<?xml version="1.0" encoding="UTF-8"?>
<rdf:RDF xmlns:rdf="http://www.w3.org/1999/02/22-rdf-syntax-ns#"
         xmlns:skos="http://www.w3.org/2004/02/skos/core#"
         xmlns:foaf="http://xmlns.com/foaf/0.1/"
         xmlns:gml="http://www.opengis.net/gml#"
         xmlns:dc="http://purl.org/dc/elements/1.1/"
         xmlns:dct="http://purl.org/dc/terms/">
   <skos:ConceptScheme rdf:about="urn:marlin.csiro.au:sourceregister:conceptscheme:1.0">
      <dc:identifier>urn:marlin.csiro.au:sourceregister</dc:identifier>
      <dc:title>CSIRO Source List</dc:title>
      <dc:description>CSIRO Oceans and Atmosphere list of Source names and descriptions</dc:description>
      <dc:URI>http://www.marlin.csiro.au/geonetwork/srv/eng/xml.metadata.get?uuid=urn:marlin.csiro.au:sourceregister</dc:URI>
      <dct:modified>2012-06-30</dct:modified>
      <dc:creator>
         <foaf:Organization>
            <foaf:name>CSIRO Oceans and Atmosphere Data Centre</foaf:name>
         </foaf:Organization>
      </dc:creator>
      <dc:publisher/>
      <dct:issued>2016-09-23T11:14:53</dct:issued>
   </skos:ConceptScheme>
   <skos:Concept rdf:about="urn:marlin.csiro.au:sourceregister:concept:216">
      <skos:prefLabel xml:lang="en">Ship: Gwendoline May</skos:prefLabel>
      <skos:inScheme rdf:resource="urn:marlin.csiro.au:sourceregister:conceptscheme:1.0"/>
      <skos:definition xml:lang="en">Type: Ship Description: None</skos:definition>
      <skos:scopeNote xml:lang="en">Ship: Gwendoline May: Type: Ship Description: None</skos:scopeNote>
   </skos:Concept>
   <skos:Concept rdf:about="urn:marlin.csiro.au:sourceregister:concept:217">
      <skos:prefLabel xml:lang="en">Model: BCC-CM1, China</skos:prefLabel>
      <skos:inScheme rdf:resource="urn:marlin.csiro.au:sourceregister:conceptscheme:1.0"/>
      <skos:definition xml:lang="en">Type: Model Description: Beijing Climate Center, National Climate Center Model
BCC-CM1, China</skos:definition>
      <skos:scopeNote xml:lang="en">Model: BCC-CM1, China: Type: Model Description: Beijing Climate Center, National Climate Center Model
BCC-CM1, China</skos:scopeNote>
   </skos:Concept>
   <skos:Concept rdf:about="urn:marlin.csiro.au:sourceregister:concept:246">
      <skos:prefLabel xml:lang="en">Model: CSIRO CCAM RCM</skos:prefLabel>
      <skos:inScheme rdf:resource="urn:marlin.csiro.au:sourceregister:conceptscheme:1.0"/>
      <skos:definition xml:lang="en">Type: Model Description: CCAM (Cubic Conformal Atmospheric Model) RCM (Regional Climate Model)</skos:definition>
      <skos:scopeNote xml:lang="en">Model: CSIRO CCAM RCM: Type: Model Description: CCAM (Cubic Conformal Atmospheric Model) RCM (Regional Climate Model)</skos:scopeNote>
   </skos:Concept>
   <skos:Concept rdf:about="urn:marlin.csiro.au:sourceregister:concept:224">
      <skos:prefLabel xml:lang="en">Model: GFDL-CM2.1, USA</skos:prefLabel>
      <skos:inScheme rdf:resource="urn:marlin.csiro.au:sourceregister:conceptscheme:1.0"/>
      <skos:definition xml:lang="en">Type: Model Description: The Geophysical Fluid Dynamics Laboratory, USA Climate System Model version 2.1 (2005) is a global coupled model representing atmosphere, land surface, oceans and sea ice. Model components consist of:
CM2.0 - AOGCM
AM2P13 &amp;#8211; atmosphere
OM3P4 - ocean
LM2 - land
SIS &amp;#8211; sea ice</skos:definition>
      <skos:scopeNote xml:lang="en">Model: GFDL-CM2.1, USA: Type: Model Description: The Geophysical Fluid Dynamics Laboratory, USA Climate System Model version 2.1 (2005) is a global coupled model representing atmosphere, land surface, oceans and sea ice. Model components consist of:
CM2.0 - AOGCM
AM2P13 &amp;#8211; atmosphere
OM3P4 - ocean
LM2 - land
SIS &amp;#8211; sea ice</skos:scopeNote>
   </skos:Concept>
   <skos:Concept rdf:about="urn:marlin.csiro.au:sourceregister:concept:227">
      <skos:prefLabel xml:lang="en">Model: GISS-EH2, USA (NASA)</skos:prefLabel>
      <skos:inScheme rdf:resource="urn:marlin.csiro.au:sourceregister:conceptscheme:1.0"/>
      <skos:definition xml:lang="en">Type: Model Description: NASA Goddard Institute for Space Studies (NASA/GISS) global climate model version E-H2 (2004) is a global coupled model representing atmosphere, land surface, oceans and sea ice. Model components consist of:
Atmospheric and sea ice model:
GISS ModelE (Schmidt et al, 2005, J. Clim, accepted)
Ocean models:
GISS-ModelE-H2 - HYCOM2 (Bleck 2000; 2002)</skos:definition>
      <skos:scopeNote xml:lang="en">Model: GISS-EH2, USA (NASA): Type: Model Description: NASA Goddard Institute for Space Studies (NASA/GISS) global climate model version E-H2 (2004) is a global coupled model representing atmosphere, land surface, oceans and sea ice. Model components consist of:
Atmospheric and sea ice model:
GISS ModelE (Schmidt et al, 2005, J. Clim, accepted)
Ocean models:
GISS-ModelE-H2 - HYCOM2 (Bleck 2000; 2002)</skos:scopeNote>
   </skos:Concept>
   <skos:Concept rdf:about="urn:marlin.csiro.au:sourceregister:concept:228">
      <skos:prefLabel xml:lang="en">Model: GISS-ER, USA (NASA)</skos:prefLabel>
      <skos:inScheme rdf:resource="urn:marlin.csiro.au:sourceregister:conceptscheme:1.0"/>
      <skos:definition xml:lang="en">Type: Model Description: NASA Goddard Institute for Space Studies (NASA/GISS) global climate model version E-R (2004) is a global coupled model representing atmosphere, land surface, oceans and sea ice. GISS-ER: ModelE20/Russell 4x5xL20. Model components consist of:
Atmospheric and sea ice model:
GISS ModelE (Schmidt et al, 2005, J. Clim, accepted)
Ocean models:
GISS-ModelE-R - Russell et al (1995; 2000)</skos:definition>
      <skos:scopeNote xml:lang="en">Model: GISS-ER, USA (NASA): Type: Model Description: NASA Goddard Institute for Space Studies (NASA/GISS) global climate model version E-R (2004) is a global coupled model representing atmosphere, land surface, oceans and sea ice. GISS-ER: ModelE20/Russell 4x5xL20. Model components consist of:
Atmospheric and sea ice model:
GISS ModelE (Schmidt et al, 2005, J. Clim, accepted)
Ocean models:
GISS-ModelE-R - Russell et al (1995; 2000)</skos:scopeNote>
   </skos:Concept>
   <skos:Concept rdf:about="urn:marlin.csiro.au:sourceregister:concept:229">
      <skos:prefLabel xml:lang="en">Model: IAP FGOALS-G1.0, China</skos:prefLabel>
      <skos:inScheme rdf:resource="urn:marlin.csiro.au:sourceregister:conceptscheme:1.0"/>
      <skos:definition xml:lang="en">Type: Model Description: LASG (Laboratory of Numerical Modeling for Atmospheric Sciences &amp; Geophysical Fluid Dynamics), Institute of Atmospheric Physics, Chinese Academy of Sciences, Global climate model version FGOALS-G1.0 (2004) is a global coupled model representing atmosphere, sea ice, land surface, and oceans. Model components consist of:
Name of the coupled GCM: FGOALS1.0_g
Name of AGCM: GAMIL1.0
Name of OGCM: LICOM1.0
Name of sea ice model: NCAR CSIM4
Name of land model: NCAR CLM2</skos:definition>
      <skos:scopeNote xml:lang="en">Model: IAP FGOALS-G1.0, China: Type: Model Description: LASG (Laboratory of Numerical Modeling for Atmospheric Sciences &amp; Geophysical Fluid Dynamics), Institute of Atmospheric Physics, Chinese Academy of Sciences, Global climate model version FGOALS-G1.0 (2004) is a global coupled model representing atmosphere, sea ice, land surface, and oceans. Model components consist of:
Name of the coupled GCM: FGOALS1.0_g
Name of AGCM: GAMIL1.0
Name of OGCM: LICOM1.0
Name of sea ice model: NCAR CSIM4
Name of land model: NCAR CLM2</skos:scopeNote>
   </skos:Concept>
   <skos:Concept rdf:about="urn:marlin.csiro.au:sourceregister:concept:231">
      <skos:prefLabel xml:lang="en">Model: IPSL-CM4, France</skos:prefLabel>
      <skos:inScheme rdf:resource="urn:marlin.csiro.au:sourceregister:conceptscheme:1.0"/>
      <skos:definition xml:lang="en">Type: Model Description: Institut Pierre Simon Laplace(IPSL), France global climate model version IPSL-CM4 (2005) is a global coupled model representing atmosphere, land surface, oceans and sea ice. Model components consist of:
coupled model: IPSL-CM4 (TAR = IPCL-CM2)
&amp;#8226; atmosphere: LMDZ-4 (TAR = LMD5)
&amp;#8226; land-vegetation: ORCHIDEE (TAR = SECHIBA)
&amp;#8226; ocean: ORCA (TAR = OPA-7)
&amp;#8226; sea-ice: LIM (TAR = IGLOO)</skos:definition>
      <skos:scopeNote xml:lang="en">Model: IPSL-CM4, France: Type: Model Description: Institut Pierre Simon Laplace(IPSL), France global climate model version IPSL-CM4 (2005) is a global coupled model representing atmosphere, land surface, oceans and sea ice. Model components consist of:
coupled model: IPSL-CM4 (TAR = IPCL-CM2)
&amp;#8226; atmosphere: LMDZ-4 (TAR = LMD5)
&amp;#8226; land-vegetation: ORCHIDEE (TAR = SECHIBA)
&amp;#8226; ocean: ORCA (TAR = OPA-7)
&amp;#8226; sea-ice: LIM (TAR = IGLOO)</skos:scopeNote>
   </skos:Concept>
   <skos:Concept rdf:about="urn:marlin.csiro.au:sourceregister:concept:234">
      <skos:prefLabel xml:lang="en">Model: MIUB-ECHO-G, Germany/Korea</skos:prefLabel>
      <skos:inScheme rdf:resource="urn:marlin.csiro.au:sourceregister:conceptscheme:1.0"/>
      <skos:definition xml:lang="en">Type: Model Description: Meteorological Institute of the University of Bonn (Germany), Institute of KMA (Korea) global climate model version ECHO-G (2005) is a global coupled model representing atmosphere, land surface, oceans and sea ice. Model components consist of: coupled model: ECHO-G = ECHAM4 + HOPE-G</skos:definition>
      <skos:scopeNote xml:lang="en">Model: MIUB-ECHO-G, Germany/Korea: Type: Model Description: Meteorological Institute of the University of Bonn (Germany), Institute of KMA (Korea) global climate model version ECHO-G (2005) is a global coupled model representing atmosphere, land surface, oceans and sea ice. Model components consist of: coupled model: ECHO-G = ECHAM4 + HOPE-G</skos:scopeNote>
   </skos:Concept>
   <skos:Concept rdf:about="urn:marlin.csiro.au:sourceregister:concept:235">
      <skos:prefLabel xml:lang="en">Model: MPI-ECHAM5, Germany</skos:prefLabel>
      <skos:inScheme rdf:resource="urn:marlin.csiro.au:sourceregister:conceptscheme:1.0"/>
      <skos:definition xml:lang="en">Type: Model Description: Max Planck Institute for Meteorology, Germany global climate model version ECHAM5(2005) is a global coupled model representing atmosphere, land surface, oceans and sea ice. GISS-ER: ModelE20/Russell 4x5xL20. Model components consist of: ECHAM5/MPI-OM. Resolution: Atmospheric: T63 L31 (TAR = T42 L19), Ocean: 1.5 deg, conformal mapping.</skos:definition>
      <skos:scopeNote xml:lang="en">Model: MPI-ECHAM5, Germany: Type: Model Description: Max Planck Institute for Meteorology, Germany global climate model version ECHAM5(2005) is a global coupled model representing atmosphere, land surface, oceans and sea ice. GISS-ER: ModelE20/Russell 4x5xL20. Model components consist of: ECHAM5/MPI-OM. Resolution: Atmospheric: T63 L31 (TAR = T42 L19), Ocean: 1.5 deg, conformal mapping.</skos:scopeNote>
   </skos:Concept>
   <skos:Concept rdf:about="urn:marlin.csiro.au:sourceregister:concept:236">
      <skos:prefLabel xml:lang="en">Model: MRI-CGCM2.3.2, Japan</skos:prefLabel>
      <skos:inScheme rdf:resource="urn:marlin.csiro.au:sourceregister:conceptscheme:1.0"/>
      <skos:definition xml:lang="en">Type: Model Description: Meteorological Research Institute, Meteorological Agency (Japan) global climate model version MRI-CGCM2.3.2 (2003) is a global coupled climate model representing atmosphere, land surface, oceans and sea ice. Coupled model: MRI-CGCM2.3.2, atmosperic: AGCM (MRI/JMA98)resolution T42(approx. 2.8 degrees), Ocean/land: MRI-CGCM2 Resolution: 2.5 degree (longitude) x 2.0 degree (latitude, poleward of 12S and 12N) ~ 0.5 (4S-4N)</skos:definition>
      <skos:scopeNote xml:lang="en">Model: MRI-CGCM2.3.2, Japan: Type: Model Description: Meteorological Research Institute, Meteorological Agency (Japan) global climate model version MRI-CGCM2.3.2 (2003) is a global coupled climate model representing atmosphere, land surface, oceans and sea ice. Coupled model: MRI-CGCM2.3.2, atmosperic: AGCM (MRI/JMA98)resolution T42(approx. 2.8 degrees), Ocean/land: MRI-CGCM2 Resolution: 2.5 degree (longitude) x 2.0 degree (latitude, poleward of 12S and 12N) ~ 0.5 (4S-4N)</skos:scopeNote>
   </skos:Concept>
   <skos:Concept rdf:about="urn:marlin.csiro.au:sourceregister:concept:237">
      <skos:prefLabel xml:lang="en">Model: NCAR CCSM3, USA</skos:prefLabel>
      <skos:inScheme rdf:resource="urn:marlin.csiro.au:sourceregister:conceptscheme:1.0"/>
      <skos:definition xml:lang="en">Type: Model Description: National Center for Atmospheric Research (NCAR)USA coupled global climate model version CCSM3 (2004) is a global coupled model representing atmosphere, sea ice, land surface and oceans. Model components consist of:
Coupled model - Community Climate System Model, version 3.0 (CCSM3) 
Atmosphere - Community Atmosphere Model, version 3.0 (CAM3)
Ocean - Parallel Ocean Program, version 1.4.3 (POP 1.4.3)
Sea ice - Community Sea Ice Model, version 5.0 (CSIM5)
Land - Community Land Model, version 3.0 (CLM3)</skos:definition>
      <skos:scopeNote xml:lang="en">Model: NCAR CCSM3, USA: Type: Model Description: National Center for Atmospheric Research (NCAR)USA coupled global climate model version CCSM3 (2004) is a global coupled model representing atmosphere, sea ice, land surface and oceans. Model components consist of:
Coupled model - Community Climate System Model, version 3.0 (CCSM3) 
Atmosphere - Community Atmosphere Model, version 3.0 (CAM3)
Ocean - Parallel Ocean Program, version 1.4.3 (POP 1.4.3)
Sea ice - Community Sea Ice Model, version 5.0 (CSIM5)
Land - Community Land Model, version 3.0 (CLM3)</skos:scopeNote>
   </skos:Concept>
   <skos:Concept rdf:about="urn:marlin.csiro.au:sourceregister:concept:245">
      <skos:prefLabel xml:lang="en">Ship: Akademik Mstislav Keldysh</skos:prefLabel>
      <skos:inScheme rdf:resource="urn:marlin.csiro.au:sourceregister:conceptscheme:1.0"/>
      <skos:definition xml:lang="en">Type: Ship Description: The R/V Akademik Mstislav Keldysh is a 6,240 ton Russian scientific research vessel, owned by the Moscow-based Shirshov Institute of Oceanology of the Russian Academy of Science.  It usually has 90 people onboard (45 crew members, 20 or more pilots, engineers and technicians, 10 to 12 scientists and about 12 passengers). Among its special accommodations are 17 laboratories and a library.
The ship was built in Rauma, Finland by Hollming OY for the Soviet Academy of Sciences and completed on December 28, 1980. It started operations on March 15, 1981 for the Soviet Union. The MIR submersibles were added to her equipment in 1987. (From Wikipedia)</skos:definition>
      <skos:scopeNote xml:lang="en">Ship: Akademik Mstislav Keldysh: Type: Ship Description: The R/V Akademik Mstislav Keldysh is a 6,240 ton Russian scientific research vessel, owned by the Moscow-based Shirshov Institute of Oceanology of the Russian Academy of Science.  It usually has 90 people onboard (45 crew members, 20 or more pilots, engineers and technicians, 10 to 12 scientists and about 12 passengers). Among its special accommodations are 17 laboratories and a library.
The ship was built in Rauma, Finland by Hollming OY for the Soviet Academy of Sciences and completed on December 28, 1980. It started operations on March 15, 1981 for the Soviet Union. The MIR submersibles were added to her equipment in 1987. (From Wikipedia)</skos:scopeNote>
   </skos:Concept>
   <skos:Concept rdf:about="urn:marlin.csiro.au:sourceregister:concept:239">
      <skos:prefLabel xml:lang="en">Model: NCAR PCM, USA</skos:prefLabel>
      <skos:inScheme rdf:resource="urn:marlin.csiro.au:sourceregister:conceptscheme:1.0"/>
      <skos:definition xml:lang="en">Type: Model Description: National Center for Atmospheric Research (NCAR)USA coupled global climate model version PCM (1998) is a global coupled model representing atmosphere, sea ice, land surface and oceans. Model components consist of:
Coupled model - Parallel Climate Model (PCM)
Atmosphere - Community Climate Model
Ocean - Parallel Ocean Program
Sea ice - Community Sea Ice Model
Land - Land Surface Model (LSM)</skos:definition>
      <skos:scopeNote xml:lang="en">Model: NCAR PCM, USA: Type: Model Description: National Center for Atmospheric Research (NCAR)USA coupled global climate model version PCM (1998) is a global coupled model representing atmosphere, sea ice, land surface and oceans. Model components consist of:
Coupled model - Parallel Climate Model (PCM)
Atmosphere - Community Climate Model
Ocean - Parallel Ocean Program
Sea ice - Community Sea Ice Model
Land - Land Surface Model (LSM)</skos:scopeNote>
   </skos:Concept>
   <skos:Concept rdf:about="urn:marlin.csiro.au:sourceregister:concept:240">
      <skos:prefLabel xml:lang="en">Model: UKMO-HadCM3, UK</skos:prefLabel>
      <skos:inScheme rdf:resource="urn:marlin.csiro.au:sourceregister:conceptscheme:1.0"/>
      <skos:definition xml:lang="en">Type: Model Description: Hadley Centre for Climate Prediction and Research Met Office UK, coupled global climate model version HadCM3 (2000) is a global coupled model representing atmosphere, sea ice, land surface and oceans. Resolution: Atmospheric - 2.75o lat x 3.75o lon, Ocean sea ice &amp; land - 1.25o x 1.25o.</skos:definition>
      <skos:scopeNote xml:lang="en">Model: UKMO-HadCM3, UK: Type: Model Description: Hadley Centre for Climate Prediction and Research Met Office UK, coupled global climate model version HadCM3 (2000) is a global coupled model representing atmosphere, sea ice, land surface and oceans. Resolution: Atmospheric - 2.75o lat x 3.75o lon, Ocean sea ice &amp; land - 1.25o x 1.25o.</skos:scopeNote>
   </skos:Concept>
   <skos:Concept rdf:about="urn:marlin.csiro.au:sourceregister:concept:243">
      <skos:prefLabel xml:lang="en">Model: INGV-SXG, Italy </skos:prefLabel>
      <skos:inScheme rdf:resource="urn:marlin.csiro.au:sourceregister:conceptscheme:1.0"/>
      <skos:definition xml:lang="en">Type: Model Description: Instituto Nazionale di Geofisica e Vulcanologia Global climate model version INGV-SXG is a global coupled model representing atmosphere, sea ice, land surface, and oceans. Model components consist of: INGV-SXG (SINTEX-G). ECHAM4.6, OPA8.2, LIM(Louvain-La-Neuve sea-ice model).(2005)
Resolution:
Atmosphere - horizontal res: T106 (about 1.125o x1.125o).vertical res: L19
Ocean OPA8.2 -
Quasi-isotrope tri-polar grid (2 poles in the northern hemisphere, one over Canada and the other over Siberia. 2° resolution Mercator grid (i.e.&amp;#1048615;x=&amp;#1048615;y) with enhanced meridional resolution in the vicinity of the equator and in Med and Red seas (1°)
sea ice LIM - Horizontal resolution: same as ocean model (2° in longitude and roughly 2° cos(phi) in latitude; equations for ice motion and transport written in curvilinear, orthogonal coordinates; staggered spatial grid of type B). Layers: 3 (1 in snow and 2 in ice), Thickness categories: 2 (level ice and leads).</skos:definition>
      <skos:scopeNote xml:lang="en">Model: INGV-SXG, Italy : Type: Model Description: Instituto Nazionale di Geofisica e Vulcanologia Global climate model version INGV-SXG is a global coupled model representing atmosphere, sea ice, land surface, and oceans. Model components consist of: INGV-SXG (SINTEX-G). ECHAM4.6, OPA8.2, LIM(Louvain-La-Neuve sea-ice model).(2005)
Resolution:
Atmosphere - horizontal res: T106 (about 1.125o x1.125o).vertical res: L19
Ocean OPA8.2 -
Quasi-isotrope tri-polar grid (2 poles in the northern hemisphere, one over Canada and the other over Siberia. 2° resolution Mercator grid (i.e.&amp;#1048615;x=&amp;#1048615;y) with enhanced meridional resolution in the vicinity of the equator and in Med and Red seas (1°)
sea ice LIM - Horizontal resolution: same as ocean model (2° in longitude and roughly 2° cos(phi) in latitude; equations for ice motion and transport written in curvilinear, orthogonal coordinates; staggered spatial grid of type B). Layers: 3 (1 in snow and 2 in ice), Thickness categories: 2 (level ice and leads).</skos:scopeNote>
   </skos:Concept>
   <skos:Concept rdf:about="urn:marlin.csiro.au:sourceregister:concept:251">
      <skos:prefLabel xml:lang="en">Model: NRL/FNMOC</skos:prefLabel>
      <skos:inScheme rdf:resource="urn:marlin.csiro.au:sourceregister:conceptscheme:1.0"/>
      <skos:definition xml:lang="en">Type: Model Description: Naval Research Laboratory/ Fleet Numerical Meteorology &amp; Oceanography Center
</skos:definition>
      <skos:scopeNote xml:lang="en">Model: NRL/FNMOC: Type: Model Description: Naval Research Laboratory/ Fleet Numerical Meteorology &amp; Oceanography Center
</skos:scopeNote>
   </skos:Concept>
   <skos:Concept rdf:about="urn:marlin.csiro.au:sourceregister:concept:253">
      <skos:prefLabel xml:lang="en">Model: ECMWF</skos:prefLabel>
      <skos:inScheme rdf:resource="urn:marlin.csiro.au:sourceregister:conceptscheme:1.0"/>
      <skos:definition xml:lang="en">Type: Model Description: European Center for Medium range Weather Forecasting(EMCWF)
European Union Framework 5 project
</skos:definition>
      <skos:scopeNote xml:lang="en">Model: ECMWF: Type: Model Description: European Center for Medium range Weather Forecasting(EMCWF)
European Union Framework 5 project
</skos:scopeNote>
   </skos:Concept>
   <skos:Concept rdf:about="urn:marlin.csiro.au:sourceregister:concept:256">
      <skos:prefLabel xml:lang="en">Model: CMAP</skos:prefLabel>
      <skos:inScheme rdf:resource="urn:marlin.csiro.au:sourceregister:conceptscheme:1.0"/>
      <skos:definition xml:lang="en">Type: Model Description: Climate Prediction Center (CPC) Merged Analysis of Precipitation (CMAP)
</skos:definition>
      <skos:scopeNote xml:lang="en">Model: CMAP: Type: Model Description: Climate Prediction Center (CPC) Merged Analysis of Precipitation (CMAP)
</skos:scopeNote>
   </skos:Concept>
   <skos:Concept rdf:about="urn:marlin.csiro.au:sourceregister:concept:257">
      <skos:prefLabel xml:lang="en">Model: SODA</skos:prefLabel>
      <skos:inScheme rdf:resource="urn:marlin.csiro.au:sourceregister:conceptscheme:1.0"/>
      <skos:definition xml:lang="en">Type: Model Description: University of Maryland, SODA (simple oceanographic data assimilation) reanalysis.</skos:definition>
      <skos:scopeNote xml:lang="en">Model: SODA: Type: Model Description: University of Maryland, SODA (simple oceanographic data assimilation) reanalysis.</skos:scopeNote>
   </skos:Concept>
   <skos:Concept rdf:about="urn:marlin.csiro.au:sourceregister:concept:258">
      <skos:prefLabel xml:lang="en">Ship: Adriatic Perl</skos:prefLabel>
      <skos:inScheme rdf:resource="urn:marlin.csiro.au:sourceregister:conceptscheme:1.0"/>
      <skos:definition xml:lang="en">Type: Ship Description: None</skos:definition>
      <skos:scopeNote xml:lang="en">Ship: Adriatic Perl: Type: Ship Description: None</skos:scopeNote>
   </skos:Concept>
   <skos:Concept rdf:about="urn:marlin.csiro.au:sourceregister:concept:222">
      <skos:prefLabel xml:lang="en">Model: CNRM-CM3, France</skos:prefLabel>
      <skos:inScheme rdf:resource="urn:marlin.csiro.au:sourceregister:conceptscheme:1.0"/>
      <skos:definition xml:lang="en">Type: Model Description: Centre National de Recherches Météorologiques, Météo France, France - CNRM-CM3
Atmosphere: ARPEGE-Climat version 3
Ocean: OPA 8.1
Sea-ice: GELATO 2

The CNRM-CM3 global coupled system is the third version of the ocean-atmosphere model initially developed at CERFACS (Toulouse, France), then regularlarly updated at Center National Weather Research  (CNRM, METEO-FRANCE, Toulouse).
This model consisted initially of ARPEGE-Climat 2 AGCM (CNRM, Déqué et al., 1994; Déqué and Piedelievre, 1995, Déqué et al., 1998; Gibelin and Déqué, 2003) and OPA7 OGCM (LODyC, CNRS-IPSL, Paris).
These components were updated respectively to ARPEGE-Climat 3 and OPA8.
CNRM-CM3 also now includes a parameterization of the homogeneous and heterogeneous chemistry of ozone (Cariolle et al., 1990), a sea ice model, GELATO2 (Salas-Mélia, 2002), and TRIP river routing from Tokyo University (Oki and Sud, 1998; Oki et al., 1999).
ARPEGE-Climat 3 is a spectral model (truncation T63, 128x64, about 2.8° resolution, and 45 levels), OPA8 (31 levels) and GELATO2 are both grid point models and share the same mesh of 182x152 points.
It corresponds to a resolution of about 2° in longitude, the latitudinal resolution varying from 0.5° near the equator to roughly 2° in polar regions.
The couplings between the different models are manage</skos:definition>
      <skos:scopeNote xml:lang="en">Model: CNRM-CM3, France: Type: Model Description: Centre National de Recherches Météorologiques, Météo France, France - CNRM-CM3
Atmosphere: ARPEGE-Climat version 3
Ocean: OPA 8.1
Sea-ice: GELATO 2

The CNRM-CM3 global coupled system is the third version of the ocean-atmosphere model initially developed at CERFACS (Toulouse, France), then regularlarly updated at Center National Weather Research  (CNRM, METEO-FRANCE, Toulouse).
This model consisted initially of ARPEGE-Climat 2 AGCM (CNRM, Déqué et al., 1994; Déqué and Piedelievre, 1995, Déqué et al., 1998; Gibelin and Déqué, 2003) and OPA7 OGCM (LODyC, CNRS-IPSL, Paris).
These components were updated respectively to ARPEGE-Climat 3 and OPA8.
CNRM-CM3 also now includes a parameterization of the homogeneous and heterogeneous chemistry of ozone (Cariolle et al., 1990), a sea ice model, GELATO2 (Salas-Mélia, 2002), and TRIP river routing from Tokyo University (Oki and Sud, 1998; Oki et al., 1999).
ARPEGE-Climat 3 is a spectral model (truncation T63, 128x64, about 2.8° resolution, and 45 levels), OPA8 (31 levels) and GELATO2 are both grid point models and share the same mesh of 182x152 points.
It corresponds to a resolution of about 2° in longitude, the latitudinal resolution varying from 0.5° near the equator to roughly 2° in polar regions.
The couplings between the different models are manage</skos:scopeNote>
   </skos:Concept>
   <skos:Concept rdf:about="urn:marlin.csiro.au:sourceregister:concept:223">
      <skos:prefLabel xml:lang="en">Model: GFDL-CM2.0, USA</skos:prefLabel>
      <skos:inScheme rdf:resource="urn:marlin.csiro.au:sourceregister:conceptscheme:1.0"/>
      <skos:definition xml:lang="en">Type: Model Description: The Geophysical Fluid Dynamics Laboratory, USA Climate System Model version 2.0 (2005) is a global coupled model representing atmosphere, land surface, oceans and sea ice. Model components consist of:
CM2.0 - AOGCM
AM2P13 &amp;#8211; atmosphere
OM3P4 - ocean
LM2 - land
SIS &amp;#8211; sea ice</skos:definition>
      <skos:scopeNote xml:lang="en">Model: GFDL-CM2.0, USA: Type: Model Description: The Geophysical Fluid Dynamics Laboratory, USA Climate System Model version 2.0 (2005) is a global coupled model representing atmosphere, land surface, oceans and sea ice. Model components consist of:
CM2.0 - AOGCM
AM2P13 &amp;#8211; atmosphere
OM3P4 - ocean
LM2 - land
SIS &amp;#8211; sea ice</skos:scopeNote>
   </skos:Concept>
   <skos:Concept rdf:about="urn:marlin.csiro.au:sourceregister:concept:225">
      <skos:prefLabel xml:lang="en">Model: GISS-AOM, USA (NASA)</skos:prefLabel>
      <skos:inScheme rdf:resource="urn:marlin.csiro.au:sourceregister:conceptscheme:1.0"/>
      <skos:definition xml:lang="en">Type: Model Description: NASA Goddard Institute for Space Studies (NASA/GISS) global climate model,
Model version AOM 4x3(2004) atmosphere/ocean model.</skos:definition>
      <skos:scopeNote xml:lang="en">Model: GISS-AOM, USA (NASA): Type: Model Description: NASA Goddard Institute for Space Studies (NASA/GISS) global climate model,
Model version AOM 4x3(2004) atmosphere/ocean model.</skos:scopeNote>
   </skos:Concept>
   <skos:Concept rdf:about="urn:marlin.csiro.au:sourceregister:concept:226">
      <skos:prefLabel xml:lang="en">Model: GISS-EH, USA (NASA)</skos:prefLabel>
      <skos:inScheme rdf:resource="urn:marlin.csiro.au:sourceregister:conceptscheme:1.0"/>
      <skos:definition xml:lang="en">Type: Model Description: NASA Goddard Institute for Space Studies (NASA/GISS) global climate model version E-H (2004) is a global coupled model representing atmosphere, land surface, oceans and sea ice. Model components consist of:
Atmospheric and sea ice model:
GISS ModelE (Schmidt et al, 2005, J. Clim, accepted)
Ocean models:
GISS-ModelE-H - HYCOM (Bleck 2000; 2002)</skos:definition>
      <skos:scopeNote xml:lang="en">Model: GISS-EH, USA (NASA): Type: Model Description: NASA Goddard Institute for Space Studies (NASA/GISS) global climate model version E-H (2004) is a global coupled model representing atmosphere, land surface, oceans and sea ice. Model components consist of:
Atmospheric and sea ice model:
GISS ModelE (Schmidt et al, 2005, J. Clim, accepted)
Ocean models:
GISS-ModelE-H - HYCOM (Bleck 2000; 2002)</skos:scopeNote>
   </skos:Concept>
   <skos:Concept rdf:about="urn:marlin.csiro.au:sourceregister:concept:230">
      <skos:prefLabel xml:lang="en">Model: INMCM3.0, Russia</skos:prefLabel>
      <skos:inScheme rdf:resource="urn:marlin.csiro.au:sourceregister:conceptscheme:1.0"/>
      <skos:definition xml:lang="en">Type: Model Description: Institute of Numerical Mathematics, Russian Academy of Science, Russia global climate model version INMCM3.0 (2004) is a global coupled model representing atmosphere, land surface, oceans and sea ice.
</skos:definition>
      <skos:scopeNote xml:lang="en">Model: INMCM3.0, Russia: Type: Model Description: Institute of Numerical Mathematics, Russian Academy of Science, Russia global climate model version INMCM3.0 (2004) is a global coupled model representing atmosphere, land surface, oceans and sea ice.
</skos:scopeNote>
   </skos:Concept>
   <skos:Concept rdf:about="urn:marlin.csiro.au:sourceregister:concept:232">
      <skos:prefLabel xml:lang="en">Model: MIROC3.2(hires), Japan</skos:prefLabel>
      <skos:inScheme rdf:resource="urn:marlin.csiro.au:sourceregister:conceptscheme:1.0"/>
      <skos:definition xml:lang="en">Type: Model Description: Center for Climate System Research, University of Tokyo Japan  Global climate model version MIROC3.2(hires) (2004) is a global coupled model representing atmosphere, sea ice, land surface, and oceans. Model components consist of:
Coupled model: MIROC3.2 (Model for Interdisciplinary Research on Climate)
Atmospheric model: CCSR/NIES/FRCGC AGCM5.7b
Ocean &amp; sea ice model: COCO3.3 (CCSR Ocean Component model)
Land surface model: MATSIRO (Minimal Advanced Treatments of Surface
Interaction and Runoff)</skos:definition>
      <skos:scopeNote xml:lang="en">Model: MIROC3.2(hires), Japan: Type: Model Description: Center for Climate System Research, University of Tokyo Japan  Global climate model version MIROC3.2(hires) (2004) is a global coupled model representing atmosphere, sea ice, land surface, and oceans. Model components consist of:
Coupled model: MIROC3.2 (Model for Interdisciplinary Research on Climate)
Atmospheric model: CCSR/NIES/FRCGC AGCM5.7b
Ocean &amp; sea ice model: COCO3.3 (CCSR Ocean Component model)
Land surface model: MATSIRO (Minimal Advanced Treatments of Surface
Interaction and Runoff)</skos:scopeNote>
   </skos:Concept>
   <skos:Concept rdf:about="urn:marlin.csiro.au:sourceregister:concept:233">
      <skos:prefLabel xml:lang="en">Model: MIROC3.2(medres)</skos:prefLabel>
      <skos:inScheme rdf:resource="urn:marlin.csiro.au:sourceregister:conceptscheme:1.0"/>
      <skos:definition xml:lang="en">Type: Model Description: Center for Climate System Research, University of Tokyo Japan  Global climate model version MIROC3.2(medres) (2004) is a global coupled model representing atmosphere, sea ice, land surface, and oceans. Model components consist of:
Coupled model: MIROC3.2 (Model for Interdisciplinary Research on Climate)
Atmospheric model: CCSR/NIES/FRCGC AGCM5.7b
Ocean &amp; sea ice model: COCO3.3 (CCSR Ocean Component model)
Land surface model: MATSIRO (Minimal Advanced Treatments of Surface Interaction and Runoff)
Resolution: atmos-T42L20 ocean-1.4Long, .5to1.4 Lat, 43 levels.

</skos:definition>
      <skos:scopeNote xml:lang="en">Model: MIROC3.2(medres): Type: Model Description: Center for Climate System Research, University of Tokyo Japan  Global climate model version MIROC3.2(medres) (2004) is a global coupled model representing atmosphere, sea ice, land surface, and oceans. Model components consist of:
Coupled model: MIROC3.2 (Model for Interdisciplinary Research on Climate)
Atmospheric model: CCSR/NIES/FRCGC AGCM5.7b
Ocean &amp; sea ice model: COCO3.3 (CCSR Ocean Component model)
Land surface model: MATSIRO (Minimal Advanced Treatments of Surface Interaction and Runoff)
Resolution: atmos-T42L20 ocean-1.4Long, .5to1.4 Lat, 43 levels.

</skos:scopeNote>
   </skos:Concept>
   <skos:Concept rdf:about="urn:marlin.csiro.au:sourceregister:concept:242">
      <skos:prefLabel xml:lang="en">Model: UKMO HadGEM1, UK</skos:prefLabel>
      <skos:inScheme rdf:resource="urn:marlin.csiro.au:sourceregister:conceptscheme:1.0"/>
      <skos:definition xml:lang="en">Type: Model Description: Hadley Centre for Climate Prediction and Research/Met Office UK, coupled global climate model version HadGEM1 (2006) is a global coupled model representing atmosphere, sea ice, land surface and oceans. Model components consist of:
Coupled model - UKMO HadGEM1 
Atmospheric component - (HadGAM1) - includes land and river routing components
Oceanic component - (HadGOM1) - includes sea ice component
Sea ice component - (HadGOM1)
Land component - (MOSES-2) - Met Office Surface Exchange Scheme, version 2
River routing - (TRIP) - Total Runoff Integrating Pathways 
</skos:definition>
      <skos:scopeNote xml:lang="en">Model: UKMO HadGEM1, UK: Type: Model Description: Hadley Centre for Climate Prediction and Research/Met Office UK, coupled global climate model version HadGEM1 (2006) is a global coupled model representing atmosphere, sea ice, land surface and oceans. Model components consist of:
Coupled model - UKMO HadGEM1 
Atmospheric component - (HadGAM1) - includes land and river routing components
Oceanic component - (HadGOM1) - includes sea ice component
Sea ice component - (HadGOM1)
Land component - (MOSES-2) - Met Office Surface Exchange Scheme, version 2
River routing - (TRIP) - Total Runoff Integrating Pathways 
</skos:scopeNote>
   </skos:Concept>
   <skos:Concept rdf:about="urn:marlin.csiro.au:sourceregister:concept:248">
      <skos:prefLabel xml:lang="en">Model: NCEP/NCAR</skos:prefLabel>
      <skos:inScheme rdf:resource="urn:marlin.csiro.au:sourceregister:conceptscheme:1.0"/>
      <skos:definition xml:lang="en">Type: Model Description: National Centers for Enviromental Prediction
</skos:definition>
      <skos:scopeNote xml:lang="en">Model: NCEP/NCAR: Type: Model Description: National Centers for Enviromental Prediction
</skos:scopeNote>
   </skos:Concept>
   <skos:Concept rdf:about="urn:marlin.csiro.au:sourceregister:concept:249">
      <skos:prefLabel xml:lang="en">Ship: Ngerin</skos:prefLabel>
      <skos:inScheme rdf:resource="urn:marlin.csiro.au:sourceregister:conceptscheme:1.0"/>
      <skos:definition xml:lang="en">Type: Ship Description: MRV Ngerin: South Australian Research and Development Institute (SARDI) Aquatic Sciences marine research vessel, see url - http://www.sardi.sa.gov.au/pages/fisheries/sas/fac/mrv_ngerin.htm</skos:definition>
      <skos:scopeNote xml:lang="en">Ship: Ngerin: Type: Ship Description: MRV Ngerin: South Australian Research and Development Institute (SARDI) Aquatic Sciences marine research vessel, see url - http://www.sardi.sa.gov.au/pages/fisheries/sas/fac/mrv_ngerin.htm</skos:scopeNote>
   </skos:Concept>
   <skos:Concept rdf:about="urn:marlin.csiro.au:sourceregister:concept:250">
      <skos:prefLabel xml:lang="en">Model: NCEP</skos:prefLabel>
      <skos:inScheme rdf:resource="urn:marlin.csiro.au:sourceregister:conceptscheme:1.0"/>
      <skos:definition xml:lang="en">Type: Model Description: National Centers for Environmental Prediction
</skos:definition>
      <skos:scopeNote xml:lang="en">Model: NCEP: Type: Model Description: National Centers for Environmental Prediction
</skos:scopeNote>
   </skos:Concept>
   <skos:Concept rdf:about="urn:marlin.csiro.au:sourceregister:concept:252">
      <skos:prefLabel xml:lang="en">Model: DWD-GPCC</skos:prefLabel>
      <skos:inScheme rdf:resource="urn:marlin.csiro.au:sourceregister:conceptscheme:1.0"/>
      <skos:definition xml:lang="en">Type: Model Description: Deutscher Wetterdienst (DWD, National Meteorological Service of Germany)
Global Precipitation Climatology Centre(GPCC)</skos:definition>
      <skos:scopeNote xml:lang="en">Model: DWD-GPCC: Type: Model Description: Deutscher Wetterdienst (DWD, National Meteorological Service of Germany)
Global Precipitation Climatology Centre(GPCC)</skos:scopeNote>
   </skos:Concept>
   <skos:Concept rdf:about="urn:marlin.csiro.au:sourceregister:concept:254">
      <skos:prefLabel xml:lang="en">Model: UKMO HADISST</skos:prefLabel>
      <skos:inScheme rdf:resource="urn:marlin.csiro.au:sourceregister:conceptscheme:1.0"/>
      <skos:definition xml:lang="en">Type: Model Description: Hadley Centre for Climate Prediction and Research/Met Office UK
(HadISST, Version 1.1)</skos:definition>
      <skos:scopeNote xml:lang="en">Model: UKMO HADISST: Type: Model Description: Hadley Centre for Climate Prediction and Research/Met Office UK
(HadISST, Version 1.1)</skos:scopeNote>
   </skos:Concept>
   <skos:Concept rdf:about="urn:marlin.csiro.au:sourceregister:concept:255">
      <skos:prefLabel xml:lang="en">Observational: BOM (Bureau of Meteorology)</skos:prefLabel>
      <skos:inScheme rdf:resource="urn:marlin.csiro.au:sourceregister:conceptscheme:1.0"/>
      <skos:definition xml:lang="en">Type: Observational Description: Bureau of Meteorology Australia
</skos:definition>
      <skos:scopeNote xml:lang="en">Observational: BOM (Bureau of Meteorology): Type: Observational Description: Bureau of Meteorology Australia
</skos:scopeNote>
   </skos:Concept>
   <skos:Concept rdf:about="urn:marlin.csiro.au:sourceregister:concept:259">
      <skos:prefLabel xml:lang="en">Observational: ARGO</skos:prefLabel>
      <skos:inScheme rdf:resource="urn:marlin.csiro.au:sourceregister:conceptscheme:1.0"/>
      <skos:definition xml:lang="en">Type: Observational Description: Advanced Research and Global Observation satellites
Part of the World Climate Research Programme&amp;#8217;s Climate Variability and Predictability project (CLIVAR), Global Ocean Data Assimilation Experiment (GODAE), Global Ocean Observing System (GOOS).
</skos:definition>
      <skos:scopeNote xml:lang="en">Observational: ARGO: Type: Observational Description: Advanced Research and Global Observation satellites
Part of the World Climate Research Programme&amp;#8217;s Climate Variability and Predictability project (CLIVAR), Global Ocean Data Assimilation Experiment (GODAE), Global Ocean Observing System (GOOS).
</skos:scopeNote>
   </skos:Concept>
   <skos:Concept rdf:about="urn:marlin.csiro.au:sourceregister:concept:260">
      <skos:prefLabel xml:lang="en">Ship: Bluefin</skos:prefLabel>
      <skos:inScheme rdf:resource="urn:marlin.csiro.au:sourceregister:conceptscheme:1.0"/>
      <skos:definition xml:lang="en">Type: Ship Description: Bluefin, Australian Maritime College (AMC) 34.5m fisheries training vessel, is powered by a Caterpillar D398 main engine. Fitted with a controllable pitch propeller and bow thruster, it is capable of cruising all Australian waters. 
Bluefin engages in stern trawling, both bottom and midwater, purse seining and prawn trawling. It can also be used to demonstrate other fishing methods on and beyond the continental shelf. Fish handling and storage capabilities include a refrigerated ice room, blast freezer, and refrigerated salt water and chilled water systems.
Bluefin is equipped with a range of electronic equipment including a Simrad EK60 (38&amp;120kHz) scientific echo sounder, OLEX 3D bottom mapping plotter, JRC Raster scan 96nm Radar, Simrad SQ270 sonar, Furuno ARPA radar, colour and monochrome underwater cameras.</skos:definition>
      <skos:scopeNote xml:lang="en">Ship: Bluefin: Type: Ship Description: Bluefin, Australian Maritime College (AMC) 34.5m fisheries training vessel, is powered by a Caterpillar D398 main engine. Fitted with a controllable pitch propeller and bow thruster, it is capable of cruising all Australian waters. 
Bluefin engages in stern trawling, both bottom and midwater, purse seining and prawn trawling. It can also be used to demonstrate other fishing methods on and beyond the continental shelf. Fish handling and storage capabilities include a refrigerated ice room, blast freezer, and refrigerated salt water and chilled water systems.
Bluefin is equipped with a range of electronic equipment including a Simrad EK60 (38&amp;120kHz) scientific echo sounder, OLEX 3D bottom mapping plotter, JRC Raster scan 96nm Radar, Simrad SQ270 sonar, Furuno ARPA radar, colour and monochrome underwater cameras.</skos:scopeNote>
   </skos:Concept>
   <skos:Concept rdf:about="urn:marlin.csiro.au:sourceregister:concept:261">
      <skos:prefLabel xml:lang="en">Coastal Station: Aspendale</skos:prefLabel>
      <skos:inScheme rdf:resource="urn:marlin.csiro.au:sourceregister:conceptscheme:1.0"/>
      <skos:definition xml:lang="en">Type: Coastal Station Description: Aspendale Bayside Air Quality Station
107 Station St Aspendale, VIC 3195</skos:definition>
      <skos:scopeNote xml:lang="en">Coastal Station: Aspendale: Type: Coastal Station Description: Aspendale Bayside Air Quality Station
107 Station St Aspendale, VIC 3195</skos:scopeNote>
   </skos:Concept>
   <skos:Concept rdf:about="urn:marlin.csiro.au:sourceregister:concept:262">
      <skos:prefLabel xml:lang="en">Model: RAMS</skos:prefLabel>
      <skos:inScheme rdf:resource="urn:marlin.csiro.au:sourceregister:conceptscheme:1.0"/>
      <skos:definition xml:lang="en">Type: Model Description: Colorado State University - Regional Atmospheric Modeling System
(Dynamic Downscaling)
</skos:definition>
      <skos:scopeNote xml:lang="en">Model: RAMS: Type: Model Description: Colorado State University - Regional Atmospheric Modeling System
(Dynamic Downscaling)
</skos:scopeNote>
   </skos:Concept>
   <skos:Concept rdf:about="urn:marlin.csiro.au:sourceregister:concept:267">
      <skos:prefLabel xml:lang="en">Coastal Station: Cape Matatula</skos:prefLabel>
      <skos:inScheme rdf:resource="urn:marlin.csiro.au:sourceregister:conceptscheme:1.0"/>
      <skos:definition xml:lang="en">Type: Coastal Station Description: Cape Matatula - American Samoa 
(14° S, 171° W)</skos:definition>
      <skos:scopeNote xml:lang="en">Coastal Station: Cape Matatula: Type: Coastal Station Description: Cape Matatula - American Samoa 
(14° S, 171° W)</skos:scopeNote>
   </skos:Concept>
   <skos:Concept rdf:about="urn:marlin.csiro.au:sourceregister:concept:264">
      <skos:prefLabel xml:lang="en">Coastal Station: Cape Grim</skos:prefLabel>
      <skos:inScheme rdf:resource="urn:marlin.csiro.au:sourceregister:conceptscheme:1.0"/>
      <skos:definition xml:lang="en">Type: Coastal Station Description: Cape Grim Baseline Air Pollution Station Tasmania
(41° S, 145° E)</skos:definition>
      <skos:scopeNote xml:lang="en">Coastal Station: Cape Grim: Type: Coastal Station Description: Cape Grim Baseline Air Pollution Station Tasmania
(41° S, 145° E)</skos:scopeNote>
   </skos:Concept>
   <skos:Concept rdf:about="urn:marlin.csiro.au:sourceregister:concept:265">
      <skos:prefLabel xml:lang="en">Coastal Station: Mace Head</skos:prefLabel>
      <skos:inScheme rdf:resource="urn:marlin.csiro.au:sourceregister:conceptscheme:1.0"/>
      <skos:definition xml:lang="en">Type: Coastal Station Description: Mace Head - Ireland
(53° N, 10° W)</skos:definition>
      <skos:scopeNote xml:lang="en">Coastal Station: Mace Head: Type: Coastal Station Description: Mace Head - Ireland
(53° N, 10° W)</skos:scopeNote>
   </skos:Concept>
   <skos:Concept rdf:about="urn:marlin.csiro.au:sourceregister:concept:266">
      <skos:prefLabel xml:lang="en">Coastal Station: Trinidad Head</skos:prefLabel>
      <skos:inScheme rdf:resource="urn:marlin.csiro.au:sourceregister:conceptscheme:1.0"/>
      <skos:definition xml:lang="en">Type: Coastal Station Description: Trinidad Head - California
(41° N, 124° W)</skos:definition>
      <skos:scopeNote xml:lang="en">Coastal Station: Trinidad Head: Type: Coastal Station Description: Trinidad Head - California
(41° N, 124° W)</skos:scopeNote>
   </skos:Concept>
   <skos:Concept rdf:about="urn:marlin.csiro.au:sourceregister:concept:268">
      <skos:prefLabel xml:lang="en">Coastal Station: Ragged Point</skos:prefLabel>
      <skos:inScheme rdf:resource="urn:marlin.csiro.au:sourceregister:conceptscheme:1.0"/>
      <skos:definition xml:lang="en">Type: Coastal Station Description: Ragged Point - Barbados
(13° N, 59° W)</skos:definition>
      <skos:scopeNote xml:lang="en">Coastal Station: Ragged Point: Type: Coastal Station Description: Ragged Point - Barbados
(13° N, 59° W)</skos:scopeNote>
   </skos:Concept>
   <skos:Concept rdf:about="urn:marlin.csiro.au:sourceregister:concept:269">
      <skos:prefLabel xml:lang="en">Coastal Station: Monte Cimone</skos:prefLabel>
      <skos:inScheme rdf:resource="urn:marlin.csiro.au:sourceregister:conceptscheme:1.0"/>
      <skos:definition xml:lang="en">Type: Coastal Station Description: Monte Cimone - Italy
</skos:definition>
      <skos:scopeNote xml:lang="en">Coastal Station: Monte Cimone: Type: Coastal Station Description: Monte Cimone - Italy
</skos:scopeNote>
   </skos:Concept>
   <skos:Concept rdf:about="urn:marlin.csiro.au:sourceregister:concept:270">
      <skos:prefLabel xml:lang="en">Coastal Station: Ny-Alesund </skos:prefLabel>
      <skos:inScheme rdf:resource="urn:marlin.csiro.au:sourceregister:conceptscheme:1.0"/>
      <skos:definition xml:lang="en">Type: Coastal Station Description: Ny-Alesund - Svalbard, Norway
</skos:definition>
      <skos:scopeNote xml:lang="en">Coastal Station: Ny-Alesund : Type: Coastal Station Description: Ny-Alesund - Svalbard, Norway
</skos:scopeNote>
   </skos:Concept>
   <skos:Concept rdf:about="urn:marlin.csiro.au:sourceregister:concept:271">
      <skos:prefLabel xml:lang="en">Coastal Station: Jungfraujoch</skos:prefLabel>
      <skos:inScheme rdf:resource="urn:marlin.csiro.au:sourceregister:conceptscheme:1.0"/>
      <skos:definition xml:lang="en">Type: Coastal Station Description: Jungfraujoch - Switzerland</skos:definition>
      <skos:scopeNote xml:lang="en">Coastal Station: Jungfraujoch: Type: Coastal Station Description: Jungfraujoch - Switzerland</skos:scopeNote>
   </skos:Concept>
   <skos:Concept rdf:about="urn:marlin.csiro.au:sourceregister:concept:273">
      <skos:prefLabel xml:lang="en">Coastal Station: Gosan</skos:prefLabel>
      <skos:inScheme rdf:resource="urn:marlin.csiro.au:sourceregister:conceptscheme:1.0"/>
      <skos:definition xml:lang="en">Type: Coastal Station Description: Gosan - Korea
</skos:definition>
      <skos:scopeNote xml:lang="en">Coastal Station: Gosan: Type: Coastal Station Description: Gosan - Korea
</skos:scopeNote>
   </skos:Concept>
   <skos:Concept rdf:about="urn:marlin.csiro.au:sourceregister:concept:274">
      <skos:prefLabel xml:lang="en">Coastal Station: Hateruma</skos:prefLabel>
      <skos:inScheme rdf:resource="urn:marlin.csiro.au:sourceregister:conceptscheme:1.0"/>
      <skos:definition xml:lang="en">Type: Coastal Station Description: Hateruma - Japan</skos:definition>
      <skos:scopeNote xml:lang="en">Coastal Station: Hateruma: Type: Coastal Station Description: Hateruma - Japan</skos:scopeNote>
   </skos:Concept>
   <skos:Concept rdf:about="urn:marlin.csiro.au:sourceregister:concept:275">
      <skos:prefLabel xml:lang="en">Coastal Station: Adrigole</skos:prefLabel>
      <skos:inScheme rdf:resource="urn:marlin.csiro.au:sourceregister:conceptscheme:1.0"/>
      <skos:definition xml:lang="en">Type: Coastal Station Description: Adrigole-Ireland (52° N, 10° W)
No longer used?. Replaced by Mace Head, Ireland</skos:definition>
      <skos:scopeNote xml:lang="en">Coastal Station: Adrigole: Type: Coastal Station Description: Adrigole-Ireland (52° N, 10° W)
No longer used?. Replaced by Mace Head, Ireland</skos:scopeNote>
   </skos:Concept>
   <skos:Concept rdf:about="urn:marlin.csiro.au:sourceregister:concept:195">
      <skos:prefLabel xml:lang="en">Satellite: Envisat</skos:prefLabel>
      <skos:inScheme rdf:resource="urn:marlin.csiro.au:sourceregister:conceptscheme:1.0"/>
      <skos:definition xml:lang="en">Type: Satellite Description: European Space Agency Satellite</skos:definition>
      <skos:scopeNote xml:lang="en">Satellite: Envisat: Type: Satellite Description: European Space Agency Satellite</skos:scopeNote>
   </skos:Concept>
   <skos:Concept rdf:about="urn:marlin.csiro.au:sourceregister:concept:196">
      <skos:prefLabel xml:lang="en">Ship: Maritime Image</skos:prefLabel>
      <skos:inScheme rdf:resource="urn:marlin.csiro.au:sourceregister:conceptscheme:1.0"/>
      <skos:definition xml:lang="en">Type: Ship Description: The Maritime Image is an 18 training vessel operated by the Western Australian 
Maritime Training Centre Fremantle, a part of TAFE
(http://www.challengertafe.wa.edu.au/)</skos:definition>
      <skos:scopeNote xml:lang="en">Ship: Maritime Image: Type: Ship Description: The Maritime Image is an 18 training vessel operated by the Western Australian 
Maritime Training Centre Fremantle, a part of TAFE
(http://www.challengertafe.wa.edu.au/)</skos:scopeNote>
   </skos:Concept>
   <skos:Concept rdf:about="urn:marlin.csiro.au:sourceregister:concept:197">
      <skos:prefLabel xml:lang="en">Ship: Naturaliste</skos:prefLabel>
      <skos:inScheme rdf:resource="urn:marlin.csiro.au:sourceregister:conceptscheme:1.0"/>
      <skos:definition xml:lang="en">Type: Ship Description: Western Australian Department of Fisheries research vessel.</skos:definition>
      <skos:scopeNote xml:lang="en">Ship: Naturaliste: Type: Ship Description: Western Australian Department of Fisheries research vessel.</skos:scopeNote>
   </skos:Concept>
   <skos:Concept rdf:about="urn:marlin.csiro.au:sourceregister:concept:198">
      <skos:prefLabel xml:lang="en">Mooring: SRFME: Two-Rocks moorings (2004 - 2005)</skos:prefLabel>
      <skos:inScheme rdf:resource="urn:marlin.csiro.au:sourceregister:conceptscheme:1.0"/>
      <skos:definition xml:lang="en">Type: Mooring Description: None</skos:definition>
      <skos:scopeNote xml:lang="en">Mooring: SRFME: Two-Rocks moorings (2004 - 2005): Type: Mooring Description: None</skos:scopeNote>
   </skos:Concept>
   <skos:Concept rdf:about="urn:marlin.csiro.au:sourceregister:concept:203">
      <skos:prefLabel xml:lang="en">Locality: SRFME: Perth Dive Sites</skos:prefLabel>
      <skos:inScheme rdf:resource="urn:marlin.csiro.au:sourceregister:conceptscheme:1.0"/>
      <skos:definition xml:lang="en">Type: Locality Description: Dive Sites used for the Coastal Ecosystems and Biodiversity component of SRFME
</skos:definition>
      <skos:scopeNote xml:lang="en">Locality: SRFME: Perth Dive Sites: Type: Locality Description: Dive Sites used for the Coastal Ecosystems and Biodiversity component of SRFME
</skos:scopeNote>
   </skos:Concept>
   <skos:Concept rdf:about="urn:marlin.csiro.au:sourceregister:concept:204">
      <skos:prefLabel xml:lang="en">Locality: SRFME: Rottnest Island Dive Sites</skos:prefLabel>
      <skos:inScheme rdf:resource="urn:marlin.csiro.au:sourceregister:conceptscheme:1.0"/>
      <skos:definition xml:lang="en">Type: Locality Description: Dive Sites used for the Coastal Ecosystems and Biodiversity component of SRFME</skos:definition>
      <skos:scopeNote xml:lang="en">Locality: SRFME: Rottnest Island Dive Sites: Type: Locality Description: Dive Sites used for the Coastal Ecosystems and Biodiversity component of SRFME</skos:scopeNote>
   </skos:Concept>
   <skos:Concept rdf:about="urn:marlin.csiro.au:sourceregister:concept:76">
      <skos:prefLabel xml:lang="en">Ship: Estelle Star</skos:prefLabel>
      <skos:inScheme rdf:resource="urn:marlin.csiro.au:sourceregister:conceptscheme:1.0"/>
      <skos:definition xml:lang="en">Type: Ship Description: FV Estelle Star.&lt;BR&gt;
85 ft long; chartered for tuna research off Albany from August 1961 or July 1962. Owned and skippered by Ken Lidwell.&lt;BR&gt;
Vivienne Mawson, David J. Tranter and Alan F. Pearce (1988). &lt;I&gt;CSIRO at sea : fifty years of marine science&lt;/I&gt;, (pp. 206)&lt;BR&gt;CSIRO Marine Laboratories.
&lt;BR&gt;
Chartered for tuna research in Western Australian waters. Began charter in Port Lincoln, 31 July 1961 (survey started 1 August 1961).&lt;br&gt;
Hynd, J. S. and Vaux, D. (1963). Report of a survey for tuna in Western Australian waters. Report. Division of Fisheries and Oceanography. CSIRO Australia, no. 37.</skos:definition>
      <skos:scopeNote xml:lang="en">Ship: Estelle Star: Type: Ship Description: FV Estelle Star.&lt;BR&gt;
85 ft long; chartered for tuna research off Albany from August 1961 or July 1962. Owned and skippered by Ken Lidwell.&lt;BR&gt;
Vivienne Mawson, David J. Tranter and Alan F. Pearce (1988). &lt;I&gt;CSIRO at sea : fifty years of marine science&lt;/I&gt;, (pp. 206)&lt;BR&gt;CSIRO Marine Laboratories.
&lt;BR&gt;
Chartered for tuna research in Western Australian waters. Began charter in Port Lincoln, 31 July 1961 (survey started 1 August 1961).&lt;br&gt;
Hynd, J. S. and Vaux, D. (1963). Report of a survey for tuna in Western Australian waters. Report. Division of Fisheries and Oceanography. CSIRO Australia, no. 37.</skos:scopeNote>
   </skos:Concept>
   <skos:Concept rdf:about="urn:marlin.csiro.au:sourceregister:concept:208">
      <skos:prefLabel xml:lang="en">Ship: Roslind Star</skos:prefLabel>
      <skos:inScheme rdf:resource="urn:marlin.csiro.au:sourceregister:conceptscheme:1.0"/>
      <skos:definition xml:lang="en">Type: Ship Description: None</skos:definition>
      <skos:scopeNote xml:lang="en">Ship: Roslind Star: Type: Ship Description: None</skos:scopeNote>
   </skos:Concept>
   <skos:Concept rdf:about="urn:marlin.csiro.au:sourceregister:concept:209">
      <skos:prefLabel xml:lang="en">Ship: Two Freddies</skos:prefLabel>
      <skos:inScheme rdf:resource="urn:marlin.csiro.au:sourceregister:conceptscheme:1.0"/>
      <skos:definition xml:lang="en">Type: Ship Description: Chartered vessel for Tasmanian tuna survey.
</skos:definition>
      <skos:scopeNote xml:lang="en">Ship: Two Freddies: Type: Ship Description: Chartered vessel for Tasmanian tuna survey.
</skos:scopeNote>
   </skos:Concept>
   <skos:Concept rdf:about="urn:marlin.csiro.au:sourceregister:concept:210">
      <skos:prefLabel xml:lang="en">Ship: Rosebud</skos:prefLabel>
      <skos:inScheme rdf:resource="urn:marlin.csiro.au:sourceregister:conceptscheme:1.0"/>
      <skos:definition xml:lang="en">Type: Ship Description: Chartered vessel for Tasmanian tuna survey</skos:definition>
      <skos:scopeNote xml:lang="en">Ship: Rosebud: Type: Ship Description: Chartered vessel for Tasmanian tuna survey</skos:scopeNote>
   </skos:Concept>
   <skos:Concept rdf:about="urn:marlin.csiro.au:sourceregister:concept:212">
      <skos:prefLabel xml:lang="en">Ship: Catriona B</skos:prefLabel>
      <skos:inScheme rdf:resource="urn:marlin.csiro.au:sourceregister:conceptscheme:1.0"/>
      <skos:definition xml:lang="en">Type: Ship Description: Chartered fishing vessel for tuna tagging.</skos:definition>
      <skos:scopeNote xml:lang="en">Ship: Catriona B: Type: Ship Description: Chartered fishing vessel for tuna tagging.</skos:scopeNote>
   </skos:Concept>
   <skos:Concept rdf:about="urn:marlin.csiro.au:sourceregister:concept:215">
      <skos:prefLabel xml:lang="en">Model: CSIRO Global Climate model Mk3.5</skos:prefLabel>
      <skos:inScheme rdf:resource="urn:marlin.csiro.au:sourceregister:conceptscheme:1.0"/>
      <skos:definition xml:lang="en">Type: Model Description: The CSIRO Mk 3.5 Climate System Model (2007) is a global coupled model representing atmosphere, land surface, oceans and sea ice. It is a development from the Mk 1, Mk 2 and Mk 3.0 models and is current as at 2008.</skos:definition>
      <skos:scopeNote xml:lang="en">Model: CSIRO Global Climate model Mk3.5: Type: Model Description: The CSIRO Mk 3.5 Climate System Model (2007) is a global coupled model representing atmosphere, land surface, oceans and sea ice. It is a development from the Mk 1, Mk 2 and Mk 3.0 models and is current as at 2008.</skos:scopeNote>
   </skos:Concept>
   <skos:Concept rdf:about="urn:marlin.csiro.au:sourceregister:concept:202">
      <skos:prefLabel xml:lang="en">Locality: SRFME: Jurien Bay Dive Sites</skos:prefLabel>
      <skos:inScheme rdf:resource="urn:marlin.csiro.au:sourceregister:conceptscheme:1.0"/>
      <skos:definition xml:lang="en">Type: Locality Description: Dive Sites used for the Coastal Ecosystems and Biodiversity component of SRFME
</skos:definition>
      <skos:scopeNote xml:lang="en">Locality: SRFME: Jurien Bay Dive Sites: Type: Locality Description: Dive Sites used for the Coastal Ecosystems and Biodiversity component of SRFME
</skos:scopeNote>
   </skos:Concept>
   <skos:Concept rdf:about="urn:marlin.csiro.au:sourceregister:concept:199">
      <skos:prefLabel xml:lang="en">Locality: SRFME: Geographe Bay Dive Sites</skos:prefLabel>
      <skos:inScheme rdf:resource="urn:marlin.csiro.au:sourceregister:conceptscheme:1.0"/>
      <skos:definition xml:lang="en">Type: Locality Description: Dive Sites used for the Coastal Ecosystems and Biodiversity component of SRFME</skos:definition>
      <skos:scopeNote xml:lang="en">Locality: SRFME: Geographe Bay Dive Sites: Type: Locality Description: Dive Sites used for the Coastal Ecosystems and Biodiversity component of SRFME</skos:scopeNote>
   </skos:Concept>
   <skos:Concept rdf:about="urn:marlin.csiro.au:sourceregister:concept:205">
      <skos:prefLabel xml:lang="en">Locality: SRFME: Capes Dive Sites</skos:prefLabel>
      <skos:inScheme rdf:resource="urn:marlin.csiro.au:sourceregister:conceptscheme:1.0"/>
      <skos:definition xml:lang="en">Type: Locality Description: Dive Sites used for the Coastal Ecosystems and Biodiversity component of SRFME</skos:definition>
      <skos:scopeNote xml:lang="en">Locality: SRFME: Capes Dive Sites: Type: Locality Description: Dive Sites used for the Coastal Ecosystems and Biodiversity component of SRFME</skos:scopeNote>
   </skos:Concept>
   <skos:Concept rdf:about="urn:marlin.csiro.au:sourceregister:concept:8">
      <skos:prefLabel xml:lang="en">Ship: Southern Surveyor</skos:prefLabel>
      <skos:inScheme rdf:resource="urn:marlin.csiro.au:sourceregister:conceptscheme:1.0"/>
      <skos:definition xml:lang="en">Type: Ship Description: 66 m stern trawler built in 1972. Purchased by CSIRO in 1988 and extensively refitted for fisheries research. Refitted again in 2002 - 2003 to be operated by CSIRO on behalf of the nation as a National Facility. It operated as the Marine National Facility between 2003 and 2014. Length Overall: 66.1 m, between perpendiculars 61.4 m Beam: 12.3 m Draft: 5.3 m Lloyds Classification: 100A1 LMC UMS Gross tonnage: 1594 t Australian Register of Shipping Official Number: 851249</skos:definition>
      <skos:scopeNote xml:lang="en">Ship: Southern Surveyor: Type: Ship Description: 66 m stern trawler built in 1972. Purchased by CSIRO in 1988 and extensively refitted for fisheries research. Refitted again in 2002 - 2003 to be operated by CSIRO on behalf of the nation as a National Facility. It operated as the Marine National Facility between 2003 and 2014. Length Overall: 66.1 m, between perpendiculars 61.4 m Beam: 12.3 m Draft: 5.3 m Lloyds Classification: 100A1 LMC UMS Gross tonnage: 1594 t Australian Register of Shipping Official Number: 851249</skos:scopeNote>
   </skos:Concept>
   <skos:Concept rdf:about="urn:marlin.csiro.au:sourceregister:concept:207">
      <skos:prefLabel xml:lang="en">Ship: Fukushima Maru</skos:prefLabel>
      <skos:inScheme rdf:resource="urn:marlin.csiro.au:sourceregister:conceptscheme:1.0"/>
      <skos:definition xml:lang="en">Type: Ship Description: None</skos:definition>
      <skos:scopeNote xml:lang="en">Ship: Fukushima Maru: Type: Ship Description: None</skos:scopeNote>
   </skos:Concept>
   <skos:Concept rdf:about="urn:marlin.csiro.au:sourceregister:concept:211">
      <skos:prefLabel xml:lang="en">Ship: Suruga Maru</skos:prefLabel>
      <skos:inScheme rdf:resource="urn:marlin.csiro.au:sourceregister:conceptscheme:1.0"/>
      <skos:definition xml:lang="en">Type: Ship Description: Fishing vessel under charter to the Japanese Fisheries Agency for exploratory fishing operations off the Australian coast. Accommodation provided for CSIRO and other observers.</skos:definition>
      <skos:scopeNote xml:lang="en">Ship: Suruga Maru: Type: Ship Description: Fishing vessel under charter to the Japanese Fisheries Agency for exploratory fishing operations off the Australian coast. Accommodation provided for CSIRO and other observers.</skos:scopeNote>
   </skos:Concept>
   <skos:Concept rdf:about="urn:marlin.csiro.au:sourceregister:concept:213">
      <skos:prefLabel xml:lang="en">Ship: Gondwana</skos:prefLabel>
      <skos:inScheme rdf:resource="urn:marlin.csiro.au:sourceregister:conceptscheme:1.0"/>
      <skos:definition xml:lang="en">Type: Ship Description: Charter vessel</skos:definition>
      <skos:scopeNote xml:lang="en">Ship: Gondwana: Type: Ship Description: Charter vessel</skos:scopeNote>
   </skos:Concept>
   <skos:Concept rdf:about="urn:marlin.csiro.au:sourceregister:concept:214">
      <skos:prefLabel xml:lang="en">Model: CSIRO Global Climate model Mk3.0</skos:prefLabel>
      <skos:inScheme rdf:resource="urn:marlin.csiro.au:sourceregister:conceptscheme:1.0"/>
      <skos:definition xml:lang="en">Type: Model Description: The CSIRO Mk 3.0 Climate System Model (2002) is a global coupled model representing atmosphere, land surface, oceans and sea ice. It is a development from the Mk 1 and Mk 2 models and preceeds the CSIRO Mk 3.5 model, current as at 2008.</skos:definition>
      <skos:scopeNote xml:lang="en">Model: CSIRO Global Climate model Mk3.0: Type: Model Description: The CSIRO Mk 3.0 Climate System Model (2002) is a global coupled model representing atmosphere, land surface, oceans and sea ice. It is a development from the Mk 1 and Mk 2 models and preceeds the CSIRO Mk 3.5 model, current as at 2008.</skos:scopeNote>
   </skos:Concept>
   <skos:Concept rdf:about="urn:marlin.csiro.au:sourceregister:concept:191">
      <skos:prefLabel xml:lang="en">Ship: Tangaroa</skos:prefLabel>
      <skos:inScheme rdf:resource="urn:marlin.csiro.au:sourceregister:conceptscheme:1.0"/>
      <skos:definition xml:lang="en">Type: Ship Description: Research Vessel of NIWA, New Zealand</skos:definition>
      <skos:scopeNote xml:lang="en">Ship: Tangaroa: Type: Ship Description: Research Vessel of NIWA, New Zealand</skos:scopeNote>
   </skos:Concept>
   <skos:Concept rdf:about="urn:marlin.csiro.au:sourceregister:concept:193">
      <skos:prefLabel xml:lang="en">Coastal Station: Marmion Reef</skos:prefLabel>
      <skos:inScheme rdf:resource="urn:marlin.csiro.au:sourceregister:conceptscheme:1.0"/>
      <skos:definition xml:lang="en">Type: Coastal Station Description: A group of 22 stations over Marmion Reef WA</skos:definition>
      <skos:scopeNote xml:lang="en">Coastal Station: Marmion Reef: Type: Coastal Station Description: A group of 22 stations over Marmion Reef WA</skos:scopeNote>
   </skos:Concept>
   <skos:Concept rdf:about="urn:marlin.csiro.au:sourceregister:concept:189">
      <skos:prefLabel xml:lang="en">Ship: Raptis Pearl</skos:prefLabel>
      <skos:inScheme rdf:resource="urn:marlin.csiro.au:sourceregister:conceptscheme:1.0"/>
      <skos:definition xml:lang="en">Type: Ship Description: Fishing Vessel</skos:definition>
      <skos:scopeNote xml:lang="en">Ship: Raptis Pearl: Type: Ship Description: Fishing Vessel</skos:scopeNote>
   </skos:Concept>
   <skos:Concept rdf:about="urn:marlin.csiro.au:sourceregister:concept:194">
      <skos:prefLabel xml:lang="en">Ship: Challenger</skos:prefLabel>
      <skos:inScheme rdf:resource="urn:marlin.csiro.au:sourceregister:conceptscheme:1.0"/>
      <skos:definition xml:lang="en">Type: Ship Description: None</skos:definition>
      <skos:scopeNote xml:lang="en">Ship: Challenger: Type: Ship Description: None</skos:scopeNote>
   </skos:Concept>
   <skos:Concept rdf:about="urn:marlin.csiro.au:sourceregister:concept:184">
      <skos:prefLabel xml:lang="en">Ship: Rama</skos:prefLabel>
      <skos:inScheme rdf:resource="urn:marlin.csiro.au:sourceregister:conceptscheme:1.0"/>
      <skos:definition xml:lang="en">Type: Ship Description: 14.6m Prawn Trawler chartered for Gulf of Carpentaria prawn surveys (July 1963 - July 1965)</skos:definition>
      <skos:scopeNote xml:lang="en">Ship: Rama: Type: Ship Description: 14.6m Prawn Trawler chartered for Gulf of Carpentaria prawn surveys (July 1963 - July 1965)</skos:scopeNote>
   </skos:Concept>
   <skos:Concept rdf:about="urn:marlin.csiro.au:sourceregister:concept:185">
      <skos:prefLabel xml:lang="en">Ship: Maxim</skos:prefLabel>
      <skos:inScheme rdf:resource="urn:marlin.csiro.au:sourceregister:conceptscheme:1.0"/>
      <skos:definition xml:lang="en">Type: Ship Description: Chartered commercial prawn trawler.
Hull material: Steel 
Length: 19.5 metres     
Built: 1976
Engine: 298kw
Transit speed 9.47 knots	
Maxim fished commercially in the Northern Prawn Fishery from 1985 to 1992.</skos:definition>
      <skos:scopeNote xml:lang="en">Ship: Maxim: Type: Ship Description: Chartered commercial prawn trawler.
Hull material: Steel 
Length: 19.5 metres     
Built: 1976
Engine: 298kw
Transit speed 9.47 knots	
Maxim fished commercially in the Northern Prawn Fishery from 1985 to 1992.</skos:scopeNote>
   </skos:Concept>
   <skos:Concept rdf:about="urn:marlin.csiro.au:sourceregister:concept:187">
      <skos:prefLabel xml:lang="en">Ship: Judy B</skos:prefLabel>
      <skos:inScheme rdf:resource="urn:marlin.csiro.au:sourceregister:conceptscheme:1.0"/>
      <skos:definition xml:lang="en">Type: Ship Description: Chartered commercial prawn trawler.
Vessel name: Judy B 
Vessel Code: JB (sometimes TP)
Hull material: timber             
Length:   19.9m
Built: 1970
Engine: 205kw	
Transit speed 9.1 knots	
Judy B fished commercially in the NPF from 1975-79 and 1982-86.</skos:definition>
      <skos:scopeNote xml:lang="en">Ship: Judy B: Type: Ship Description: Chartered commercial prawn trawler.
Vessel name: Judy B 
Vessel Code: JB (sometimes TP)
Hull material: timber             
Length:   19.9m
Built: 1970
Engine: 205kw	
Transit speed 9.1 knots	
Judy B fished commercially in the NPF from 1975-79 and 1982-86.</skos:scopeNote>
   </skos:Concept>
   <skos:Concept rdf:about="urn:marlin.csiro.au:sourceregister:concept:1">
      <skos:prefLabel xml:lang="en">Ship: Aurora Australis</skos:prefLabel>
      <skos:inScheme rdf:resource="urn:marlin.csiro.au:sourceregister:conceptscheme:1.0"/>
      <skos:definition xml:lang="en">Type: Ship Description: Research vessel of the Australian Antarctic Division.
&lt;br&gt;
RSV Aurora Australis was built in Newcastle in 1989, and sails under the Australian flag with an Australian crew. The vessel is 94.91 metres long, has a dead weight of 3893 tonnes, and is classed as an Ice Class 1A Super Icebreaker under Lloyd's Register of Shipping + 100 A1 + LMC UMS DP (CM): CASPR Class 2 Amidships, Class 3 fore and aft.
&lt;br&gt;
The vessel has accommodation for 24 crew and 109 expeditioners, and is owned and managed by P&amp;O Polar Australia Pty Ltd.
&lt;br&gt;
Further information about this vessel is available at the URL http://www.cms.udel.edu/ships/country/Australia/Aurora_Australis/</skos:definition>
      <skos:scopeNote xml:lang="en">Ship: Aurora Australis: Type: Ship Description: Research vessel of the Australian Antarctic Division.
&lt;br&gt;
RSV Aurora Australis was built in Newcastle in 1989, and sails under the Australian flag with an Australian crew. The vessel is 94.91 metres long, has a dead weight of 3893 tonnes, and is classed as an Ice Class 1A Super Icebreaker under Lloyd's Register of Shipping + 100 A1 + LMC UMS DP (CM): CASPR Class 2 Amidships, Class 3 fore and aft.
&lt;br&gt;
The vessel has accommodation for 24 crew and 109 expeditioners, and is owned and managed by P&amp;O Polar Australia Pty Ltd.
&lt;br&gt;
Further information about this vessel is available at the URL http://www.cms.udel.edu/ships/country/Australia/Aurora_Australis/</skos:scopeNote>
   </skos:Concept>
   <skos:Concept rdf:about="urn:marlin.csiro.au:sourceregister:concept:2">
      <skos:prefLabel xml:lang="en">Ship: Courageous</skos:prefLabel>
      <skos:inScheme rdf:resource="urn:marlin.csiro.au:sourceregister:conceptscheme:1.0"/>
      <skos:definition xml:lang="en">Type: Ship Description: 28m stern ramp trawler, chartered September 1975 to August 1979 for fisheries research. Completed 52 cruises for Division of Fisheries and Oceanography around Australia.
</skos:definition>
      <skos:scopeNote xml:lang="en">Ship: Courageous: Type: Ship Description: 28m stern ramp trawler, chartered September 1975 to August 1979 for fisheries research. Completed 52 cruises for Division of Fisheries and Oceanography around Australia.
</skos:scopeNote>
   </skos:Concept>
   <skos:Concept rdf:about="urn:marlin.csiro.au:sourceregister:concept:3">
      <skos:prefLabel xml:lang="en">Ship: Derwent Hunter</skos:prefLabel>
      <skos:inScheme rdf:resource="urn:marlin.csiro.au:sourceregister:conceptscheme:1.0"/>
      <skos:definition xml:lang="en">Type: Ship Description: 72 ft auxiliary schooner, built 1946. Initially chartered, then purchased in 1950 by CSIRO for fisheries and oceanographic work; sold in 1962.&lt;br&gt;
(Powered by a 68 hp Gardner diesel with two Kelvin Hughes echosounders, a type 24D and a Type 24E - taken from Division of Fisheries and Oceanography report 27).&lt;br&gt;
Principal operations:&lt;br&gt;
- 1950-1955: shark tagging and droplining for deep-sea trevalla, chiefly off Tasmania&lt;br&gt;
- 1956-59: Oceanographic studies in Coral Sea, plus plankton and hydrographic studies in the Tasman Sea&lt;br&gt;
- 1959-1962: Tuna longlining off NSW, Victoria and Tasmania.</skos:definition>
      <skos:scopeNote xml:lang="en">Ship: Derwent Hunter: Type: Ship Description: 72 ft auxiliary schooner, built 1946. Initially chartered, then purchased in 1950 by CSIRO for fisheries and oceanographic work; sold in 1962.&lt;br&gt;
(Powered by a 68 hp Gardner diesel with two Kelvin Hughes echosounders, a type 24D and a Type 24E - taken from Division of Fisheries and Oceanography report 27).&lt;br&gt;
Principal operations:&lt;br&gt;
- 1950-1955: shark tagging and droplining for deep-sea trevalla, chiefly off Tasmania&lt;br&gt;
- 1956-59: Oceanographic studies in Coral Sea, plus plankton and hydrographic studies in the Tasman Sea&lt;br&gt;
- 1959-1962: Tuna longlining off NSW, Victoria and Tasmania.</skos:scopeNote>
   </skos:Concept>
   <skos:Concept rdf:about="urn:marlin.csiro.au:sourceregister:concept:4">
      <skos:prefLabel xml:lang="en">Ship: Diamantina</skos:prefLabel>
      <skos:inScheme rdf:resource="urn:marlin.csiro.au:sourceregister:conceptscheme:1.0"/>
      <skos:definition xml:lang="en">Type: Ship Description: 300 ft RAN frigate, loaned to CSIRO for oceanographic work from 1959 to late 1970s(?). Most of its early work was undertaken in the Indian Ocean.

</skos:definition>
      <skos:scopeNote xml:lang="en">Ship: Diamantina: Type: Ship Description: 300 ft RAN frigate, loaned to CSIRO for oceanographic work from 1959 to late 1970s(?). Most of its early work was undertaken in the Indian Ocean.

</skos:scopeNote>
   </skos:Concept>
   <skos:Concept rdf:about="urn:marlin.csiro.au:sourceregister:concept:5">
      <skos:prefLabel xml:lang="en">Ship: Franklin</skos:prefLabel>
      <skos:inScheme rdf:resource="urn:marlin.csiro.au:sourceregister:conceptscheme:1.0"/>
      <skos:definition xml:lang="en">Type: Ship Description: Purpose built oceanographic research vessel, commissioned by CSIRO Division of Oceanography in 1985. Operated by CSIRO on behalf of the nation as the Marine National Facility until 2002. Overall length: 55.2m Breadth moulded: 11.8m Draft: 3.8m Engine output: 1598 kW Bow-thruster: 5 t thrust Stern-thruster: 4.5 t thrust Displacement: 1187 t Design speed: 13 knots.</skos:definition>
      <skos:scopeNote xml:lang="en">Ship: Franklin: Type: Ship Description: Purpose built oceanographic research vessel, commissioned by CSIRO Division of Oceanography in 1985. Operated by CSIRO on behalf of the nation as the Marine National Facility until 2002. Overall length: 55.2m Breadth moulded: 11.8m Draft: 3.8m Engine output: 1598 kW Bow-thruster: 5 t thrust Stern-thruster: 4.5 t thrust Displacement: 1187 t Design speed: 13 knots.</skos:scopeNote>
   </skos:Concept>
   <skos:Concept rdf:about="urn:marlin.csiro.au:sourceregister:concept:6">
      <skos:prefLabel xml:lang="en">Ship: Kimbla</skos:prefLabel>
      <skos:inScheme rdf:resource="urn:marlin.csiro.au:sourceregister:conceptscheme:1.0"/>
      <skos:definition xml:lang="en">Type: Ship Description: RAN hydrographic ship, loaned to CSIRO at intervals, 1959 then 1966-1973 for oceanographic work, mostly on the Australian east coast.</skos:definition>
      <skos:scopeNote xml:lang="en">Ship: Kimbla: Type: Ship Description: RAN hydrographic ship, loaned to CSIRO at intervals, 1959 then 1966-1973 for oceanographic work, mostly on the Australian east coast.</skos:scopeNote>
   </skos:Concept>
   <skos:Concept rdf:about="urn:marlin.csiro.au:sourceregister:concept:7">
      <skos:prefLabel xml:lang="en">Ship: Soela</skos:prefLabel>
      <skos:inScheme rdf:resource="urn:marlin.csiro.au:sourceregister:conceptscheme:1.0"/>
      <skos:definition xml:lang="en">Type: Ship Description: 53 m deep-sea trawler, chartered by CSIRO 1979-1989 for fisheries research. 

Further information about this vessel is available at the URL http://www.cms.udel.edu/ships/country/Australia/soela.html


</skos:definition>
      <skos:scopeNote xml:lang="en">Ship: Soela: Type: Ship Description: 53 m deep-sea trawler, chartered by CSIRO 1979-1989 for fisheries research. 

Further information about this vessel is available at the URL http://www.cms.udel.edu/ships/country/Australia/soela.html


</skos:scopeNote>
   </skos:Concept>
   <skos:Concept rdf:about="urn:marlin.csiro.au:sourceregister:concept:9">
      <skos:prefLabel xml:lang="en">Ship: Sprightly</skos:prefLabel>
      <skos:inScheme rdf:resource="urn:marlin.csiro.au:sourceregister:conceptscheme:1.0"/>
      <skos:definition xml:lang="en">Type: Ship Description: 43.5 m oceanographic research vessel, chartered by CSIRO 1973-1983. Principal activities:
   1973-1976: western rock lobster studies off Western Australia
   1977-1983: oceanographic work, Gulf of Carpentaria and Australian east coast.
Hull material:  steel</skos:definition>
      <skos:scopeNote xml:lang="en">Ship: Sprightly: Type: Ship Description: 43.5 m oceanographic research vessel, chartered by CSIRO 1973-1983. Principal activities:
   1973-1976: western rock lobster studies off Western Australia
   1977-1983: oceanographic work, Gulf of Carpentaria and Australian east coast.
Hull material:  steel</skos:scopeNote>
   </skos:Concept>
   <skos:Concept rdf:about="urn:marlin.csiro.au:sourceregister:concept:10">
      <skos:prefLabel xml:lang="en">Ship: Stanley Fowler</skos:prefLabel>
      <skos:inScheme rdf:resource="urn:marlin.csiro.au:sourceregister:conceptscheme:1.0"/>
      <skos:definition xml:lang="en">Type: Ship Description: 65 ft motor vessel, loaned by RAN to CSIRO, 1948-1951 for fisheries and hydrological surveys.</skos:definition>
      <skos:scopeNote xml:lang="en">Ship: Stanley Fowler: Type: Ship Description: 65 ft motor vessel, loaned by RAN to CSIRO, 1948-1951 for fisheries and hydrological surveys.</skos:scopeNote>
   </skos:Concept>
   <skos:Concept rdf:about="urn:marlin.csiro.au:sourceregister:concept:11">
      <skos:prefLabel xml:lang="en">Ship: Warreen</skos:prefLabel>
      <skos:inScheme rdf:resource="urn:marlin.csiro.au:sourceregister:conceptscheme:1.0"/>
      <skos:definition xml:lang="en">Type: Ship Description: 82 ft purse-seine motor vessel, commissioned by CSIRO in 1938. The Division's first research vessel, in use 1938-1942 and 1947-1951. Used for exploratory fishing, plankton and hydrological investigations. Decommissioned 1951.</skos:definition>
      <skos:scopeNote xml:lang="en">Ship: Warreen: Type: Ship Description: 82 ft purse-seine motor vessel, commissioned by CSIRO in 1938. The Division's first research vessel, in use 1938-1942 and 1947-1951. Used for exploratory fishing, plankton and hydrological investigations. Decommissioned 1951.</skos:scopeNote>
   </skos:Concept>
   <skos:Concept rdf:about="urn:marlin.csiro.au:sourceregister:concept:12">
      <skos:prefLabel xml:lang="en">Ship: Gascoyne</skos:prefLabel>
      <skos:inScheme rdf:resource="urn:marlin.csiro.au:sourceregister:conceptscheme:1.0"/>
      <skos:definition xml:lang="en">Type: Ship Description: 300 ft RAN frigate, loaned to CSIRO for oceanographic work, 1960-1965.</skos:definition>
      <skos:scopeNote xml:lang="en">Ship: Gascoyne: Type: Ship Description: 300 ft RAN frigate, loaned to CSIRO for oceanographic work, 1960-1965.</skos:scopeNote>
   </skos:Concept>
   <skos:Concept rdf:about="urn:marlin.csiro.au:sourceregister:concept:13">
      <skos:prefLabel xml:lang="en">Ship: Liawenee</skos:prefLabel>
      <skos:inScheme rdf:resource="urn:marlin.csiro.au:sourceregister:conceptscheme:1.0"/>
      <skos:definition xml:lang="en">Type: Ship Description: 75 ft motor vessel, chartered by CSIRO from Tasmanian Government, 1946-1951 for fishing trials and hydrography in Tasmanian waters.</skos:definition>
      <skos:scopeNote xml:lang="en">Ship: Liawenee: Type: Ship Description: 75 ft motor vessel, chartered by CSIRO from Tasmanian Government, 1946-1951 for fishing trials and hydrography in Tasmanian waters.</skos:scopeNote>
   </skos:Concept>
   <skos:Concept rdf:about="urn:marlin.csiro.au:sourceregister:concept:14">
      <skos:prefLabel xml:lang="en">Ship: Gahleru</skos:prefLabel>
      <skos:inScheme rdf:resource="urn:marlin.csiro.au:sourceregister:conceptscheme:1.0"/>
      <skos:definition xml:lang="en">Type: Ship Description: 45 ft auxiliary wooden ketch, commisioned 1951 by CSIRO and used for pearl shell research in Thursday Island, 1951-1962.

</skos:definition>
      <skos:scopeNote xml:lang="en">Ship: Gahleru: Type: Ship Description: 45 ft auxiliary wooden ketch, commisioned 1951 by CSIRO and used for pearl shell research in Thursday Island, 1951-1962.

</skos:scopeNote>
   </skos:Concept>
   <skos:Concept rdf:about="urn:marlin.csiro.au:sourceregister:concept:16">
      <skos:prefLabel xml:lang="en">Ship: Magga Dan</skos:prefLabel>
      <skos:inScheme rdf:resource="urn:marlin.csiro.au:sourceregister:conceptscheme:1.0"/>
      <skos:definition xml:lang="en">Type: Ship Description: Research vessel chartered by the Antarctic Division (Department of Australian Affairs, Australia) around the period 1959-1961 (possibly longer?).


</skos:definition>
      <skos:scopeNote xml:lang="en">Ship: Magga Dan: Type: Ship Description: Research vessel chartered by the Antarctic Division (Department of Australian Affairs, Australia) around the period 1959-1961 (possibly longer?).


</skos:scopeNote>
   </skos:Concept>
   <skos:Concept rdf:about="urn:marlin.csiro.au:sourceregister:concept:17">
      <skos:prefLabel xml:lang="en">Ship: Pride of Eden</skos:prefLabel>
      <skos:inScheme rdf:resource="urn:marlin.csiro.au:sourceregister:conceptscheme:1.0"/>
      <skos:definition xml:lang="en">Type: Ship Description: Chartered fishing vessel 1989
L.O.A.: 53.64m
L.W.L.: 52.84m
Breadth Mid: 11.58m
Depth Mid: 4.27m
Draught: 6.65m
Deadweight: 700 Tonnes</skos:definition>
      <skos:scopeNote xml:lang="en">Ship: Pride of Eden: Type: Ship Description: Chartered fishing vessel 1989
L.O.A.: 53.64m
L.W.L.: 52.84m
Breadth Mid: 11.58m
Depth Mid: 4.27m
Draught: 6.65m
Deadweight: 700 Tonnes</skos:scopeNote>
   </skos:Concept>
   <skos:Concept rdf:about="urn:marlin.csiro.au:sourceregister:concept:18">
      <skos:prefLabel xml:lang="en">Ship: Rachel</skos:prefLabel>
      <skos:inScheme rdf:resource="urn:marlin.csiro.au:sourceregister:conceptscheme:1.0"/>
      <skos:definition xml:lang="en">Type: Ship Description: Chartered fishing vessel</skos:definition>
      <skos:scopeNote xml:lang="en">Ship: Rachel: Type: Ship Description: Chartered fishing vessel</skos:scopeNote>
   </skos:Concept>
   <skos:Concept rdf:about="urn:marlin.csiro.au:sourceregister:concept:19">
      <skos:prefLabel xml:lang="en">Ship: Marelda</skos:prefLabel>
      <skos:inScheme rdf:resource="urn:marlin.csiro.au:sourceregister:conceptscheme:1.0"/>
      <skos:definition xml:lang="en">Type: Ship Description: Fishery Research Vessel Marelda&lt;BR&gt;
Skippered by Ron Greig. 36 fr launch, built in 1946; used 1948-70 from Dunwich field station in Moreton Bay, then in Eden, Queensland, for esturaine fish, tuna, whale-marking and prawns.&lt;BR&gt;
Auxiliary wooden cutter; 48 Hp diesel.&lt;BR&gt;
Vivienne Mawson, David J. Tranter and Alan F. Pearce (1988). &lt;I&gt;CSIRO at sea : fifty years of marine science&lt;/I&gt;, (pp. 207)&lt;BR&gt;CSIRO Marine Laboratories.</skos:definition>
      <skos:scopeNote xml:lang="en">Ship: Marelda: Type: Ship Description: Fishery Research Vessel Marelda&lt;BR&gt;
Skippered by Ron Greig. 36 fr launch, built in 1946; used 1948-70 from Dunwich field station in Moreton Bay, then in Eden, Queensland, for esturaine fish, tuna, whale-marking and prawns.&lt;BR&gt;
Auxiliary wooden cutter; 48 Hp diesel.&lt;BR&gt;
Vivienne Mawson, David J. Tranter and Alan F. Pearce (1988). &lt;I&gt;CSIRO at sea : fifty years of marine science&lt;/I&gt;, (pp. 207)&lt;BR&gt;CSIRO Marine Laboratories.</skos:scopeNote>
   </skos:Concept>
   <skos:Concept rdf:about="urn:marlin.csiro.au:sourceregister:concept:20">
      <skos:prefLabel xml:lang="en">Ship: Flinders</skos:prefLabel>
      <skos:inScheme rdf:resource="urn:marlin.csiro.au:sourceregister:conceptscheme:1.0"/>
      <skos:definition xml:lang="en">Type: Ship Description: R.V. Flinders: 

Operated by the Department of Fisheries and Fauna (WA) as a mid-water trawler. Build at a cost of $148,000 was launched on November 10, 1967 at the Dillinham Shipyards at North Fremantle. Extensively re-fit in 1988 at a cost of $350,000.

Length:       20m, 
Displacement: 110 tonnes, 
Main engine:  Gardner 8L3B, 230 hp,  
Winches:      hydraulic Dunstan pot winch, hydraulic anchor windlass and hydraulic double ring trawl.
Navigation:   GPS, sonar, dual frequency echo sounder, auto-pilot, radar and VHF and MF/HF radio.

Replaced in 2001 by the new 22.7 metre research vessel R.V. Naturaliste.</skos:definition>
      <skos:scopeNote xml:lang="en">Ship: Flinders: Type: Ship Description: R.V. Flinders: 

Operated by the Department of Fisheries and Fauna (WA) as a mid-water trawler. Build at a cost of $148,000 was launched on November 10, 1967 at the Dillinham Shipyards at North Fremantle. Extensively re-fit in 1988 at a cost of $350,000.

Length:       20m, 
Displacement: 110 tonnes, 
Main engine:  Gardner 8L3B, 230 hp,  
Winches:      hydraulic Dunstan pot winch, hydraulic anchor windlass and hydraulic double ring trawl.
Navigation:   GPS, sonar, dual frequency echo sounder, auto-pilot, radar and VHF and MF/HF radio.

Replaced in 2001 by the new 22.7 metre research vessel R.V. Naturaliste.</skos:scopeNote>
   </skos:Concept>
   <skos:Concept rdf:about="urn:marlin.csiro.au:sourceregister:concept:21">
      <skos:prefLabel xml:lang="en">Coastal Station: Port Hacking 50m station</skos:prefLabel>
      <skos:inScheme rdf:resource="urn:marlin.csiro.au:sourceregister:conceptscheme:1.0"/>
      <skos:definition xml:lang="en">Type: Coastal Station Description: None</skos:definition>
      <skos:scopeNote xml:lang="en">Coastal Station: Port Hacking 50m station: Type: Coastal Station Description: None</skos:scopeNote>
   </skos:Concept>
   <skos:Concept rdf:about="urn:marlin.csiro.au:sourceregister:concept:22">
      <skos:prefLabel xml:lang="en">Ship: Lancelin</skos:prefLabel>
      <skos:inScheme rdf:resource="urn:marlin.csiro.au:sourceregister:conceptscheme:1.0"/>
      <skos:definition xml:lang="en">Type: Ship Description: Patrol vessel</skos:definition>
      <skos:scopeNote xml:lang="en">Ship: Lancelin: Type: Ship Description: Patrol vessel</skos:scopeNote>
   </skos:Concept>
   <skos:Concept rdf:about="urn:marlin.csiro.au:sourceregister:concept:23">
      <skos:prefLabel xml:lang="en">Ship: Islander VI</skos:prefLabel>
      <skos:inScheme rdf:resource="urn:marlin.csiro.au:sourceregister:conceptscheme:1.0"/>
      <skos:definition xml:lang="en">Type: Ship Description: Fishing vessel
</skos:definition>
      <skos:scopeNote xml:lang="en">Ship: Islander VI: Type: Ship Description: Fishing vessel
</skos:scopeNote>
   </skos:Concept>
   <skos:Concept rdf:about="urn:marlin.csiro.au:sourceregister:concept:24">
      <skos:prefLabel xml:lang="en">Ship: Megisti Star</skos:prefLabel>
      <skos:inScheme rdf:resource="urn:marlin.csiro.au:sourceregister:conceptscheme:1.0"/>
      <skos:definition xml:lang="en">Type: Ship Description: Fishing vessel
</skos:definition>
      <skos:scopeNote xml:lang="en">Ship: Megisti Star: Type: Ship Description: Fishing vessel
</skos:scopeNote>
   </skos:Concept>
   <skos:Concept rdf:about="urn:marlin.csiro.au:sourceregister:concept:25">
      <skos:prefLabel xml:lang="en">Ship: Petuna Endeavour</skos:prefLabel>
      <skos:inScheme rdf:resource="urn:marlin.csiro.au:sourceregister:conceptscheme:1.0"/>
      <skos:definition xml:lang="en">Type: Ship Description: Charter Fishing vessel</skos:definition>
      <skos:scopeNote xml:lang="en">Ship: Petuna Endeavour: Type: Ship Description: Charter Fishing vessel</skos:scopeNote>
   </skos:Concept>
   <skos:Concept rdf:about="urn:marlin.csiro.au:sourceregister:concept:26">
      <skos:prefLabel xml:lang="en">Ship: Tasmanian Enterprise</skos:prefLabel>
      <skos:inScheme rdf:resource="urn:marlin.csiro.au:sourceregister:conceptscheme:1.0"/>
      <skos:definition xml:lang="en">Type: Ship Description: Fishing Vessel
</skos:definition>
      <skos:scopeNote xml:lang="en">Ship: Tasmanian Enterprise: Type: Ship Description: Fishing Vessel
</skos:scopeNote>
   </skos:Concept>
   <skos:Concept rdf:about="urn:marlin.csiro.au:sourceregister:concept:27">
      <skos:prefLabel xml:lang="en">Locality: Albatross Bay</skos:prefLabel>
      <skos:inScheme rdf:resource="urn:marlin.csiro.au:sourceregister:conceptscheme:1.0"/>
      <skos:definition xml:lang="en">Type: Locality Description: Albatross Bay study area (NE Gulf of Carpentaria)
</skos:definition>
      <skos:scopeNote xml:lang="en">Locality: Albatross Bay: Type: Locality Description: Albatross Bay study area (NE Gulf of Carpentaria)
</skos:scopeNote>
   </skos:Concept>
   <skos:Concept rdf:about="urn:marlin.csiro.au:sourceregister:concept:28">
      <skos:prefLabel xml:lang="en">Ship: Te Tautai</skos:prefLabel>
      <skos:inScheme rdf:resource="urn:marlin.csiro.au:sourceregister:conceptscheme:1.0"/>
      <skos:definition xml:lang="en">Type: Ship Description: Note
This vessel was originally assigned code TT, and is referred to as such in the lone voyage plan we hold.
The code was changed to TeT in 2009 as the TT code was requested for another vesse.</skos:definition>
      <skos:scopeNote xml:lang="en">Ship: Te Tautai: Type: Ship Description: Note
This vessel was originally assigned code TT, and is referred to as such in the lone voyage plan we hold.
The code was changed to TeT in 2009 as the TT code was requested for another vesse.</skos:scopeNote>
   </skos:Concept>
   <skos:Concept rdf:about="urn:marlin.csiro.au:sourceregister:concept:29">
      <skos:prefLabel xml:lang="en">Coastal Station: Albany</skos:prefLabel>
      <skos:inScheme rdf:resource="urn:marlin.csiro.au:sourceregister:conceptscheme:1.0"/>
      <skos:definition xml:lang="en">Type: Coastal Station Description: None</skos:definition>
      <skos:scopeNote xml:lang="en">Coastal Station: Albany: Type: Coastal Station Description: None</skos:scopeNote>
   </skos:Concept>
   <skos:Concept rdf:about="urn:marlin.csiro.au:sourceregister:concept:30">
      <skos:prefLabel xml:lang="en">Coastal Station: Albatross Island</skos:prefLabel>
      <skos:inScheme rdf:resource="urn:marlin.csiro.au:sourceregister:conceptscheme:1.0"/>
      <skos:definition xml:lang="en">Type: Coastal Station Description: None</skos:definition>
      <skos:scopeNote xml:lang="en">Coastal Station: Albatross Island: Type: Coastal Station Description: None</skos:scopeNote>
   </skos:Concept>
   <skos:Concept rdf:about="urn:marlin.csiro.au:sourceregister:concept:31">
      <skos:prefLabel xml:lang="en">Coastal Station: Barrow Island</skos:prefLabel>
      <skos:inScheme rdf:resource="urn:marlin.csiro.au:sourceregister:conceptscheme:1.0"/>
      <skos:definition xml:lang="en">Type: Coastal Station Description: None</skos:definition>
      <skos:scopeNote xml:lang="en">Coastal Station: Barrow Island: Type: Coastal Station Description: None</skos:scopeNote>
   </skos:Concept>
   <skos:Concept rdf:about="urn:marlin.csiro.au:sourceregister:concept:32">
      <skos:prefLabel xml:lang="en">Coastal Station: Batemans Bay</skos:prefLabel>
      <skos:inScheme rdf:resource="urn:marlin.csiro.au:sourceregister:conceptscheme:1.0"/>
      <skos:definition xml:lang="en">Type: Coastal Station Description: None</skos:definition>
      <skos:scopeNote xml:lang="en">Coastal Station: Batemans Bay: Type: Coastal Station Description: None</skos:scopeNote>
   </skos:Concept>
   <skos:Concept rdf:about="urn:marlin.csiro.au:sourceregister:concept:33">
      <skos:prefLabel xml:lang="en">Coastal Station: Bermagui</skos:prefLabel>
      <skos:inScheme rdf:resource="urn:marlin.csiro.au:sourceregister:conceptscheme:1.0"/>
      <skos:definition xml:lang="en">Type: Coastal Station Description: None</skos:definition>
      <skos:scopeNote xml:lang="en">Coastal Station: Bermagui: Type: Coastal Station Description: None</skos:scopeNote>
   </skos:Concept>
   <skos:Concept rdf:about="urn:marlin.csiro.au:sourceregister:concept:34">
      <skos:prefLabel xml:lang="en">Coastal Station: Boobie Island</skos:prefLabel>
      <skos:inScheme rdf:resource="urn:marlin.csiro.au:sourceregister:conceptscheme:1.0"/>
      <skos:definition xml:lang="en">Type: Coastal Station Description: None</skos:definition>
      <skos:scopeNote xml:lang="en">Coastal Station: Boobie Island: Type: Coastal Station Description: None</skos:scopeNote>
   </skos:Concept>
   <skos:Concept rdf:about="urn:marlin.csiro.au:sourceregister:concept:35">
      <skos:prefLabel xml:lang="en">Coastal Station: Botany Bay</skos:prefLabel>
      <skos:inScheme rdf:resource="urn:marlin.csiro.au:sourceregister:conceptscheme:1.0"/>
      <skos:definition xml:lang="en">Type: Coastal Station Description: None</skos:definition>
      <skos:scopeNote xml:lang="en">Coastal Station: Botany Bay: Type: Coastal Station Description: None</skos:scopeNote>
   </skos:Concept>
   <skos:Concept rdf:about="urn:marlin.csiro.au:sourceregister:concept:36">
      <skos:prefLabel xml:lang="en">Coastal Station: Broulee Island</skos:prefLabel>
      <skos:inScheme rdf:resource="urn:marlin.csiro.au:sourceregister:conceptscheme:1.0"/>
      <skos:definition xml:lang="en">Type: Coastal Station Description: None</skos:definition>
      <skos:scopeNote xml:lang="en">Coastal Station: Broulee Island: Type: Coastal Station Description: None</skos:scopeNote>
   </skos:Concept>
   <skos:Concept rdf:about="urn:marlin.csiro.au:sourceregister:concept:37">
      <skos:prefLabel xml:lang="en">Coastal Station: Byron Bay</skos:prefLabel>
      <skos:inScheme rdf:resource="urn:marlin.csiro.au:sourceregister:conceptscheme:1.0"/>
      <skos:definition xml:lang="en">Type: Coastal Station Description: None</skos:definition>
      <skos:scopeNote xml:lang="en">Coastal Station: Byron Bay: Type: Coastal Station Description: None</skos:scopeNote>
   </skos:Concept>
   <skos:Concept rdf:about="urn:marlin.csiro.au:sourceregister:concept:38">
      <skos:prefLabel xml:lang="en">Coastal Station: Cliff Head</skos:prefLabel>
      <skos:inScheme rdf:resource="urn:marlin.csiro.au:sourceregister:conceptscheme:1.0"/>
      <skos:definition xml:lang="en">Type: Coastal Station Description: None</skos:definition>
      <skos:scopeNote xml:lang="en">Coastal Station: Cliff Head: Type: Coastal Station Description: None</skos:scopeNote>
   </skos:Concept>
   <skos:Concept rdf:about="urn:marlin.csiro.au:sourceregister:concept:39">
      <skos:prefLabel xml:lang="en">Coastal Station: Coffs Harbour</skos:prefLabel>
      <skos:inScheme rdf:resource="urn:marlin.csiro.au:sourceregister:conceptscheme:1.0"/>
      <skos:definition xml:lang="en">Type: Coastal Station Description: None</skos:definition>
      <skos:scopeNote xml:lang="en">Coastal Station: Coffs Harbour: Type: Coastal Station Description: None</skos:scopeNote>
   </skos:Concept>
   <skos:Concept rdf:about="urn:marlin.csiro.au:sourceregister:concept:40">
      <skos:prefLabel xml:lang="en">Coastal Station: Crowdy Head</skos:prefLabel>
      <skos:inScheme rdf:resource="urn:marlin.csiro.au:sourceregister:conceptscheme:1.0"/>
      <skos:definition xml:lang="en">Type: Coastal Station Description: None</skos:definition>
      <skos:scopeNote xml:lang="en">Coastal Station: Crowdy Head: Type: Coastal Station Description: None</skos:scopeNote>
   </skos:Concept>
   <skos:Concept rdf:about="urn:marlin.csiro.au:sourceregister:concept:41">
      <skos:prefLabel xml:lang="en">Coastal Station: Diamond Head</skos:prefLabel>
      <skos:inScheme rdf:resource="urn:marlin.csiro.au:sourceregister:conceptscheme:1.0"/>
      <skos:definition xml:lang="en">Type: Coastal Station Description: None</skos:definition>
      <skos:scopeNote xml:lang="en">Coastal Station: Diamond Head: Type: Coastal Station Description: None</skos:scopeNote>
   </skos:Concept>
   <skos:Concept rdf:about="urn:marlin.csiro.au:sourceregister:concept:42">
      <skos:prefLabel xml:lang="en">Coastal Station: Eden</skos:prefLabel>
      <skos:inScheme rdf:resource="urn:marlin.csiro.au:sourceregister:conceptscheme:1.0"/>
      <skos:definition xml:lang="en">Type: Coastal Station Description: None</skos:definition>
      <skos:scopeNote xml:lang="en">Coastal Station: Eden: Type: Coastal Station Description: None</skos:scopeNote>
   </skos:Concept>
   <skos:Concept rdf:about="urn:marlin.csiro.au:sourceregister:concept:43">
      <skos:prefLabel xml:lang="en">Coastal Station: Evans Head</skos:prefLabel>
      <skos:inScheme rdf:resource="urn:marlin.csiro.au:sourceregister:conceptscheme:1.0"/>
      <skos:definition xml:lang="en">Type: Coastal Station Description: None</skos:definition>
      <skos:scopeNote xml:lang="en">Coastal Station: Evans Head: Type: Coastal Station Description: None</skos:scopeNote>
   </skos:Concept>
   <skos:Concept rdf:about="urn:marlin.csiro.au:sourceregister:concept:44">
      <skos:prefLabel xml:lang="en">Coastal Station: Garden Island</skos:prefLabel>
      <skos:inScheme rdf:resource="urn:marlin.csiro.au:sourceregister:conceptscheme:1.0"/>
      <skos:definition xml:lang="en">Type: Coastal Station Description: None</skos:definition>
      <skos:scopeNote xml:lang="en">Coastal Station: Garden Island: Type: Coastal Station Description: None</skos:scopeNote>
   </skos:Concept>
   <skos:Concept rdf:about="urn:marlin.csiro.au:sourceregister:concept:45">
      <skos:prefLabel xml:lang="en">Coastal Station: Heron Island</skos:prefLabel>
      <skos:inScheme rdf:resource="urn:marlin.csiro.au:sourceregister:conceptscheme:1.0"/>
      <skos:definition xml:lang="en">Type: Coastal Station Description: None</skos:definition>
      <skos:scopeNote xml:lang="en">Coastal Station: Heron Island: Type: Coastal Station Description: None</skos:scopeNote>
   </skos:Concept>
   <skos:Concept rdf:about="urn:marlin.csiro.au:sourceregister:concept:46">
      <skos:prefLabel xml:lang="en">Coastal Station: Jervis Bay</skos:prefLabel>
      <skos:inScheme rdf:resource="urn:marlin.csiro.au:sourceregister:conceptscheme:1.0"/>
      <skos:definition xml:lang="en">Type: Coastal Station Description: None</skos:definition>
      <skos:scopeNote xml:lang="en">Coastal Station: Jervis Bay: Type: Coastal Station Description: None</skos:scopeNote>
   </skos:Concept>
   <skos:Concept rdf:about="urn:marlin.csiro.au:sourceregister:concept:47">
      <skos:prefLabel xml:lang="en">Coastal Station: Jurien Bay</skos:prefLabel>
      <skos:inScheme rdf:resource="urn:marlin.csiro.au:sourceregister:conceptscheme:1.0"/>
      <skos:definition xml:lang="en">Type: Coastal Station Description: None</skos:definition>
      <skos:scopeNote xml:lang="en">Coastal Station: Jurien Bay: Type: Coastal Station Description: None</skos:scopeNote>
   </skos:Concept>
   <skos:Concept rdf:about="urn:marlin.csiro.au:sourceregister:concept:48">
      <skos:prefLabel xml:lang="en">Coastal Station: Kiama</skos:prefLabel>
      <skos:inScheme rdf:resource="urn:marlin.csiro.au:sourceregister:conceptscheme:1.0"/>
      <skos:definition xml:lang="en">Type: Coastal Station Description: None</skos:definition>
      <skos:scopeNote xml:lang="en">Coastal Station: Kiama: Type: Coastal Station Description: None</skos:scopeNote>
   </skos:Concept>
   <skos:Concept rdf:about="urn:marlin.csiro.au:sourceregister:concept:49">
      <skos:prefLabel xml:lang="en">Coastal Station: Laurieton</skos:prefLabel>
      <skos:inScheme rdf:resource="urn:marlin.csiro.au:sourceregister:conceptscheme:1.0"/>
      <skos:definition xml:lang="en">Type: Coastal Station Description: None</skos:definition>
      <skos:scopeNote xml:lang="en">Coastal Station: Laurieton: Type: Coastal Station Description: None</skos:scopeNote>
   </skos:Concept>
   <skos:Concept rdf:about="urn:marlin.csiro.au:sourceregister:concept:50">
      <skos:prefLabel xml:lang="en">Coastal Station: Lennox Head</skos:prefLabel>
      <skos:inScheme rdf:resource="urn:marlin.csiro.au:sourceregister:conceptscheme:1.0"/>
      <skos:definition xml:lang="en">Type: Coastal Station Description: None</skos:definition>
      <skos:scopeNote xml:lang="en">Coastal Station: Lennox Head: Type: Coastal Station Description: None</skos:scopeNote>
   </skos:Concept>
   <skos:Concept rdf:about="urn:marlin.csiro.au:sourceregister:concept:51">
      <skos:prefLabel xml:lang="en">Coastal Station: Lizard Island</skos:prefLabel>
      <skos:inScheme rdf:resource="urn:marlin.csiro.au:sourceregister:conceptscheme:1.0"/>
      <skos:definition xml:lang="en">Type: Coastal Station Description: None</skos:definition>
      <skos:scopeNote xml:lang="en">Coastal Station: Lizard Island: Type: Coastal Station Description: None</skos:scopeNote>
   </skos:Concept>
   <skos:Concept rdf:about="urn:marlin.csiro.au:sourceregister:concept:52">
      <skos:prefLabel xml:lang="en">Coastal Station: Lord Howe Island</skos:prefLabel>
      <skos:inScheme rdf:resource="urn:marlin.csiro.au:sourceregister:conceptscheme:1.0"/>
      <skos:definition xml:lang="en">Type: Coastal Station Description: None</skos:definition>
      <skos:scopeNote xml:lang="en">Coastal Station: Lord Howe Island: Type: Coastal Station Description: None</skos:scopeNote>
   </skos:Concept>
   <skos:Concept rdf:about="urn:marlin.csiro.au:sourceregister:concept:53">
      <skos:prefLabel xml:lang="en">Coastal Station: Low Head</skos:prefLabel>
      <skos:inScheme rdf:resource="urn:marlin.csiro.au:sourceregister:conceptscheme:1.0"/>
      <skos:definition xml:lang="en">Type: Coastal Station Description: None</skos:definition>
      <skos:scopeNote xml:lang="en">Coastal Station: Low Head: Type: Coastal Station Description: None</skos:scopeNote>
   </skos:Concept>
   <skos:Concept rdf:about="urn:marlin.csiro.au:sourceregister:concept:54">
      <skos:prefLabel xml:lang="en">Coastal Station: Low Isles</skos:prefLabel>
      <skos:inScheme rdf:resource="urn:marlin.csiro.au:sourceregister:conceptscheme:1.0"/>
      <skos:definition xml:lang="en">Type: Coastal Station Description: None</skos:definition>
      <skos:scopeNote xml:lang="en">Coastal Station: Low Isles: Type: Coastal Station Description: None</skos:scopeNote>
   </skos:Concept>
   <skos:Concept rdf:about="urn:marlin.csiro.au:sourceregister:concept:55">
      <skos:prefLabel xml:lang="en">Coastal Station: Maria Island</skos:prefLabel>
      <skos:inScheme rdf:resource="urn:marlin.csiro.au:sourceregister:conceptscheme:1.0"/>
      <skos:definition xml:lang="en">Type: Coastal Station Description: None</skos:definition>
      <skos:scopeNote xml:lang="en">Coastal Station: Maria Island: Type: Coastal Station Description: None</skos:scopeNote>
   </skos:Concept>
   <skos:Concept rdf:about="urn:marlin.csiro.au:sourceregister:concept:56">
      <skos:prefLabel xml:lang="en">Coastal Station: Moreton Bay</skos:prefLabel>
      <skos:inScheme rdf:resource="urn:marlin.csiro.au:sourceregister:conceptscheme:1.0"/>
      <skos:definition xml:lang="en">Type: Coastal Station Description: None</skos:definition>
      <skos:scopeNote xml:lang="en">Coastal Station: Moreton Bay: Type: Coastal Station Description: None</skos:scopeNote>
   </skos:Concept>
   <skos:Concept rdf:about="urn:marlin.csiro.au:sourceregister:concept:57">
      <skos:prefLabel xml:lang="en">Coastal Station: Norfolk Island</skos:prefLabel>
      <skos:inScheme rdf:resource="urn:marlin.csiro.au:sourceregister:conceptscheme:1.0"/>
      <skos:definition xml:lang="en">Type: Coastal Station Description: None</skos:definition>
      <skos:scopeNote xml:lang="en">Coastal Station: Norfolk Island: Type: Coastal Station Description: None</skos:scopeNote>
   </skos:Concept>
   <skos:Concept rdf:about="urn:marlin.csiro.au:sourceregister:concept:58">
      <skos:prefLabel xml:lang="en">Coastal Station: Port Hacking 100m station</skos:prefLabel>
      <skos:inScheme rdf:resource="urn:marlin.csiro.au:sourceregister:conceptscheme:1.0"/>
      <skos:definition xml:lang="en">Type: Coastal Station Description: None</skos:definition>
      <skos:scopeNote xml:lang="en">Coastal Station: Port Hacking 100m station: Type: Coastal Station Description: None</skos:scopeNote>
   </skos:Concept>
   <skos:Concept rdf:about="urn:marlin.csiro.au:sourceregister:concept:59">
      <skos:prefLabel xml:lang="en">Coastal Station: Port Jackson</skos:prefLabel>
      <skos:inScheme rdf:resource="urn:marlin.csiro.au:sourceregister:conceptscheme:1.0"/>
      <skos:definition xml:lang="en">Type: Coastal Station Description: None</skos:definition>
      <skos:scopeNote xml:lang="en">Coastal Station: Port Jackson: Type: Coastal Station Description: None</skos:scopeNote>
   </skos:Concept>
   <skos:Concept rdf:about="urn:marlin.csiro.au:sourceregister:concept:60">
      <skos:prefLabel xml:lang="en">Coastal Station: Port Macdonnell</skos:prefLabel>
      <skos:inScheme rdf:resource="urn:marlin.csiro.au:sourceregister:conceptscheme:1.0"/>
      <skos:definition xml:lang="en">Type: Coastal Station Description: None</skos:definition>
      <skos:scopeNote xml:lang="en">Coastal Station: Port Macdonnell: Type: Coastal Station Description: None</skos:scopeNote>
   </skos:Concept>
   <skos:Concept rdf:about="urn:marlin.csiro.au:sourceregister:concept:61">
      <skos:prefLabel xml:lang="en">Coastal Station: Port Macquarie</skos:prefLabel>
      <skos:inScheme rdf:resource="urn:marlin.csiro.au:sourceregister:conceptscheme:1.0"/>
      <skos:definition xml:lang="en">Type: Coastal Station Description: None</skos:definition>
      <skos:scopeNote xml:lang="en">Coastal Station: Port Macquarie: Type: Coastal Station Description: None</skos:scopeNote>
   </skos:Concept>
   <skos:Concept rdf:about="urn:marlin.csiro.au:sourceregister:concept:62">
      <skos:prefLabel xml:lang="en">Coastal Station: Port Phillip Heads</skos:prefLabel>
      <skos:inScheme rdf:resource="urn:marlin.csiro.au:sourceregister:conceptscheme:1.0"/>
      <skos:definition xml:lang="en">Type: Coastal Station Description: None</skos:definition>
      <skos:scopeNote xml:lang="en">Coastal Station: Port Phillip Heads: Type: Coastal Station Description: None</skos:scopeNote>
   </skos:Concept>
   <skos:Concept rdf:about="urn:marlin.csiro.au:sourceregister:concept:63">
      <skos:prefLabel xml:lang="en">Coastal Station: Port Stephens</skos:prefLabel>
      <skos:inScheme rdf:resource="urn:marlin.csiro.au:sourceregister:conceptscheme:1.0"/>
      <skos:definition xml:lang="en">Type: Coastal Station Description: None</skos:definition>
      <skos:scopeNote xml:lang="en">Coastal Station: Port Stephens: Type: Coastal Station Description: None</skos:scopeNote>
   </skos:Concept>
   <skos:Concept rdf:about="urn:marlin.csiro.au:sourceregister:concept:64">
      <skos:prefLabel xml:lang="en">Coastal Station: Rottnest Island</skos:prefLabel>
      <skos:inScheme rdf:resource="urn:marlin.csiro.au:sourceregister:conceptscheme:1.0"/>
      <skos:definition xml:lang="en">Type: Coastal Station Description: None</skos:definition>
      <skos:scopeNote xml:lang="en">Coastal Station: Rottnest Island: Type: Coastal Station Description: None</skos:scopeNote>
   </skos:Concept>
   <skos:Concept rdf:about="urn:marlin.csiro.au:sourceregister:concept:65">
      <skos:prefLabel xml:lang="en">Coastal Station: St Helens</skos:prefLabel>
      <skos:inScheme rdf:resource="urn:marlin.csiro.au:sourceregister:conceptscheme:1.0"/>
      <skos:definition xml:lang="en">Type: Coastal Station Description: None</skos:definition>
      <skos:scopeNote xml:lang="en">Coastal Station: St Helens: Type: Coastal Station Description: None</skos:scopeNote>
   </skos:Concept>
   <skos:Concept rdf:about="urn:marlin.csiro.au:sourceregister:concept:66">
      <skos:prefLabel xml:lang="en">Coastal Station: Seven Mile Beach</skos:prefLabel>
      <skos:inScheme rdf:resource="urn:marlin.csiro.au:sourceregister:conceptscheme:1.0"/>
      <skos:definition xml:lang="en">Type: Coastal Station Description: None</skos:definition>
      <skos:scopeNote xml:lang="en">Coastal Station: Seven Mile Beach: Type: Coastal Station Description: None</skos:scopeNote>
   </skos:Concept>
   <skos:Concept rdf:about="urn:marlin.csiro.au:sourceregister:concept:67">
      <skos:prefLabel xml:lang="en">Coastal Station: Ulladulla</skos:prefLabel>
      <skos:inScheme rdf:resource="urn:marlin.csiro.au:sourceregister:conceptscheme:1.0"/>
      <skos:definition xml:lang="en">Type: Coastal Station Description: None</skos:definition>
      <skos:scopeNote xml:lang="en">Coastal Station: Ulladulla: Type: Coastal Station Description: None</skos:scopeNote>
   </skos:Concept>
   <skos:Concept rdf:about="urn:marlin.csiro.au:sourceregister:concept:68">
      <skos:prefLabel xml:lang="en">Coastal Station: Wollongong</skos:prefLabel>
      <skos:inScheme rdf:resource="urn:marlin.csiro.au:sourceregister:conceptscheme:1.0"/>
      <skos:definition xml:lang="en">Type: Coastal Station Description: None</skos:definition>
      <skos:scopeNote xml:lang="en">Coastal Station: Wollongong: Type: Coastal Station Description: None</skos:scopeNote>
   </skos:Concept>
   <skos:Concept rdf:about="urn:marlin.csiro.au:sourceregister:concept:69">
      <skos:prefLabel xml:lang="en">Coastal Station: Yamba</skos:prefLabel>
      <skos:inScheme rdf:resource="urn:marlin.csiro.au:sourceregister:conceptscheme:1.0"/>
      <skos:definition xml:lang="en">Type: Coastal Station Description: None</skos:definition>
      <skos:scopeNote xml:lang="en">Coastal Station: Yamba: Type: Coastal Station Description: None</skos:scopeNote>
   </skos:Concept>
   <skos:Concept rdf:about="urn:marlin.csiro.au:sourceregister:concept:71">
      <skos:prefLabel xml:lang="en">Ship: Fairwind</skos:prefLabel>
      <skos:inScheme rdf:resource="urn:marlin.csiro.au:sourceregister:conceptscheme:1.0"/>
      <skos:definition xml:lang="en">Type: Ship Description: None</skos:definition>
      <skos:scopeNote xml:lang="en">Ship: Fairwind: Type: Ship Description: None</skos:scopeNote>
   </skos:Concept>
   <skos:Concept rdf:about="urn:marlin.csiro.au:sourceregister:concept:70">
      <skos:prefLabel xml:lang="en">Ship: Southern Endeavour</skos:prefLabel>
      <skos:inScheme rdf:resource="urn:marlin.csiro.au:sourceregister:conceptscheme:1.0"/>
      <skos:definition xml:lang="en">Type: Ship Description: None</skos:definition>
      <skos:scopeNote xml:lang="en">Ship: Southern Endeavour: Type: Ship Description: None</skos:scopeNote>
   </skos:Concept>
   <skos:Concept rdf:about="urn:marlin.csiro.au:sourceregister:concept:72">
      <skos:prefLabel xml:lang="en">Ship: Cook</skos:prefLabel>
      <skos:inScheme rdf:resource="urn:marlin.csiro.au:sourceregister:conceptscheme:1.0"/>
      <skos:definition xml:lang="en">Type: Ship Description: HMS Cook (K638/A307) was a Bay-class frigate of the British Royal Navy which served as a survey ship.

Class &amp; type: Bay-class frigate
Overall length 307 ft 3 in (93.65 m)

Commissioned: 6 June 1950
Decommissioned: 1 May 1964</skos:definition>
      <skos:scopeNote xml:lang="en">Ship: Cook: Type: Ship Description: HMS Cook (K638/A307) was a Bay-class frigate of the British Royal Navy which served as a survey ship.

Class &amp; type: Bay-class frigate
Overall length 307 ft 3 in (93.65 m)

Commissioned: 6 June 1950
Decommissioned: 1 May 1964</skos:scopeNote>
   </skos:Concept>
   <skos:Concept rdf:about="urn:marlin.csiro.au:sourceregister:concept:73">
      <skos:prefLabel xml:lang="en">Ship: Dana</skos:prefLabel>
      <skos:inScheme rdf:resource="urn:marlin.csiro.au:sourceregister:conceptscheme:1.0"/>
      <skos:definition xml:lang="en">Type: Ship Description: None</skos:definition>
      <skos:scopeNote xml:lang="en">Ship: Dana: Type: Ship Description: None</skos:scopeNote>
   </skos:Concept>
   <skos:Concept rdf:about="urn:marlin.csiro.au:sourceregister:concept:75">
      <skos:prefLabel xml:lang="en">Ship: Umitaka Maru</skos:prefLabel>
      <skos:inScheme rdf:resource="urn:marlin.csiro.au:sourceregister:conceptscheme:1.0"/>
      <skos:definition xml:lang="en">Type: Ship Description: None</skos:definition>
      <skos:scopeNote xml:lang="en">Ship: Umitaka Maru: Type: Ship Description: None</skos:scopeNote>
   </skos:Concept>
   <skos:Concept rdf:about="urn:marlin.csiro.au:sourceregister:concept:77">
      <skos:prefLabel xml:lang="en">Ship: Queenborough</skos:prefLabel>
      <skos:inScheme rdf:resource="urn:marlin.csiro.au:sourceregister:conceptscheme:1.0"/>
      <skos:definition xml:lang="en">Type: Ship Description: HMAS Queenborough.&lt;BR&gt;
RAN frigate on loan to CSIRO in 1958 for work in the Tasman and Coral Seas.</skos:definition>
      <skos:scopeNote xml:lang="en">Ship: Queenborough: Type: Ship Description: HMAS Queenborough.&lt;BR&gt;
RAN frigate on loan to CSIRO in 1958 for work in the Tasman and Coral Seas.</skos:scopeNote>
   </skos:Concept>
   <skos:Concept rdf:about="urn:marlin.csiro.au:sourceregister:concept:78">
      <skos:prefLabel xml:lang="en">Ship: Ob</skos:prefLabel>
      <skos:inScheme rdf:resource="urn:marlin.csiro.au:sourceregister:conceptscheme:1.0"/>
      <skos:definition xml:lang="en">Type: Ship Description: None</skos:definition>
      <skos:scopeNote xml:lang="en">Ship: Ob: Type: Ship Description: None</skos:scopeNote>
   </skos:Concept>
   <skos:Concept rdf:about="urn:marlin.csiro.au:sourceregister:concept:79">
      <skos:prefLabel xml:lang="en">Ship: Galathea</skos:prefLabel>
      <skos:inScheme rdf:resource="urn:marlin.csiro.au:sourceregister:conceptscheme:1.0"/>
      <skos:definition xml:lang="en">Type: Ship Description: None</skos:definition>
      <skos:scopeNote xml:lang="en">Ship: Galathea: Type: Ship Description: None</skos:scopeNote>
   </skos:Concept>
   <skos:Concept rdf:about="urn:marlin.csiro.au:sourceregister:concept:80">
      <skos:prefLabel xml:lang="en">Ship: Warrego</skos:prefLabel>
      <skos:inScheme rdf:resource="urn:marlin.csiro.au:sourceregister:conceptscheme:1.0"/>
      <skos:definition xml:lang="en">Type: Ship Description: None</skos:definition>
      <skos:scopeNote xml:lang="en">Ship: Warrego: Type: Ship Description: None</skos:scopeNote>
   </skos:Concept>
   <skos:Concept rdf:about="urn:marlin.csiro.au:sourceregister:concept:81">
      <skos:prefLabel xml:lang="en">Ship: Kalinda</skos:prefLabel>
      <skos:inScheme rdf:resource="urn:marlin.csiro.au:sourceregister:conceptscheme:1.0"/>
      <skos:definition xml:lang="en">Type: Ship Description: Chartered commercial prawn trawler.
Hull material:  timber
Length: 21.3m
Built: 1973
Typical trawl speed: 3.0 knots</skos:definition>
      <skos:scopeNote xml:lang="en">Ship: Kalinda: Type: Ship Description: Chartered commercial prawn trawler.
Hull material:  timber
Length: 21.3m
Built: 1973
Typical trawl speed: 3.0 knots</skos:scopeNote>
   </skos:Concept>
   <skos:Concept rdf:about="urn:marlin.csiro.au:sourceregister:concept:82">
      <skos:prefLabel xml:lang="en">Ship: Puccini</skos:prefLabel>
      <skos:inScheme rdf:resource="urn:marlin.csiro.au:sourceregister:conceptscheme:1.0"/>
      <skos:definition xml:lang="en">Type: Ship Description: None</skos:definition>
      <skos:scopeNote xml:lang="en">Ship: Puccini: Type: Ship Description: None</skos:scopeNote>
   </skos:Concept>
   <skos:Concept rdf:about="urn:marlin.csiro.au:sourceregister:concept:83">
      <skos:prefLabel xml:lang="en">Ship: Oshoro Maru</skos:prefLabel>
      <skos:inScheme rdf:resource="urn:marlin.csiro.au:sourceregister:conceptscheme:1.0"/>
      <skos:definition xml:lang="en">Type: Ship Description: None</skos:definition>
      <skos:scopeNote xml:lang="en">Ship: Oshoro Maru: Type: Ship Description: None</skos:scopeNote>
   </skos:Concept>
   <skos:Concept rdf:about="urn:marlin.csiro.au:sourceregister:concept:84">
      <skos:prefLabel xml:lang="en">Ship: (Historical Fisheries Vessel) - Investigator</skos:prefLabel>
      <skos:inScheme rdf:resource="urn:marlin.csiro.au:sourceregister:conceptscheme:1.0"/>
      <skos:definition xml:lang="en">Type: Ship Description: FRV Investigator - fisheries research vessel of the Department of Fisheries and Game, South Australia (1964); Department of Fisheries and Fauna Conservation (1965).&lt;br&gt;
??? Previously named 'Weerutta'???</skos:definition>
      <skos:scopeNote xml:lang="en">Ship: (Historical Fisheries Vessel) - Investigator: Type: Ship Description: FRV Investigator - fisheries research vessel of the Department of Fisheries and Game, South Australia (1964); Department of Fisheries and Fauna Conservation (1965).&lt;br&gt;
??? Previously named 'Weerutta'???</skos:scopeNote>
   </skos:Concept>
   <skos:Concept rdf:about="urn:marlin.csiro.au:sourceregister:concept:85">
      <skos:prefLabel xml:lang="en">Ship: Weerutta</skos:prefLabel>
      <skos:inScheme rdf:resource="urn:marlin.csiro.au:sourceregister:conceptscheme:1.0"/>
      <skos:definition xml:lang="en">Type: Ship Description: None</skos:definition>
      <skos:scopeNote xml:lang="en">Ship: Weerutta: Type: Ship Description: None</skos:scopeNote>
   </skos:Concept>
   <skos:Concept rdf:about="urn:marlin.csiro.au:sourceregister:concept:86">
      <skos:prefLabel xml:lang="en">Coastal Station: Kingfish B</skos:prefLabel>
      <skos:inScheme rdf:resource="urn:marlin.csiro.au:sourceregister:conceptscheme:1.0"/>
      <skos:definition xml:lang="en">Type: Coastal Station Description: None</skos:definition>
      <skos:scopeNote xml:lang="en">Coastal Station: Kingfish B: Type: Coastal Station Description: None</skos:scopeNote>
   </skos:Concept>
   <skos:Concept rdf:about="urn:marlin.csiro.au:sourceregister:concept:87">
      <skos:prefLabel xml:lang="en">Ship: Kakuyo Maru</skos:prefLabel>
      <skos:inScheme rdf:resource="urn:marlin.csiro.au:sourceregister:conceptscheme:1.0"/>
      <skos:definition xml:lang="en">Type: Ship Description: None</skos:definition>
      <skos:scopeNote xml:lang="en">Ship: Kakuyo Maru: Type: Ship Description: None</skos:scopeNote>
   </skos:Concept>
   <skos:Concept rdf:about="urn:marlin.csiro.au:sourceregister:concept:88">
      <skos:prefLabel xml:lang="en">Ship: Penaeus</skos:prefLabel>
      <skos:inScheme rdf:resource="urn:marlin.csiro.au:sourceregister:conceptscheme:1.0"/>
      <skos:definition xml:lang="en">Type: Ship Description: RV Penaueus.&lt;BR&gt;
11.6m bondwood prawn trawler used in Moreton Bay on the East Coast Prawn Project; 145 BHP Detroit diesel; range 400 miles, max. speed 9.5 knots; built in Brisbane in 1972.&lt;BR&gt;
Vivienne Mawson, David J. Tranter and Alan F. Pearce (1988). &lt;I&gt;CSIRO at sea : fifty years of marine science&lt;/I&gt;, (pp. 208)&lt;BR&gt;CSIRO Marine Laboratories.</skos:definition>
      <skos:scopeNote xml:lang="en">Ship: Penaeus: Type: Ship Description: RV Penaueus.&lt;BR&gt;
11.6m bondwood prawn trawler used in Moreton Bay on the East Coast Prawn Project; 145 BHP Detroit diesel; range 400 miles, max. speed 9.5 knots; built in Brisbane in 1972.&lt;BR&gt;
Vivienne Mawson, David J. Tranter and Alan F. Pearce (1988). &lt;I&gt;CSIRO at sea : fifty years of marine science&lt;/I&gt;, (pp. 208)&lt;BR&gt;CSIRO Marine Laboratories.</skos:scopeNote>
   </skos:Concept>
   <skos:Concept rdf:about="urn:marlin.csiro.au:sourceregister:concept:89">
      <skos:prefLabel xml:lang="en">Ship: Anson</skos:prefLabel>
      <skos:inScheme rdf:resource="urn:marlin.csiro.au:sourceregister:conceptscheme:1.0"/>
      <skos:definition xml:lang="en">Type: Ship Description: None</skos:definition>
      <skos:scopeNote xml:lang="en">Ship: Anson: Type: Ship Description: None</skos:scopeNote>
   </skos:Concept>
   <skos:Concept rdf:about="urn:marlin.csiro.au:sourceregister:concept:90">
      <skos:prefLabel xml:lang="en">Ship: Favourite</skos:prefLabel>
      <skos:inScheme rdf:resource="urn:marlin.csiro.au:sourceregister:conceptscheme:1.0"/>
      <skos:definition xml:lang="en">Type: Ship Description: None</skos:definition>
      <skos:scopeNote xml:lang="en">Ship: Favourite: Type: Ship Description: None</skos:scopeNote>
   </skos:Concept>
   <skos:Concept rdf:about="urn:marlin.csiro.au:sourceregister:concept:91">
      <skos:prefLabel xml:lang="en">Ship: Coriolis</skos:prefLabel>
      <skos:inScheme rdf:resource="urn:marlin.csiro.au:sourceregister:conceptscheme:1.0"/>
      <skos:definition xml:lang="en">Type: Ship Description: None</skos:definition>
      <skos:scopeNote xml:lang="en">Ship: Coriolis: Type: Ship Description: None</skos:scopeNote>
   </skos:Concept>
   <skos:Concept rdf:about="urn:marlin.csiro.au:sourceregister:concept:92">
      <skos:prefLabel xml:lang="en">Ship: Degei</skos:prefLabel>
      <skos:inScheme rdf:resource="urn:marlin.csiro.au:sourceregister:conceptscheme:1.0"/>
      <skos:definition xml:lang="en">Type: Ship Description: None</skos:definition>
      <skos:scopeNote xml:lang="en">Ship: Degei: Type: Ship Description: None</skos:scopeNote>
   </skos:Concept>
   <skos:Concept rdf:about="urn:marlin.csiro.au:sourceregister:concept:93">
      <skos:prefLabel xml:lang="en">Ship: Changi</skos:prefLabel>
      <skos:inScheme rdf:resource="urn:marlin.csiro.au:sourceregister:conceptscheme:1.0"/>
      <skos:definition xml:lang="en">Type: Ship Description: None</skos:definition>
      <skos:scopeNote xml:lang="en">Ship: Changi: Type: Ship Description: None</skos:scopeNote>
   </skos:Concept>
   <skos:Concept rdf:about="urn:marlin.csiro.au:sourceregister:concept:95">
      <skos:prefLabel xml:lang="en">Ship: Cape Don</skos:prefLabel>
      <skos:inScheme rdf:resource="urn:marlin.csiro.au:sourceregister:conceptscheme:1.0"/>
      <skos:definition xml:lang="en">Type: Ship Description: None</skos:definition>
      <skos:scopeNote xml:lang="en">Ship: Cape Don: Type: Ship Description: None</skos:scopeNote>
   </skos:Concept>
   <skos:Concept rdf:about="urn:marlin.csiro.au:sourceregister:concept:96">
      <skos:prefLabel xml:lang="en">Ship: Eastwind</skos:prefLabel>
      <skos:inScheme rdf:resource="urn:marlin.csiro.au:sourceregister:conceptscheme:1.0"/>
      <skos:definition xml:lang="en">Type: Ship Description: None</skos:definition>
      <skos:scopeNote xml:lang="en">Ship: Eastwind: Type: Ship Description: None</skos:scopeNote>
   </skos:Concept>
   <skos:Concept rdf:about="urn:marlin.csiro.au:sourceregister:concept:97">
      <skos:prefLabel xml:lang="en">Coastal Station: Cape Pillar</skos:prefLabel>
      <skos:inScheme rdf:resource="urn:marlin.csiro.au:sourceregister:conceptscheme:1.0"/>
      <skos:definition xml:lang="en">Type: Coastal Station Description: None</skos:definition>
      <skos:scopeNote xml:lang="en">Coastal Station: Cape Pillar: Type: Coastal Station Description: None</skos:scopeNote>
   </skos:Concept>
   <skos:Concept rdf:about="urn:marlin.csiro.au:sourceregister:concept:98">
      <skos:prefLabel xml:lang="en">Coastal Station: Nickol Bay</skos:prefLabel>
      <skos:inScheme rdf:resource="urn:marlin.csiro.au:sourceregister:conceptscheme:1.0"/>
      <skos:definition xml:lang="en">Type: Coastal Station Description: None</skos:definition>
      <skos:scopeNote xml:lang="en">Coastal Station: Nickol Bay: Type: Coastal Station Description: None</skos:scopeNote>
   </skos:Concept>
   <skos:Concept rdf:about="urn:marlin.csiro.au:sourceregister:concept:99">
      <skos:prefLabel xml:lang="en">Coastal Station: Tin Can Bay</skos:prefLabel>
      <skos:inScheme rdf:resource="urn:marlin.csiro.au:sourceregister:conceptscheme:1.0"/>
      <skos:definition xml:lang="en">Type: Coastal Station Description: None</skos:definition>
      <skos:scopeNote xml:lang="en">Coastal Station: Tin Can Bay: Type: Coastal Station Description: None</skos:scopeNote>
   </skos:Concept>
   <skos:Concept rdf:about="urn:marlin.csiro.au:sourceregister:concept:100">
      <skos:prefLabel xml:lang="en">Coastal Station: Warrnambool</skos:prefLabel>
      <skos:inScheme rdf:resource="urn:marlin.csiro.au:sourceregister:conceptscheme:1.0"/>
      <skos:definition xml:lang="en">Type: Coastal Station Description: None</skos:definition>
      <skos:scopeNote xml:lang="en">Coastal Station: Warrnambool: Type: Coastal Station Description: None</skos:scopeNote>
   </skos:Concept>
   <skos:Concept rdf:about="urn:marlin.csiro.au:sourceregister:concept:101">
      <skos:prefLabel xml:lang="en">Coastal Station: Bougainville</skos:prefLabel>
      <skos:inScheme rdf:resource="urn:marlin.csiro.au:sourceregister:conceptscheme:1.0"/>
      <skos:definition xml:lang="en">Type: Coastal Station Description: None</skos:definition>
      <skos:scopeNote xml:lang="en">Coastal Station: Bougainville: Type: Coastal Station Description: None</skos:scopeNote>
   </skos:Concept>
   <skos:Concept rdf:about="urn:marlin.csiro.au:sourceregister:concept:102">
      <skos:prefLabel xml:lang="en">Coastal Station: Broome</skos:prefLabel>
      <skos:inScheme rdf:resource="urn:marlin.csiro.au:sourceregister:conceptscheme:1.0"/>
      <skos:definition xml:lang="en">Type: Coastal Station Description: None</skos:definition>
      <skos:scopeNote xml:lang="en">Coastal Station: Broome: Type: Coastal Station Description: None</skos:scopeNote>
   </skos:Concept>
   <skos:Concept rdf:about="urn:marlin.csiro.au:sourceregister:concept:103">
      <skos:prefLabel xml:lang="en">Coastal Station: Lake Cathie</skos:prefLabel>
      <skos:inScheme rdf:resource="urn:marlin.csiro.au:sourceregister:conceptscheme:1.0"/>
      <skos:definition xml:lang="en">Type: Coastal Station Description: None</skos:definition>
      <skos:scopeNote xml:lang="en">Coastal Station: Lake Cathie: Type: Coastal Station Description: None</skos:scopeNote>
   </skos:Concept>
   <skos:Concept rdf:about="urn:marlin.csiro.au:sourceregister:concept:104">
      <skos:prefLabel xml:lang="en">Coastal Station: Geraldton</skos:prefLabel>
      <skos:inScheme rdf:resource="urn:marlin.csiro.au:sourceregister:conceptscheme:1.0"/>
      <skos:definition xml:lang="en">Type: Coastal Station Description: None</skos:definition>
      <skos:scopeNote xml:lang="en">Coastal Station: Geraldton: Type: Coastal Station Description: None</skos:scopeNote>
   </skos:Concept>
   <skos:Concept rdf:about="urn:marlin.csiro.au:sourceregister:concept:105">
      <skos:prefLabel xml:lang="en">Coastal Station: Augusta</skos:prefLabel>
      <skos:inScheme rdf:resource="urn:marlin.csiro.au:sourceregister:conceptscheme:1.0"/>
      <skos:definition xml:lang="en">Type: Coastal Station Description: None</skos:definition>
      <skos:scopeNote xml:lang="en">Coastal Station: Augusta: Type: Coastal Station Description: None</skos:scopeNote>
   </skos:Concept>
   <skos:Concept rdf:about="urn:marlin.csiro.au:sourceregister:concept:106">
      <skos:prefLabel xml:lang="en">Coastal Station: Esperance</skos:prefLabel>
      <skos:inScheme rdf:resource="urn:marlin.csiro.au:sourceregister:conceptscheme:1.0"/>
      <skos:definition xml:lang="en">Type: Coastal Station Description: None</skos:definition>
      <skos:scopeNote xml:lang="en">Coastal Station: Esperance: Type: Coastal Station Description: None</skos:scopeNote>
   </skos:Concept>
   <skos:Concept rdf:about="urn:marlin.csiro.au:sourceregister:concept:107">
      <skos:prefLabel xml:lang="en">Coastal Station: Cape Sorell</skos:prefLabel>
      <skos:inScheme rdf:resource="urn:marlin.csiro.au:sourceregister:conceptscheme:1.0"/>
      <skos:definition xml:lang="en">Type: Coastal Station Description: None</skos:definition>
      <skos:scopeNote xml:lang="en">Coastal Station: Cape Sorell: Type: Coastal Station Description: None</skos:scopeNote>
   </skos:Concept>
   <skos:Concept rdf:about="urn:marlin.csiro.au:sourceregister:concept:108">
      <skos:prefLabel xml:lang="en">Locality: Hillarys Transect</skos:prefLabel>
      <skos:inScheme rdf:resource="urn:marlin.csiro.au:sourceregister:conceptscheme:1.0"/>
      <skos:definition xml:lang="en">Type: Locality Description: 4 km transect oceanographic transect, westwards from Hillarys Marina, Perth</skos:definition>
      <skos:scopeNote xml:lang="en">Locality: Hillarys Transect: Type: Locality Description: 4 km transect oceanographic transect, westwards from Hillarys Marina, Perth</skos:scopeNote>
   </skos:Concept>
   <skos:Concept rdf:about="urn:marlin.csiro.au:sourceregister:concept:109">
      <skos:prefLabel xml:lang="en">Ship: Saxon Progress</skos:prefLabel>
      <skos:inScheme rdf:resource="urn:marlin.csiro.au:sourceregister:conceptscheme:1.0"/>
      <skos:definition xml:lang="en">Type: Ship Description: Commercial Fishing Vessel
</skos:definition>
      <skos:scopeNote xml:lang="en">Ship: Saxon Progress: Type: Ship Description: Commercial Fishing Vessel
</skos:scopeNote>
   </skos:Concept>
   <skos:Concept rdf:about="urn:marlin.csiro.au:sourceregister:concept:110">
      <skos:prefLabel xml:lang="en">Ship: Berg-1</skos:prefLabel>
      <skos:inScheme rdf:resource="urn:marlin.csiro.au:sourceregister:conceptscheme:1.0"/>
      <skos:definition xml:lang="en">Type: Ship Description: Russian Fishery Vessel</skos:definition>
      <skos:scopeNote xml:lang="en">Ship: Berg-1: Type: Ship Description: Russian Fishery Vessel</skos:scopeNote>
   </skos:Concept>
   <skos:Concept rdf:about="urn:marlin.csiro.au:sourceregister:concept:111">
      <skos:prefLabel xml:lang="en">Ship: Berg-2</skos:prefLabel>
      <skos:inScheme rdf:resource="urn:marlin.csiro.au:sourceregister:conceptscheme:1.0"/>
      <skos:definition xml:lang="en">Type: Ship Description: Russian Fishery Vessel</skos:definition>
      <skos:scopeNote xml:lang="en">Ship: Berg-2: Type: Ship Description: Russian Fishery Vessel</skos:scopeNote>
   </skos:Concept>
   <skos:Concept rdf:about="urn:marlin.csiro.au:sourceregister:concept:112">
      <skos:prefLabel xml:lang="en">Ship: Seskar</skos:prefLabel>
      <skos:inScheme rdf:resource="urn:marlin.csiro.au:sourceregister:conceptscheme:1.0"/>
      <skos:definition xml:lang="en">Type: Ship Description: Russian Fishery Vessel</skos:definition>
      <skos:scopeNote xml:lang="en">Ship: Seskar: Type: Ship Description: Russian Fishery Vessel</skos:scopeNote>
   </skos:Concept>
   <skos:Concept rdf:about="urn:marlin.csiro.au:sourceregister:concept:113">
      <skos:prefLabel xml:lang="en">Ship: Raduga</skos:prefLabel>
      <skos:inScheme rdf:resource="urn:marlin.csiro.au:sourceregister:conceptscheme:1.0"/>
      <skos:definition xml:lang="en">Type: Ship Description: Russian Fishery Vessel</skos:definition>
      <skos:scopeNote xml:lang="en">Ship: Raduga: Type: Ship Description: Russian Fishery Vessel</skos:scopeNote>
   </skos:Concept>
   <skos:Concept rdf:about="urn:marlin.csiro.au:sourceregister:concept:114">
      <skos:prefLabel xml:lang="en">Ship: Lira</skos:prefLabel>
      <skos:inScheme rdf:resource="urn:marlin.csiro.au:sourceregister:conceptscheme:1.0"/>
      <skos:definition xml:lang="en">Type: Ship Description: Russian Fishery Vessel</skos:definition>
      <skos:scopeNote xml:lang="en">Ship: Lira: Type: Ship Description: Russian Fishery Vessel</skos:scopeNote>
   </skos:Concept>
   <skos:Concept rdf:about="urn:marlin.csiro.au:sourceregister:concept:115">
      <skos:prefLabel xml:lang="en">Ship: Berg-3</skos:prefLabel>
      <skos:inScheme rdf:resource="urn:marlin.csiro.au:sourceregister:conceptscheme:1.0"/>
      <skos:definition xml:lang="en">Type: Ship Description: Russian Fishery Vessel</skos:definition>
      <skos:scopeNote xml:lang="en">Ship: Berg-3: Type: Ship Description: Russian Fishery Vessel</skos:scopeNote>
   </skos:Concept>
   <skos:Concept rdf:about="urn:marlin.csiro.au:sourceregister:concept:116">
      <skos:prefLabel xml:lang="en">Ship: Korifei</skos:prefLabel>
      <skos:inScheme rdf:resource="urn:marlin.csiro.au:sourceregister:conceptscheme:1.0"/>
      <skos:definition xml:lang="en">Type: Ship Description: Russian Fishery Vessel</skos:definition>
      <skos:scopeNote xml:lang="en">Ship: Korifei: Type: Ship Description: Russian Fishery Vessel</skos:scopeNote>
   </skos:Concept>
   <skos:Concept rdf:about="urn:marlin.csiro.au:sourceregister:concept:117">
      <skos:prefLabel xml:lang="en">Ship: Sutchan</skos:prefLabel>
      <skos:inScheme rdf:resource="urn:marlin.csiro.au:sourceregister:conceptscheme:1.0"/>
      <skos:definition xml:lang="en">Type: Ship Description: Russian Fishery Vessel</skos:definition>
      <skos:scopeNote xml:lang="en">Ship: Sutchan: Type: Ship Description: Russian Fishery Vessel</skos:scopeNote>
   </skos:Concept>
   <skos:Concept rdf:about="urn:marlin.csiro.au:sourceregister:concept:118">
      <skos:prefLabel xml:lang="en">Ship: Pr. Deruygin</skos:prefLabel>
      <skos:inScheme rdf:resource="urn:marlin.csiro.au:sourceregister:conceptscheme:1.0"/>
      <skos:definition xml:lang="en">Type: Ship Description: Russian Fishery Vessel</skos:definition>
      <skos:scopeNote xml:lang="en">Ship: Pr. Deruygin: Type: Ship Description: Russian Fishery Vessel</skos:scopeNote>
   </skos:Concept>
   <skos:Concept rdf:about="urn:marlin.csiro.au:sourceregister:concept:119">
      <skos:prefLabel xml:lang="en">Ship: Prometey</skos:prefLabel>
      <skos:inScheme rdf:resource="urn:marlin.csiro.au:sourceregister:conceptscheme:1.0"/>
      <skos:definition xml:lang="en">Type: Ship Description: Russian Fishery Vessel</skos:definition>
      <skos:scopeNote xml:lang="en">Ship: Prometey: Type: Ship Description: Russian Fishery Vessel</skos:scopeNote>
   </skos:Concept>
   <skos:Concept rdf:about="urn:marlin.csiro.au:sourceregister:concept:120">
      <skos:prefLabel xml:lang="en">Ship: SRTM 8-449</skos:prefLabel>
      <skos:inScheme rdf:resource="urn:marlin.csiro.au:sourceregister:conceptscheme:1.0"/>
      <skos:definition xml:lang="en">Type: Ship Description: Russian Fishery Vessel</skos:definition>
      <skos:scopeNote xml:lang="en">Ship: SRTM 8-449: Type: Ship Description: Russian Fishery Vessel</skos:scopeNote>
   </skos:Concept>
   <skos:Concept rdf:about="urn:marlin.csiro.au:sourceregister:concept:121">
      <skos:prefLabel xml:lang="en">Ship: Alba</skos:prefLabel>
      <skos:inScheme rdf:resource="urn:marlin.csiro.au:sourceregister:conceptscheme:1.0"/>
      <skos:definition xml:lang="en">Type: Ship Description: Russian Fishery Vessel</skos:definition>
      <skos:scopeNote xml:lang="en">Ship: Alba: Type: Ship Description: Russian Fishery Vessel</skos:scopeNote>
   </skos:Concept>
   <skos:Concept rdf:about="urn:marlin.csiro.au:sourceregister:concept:122">
      <skos:prefLabel xml:lang="en">Ship: Poseidon</skos:prefLabel>
      <skos:inScheme rdf:resource="urn:marlin.csiro.au:sourceregister:conceptscheme:1.0"/>
      <skos:definition xml:lang="en">Type: Ship Description: Russian Fishery Vessel</skos:definition>
      <skos:scopeNote xml:lang="en">Ship: Poseidon: Type: Ship Description: Russian Fishery Vessel</skos:scopeNote>
   </skos:Concept>
   <skos:Concept rdf:about="urn:marlin.csiro.au:sourceregister:concept:123">
      <skos:prefLabel xml:lang="en">Ship: Equator</skos:prefLabel>
      <skos:inScheme rdf:resource="urn:marlin.csiro.au:sourceregister:conceptscheme:1.0"/>
      <skos:definition xml:lang="en">Type: Ship Description: Russian Fishery Vessel</skos:definition>
      <skos:scopeNote xml:lang="en">Ship: Equator: Type: Ship Description: Russian Fishery Vessel</skos:scopeNote>
   </skos:Concept>
   <skos:Concept rdf:about="urn:marlin.csiro.au:sourceregister:concept:124">
      <skos:prefLabel xml:lang="en">Ship: Shantar</skos:prefLabel>
      <skos:inScheme rdf:resource="urn:marlin.csiro.au:sourceregister:conceptscheme:1.0"/>
      <skos:definition xml:lang="en">Type: Ship Description: Russian Fishery Vessel</skos:definition>
      <skos:scopeNote xml:lang="en">Ship: Shantar: Type: Ship Description: Russian Fishery Vessel</skos:scopeNote>
   </skos:Concept>
   <skos:Concept rdf:about="urn:marlin.csiro.au:sourceregister:concept:125">
      <skos:prefLabel xml:lang="en">Ship: Bacaevo</skos:prefLabel>
      <skos:inScheme rdf:resource="urn:marlin.csiro.au:sourceregister:conceptscheme:1.0"/>
      <skos:definition xml:lang="en">Type: Ship Description: Russian Fishery Vessel</skos:definition>
      <skos:scopeNote xml:lang="en">Ship: Bacaevo: Type: Ship Description: Russian Fishery Vessel</skos:scopeNote>
   </skos:Concept>
   <skos:Concept rdf:about="urn:marlin.csiro.au:sourceregister:concept:126">
      <skos:prefLabel xml:lang="en">Ship: Kamensky</skos:prefLabel>
      <skos:inScheme rdf:resource="urn:marlin.csiro.au:sourceregister:conceptscheme:1.0"/>
      <skos:definition xml:lang="en">Type: Ship Description: Russian Fishery Vessel</skos:definition>
      <skos:scopeNote xml:lang="en">Ship: Kamensky: Type: Ship Description: Russian Fishery Vessel</skos:scopeNote>
   </skos:Concept>
   <skos:Concept rdf:about="urn:marlin.csiro.au:sourceregister:concept:127">
      <skos:prefLabel xml:lang="en">Ship: Tichookeanscy</skos:prefLabel>
      <skos:inScheme rdf:resource="urn:marlin.csiro.au:sourceregister:conceptscheme:1.0"/>
      <skos:definition xml:lang="en">Type: Ship Description: Russian Fishery Vessel</skos:definition>
      <skos:scopeNote xml:lang="en">Ship: Tichookeanscy: Type: Ship Description: Russian Fishery Vessel</skos:scopeNote>
   </skos:Concept>
   <skos:Concept rdf:about="urn:marlin.csiro.au:sourceregister:concept:128">
      <skos:prefLabel xml:lang="en">Ship: Pulk. Meridian</skos:prefLabel>
      <skos:inScheme rdf:resource="urn:marlin.csiro.au:sourceregister:conceptscheme:1.0"/>
      <skos:definition xml:lang="en">Type: Ship Description: Russian Fishery Vessel</skos:definition>
      <skos:scopeNote xml:lang="en">Ship: Pulk. Meridian: Type: Ship Description: Russian Fishery Vessel</skos:scopeNote>
   </skos:Concept>
   <skos:Concept rdf:about="urn:marlin.csiro.au:sourceregister:concept:129">
      <skos:prefLabel xml:lang="en">Ship: Mys Tichy</skos:prefLabel>
      <skos:inScheme rdf:resource="urn:marlin.csiro.au:sourceregister:conceptscheme:1.0"/>
      <skos:definition xml:lang="en">Type: Ship Description: Russian Fishery Vessel</skos:definition>
      <skos:scopeNote xml:lang="en">Ship: Mys Tichy: Type: Ship Description: Russian Fishery Vessel</skos:scopeNote>
   </skos:Concept>
   <skos:Concept rdf:about="urn:marlin.csiro.au:sourceregister:concept:130">
      <skos:prefLabel xml:lang="en">Ship: Petuna Explorer</skos:prefLabel>
      <skos:inScheme rdf:resource="urn:marlin.csiro.au:sourceregister:conceptscheme:1.0"/>
      <skos:definition xml:lang="en">Type: Ship Description: Charter Fishing Vessel
The PETUNA EXPLORER became EXPLORER S on January 2008.

Ship page:      http://maritime-connector.com/ship/explorer-s-8810061/ 
Images:         http://www.shipspotting.com/gallery/photo.php?lid=2005023 
IMO number:     8810061
Currently:      EXPLORER S
Type of ship:   TRAWLER
MMSI:           503375000
Gross tonnage:  296 tons
DWT:            303 tons
Length:         21m
Year of build:  1989
Equipment:      Simrad ES60 38KHz Echosounder

Builder PORT LINCOLN MARINE SERVICES - PORT LINCOLN, AUSTRALIA</skos:definition>
      <skos:scopeNote xml:lang="en">Ship: Petuna Explorer: Type: Ship Description: Charter Fishing Vessel
The PETUNA EXPLORER became EXPLORER S on January 2008.

Ship page:      http://maritime-connector.com/ship/explorer-s-8810061/ 
Images:         http://www.shipspotting.com/gallery/photo.php?lid=2005023 
IMO number:     8810061
Currently:      EXPLORER S
Type of ship:   TRAWLER
MMSI:           503375000
Gross tonnage:  296 tons
DWT:            303 tons
Length:         21m
Year of build:  1989
Equipment:      Simrad ES60 38KHz Echosounder

Builder PORT LINCOLN MARINE SERVICES - PORT LINCOLN, AUSTRALIA</skos:scopeNote>
   </skos:Concept>
   <skos:Concept rdf:about="urn:marlin.csiro.au:sourceregister:concept:131">
      <skos:prefLabel xml:lang="en">Mooring: ACE Cape Howe Moorings (1983)</skos:prefLabel>
      <skos:inScheme rdf:resource="urn:marlin.csiro.au:sourceregister:conceptscheme:1.0"/>
      <skos:definition xml:lang="en">Type: Mooring Description: None</skos:definition>
      <skos:scopeNote xml:lang="en">Mooring: ACE Cape Howe Moorings (1983): Type: Mooring Description: None</skos:scopeNote>
   </skos:Concept>
   <skos:Concept rdf:about="urn:marlin.csiro.au:sourceregister:concept:132">
      <skos:prefLabel xml:lang="en">Mooring: ACE Maria Island Mooring (1983)</skos:prefLabel>
      <skos:inScheme rdf:resource="urn:marlin.csiro.au:sourceregister:conceptscheme:1.0"/>
      <skos:definition xml:lang="en">Type: Mooring Description: None</skos:definition>
      <skos:scopeNote xml:lang="en">Mooring: ACE Maria Island Mooring (1983): Type: Mooring Description: None</skos:scopeNote>
   </skos:Concept>
   <skos:Concept rdf:about="urn:marlin.csiro.au:sourceregister:concept:133">
      <skos:prefLabel xml:lang="en">Mooring: ACE Newcastle Moorings (1983)</skos:prefLabel>
      <skos:inScheme rdf:resource="urn:marlin.csiro.au:sourceregister:conceptscheme:1.0"/>
      <skos:definition xml:lang="en">Type: Mooring Description: None</skos:definition>
      <skos:scopeNote xml:lang="en">Mooring: ACE Newcastle Moorings (1983): Type: Mooring Description: None</skos:scopeNote>
   </skos:Concept>
   <skos:Concept rdf:about="urn:marlin.csiro.au:sourceregister:concept:134">
      <skos:prefLabel xml:lang="en">Mooring: ACE South Solitary Island Mooring (1983)</skos:prefLabel>
      <skos:inScheme rdf:resource="urn:marlin.csiro.au:sourceregister:conceptscheme:1.0"/>
      <skos:definition xml:lang="en">Type: Mooring Description: None</skos:definition>
      <skos:scopeNote xml:lang="en">Mooring: ACE South Solitary Island Mooring (1983): Type: Mooring Description: None</skos:scopeNote>
   </skos:Concept>
   <skos:Concept rdf:about="urn:marlin.csiro.au:sourceregister:concept:135">
      <skos:prefLabel xml:lang="en">Mooring: ACE Stanwell Park Moorings (1983)</skos:prefLabel>
      <skos:inScheme rdf:resource="urn:marlin.csiro.au:sourceregister:conceptscheme:1.0"/>
      <skos:definition xml:lang="en">Type: Mooring Description: None</skos:definition>
      <skos:scopeNote xml:lang="en">Mooring: ACE Stanwell Park Moorings (1983): Type: Mooring Description: None</skos:scopeNote>
   </skos:Concept>
   <skos:Concept rdf:about="urn:marlin.csiro.au:sourceregister:concept:136">
      <skos:prefLabel xml:lang="en">Mooring: AIMS/CSIRO GBR-Coral Sea Moorings (1985)</skos:prefLabel>
      <skos:inScheme rdf:resource="urn:marlin.csiro.au:sourceregister:conceptscheme:1.0"/>
      <skos:definition xml:lang="en">Type: Mooring Description: None</skos:definition>
      <skos:scopeNote xml:lang="en">Mooring: AIMS/CSIRO GBR-Coral Sea Moorings (1985): Type: Mooring Description: None</skos:scopeNote>
   </skos:Concept>
   <skos:Concept rdf:about="urn:marlin.csiro.au:sourceregister:concept:137">
      <skos:prefLabel xml:lang="en">Mooring: Bass Strait Moorings - CSIRO (1991)</skos:prefLabel>
      <skos:inScheme rdf:resource="urn:marlin.csiro.au:sourceregister:conceptscheme:1.0"/>
      <skos:definition xml:lang="en">Type: Mooring Description: None</skos:definition>
      <skos:scopeNote xml:lang="en">Mooring: Bass Strait Moorings - CSIRO (1991): Type: Mooring Description: None</skos:scopeNote>
   </skos:Concept>
   <skos:Concept rdf:about="urn:marlin.csiro.au:sourceregister:concept:138">
      <skos:prefLabel xml:lang="en">Locality: Huon Estuary</skos:prefLabel>
      <skos:inScheme rdf:resource="urn:marlin.csiro.au:sourceregister:conceptscheme:1.0"/>
      <skos:definition xml:lang="en">Type: Locality Description: None</skos:definition>
      <skos:scopeNote xml:lang="en">Locality: Huon Estuary: Type: Locality Description: None</skos:scopeNote>
   </skos:Concept>
   <skos:Concept rdf:about="urn:marlin.csiro.au:sourceregister:concept:139">
      <skos:prefLabel xml:lang="en">Locality: Derwent Estuary</skos:prefLabel>
      <skos:inScheme rdf:resource="urn:marlin.csiro.au:sourceregister:conceptscheme:1.0"/>
      <skos:definition xml:lang="en">Type: Locality Description: None</skos:definition>
      <skos:scopeNote xml:lang="en">Locality: Derwent Estuary: Type: Locality Description: None</skos:scopeNote>
   </skos:Concept>
   <skos:Concept rdf:about="urn:marlin.csiro.au:sourceregister:concept:140">
      <skos:prefLabel xml:lang="en">Mooring: Devonport Moorings (1991-2)</skos:prefLabel>
      <skos:inScheme rdf:resource="urn:marlin.csiro.au:sourceregister:conceptscheme:1.0"/>
      <skos:definition xml:lang="en">Type: Mooring Description: None</skos:definition>
      <skos:scopeNote xml:lang="en">Mooring: Devonport Moorings (1991-2): Type: Mooring Description: None</skos:scopeNote>
   </skos:Concept>
   <skos:Concept rdf:about="urn:marlin.csiro.au:sourceregister:concept:141">
      <skos:prefLabel xml:lang="en">Mooring: Tasman Sea (L.H. Rise) Moorings (1989)</skos:prefLabel>
      <skos:inScheme rdf:resource="urn:marlin.csiro.au:sourceregister:conceptscheme:1.0"/>
      <skos:definition xml:lang="en">Type: Mooring Description: None</skos:definition>
      <skos:scopeNote xml:lang="en">Mooring: Tasman Sea (L.H. Rise) Moorings (1989): Type: Mooring Description: None</skos:scopeNote>
   </skos:Concept>
   <skos:Concept rdf:about="urn:marlin.csiro.au:sourceregister:concept:142">
      <skos:prefLabel xml:lang="en">Mooring: Arafura/G. of Carpent. Moorings (1987)</skos:prefLabel>
      <skos:inScheme rdf:resource="urn:marlin.csiro.au:sourceregister:conceptscheme:1.0"/>
      <skos:definition xml:lang="en">Type: Mooring Description: None</skos:definition>
      <skos:scopeNote xml:lang="en">Mooring: Arafura/G. of Carpent. Moorings (1987): Type: Mooring Description: None</skos:scopeNote>
   </skos:Concept>
   <skos:Concept rdf:about="urn:marlin.csiro.au:sourceregister:concept:143">
      <skos:prefLabel xml:lang="en">Mooring: Halmahera Sea Mooring (1993)</skos:prefLabel>
      <skos:inScheme rdf:resource="urn:marlin.csiro.au:sourceregister:conceptscheme:1.0"/>
      <skos:definition xml:lang="en">Type: Mooring Description: None</skos:definition>
      <skos:scopeNote xml:lang="en">Mooring: Halmahera Sea Mooring (1993): Type: Mooring Description: None</skos:scopeNote>
   </skos:Concept>
   <skos:Concept rdf:about="urn:marlin.csiro.au:sourceregister:concept:144">
      <skos:prefLabel xml:lang="en">Mooring: Heard Island Moorings (1990)</skos:prefLabel>
      <skos:inScheme rdf:resource="urn:marlin.csiro.au:sourceregister:conceptscheme:1.0"/>
      <skos:definition xml:lang="en">Type: Mooring Description: None</skos:definition>
      <skos:scopeNote xml:lang="en">Mooring: Heard Island Moorings (1990): Type: Mooring Description: None</skos:scopeNote>
   </skos:Concept>
   <skos:Concept rdf:about="urn:marlin.csiro.au:sourceregister:concept:145">
      <skos:prefLabel xml:lang="en">Mooring: ICM6 (Ningaloo Reef) Moorings (1994)</skos:prefLabel>
      <skos:inScheme rdf:resource="urn:marlin.csiro.au:sourceregister:conceptscheme:1.0"/>
      <skos:definition xml:lang="en">Type: Mooring Description: None</skos:definition>
      <skos:scopeNote xml:lang="en">Mooring: ICM6 (Ningaloo Reef) Moorings (1994): Type: Mooring Description: None</skos:scopeNote>
   </skos:Concept>
   <skos:Concept rdf:about="urn:marlin.csiro.au:sourceregister:concept:146">
      <skos:prefLabel xml:lang="en">Mooring: LUCIE: alongshore Moorings (1986-7)</skos:prefLabel>
      <skos:inScheme rdf:resource="urn:marlin.csiro.au:sourceregister:conceptscheme:1.0"/>
      <skos:definition xml:lang="en">Type: Mooring Description: None</skos:definition>
      <skos:scopeNote xml:lang="en">Mooring: LUCIE: alongshore Moorings (1986-7): Type: Mooring Description: None</skos:scopeNote>
   </skos:Concept>
   <skos:Concept rdf:about="urn:marlin.csiro.au:sourceregister:concept:147">
      <skos:prefLabel xml:lang="en">Mooring: LUCIE: Cape Mentelle Moorings (1987)</skos:prefLabel>
      <skos:inScheme rdf:resource="urn:marlin.csiro.au:sourceregister:conceptscheme:1.0"/>
      <skos:definition xml:lang="en">Type: Mooring Description: None</skos:definition>
      <skos:scopeNote xml:lang="en">Mooring: LUCIE: Cape Mentelle Moorings (1987): Type: Mooring Description: None</skos:scopeNote>
   </skos:Concept>
   <skos:Concept rdf:about="urn:marlin.csiro.au:sourceregister:concept:148">
      <skos:prefLabel xml:lang="en">Mooring: LUCIE: Dongara Moorings (1986/7)</skos:prefLabel>
      <skos:inScheme rdf:resource="urn:marlin.csiro.au:sourceregister:conceptscheme:1.0"/>
      <skos:definition xml:lang="en">Type: Mooring Description: None</skos:definition>
      <skos:scopeNote xml:lang="en">Mooring: LUCIE: Dongara Moorings (1986/7): Type: Mooring Description: None</skos:scopeNote>
   </skos:Concept>
   <skos:Concept rdf:about="urn:marlin.csiro.au:sourceregister:concept:149">
      <skos:prefLabel xml:lang="en">Mooring: Makassar Strait Moorings (1993)</skos:prefLabel>
      <skos:inScheme rdf:resource="urn:marlin.csiro.au:sourceregister:conceptscheme:1.0"/>
      <skos:definition xml:lang="en">Type: Mooring Description: None</skos:definition>
      <skos:scopeNote xml:lang="en">Mooring: Makassar Strait Moorings (1993): Type: Mooring Description: None</skos:scopeNote>
   </skos:Concept>
   <skos:Concept rdf:about="urn:marlin.csiro.au:sourceregister:concept:150">
      <skos:prefLabel xml:lang="en">Mooring: Maluku Strait Mooring (1993)</skos:prefLabel>
      <skos:inScheme rdf:resource="urn:marlin.csiro.au:sourceregister:conceptscheme:1.0"/>
      <skos:definition xml:lang="en">Type: Mooring Description: None</skos:definition>
      <skos:scopeNote xml:lang="en">Mooring: Maluku Strait Mooring (1993): Type: Mooring Description: None</skos:scopeNote>
   </skos:Concept>
   <skos:Concept rdf:about="urn:marlin.csiro.au:sourceregister:concept:151">
      <skos:prefLabel xml:lang="en">Mooring: Mertz Polynya Moorings (1998)</skos:prefLabel>
      <skos:inScheme rdf:resource="urn:marlin.csiro.au:sourceregister:conceptscheme:1.0"/>
      <skos:definition xml:lang="en">Type: Mooring Description: None</skos:definition>
      <skos:scopeNote xml:lang="en">Mooring: Mertz Polynya Moorings (1998): Type: Mooring Description: None</skos:scopeNote>
   </skos:Concept>
   <skos:Concept rdf:about="urn:marlin.csiro.au:sourceregister:concept:152">
      <skos:prefLabel xml:lang="en">Mooring: North West Shelf Moorings (1995)</skos:prefLabel>
      <skos:inScheme rdf:resource="urn:marlin.csiro.au:sourceregister:conceptscheme:1.0"/>
      <skos:definition xml:lang="en">Type: Mooring Description: None</skos:definition>
      <skos:scopeNote xml:lang="en">Mooring: North West Shelf Moorings (1995): Type: Mooring Description: None</skos:scopeNote>
   </skos:Concept>
   <skos:Concept rdf:about="urn:marlin.csiro.au:sourceregister:concept:153">
      <skos:prefLabel xml:lang="en">Mooring: South Austr. Upwelling Moorings (1989)</skos:prefLabel>
      <skos:inScheme rdf:resource="urn:marlin.csiro.au:sourceregister:conceptscheme:1.0"/>
      <skos:definition xml:lang="en">Type: Mooring Description: None</skos:definition>
      <skos:scopeNote xml:lang="en">Mooring: South Austr. Upwelling Moorings (1989): Type: Mooring Description: None</skos:scopeNote>
   </skos:Concept>
   <skos:Concept rdf:about="urn:marlin.csiro.au:sourceregister:concept:154">
      <skos:prefLabel xml:lang="en">Mooring: S. Ocean (AUSSAF) Moorings (1991-93)</skos:prefLabel>
      <skos:inScheme rdf:resource="urn:marlin.csiro.au:sourceregister:conceptscheme:1.0"/>
      <skos:definition xml:lang="en">Type: Mooring Description: None</skos:definition>
      <skos:scopeNote xml:lang="en">Mooring: S. Ocean (AUSSAF) Moorings (1991-93): Type: Mooring Description: None</skos:scopeNote>
   </skos:Concept>
   <skos:Concept rdf:about="urn:marlin.csiro.au:sourceregister:concept:155">
      <skos:prefLabel xml:lang="en">Mooring: S. Ocean (SAFDE) Moorings (1995)</skos:prefLabel>
      <skos:inScheme rdf:resource="urn:marlin.csiro.au:sourceregister:conceptscheme:1.0"/>
      <skos:definition xml:lang="en">Type: Mooring Description: None</skos:definition>
      <skos:scopeNote xml:lang="en">Mooring: S. Ocean (SAFDE) Moorings (1995): Type: Mooring Description: None</skos:scopeNote>
   </skos:Concept>
   <skos:Concept rdf:about="urn:marlin.csiro.au:sourceregister:concept:156">
      <skos:prefLabel xml:lang="en">Mooring: SEF-Gabo Reef Moorings (1996)</skos:prefLabel>
      <skos:inScheme rdf:resource="urn:marlin.csiro.au:sourceregister:conceptscheme:1.0"/>
      <skos:definition xml:lang="en">Type: Mooring Description: None</skos:definition>
      <skos:scopeNote xml:lang="en">Mooring: SEF-Gabo Reef Moorings (1996): Type: Mooring Description: None</skos:scopeNote>
   </skos:Concept>
   <skos:Concept rdf:about="urn:marlin.csiro.au:sourceregister:concept:157">
      <skos:prefLabel xml:lang="en">Mooring: Tasmania: EZ Jarosite Mooring (1988)</skos:prefLabel>
      <skos:inScheme rdf:resource="urn:marlin.csiro.au:sourceregister:conceptscheme:1.0"/>
      <skos:definition xml:lang="en">Type: Mooring Description: None</skos:definition>
      <skos:scopeNote xml:lang="en">Mooring: Tasmania: EZ Jarosite Mooring (1988): Type: Mooring Description: None</skos:scopeNote>
   </skos:Concept>
   <skos:Concept rdf:about="urn:marlin.csiro.au:sourceregister:concept:158">
      <skos:prefLabel xml:lang="en">Mooring: PCM3 (Tasman Sea) Moorings (1991-2)</skos:prefLabel>
      <skos:inScheme rdf:resource="urn:marlin.csiro.au:sourceregister:conceptscheme:1.0"/>
      <skos:definition xml:lang="en">Type: Mooring Description: None</skos:definition>
      <skos:scopeNote xml:lang="en">Mooring: PCM3 (Tasman Sea) Moorings (1991-2): Type: Mooring Description: None</skos:scopeNote>
   </skos:Concept>
   <skos:Concept rdf:about="urn:marlin.csiro.au:sourceregister:concept:159">
      <skos:prefLabel xml:lang="en">Mooring: Timor Sea Moorings (1988)</skos:prefLabel>
      <skos:inScheme rdf:resource="urn:marlin.csiro.au:sourceregister:conceptscheme:1.0"/>
      <skos:definition xml:lang="en">Type: Mooring Description: None</skos:definition>
      <skos:scopeNote xml:lang="en">Mooring: Timor Sea Moorings (1988): Type: Mooring Description: None</skos:scopeNote>
   </skos:Concept>
   <skos:Concept rdf:about="urn:marlin.csiro.au:sourceregister:concept:160">
      <skos:prefLabel xml:lang="en">Mooring: Tasmania: East Coast Moorings (1988)</skos:prefLabel>
      <skos:inScheme rdf:resource="urn:marlin.csiro.au:sourceregister:conceptscheme:1.0"/>
      <skos:definition xml:lang="en">Type: Mooring Description: None</skos:definition>
      <skos:scopeNote xml:lang="en">Mooring: Tasmania: East Coast Moorings (1988): Type: Mooring Description: None</skos:scopeNote>
   </skos:Concept>
   <skos:Concept rdf:about="urn:marlin.csiro.au:sourceregister:concept:161">
      <skos:prefLabel xml:lang="en">Mooring: Tasmania: West Coast Moorings (1988)</skos:prefLabel>
      <skos:inScheme rdf:resource="urn:marlin.csiro.au:sourceregister:conceptscheme:1.0"/>
      <skos:definition xml:lang="en">Type: Mooring Description: None</skos:definition>
      <skos:scopeNote xml:lang="en">Mooring: Tasmania: West Coast Moorings (1988): Type: Mooring Description: None</skos:scopeNote>
   </skos:Concept>
   <skos:Concept rdf:about="urn:marlin.csiro.au:sourceregister:concept:162">
      <skos:prefLabel xml:lang="en">Mooring: TOGA Equatorial Pacific Mooring (1990)</skos:prefLabel>
      <skos:inScheme rdf:resource="urn:marlin.csiro.au:sourceregister:conceptscheme:1.0"/>
      <skos:definition xml:lang="en">Type: Mooring Description: None</skos:definition>
      <skos:scopeNote xml:lang="en">Mooring: TOGA Equatorial Pacific Mooring (1990): Type: Mooring Description: None</skos:scopeNote>
   </skos:Concept>
   <skos:Concept rdf:about="urn:marlin.csiro.au:sourceregister:concept:163">
      <skos:prefLabel xml:lang="en">Mooring: TROPICS 97 - Sepik River Moorings (1997)</skos:prefLabel>
      <skos:inScheme rdf:resource="urn:marlin.csiro.au:sourceregister:conceptscheme:1.0"/>
      <skos:definition xml:lang="en">Type: Mooring Description: None</skos:definition>
      <skos:scopeNote xml:lang="en">Mooring: TROPICS 97 - Sepik River Moorings (1997): Type: Mooring Description: None</skos:scopeNote>
   </skos:Concept>
   <skos:Concept rdf:about="urn:marlin.csiro.au:sourceregister:concept:164">
      <skos:prefLabel xml:lang="en">Mooring: West Australian Basin Moorings (1995)</skos:prefLabel>
      <skos:inScheme rdf:resource="urn:marlin.csiro.au:sourceregister:conceptscheme:1.0"/>
      <skos:definition xml:lang="en">Type: Mooring Description: None</skos:definition>
      <skos:scopeNote xml:lang="en">Mooring: West Australian Basin Moorings (1995): Type: Mooring Description: None</skos:scopeNote>
   </skos:Concept>
   <skos:Concept rdf:about="urn:marlin.csiro.au:sourceregister:concept:165">
      <skos:prefLabel xml:lang="en">Mooring: SAZ Southern Ocean Moorings (1997-8)</skos:prefLabel>
      <skos:inScheme rdf:resource="urn:marlin.csiro.au:sourceregister:conceptscheme:1.0"/>
      <skos:definition xml:lang="en">Type: Mooring Description: None</skos:definition>
      <skos:scopeNote xml:lang="en">Mooring: SAZ Southern Ocean Moorings (1997-8): Type: Mooring Description: None</skos:scopeNote>
   </skos:Concept>
   <skos:Concept rdf:about="urn:marlin.csiro.au:sourceregister:concept:166">
      <skos:prefLabel xml:lang="en">Mooring: Evans Head Upwelling Moorings (1989)</skos:prefLabel>
      <skos:inScheme rdf:resource="urn:marlin.csiro.au:sourceregister:conceptscheme:1.0"/>
      <skos:definition xml:lang="en">Type: Mooring Description: None</skos:definition>
      <skos:scopeNote xml:lang="en">Mooring: Evans Head Upwelling Moorings (1989): Type: Mooring Description: None</skos:scopeNote>
   </skos:Concept>
   <skos:Concept rdf:about="urn:marlin.csiro.au:sourceregister:concept:167">
      <skos:prefLabel xml:lang="en">Mooring: Bass Strait Moorings - UNSW (1991)</skos:prefLabel>
      <skos:inScheme rdf:resource="urn:marlin.csiro.au:sourceregister:conceptscheme:1.0"/>
      <skos:definition xml:lang="en">Type: Mooring Description: None</skos:definition>
      <skos:scopeNote xml:lang="en">Mooring: Bass Strait Moorings - UNSW (1991): Type: Mooring Description: None</skos:scopeNote>
   </skos:Concept>
   <skos:Concept rdf:about="urn:marlin.csiro.au:sourceregister:concept:168">
      <skos:prefLabel xml:lang="en">Ship: Soviet Fisheries vessels  (1965-78)</skos:prefLabel>
      <skos:inScheme rdf:resource="urn:marlin.csiro.au:sourceregister:conceptscheme:1.0"/>
      <skos:definition xml:lang="en">Type: Ship Description: Russian Fishery Vessels - various</skos:definition>
      <skos:scopeNote xml:lang="en">Ship: Soviet Fisheries vessels  (1965-78): Type: Ship Description: Russian Fishery Vessels - various</skos:scopeNote>
   </skos:Concept>
   <skos:Concept rdf:about="urn:marlin.csiro.au:sourceregister:concept:169">
      <skos:prefLabel xml:lang="en">Ship: Jacqueline D</skos:prefLabel>
      <skos:inScheme rdf:resource="urn:marlin.csiro.au:sourceregister:conceptscheme:1.0"/>
      <skos:definition xml:lang="en">Type: Ship Description: Chartered commercial prawn trawler
Hull material: timber
Length: 17.4m
Built: 1969
Engine: 225kw	
Typical trawl speed: 3.2 knots</skos:definition>
      <skos:scopeNote xml:lang="en">Ship: Jacqueline D: Type: Ship Description: Chartered commercial prawn trawler
Hull material: timber
Length: 17.4m
Built: 1969
Engine: 225kw	
Typical trawl speed: 3.2 knots</skos:scopeNote>
   </skos:Concept>
   <skos:Concept rdf:about="urn:marlin.csiro.au:sourceregister:concept:170">
      <skos:prefLabel xml:lang="en">Ship: Ben Boyd</skos:prefLabel>
      <skos:inScheme rdf:resource="urn:marlin.csiro.au:sourceregister:conceptscheme:1.0"/>
      <skos:definition xml:lang="en">Type: Ship Description: None</skos:definition>
      <skos:scopeNote xml:lang="en">Ship: Ben Boyd: Type: Ship Description: None</skos:scopeNote>
   </skos:Concept>
   <skos:Concept rdf:about="urn:marlin.csiro.au:sourceregister:concept:171">
      <skos:prefLabel xml:lang="en">Ship: Erin Jay</skos:prefLabel>
      <skos:inScheme rdf:resource="urn:marlin.csiro.au:sourceregister:conceptscheme:1.0"/>
      <skos:definition xml:lang="en">Type: Ship Description: None</skos:definition>
      <skos:scopeNote xml:lang="en">Ship: Erin Jay: Type: Ship Description: None</skos:scopeNote>
   </skos:Concept>
   <skos:Concept rdf:about="urn:marlin.csiro.au:sourceregister:concept:172">
      <skos:prefLabel xml:lang="en">Ship: Imlay</skos:prefLabel>
      <skos:inScheme rdf:resource="urn:marlin.csiro.au:sourceregister:conceptscheme:1.0"/>
      <skos:definition xml:lang="en">Type: Ship Description: None</skos:definition>
      <skos:scopeNote xml:lang="en">Ship: Imlay: Type: Ship Description: None</skos:scopeNote>
   </skos:Concept>
   <skos:Concept rdf:about="urn:marlin.csiro.au:sourceregister:concept:173">
      <skos:prefLabel xml:lang="en">Ship: Starfire</skos:prefLabel>
      <skos:inScheme rdf:resource="urn:marlin.csiro.au:sourceregister:conceptscheme:1.0"/>
      <skos:definition xml:lang="en">Type: Ship Description: None</skos:definition>
      <skos:scopeNote xml:lang="en">Ship: Starfire: Type: Ship Description: None</skos:scopeNote>
   </skos:Concept>
   <skos:Concept rdf:about="urn:marlin.csiro.au:sourceregister:concept:174">
      <skos:prefLabel xml:lang="en">Ship: Celtic Rose</skos:prefLabel>
      <skos:inScheme rdf:resource="urn:marlin.csiro.au:sourceregister:conceptscheme:1.0"/>
      <skos:definition xml:lang="en">Type: Ship Description: None</skos:definition>
      <skos:scopeNote xml:lang="en">Ship: Celtic Rose: Type: Ship Description: None</skos:scopeNote>
   </skos:Concept>
   <skos:Concept rdf:about="urn:marlin.csiro.au:sourceregister:concept:175">
      <skos:prefLabel xml:lang="en">Coastal Station: Macquarie Harbour</skos:prefLabel>
      <skos:inScheme rdf:resource="urn:marlin.csiro.au:sourceregister:conceptscheme:1.0"/>
      <skos:definition xml:lang="en">Type: Coastal Station Description: None</skos:definition>
      <skos:scopeNote xml:lang="en">Coastal Station: Macquarie Harbour: Type: Coastal Station Description: None</skos:scopeNote>
   </skos:Concept>
   <skos:Concept rdf:about="urn:marlin.csiro.au:sourceregister:concept:176">
      <skos:prefLabel xml:lang="en">Coastal Station: Storm Bay</skos:prefLabel>
      <skos:inScheme rdf:resource="urn:marlin.csiro.au:sourceregister:conceptscheme:1.0"/>
      <skos:definition xml:lang="en">Type: Coastal Station Description: None</skos:definition>
      <skos:scopeNote xml:lang="en">Coastal Station: Storm Bay: Type: Coastal Station Description: None</skos:scopeNote>
   </skos:Concept>
   <skos:Concept rdf:about="urn:marlin.csiro.au:sourceregister:concept:177">
      <skos:prefLabel xml:lang="en">Mooring: S. Ocean (AMISOR) Moorings (2000-2002)</skos:prefLabel>
      <skos:inScheme rdf:resource="urn:marlin.csiro.au:sourceregister:conceptscheme:1.0"/>
      <skos:definition xml:lang="en">Type: Mooring Description: None</skos:definition>
      <skos:scopeNote xml:lang="en">Mooring: S. Ocean (AMISOR) Moorings (2000-2002): Type: Mooring Description: None</skos:scopeNote>
   </skos:Concept>
   <skos:Concept rdf:about="urn:marlin.csiro.au:sourceregister:concept:179">
      <skos:prefLabel xml:lang="en">Model: ACOM</skos:prefLabel>
      <skos:inScheme rdf:resource="urn:marlin.csiro.au:sourceregister:conceptscheme:1.0"/>
      <skos:definition xml:lang="en">Type: Model Description: Australian Community Ocean Model 
</skos:definition>
      <skos:scopeNote xml:lang="en">Model: ACOM: Type: Model Description: Australian Community Ocean Model 
</skos:scopeNote>
   </skos:Concept>
   <skos:Concept rdf:about="urn:marlin.csiro.au:sourceregister:concept:178">
      <skos:prefLabel xml:lang="en">Model: MECO</skos:prefLabel>
      <skos:inScheme rdf:resource="urn:marlin.csiro.au:sourceregister:conceptscheme:1.0"/>
      <skos:definition xml:lang="en">Type: Model Description: Model for Estuaries and Coastal Ocean</skos:definition>
      <skos:scopeNote xml:lang="en">Model: MECO: Type: Model Description: Model for Estuaries and Coastal Ocean</skos:scopeNote>
   </skos:Concept>
   <skos:Concept rdf:about="urn:marlin.csiro.au:sourceregister:concept:180">
      <skos:prefLabel xml:lang="en">Ship: Peterson</skos:prefLabel>
      <skos:inScheme rdf:resource="urn:marlin.csiro.au:sourceregister:conceptscheme:1.0"/>
      <skos:definition xml:lang="en">Type: Ship Description: 40 metre factory freezer stern trawler</skos:definition>
      <skos:scopeNote xml:lang="en">Ship: Peterson: Type: Ship Description: 40 metre factory freezer stern trawler</skos:scopeNote>
   </skos:Concept>
   <skos:Concept rdf:about="urn:marlin.csiro.au:sourceregister:concept:181">
      <skos:prefLabel xml:lang="en">Ship: Aoraki</skos:prefLabel>
      <skos:inScheme rdf:resource="urn:marlin.csiro.au:sourceregister:conceptscheme:1.0"/>
      <skos:definition xml:lang="en">Type: Ship Description: Factory freezer stern trawler. Length overall 67.5 metres.</skos:definition>
      <skos:scopeNote xml:lang="en">Ship: Aoraki: Type: Ship Description: Factory freezer stern trawler. Length overall 67.5 metres.</skos:scopeNote>
   </skos:Concept>
   <skos:Concept rdf:about="urn:marlin.csiro.au:sourceregister:concept:182">
      <skos:prefLabel xml:lang="en">Ship: Ocean Dawn</skos:prefLabel>
      <skos:inScheme rdf:resource="urn:marlin.csiro.au:sourceregister:conceptscheme:1.0"/>
      <skos:definition xml:lang="en">Type: Ship Description: 64 meter factory freezer stern trawler</skos:definition>
      <skos:scopeNote xml:lang="en">Ship: Ocean Dawn: Type: Ship Description: 64 meter factory freezer stern trawler</skos:scopeNote>
   </skos:Concept>
   <skos:Concept rdf:about="urn:marlin.csiro.au:sourceregister:concept:183">
      <skos:prefLabel xml:lang="en">Ship: Dell Richey II</skos:prefLabel>
      <skos:inScheme rdf:resource="urn:marlin.csiro.au:sourceregister:conceptscheme:1.0"/>
      <skos:definition xml:lang="en">Type: Ship Description: Fishing vessel, steel LOA 24.95m, Draft 2.6m, Beam 7.63m, Endurance 4000nm, Accomodates 12</skos:definition>
      <skos:scopeNote xml:lang="en">Ship: Dell Richey II: Type: Ship Description: Fishing vessel, steel LOA 24.95m, Draft 2.6m, Beam 7.63m, Endurance 4000nm, Accomodates 12</skos:scopeNote>
   </skos:Concept>
   <skos:Concept rdf:about="urn:marlin.csiro.au:sourceregister:concept:186">
      <skos:prefLabel xml:lang="en">Ship: Ali Baba</skos:prefLabel>
      <skos:inScheme rdf:resource="urn:marlin.csiro.au:sourceregister:conceptscheme:1.0"/>
      <skos:definition xml:lang="en">Type: Ship Description: Chartered commercial prawn trawler.
Hull material: timber
Length: 16.6m                                 
Built: 1971
Engine: 112kw	
Transit speed: 8.7 knots	
Trawl speed: 3.0 knots
</skos:definition>
      <skos:scopeNote xml:lang="en">Ship: Ali Baba: Type: Ship Description: Chartered commercial prawn trawler.
Hull material: timber
Length: 16.6m                                 
Built: 1971
Engine: 112kw	
Transit speed: 8.7 knots	
Trawl speed: 3.0 knots
</skos:scopeNote>
   </skos:Concept>
   <skos:Concept rdf:about="urn:marlin.csiro.au:sourceregister:concept:188">
      <skos:prefLabel xml:lang="en">Ship: Mesocat</skos:prefLabel>
      <skos:inScheme rdf:resource="urn:marlin.csiro.au:sourceregister:conceptscheme:1.0"/>
      <skos:definition xml:lang="en">Type: Ship Description: M.V. Mesocat 8.0m twin hulled aluminium catamaran designed and built by Gavin Mair Marine in 1995. Water line length 7.1m beam 3.5m max displacement 6.0 Tonnes. Powered by twin 225 Hp two stroke outboard engines.  Survey Class 2C.</skos:definition>
      <skos:scopeNote xml:lang="en">Ship: Mesocat: Type: Ship Description: M.V. Mesocat 8.0m twin hulled aluminium catamaran designed and built by Gavin Mair Marine in 1995. Water line length 7.1m beam 3.5m max displacement 6.0 Tonnes. Powered by twin 225 Hp two stroke outboard engines.  Survey Class 2C.</skos:scopeNote>
   </skos:Concept>
   <skos:Concept rdf:about="urn:marlin.csiro.au:sourceregister:concept:190">
      <skos:prefLabel xml:lang="en">Ship: Marion Dufresne (RV)</skos:prefLabel>
      <skos:inScheme rdf:resource="urn:marlin.csiro.au:sourceregister:conceptscheme:1.0"/>
      <skos:definition xml:lang="en">Type: Ship Description: Marion Dufresne is a general-purpose ship. Built in 1995, it provides two principal functions:&lt;BR&gt;The logistics of the French southern islands: Crozet, Kerguelen, Amsterdam, under the responsibility of the TAAF&lt;BR&gt;Oceanographical research on the major part of the oceans, under the responsibility of the IPEV</skos:definition>
      <skos:scopeNote xml:lang="en">Ship: Marion Dufresne (RV): Type: Ship Description: Marion Dufresne is a general-purpose ship. Built in 1995, it provides two principal functions:&lt;BR&gt;The logistics of the French southern islands: Crozet, Kerguelen, Amsterdam, under the responsibility of the TAAF&lt;BR&gt;Oceanographical research on the major part of the oceans, under the responsibility of the IPEV</skos:scopeNote>
   </skos:Concept>
   <skos:Concept rdf:about="urn:marlin.csiro.au:sourceregister:concept:192">
      <skos:prefLabel xml:lang="en">Ship: Lady Basten</skos:prefLabel>
      <skos:inScheme rdf:resource="urn:marlin.csiro.au:sourceregister:conceptscheme:1.0"/>
      <skos:definition xml:lang="en">Type: Ship Description: Australian Institute of Marine Science Research Vessel 1978 -</skos:definition>
      <skos:scopeNote xml:lang="en">Ship: Lady Basten: Type: Ship Description: Australian Institute of Marine Science Research Vessel 1978 -</skos:scopeNote>
   </skos:Concept>
   <skos:Concept rdf:about="urn:marlin.csiro.au:sourceregister:concept:218">
      <skos:prefLabel xml:lang="en">Model: BCCR-BCM2.0, Norway</skos:prefLabel>
      <skos:inScheme rdf:resource="urn:marlin.csiro.au:sourceregister:conceptscheme:1.0"/>
      <skos:definition xml:lang="en">Type: Model Description: Bjerknes Centre for Climate Research (BCCR), Univ. of Bergen, Norway
BCCR-BCM2.0, Norway
Bergen Climate Model (BCM) Version 2
Atmosphere/land: ARPEGE-CLIMAT Version 3
Ocean/sea ice: NERSC largely modified version of MICOM Version 2.8, with
NERSC Sea Ice Model
First used in a published application 2005</skos:definition>
      <skos:scopeNote xml:lang="en">Model: BCCR-BCM2.0, Norway: Type: Model Description: Bjerknes Centre for Climate Research (BCCR), Univ. of Bergen, Norway
BCCR-BCM2.0, Norway
Bergen Climate Model (BCM) Version 2
Atmosphere/land: ARPEGE-CLIMAT Version 3
Ocean/sea ice: NERSC largely modified version of MICOM Version 2.8, with
NERSC Sea Ice Model
First used in a published application 2005</skos:scopeNote>
   </skos:Concept>
   <skos:Concept rdf:about="urn:marlin.csiro.au:sourceregister:concept:219">
      <skos:prefLabel xml:lang="en">Model: CCCMA CGCM3.1 (t47), Canada</skos:prefLabel>
      <skos:inScheme rdf:resource="urn:marlin.csiro.au:sourceregister:conceptscheme:1.0"/>
      <skos:definition xml:lang="en">Type: Model Description: CCCMA CGCM3.1 (t47), Canada
Canadian Centre for Climate Modelling and Analysis (CCCma) Coupled Global Climate Model (CGCM3)Version 3 
The T47 version has a surface grid whose spatial resolotion is roughly 3.75 degrees lat/lon and 31 levels in the vertical. The ocean grid shares the same land mask as the atmsosphere, but has four ocean grid cells underlying every atmospheric grid cell. The ocean resolution in this case is roughly 1.85 degrees, with 29 levels in the vertical.</skos:definition>
      <skos:scopeNote xml:lang="en">Model: CCCMA CGCM3.1 (t47), Canada: Type: Model Description: CCCMA CGCM3.1 (t47), Canada
Canadian Centre for Climate Modelling and Analysis (CCCma) Coupled Global Climate Model (CGCM3)Version 3 
The T47 version has a surface grid whose spatial resolotion is roughly 3.75 degrees lat/lon and 31 levels in the vertical. The ocean grid shares the same land mask as the atmsosphere, but has four ocean grid cells underlying every atmospheric grid cell. The ocean resolution in this case is roughly 1.85 degrees, with 29 levels in the vertical.</skos:scopeNote>
   </skos:Concept>
   <skos:Concept rdf:about="urn:marlin.csiro.au:sourceregister:concept:221">
      <skos:prefLabel xml:lang="en">Model: CCCMA CGCM3.1 (t63), Canada</skos:prefLabel>
      <skos:inScheme rdf:resource="urn:marlin.csiro.au:sourceregister:conceptscheme:1.0"/>
      <skos:definition xml:lang="en">Type: Model Description: CCCMA CGCM3.1 (t63), Canada
Canadian Centre for Climate Modelling and Analysis (CCCma) Coupled Global Climate Model (CGCM3)Version 3 
The T63 version has a surface grid whose spatial resolution is roughly 2.8 degrees lat/lon and 31 levels in the vertical. As before the ocean grid shares the same land mask as the atmosphere, but in this case there are 6 ocean grids underlying every atmospheric grid cell. The ocean resolution is therefore approximately 1.4 degrees in longitude and 0.94 degrees in latitude. This provides slightly better resolution of zonal currents in the Tropics, more nearly isotropic resolution at mid latitudes, and somewhat reduced probles with converging meridians in the Arctic.</skos:definition>
      <skos:scopeNote xml:lang="en">Model: CCCMA CGCM3.1 (t63), Canada: Type: Model Description: CCCMA CGCM3.1 (t63), Canada
Canadian Centre for Climate Modelling and Analysis (CCCma) Coupled Global Climate Model (CGCM3)Version 3 
The T63 version has a surface grid whose spatial resolution is roughly 2.8 degrees lat/lon and 31 levels in the vertical. As before the ocean grid shares the same land mask as the atmosphere, but in this case there are 6 ocean grids underlying every atmospheric grid cell. The ocean resolution is therefore approximately 1.4 degrees in longitude and 0.94 degrees in latitude. This provides slightly better resolution of zonal currents in the Tropics, more nearly isotropic resolution at mid latitudes, and somewhat reduced probles with converging meridians in the Arctic.</skos:scopeNote>
   </skos:Concept>
   <skos:Concept rdf:about="urn:marlin.csiro.au:sourceregister:concept:276">
      <skos:prefLabel xml:lang="en">Coastal Station: Cape Meares</skos:prefLabel>
      <skos:inScheme rdf:resource="urn:marlin.csiro.au:sourceregister:conceptscheme:1.0"/>
      <skos:definition xml:lang="en">Type: Coastal Station Description: Cape Meares - Oregon
(45° N, 124° W)
No longer used? Replaced by Trinidad Head, (California)</skos:definition>
      <skos:scopeNote xml:lang="en">Coastal Station: Cape Meares: Type: Coastal Station Description: Cape Meares - Oregon
(45° N, 124° W)
No longer used? Replaced by Trinidad Head, (California)</skos:scopeNote>
   </skos:Concept>
   <skos:Concept rdf:about="urn:marlin.csiro.au:sourceregister:concept:280">
      <skos:prefLabel xml:lang="en">Observational: Aspendale - GASLAB</skos:prefLabel>
      <skos:inScheme rdf:resource="urn:marlin.csiro.au:sourceregister:conceptscheme:1.0"/>
      <skos:definition xml:lang="en">Type: Observational Description: CSIRO - Marine and Atmospheric Research division Aspendale,
GASLAB Global Atmospheric Laboratory </skos:definition>
      <skos:scopeNote xml:lang="en">Observational: Aspendale - GASLAB: Type: Observational Description: CSIRO - Marine and Atmospheric Research division Aspendale,
GASLAB Global Atmospheric Laboratory </skos:scopeNote>
   </skos:Concept>
   <skos:Concept rdf:about="urn:marlin.csiro.au:sourceregister:concept:288">
      <skos:prefLabel xml:lang="en">Model: SIMHYD</skos:prefLabel>
      <skos:inScheme rdf:resource="urn:marlin.csiro.au:sourceregister:conceptscheme:1.0"/>
      <skos:definition xml:lang="en">Type: Model Description: Co-operative Research Center for Catchment Hydrology - Hydrological Simulator</skos:definition>
      <skos:scopeNote xml:lang="en">Model: SIMHYD: Type: Model Description: Co-operative Research Center for Catchment Hydrology - Hydrological Simulator</skos:scopeNote>
   </skos:Concept>
   <skos:Concept rdf:about="urn:marlin.csiro.au:sourceregister:concept:289">
      <skos:prefLabel xml:lang="en">Model: SWAN</skos:prefLabel>
      <skos:inScheme rdf:resource="urn:marlin.csiro.au:sourceregister:conceptscheme:1.0"/>
      <skos:definition xml:lang="en">Type: Model Description: None</skos:definition>
      <skos:scopeNote xml:lang="en">Model: SWAN: Type: Model Description: None</skos:scopeNote>
   </skos:Concept>
   <skos:Concept rdf:about="urn:marlin.csiro.au:sourceregister:concept:277">
      <skos:prefLabel xml:lang="en">Coastal Station: Macquarie Island</skos:prefLabel>
      <skos:inScheme rdf:resource="urn:marlin.csiro.au:sourceregister:conceptscheme:1.0"/>
      <skos:definition xml:lang="en">Type: Coastal Station Description: Macquarie Island Station Antarctica 
54°30' S 158°57' E</skos:definition>
      <skos:scopeNote xml:lang="en">Coastal Station: Macquarie Island: Type: Coastal Station Description: Macquarie Island Station Antarctica 
54°30' S 158°57' E</skos:scopeNote>
   </skos:Concept>
   <skos:Concept rdf:about="urn:marlin.csiro.au:sourceregister:concept:286">
      <skos:prefLabel xml:lang="en">Ship: Lucky S</skos:prefLabel>
      <skos:inScheme rdf:resource="urn:marlin.csiro.au:sourceregister:conceptscheme:1.0"/>
      <skos:definition xml:lang="en">Type: Ship Description: Fishing Vessel from Port Lincon
</skos:definition>
      <skos:scopeNote xml:lang="en">Ship: Lucky S: Type: Ship Description: Fishing Vessel from Port Lincon
</skos:scopeNote>
   </skos:Concept>
   <skos:Concept rdf:about="urn:marlin.csiro.au:sourceregister:concept:292">
      <skos:prefLabel xml:lang="en">Ship: Hai Kung (RV)</skos:prefLabel>
      <skos:inScheme rdf:resource="urn:marlin.csiro.au:sourceregister:conceptscheme:1.0"/>
      <skos:definition xml:lang="en">Type: Ship Description: Deep sea trawling and fish research vessel.
Home Port: Keelung - Taiwan
711.58 Tonnes
56.6 m LOA</skos:definition>
      <skos:scopeNote xml:lang="en">Ship: Hai Kung (RV): Type: Ship Description: Deep sea trawling and fish research vessel.
Home Port: Keelung - Taiwan
711.58 Tonnes
56.6 m LOA</skos:scopeNote>
   </skos:Concept>
   <skos:Concept rdf:about="urn:marlin.csiro.au:sourceregister:concept:294">
      <skos:prefLabel xml:lang="en">Ship: Swordfish</skos:prefLabel>
      <skos:inScheme rdf:resource="urn:marlin.csiro.au:sourceregister:conceptscheme:1.0"/>
      <skos:definition xml:lang="en">Type: Ship Description: None</skos:definition>
      <skos:scopeNote xml:lang="en">Ship: Swordfish: Type: Ship Description: None</skos:scopeNote>
   </skos:Concept>
   <skos:Concept rdf:about="urn:marlin.csiro.au:sourceregister:concept:278">
      <skos:prefLabel xml:lang="en">Locality: Otway Basin</skos:prefLabel>
      <skos:inScheme rdf:resource="urn:marlin.csiro.au:sourceregister:conceptscheme:1.0"/>
      <skos:definition xml:lang="en">Type: Locality Description: Otway Basin</skos:definition>
      <skos:scopeNote xml:lang="en">Locality: Otway Basin: Type: Locality Description: Otway Basin</skos:scopeNote>
   </skos:Concept>
   <skos:Concept rdf:about="urn:marlin.csiro.au:sourceregister:concept:285">
      <skos:prefLabel xml:lang="en">Coastal Station: Hobart Wharf (CSIRO Labs)</skos:prefLabel>
      <skos:inScheme rdf:resource="urn:marlin.csiro.au:sourceregister:conceptscheme:1.0"/>
      <skos:definition xml:lang="en">Type: Coastal Station Description: None</skos:definition>
      <skos:scopeNote xml:lang="en">Coastal Station: Hobart Wharf (CSIRO Labs): Type: Coastal Station Description: None</skos:scopeNote>
   </skos:Concept>
   <skos:Concept rdf:about="urn:marlin.csiro.au:sourceregister:concept:295">
      <skos:prefLabel xml:lang="en">Ship: Febrina</skos:prefLabel>
      <skos:inScheme rdf:resource="urn:marlin.csiro.au:sourceregister:conceptscheme:1.0"/>
      <skos:definition xml:lang="en">Type: Ship Description: None</skos:definition>
      <skos:scopeNote xml:lang="en">Ship: Febrina: Type: Ship Description: None</skos:scopeNote>
   </skos:Concept>
   <skos:Concept rdf:about="urn:marlin.csiro.au:sourceregister:concept:282">
      <skos:prefLabel xml:lang="en">Ship: Saxon Onward</skos:prefLabel>
      <skos:inScheme rdf:resource="urn:marlin.csiro.au:sourceregister:conceptscheme:1.0"/>
      <skos:definition xml:lang="en">Type: Ship Description: Fishing Vessel Saxon Onward</skos:definition>
      <skos:scopeNote xml:lang="en">Ship: Saxon Onward: Type: Ship Description: Fishing Vessel Saxon Onward</skos:scopeNote>
   </skos:Concept>
   <skos:Concept rdf:about="urn:marlin.csiro.au:sourceregister:concept:284">
      <skos:prefLabel xml:lang="en">Ship: Rehua</skos:prefLabel>
      <skos:inScheme rdf:resource="urn:marlin.csiro.au:sourceregister:conceptscheme:1.0"/>
      <skos:definition xml:lang="en">Type: Ship Description: Fishing Vessel Rehua
</skos:definition>
      <skos:scopeNote xml:lang="en">Ship: Rehua: Type: Ship Description: Fishing Vessel Rehua
</skos:scopeNote>
   </skos:Concept>
   <skos:Concept rdf:about="urn:marlin.csiro.au:sourceregister:concept:287">
      <skos:prefLabel xml:lang="en">Mooring: WEPOCS Moorings</skos:prefLabel>
      <skos:inScheme rdf:resource="urn:marlin.csiro.au:sourceregister:conceptscheme:1.0"/>
      <skos:definition xml:lang="en">Type: Mooring Description: Western Equatorial Pacific Ocean Climate Studies (WEPOCS) Moorings</skos:definition>
      <skos:scopeNote xml:lang="en">Mooring: WEPOCS Moorings: Type: Mooring Description: Western Equatorial Pacific Ocean Climate Studies (WEPOCS) Moorings</skos:scopeNote>
   </skos:Concept>
   <skos:Concept rdf:about="urn:marlin.csiro.au:sourceregister:concept:293">
      <skos:prefLabel xml:lang="en">Ship: Coral Reeftel</skos:prefLabel>
      <skos:inScheme rdf:resource="urn:marlin.csiro.au:sourceregister:conceptscheme:1.0"/>
      <skos:definition xml:lang="en">Type: Ship Description: A catamaran, chartered by the Australian Fiseries Service.
Previously a Marlin fishery mother-ship in Cairns.</skos:definition>
      <skos:scopeNote xml:lang="en">Ship: Coral Reeftel: Type: Ship Description: A catamaran, chartered by the Australian Fiseries Service.
Previously a Marlin fishery mother-ship in Cairns.</skos:scopeNote>
   </skos:Concept>
   <skos:Concept rdf:about="urn:marlin.csiro.au:sourceregister:concept:283">
      <skos:prefLabel xml:lang="en">Ship: Riba 1</skos:prefLabel>
      <skos:inScheme rdf:resource="urn:marlin.csiro.au:sourceregister:conceptscheme:1.0"/>
      <skos:definition xml:lang="en">Type: Ship Description: Fishing Vessel Riba 1
</skos:definition>
      <skos:scopeNote xml:lang="en">Ship: Riba 1: Type: Ship Description: Fishing Vessel Riba 1
</skos:scopeNote>
   </skos:Concept>
   <skos:Concept rdf:about="urn:marlin.csiro.au:sourceregister:concept:296">
      <skos:prefLabel xml:lang="en">Ship: Flamingo Bay</skos:prefLabel>
      <skos:inScheme rdf:resource="urn:marlin.csiro.au:sourceregister:conceptscheme:1.0"/>
      <skos:definition xml:lang="en">Type: Ship Description: Fishing vessel</skos:definition>
      <skos:scopeNote xml:lang="en">Ship: Flamingo Bay: Type: Ship Description: Fishing vessel</skos:scopeNote>
   </skos:Concept>
   <skos:Concept rdf:about="urn:marlin.csiro.au:sourceregister:concept:279">
      <skos:prefLabel xml:lang="en">Ship: Cape Pillar</skos:prefLabel>
      <skos:inScheme rdf:resource="urn:marlin.csiro.au:sourceregister:conceptscheme:1.0"/>
      <skos:definition xml:lang="en">Type: Ship Description: Vessel Details copied from
http://www.researchvessels.org/ship_info_display.asp?shipID=139
12 August 2008:
Country:  	  Australia  	
NODC Code:	09CP
Owner: 	
Operator: 	Department of Transport and Communications
Address: 	Department of Transport and Communications
Adelaide Street PO Box 10000
Brisbane, Qld. 4000 Australia
Year Built: 	1964	
Main Dimensions
  	Length OA: 	73.06  m
  	Breadth: 	12.72  m
  	Freeboard to working deck: 	2.7  m
  	Max. draft: 	4.24  m</skos:definition>
      <skos:scopeNote xml:lang="en">Ship: Cape Pillar: Type: Ship Description: Vessel Details copied from
http://www.researchvessels.org/ship_info_display.asp?shipID=139
12 August 2008:
Country:  	  Australia  	
NODC Code:	09CP
Owner: 	
Operator: 	Department of Transport and Communications
Address: 	Department of Transport and Communications
Adelaide Street PO Box 10000
Brisbane, Qld. 4000 Australia
Year Built: 	1964	
Main Dimensions
  	Length OA: 	73.06  m
  	Breadth: 	12.72  m
  	Freeboard to working deck: 	2.7  m
  	Max. draft: 	4.24  m</skos:scopeNote>
   </skos:Concept>
   <skos:Concept rdf:about="urn:marlin.csiro.au:sourceregister:concept:281">
      <skos:prefLabel xml:lang="en">Ship: Dell Richey</skos:prefLabel>
      <skos:inScheme rdf:resource="urn:marlin.csiro.au:sourceregister:conceptscheme:1.0"/>
      <skos:definition xml:lang="en">Type: Ship Description: Fishing Vessel Dell Richey, typically operates from Tasmania.</skos:definition>
      <skos:scopeNote xml:lang="en">Ship: Dell Richey: Type: Ship Description: Fishing Vessel Dell Richey, typically operates from Tasmania.</skos:scopeNote>
   </skos:Concept>
   <skos:Concept rdf:about="urn:marlin.csiro.au:sourceregister:concept:290">
      <skos:prefLabel xml:lang="en">Model: Xbeach</skos:prefLabel>
      <skos:inScheme rdf:resource="urn:marlin.csiro.au:sourceregister:conceptscheme:1.0"/>
      <skos:definition xml:lang="en">Type: Model Description: None</skos:definition>
      <skos:scopeNote xml:lang="en">Model: Xbeach: Type: Model Description: None</skos:scopeNote>
   </skos:Concept>
   <skos:Concept rdf:about="urn:marlin.csiro.au:sourceregister:concept:291">
      <skos:prefLabel xml:lang="en">Ship: Thomas G Thompson (RV)</skos:prefLabel>
      <skos:inScheme rdf:resource="urn:marlin.csiro.au:sourceregister:conceptscheme:1.0"/>
      <skos:definition xml:lang="en">Type: Ship Description: The R/V THOMAS G. THOMPSON (AGOR-23) was constructed by Halter Marine
and funded by the U.S. Navy. The vessel was delivered to ONR on 8 July 1991
and is operated by the University of Washington, under a Charter Party Agreement,
on behalf of NORCOR. The R/V THOMPSON is a thoroughly modern vessel capable of
multidisciplinary research in most oceans of the world.</skos:definition>
      <skos:scopeNote xml:lang="en">Ship: Thomas G Thompson (RV): Type: Ship Description: The R/V THOMAS G. THOMPSON (AGOR-23) was constructed by Halter Marine
and funded by the U.S. Navy. The vessel was delivered to ONR on 8 July 1991
and is operated by the University of Washington, under a Charter Party Agreement,
on behalf of NORCOR. The R/V THOMPSON is a thoroughly modern vessel capable of
multidisciplinary research in most oceans of the world.</skos:scopeNote>
   </skos:Concept>
   <skos:Concept rdf:about="urn:marlin.csiro.au:sourceregister:concept:297">
      <skos:prefLabel xml:lang="en">Ship: Linnaeus (RV)</skos:prefLabel>
      <skos:inScheme rdf:resource="urn:marlin.csiro.au:sourceregister:conceptscheme:1.0"/>
      <skos:definition xml:lang="en">Type: Ship Description: The Linnaeus is a 17 metre cray fishing vessel modified for coastal oceanography.</skos:definition>
      <skos:scopeNote xml:lang="en">Ship: Linnaeus (RV): Type: Ship Description: The Linnaeus is a 17 metre cray fishing vessel modified for coastal oceanography.</skos:scopeNote>
   </skos:Concept>
   <skos:Concept rdf:about="urn:marlin.csiro.au:sourceregister:concept:298">
      <skos:prefLabel xml:lang="en">Ship: Sarda</skos:prefLabel>
      <skos:inScheme rdf:resource="urn:marlin.csiro.au:sourceregister:conceptscheme:1.0"/>
      <skos:definition xml:lang="en">Type: Ship Description: FV Sarda is a 20m longline vessel licensed to fish in Commonwealth waters. Built in 1974 of steel, she has 7 berths. She works out of Lakes Entrance, owned by Mr.Chris Currie of Bluebeard's Seafoods.
</skos:definition>
      <skos:scopeNote xml:lang="en">Ship: Sarda: Type: Ship Description: FV Sarda is a 20m longline vessel licensed to fish in Commonwealth waters. Built in 1974 of steel, she has 7 berths. She works out of Lakes Entrance, owned by Mr.Chris Currie of Bluebeard's Seafoods.
</skos:scopeNote>
   </skos:Concept>
   <skos:Concept rdf:about="urn:marlin.csiro.au:sourceregister:concept:302">
      <skos:prefLabel xml:lang="en">Ship: Kapala</skos:prefLabel>
      <skos:inScheme rdf:resource="urn:marlin.csiro.au:sourceregister:conceptscheme:1.0"/>
      <skos:definition xml:lang="en">Type: Ship Description: FRV Kapala
TYPE:     Fishing Patrol and Support Vessel,  
BUILT:    1970, York Marine - Woodburn, AUSTRALIA, 
IMO:      6924923
CALLSIGN: -
URL:      www.shipspotting.com/gallery/photo.php?lid=1467971</skos:definition>
      <skos:scopeNote xml:lang="en">Ship: Kapala: Type: Ship Description: FRV Kapala
TYPE:     Fishing Patrol and Support Vessel,  
BUILT:    1970, York Marine - Woodburn, AUSTRALIA, 
IMO:      6924923
CALLSIGN: -
URL:      www.shipspotting.com/gallery/photo.php?lid=1467971</skos:scopeNote>
   </skos:Concept>
   <skos:Concept rdf:about="urn:marlin.csiro.au:sourceregister:concept:305">
      <skos:prefLabel xml:lang="en">Ship: Kirrawa</skos:prefLabel>
      <skos:inScheme rdf:resource="urn:marlin.csiro.au:sourceregister:conceptscheme:1.0"/>
      <skos:definition xml:lang="en">Type: Ship Description: FV Kirrawa
</skos:definition>
      <skos:scopeNote xml:lang="en">Ship: Kirrawa: Type: Ship Description: FV Kirrawa
</skos:scopeNote>
   </skos:Concept>
   <skos:Concept rdf:about="urn:marlin.csiro.au:sourceregister:concept:301">
      <skos:prefLabel xml:lang="en">Ship: Nelson Bay</skos:prefLabel>
      <skos:inScheme rdf:resource="urn:marlin.csiro.au:sourceregister:conceptscheme:1.0"/>
      <skos:definition xml:lang="en">Type: Ship Description: 12 metre longliner
see http://www.virhydro.com/press/Ausmarine%20Sept%202010%20Vol%2032%20No%2011.pdf</skos:definition>
      <skos:scopeNote xml:lang="en">Ship: Nelson Bay: Type: Ship Description: 12 metre longliner
see http://www.virhydro.com/press/Ausmarine%20Sept%202010%20Vol%2032%20No%2011.pdf</skos:scopeNote>
   </skos:Concept>
   <skos:Concept rdf:about="urn:marlin.csiro.au:sourceregister:concept:303">
      <skos:prefLabel xml:lang="en">Ship: Trader Horn</skos:prefLabel>
      <skos:inScheme rdf:resource="urn:marlin.csiro.au:sourceregister:conceptscheme:1.0"/>
      <skos:definition xml:lang="en">Type: Ship Description: FV Trader Horn</skos:definition>
      <skos:scopeNote xml:lang="en">Ship: Trader Horn: Type: Ship Description: FV Trader Horn</skos:scopeNote>
   </skos:Concept>
   <skos:Concept rdf:about="urn:marlin.csiro.au:sourceregister:concept:299">
      <skos:prefLabel xml:lang="en">Ship: Diana</skos:prefLabel>
      <skos:inScheme rdf:resource="urn:marlin.csiro.au:sourceregister:conceptscheme:1.0"/>
      <skos:definition xml:lang="en">Type: Ship Description: FV Diana  is a Hobart based vessel owned by Will Mure of Mure's Fishing. IShe is a 22.8m vessel built in 2004 with 8 berths. She is equipped with long-line gear and licensed to fish in Commonwealth waters.</skos:definition>
      <skos:scopeNote xml:lang="en">Ship: Diana: Type: Ship Description: FV Diana  is a Hobart based vessel owned by Will Mure of Mure's Fishing. IShe is a 22.8m vessel built in 2004 with 8 berths. She is equipped with long-line gear and licensed to fish in Commonwealth waters.</skos:scopeNote>
   </skos:Concept>
   <skos:Concept rdf:about="urn:marlin.csiro.au:sourceregister:concept:300">
      <skos:prefLabel xml:lang="en">Ship: Claudarah</skos:prefLabel>
      <skos:inScheme rdf:resource="urn:marlin.csiro.au:sourceregister:conceptscheme:1.0"/>
      <skos:definition xml:lang="en">Type: Ship Description: Longliner (length 18.3 m. used in the Eastern Tuna &amp; Billfish Fishery. see
http://intra.wcpfc.int/Lists/Vessels/DispForm.aspx?ID=5117</skos:definition>
      <skos:scopeNote xml:lang="en">Ship: Claudarah: Type: Ship Description: Longliner (length 18.3 m. used in the Eastern Tuna &amp; Billfish Fishery. see
http://intra.wcpfc.int/Lists/Vessels/DispForm.aspx?ID=5117</skos:scopeNote>
   </skos:Concept>
   <skos:Concept rdf:about="urn:marlin.csiro.au:sourceregister:concept:304">
      <skos:prefLabel xml:lang="en">Ship: Shelley H</skos:prefLabel>
      <skos:inScheme rdf:resource="urn:marlin.csiro.au:sourceregister:conceptscheme:1.0"/>
      <skos:definition xml:lang="en">Type: Ship Description: FV Shelley H</skos:definition>
      <skos:scopeNote xml:lang="en">Ship: Shelley H: Type: Ship Description: FV Shelley H</skos:scopeNote>
   </skos:Concept>
   <skos:Concept rdf:about="urn:marlin.csiro.au:sourceregister:concept:306">
      <skos:prefLabel xml:lang="en">Ship: May Bell II</skos:prefLabel>
      <skos:inScheme rdf:resource="urn:marlin.csiro.au:sourceregister:conceptscheme:1.0"/>
      <skos:definition xml:lang="en">Type: Ship Description: FV May Bell II
</skos:definition>
      <skos:scopeNote xml:lang="en">Ship: May Bell II: Type: Ship Description: FV May Bell II
</skos:scopeNote>
   </skos:Concept>
   <skos:Concept rdf:about="urn:marlin.csiro.au:sourceregister:concept:307">
      <skos:prefLabel xml:lang="en">Ship: James Kirby (RV)</skos:prefLabel>
      <skos:inScheme rdf:resource="urn:marlin.csiro.au:sourceregister:conceptscheme:1.0"/>
      <skos:definition xml:lang="en">Type: Ship Description: James Cook University Research Vessel
Ship Type: Research Vessel (Trawler)
Length x Breadth: 19.57 m X 5.2 m
Draft: 2.15 m
Flag: Australia [AU] 
Call Sign: 2189QB

RV James Kirby is a steel hulled research vessel, purpose built based on a commercial prawn trawler hull. The all welded hulled vessel has an overall length of 19.57 metres, a moulded breadth of 5.2 metres and a draft of 2.15 metres.

The main propulsion unit is a turbo-charged Cummins NT855 marine diesel engine developing 300 BHP at 1800 revs. The engine is coupled to a variable pitch three-blade propeller giving the vessel a cruising speed of 10 knots.

http://www.jameskirby.jcu.edu.au/capabilities.html
http://www.marinetraffic.com/ais/shipdetails.aspx?MMSI=503416000</skos:definition>
      <skos:scopeNote xml:lang="en">Ship: James Kirby (RV): Type: Ship Description: James Cook University Research Vessel
Ship Type: Research Vessel (Trawler)
Length x Breadth: 19.57 m X 5.2 m
Draft: 2.15 m
Flag: Australia [AU] 
Call Sign: 2189QB

RV James Kirby is a steel hulled research vessel, purpose built based on a commercial prawn trawler hull. The all welded hulled vessel has an overall length of 19.57 metres, a moulded breadth of 5.2 metres and a draft of 2.15 metres.

The main propulsion unit is a turbo-charged Cummins NT855 marine diesel engine developing 300 BHP at 1800 revs. The engine is coupled to a variable pitch three-blade propeller giving the vessel a cruising speed of 10 knots.

http://www.jameskirby.jcu.edu.au/capabilities.html
http://www.marinetraffic.com/ais/shipdetails.aspx?MMSI=503416000</skos:scopeNote>
   </skos:Concept>
   <skos:Concept rdf:about="urn:marlin.csiro.au:sourceregister:concept:311">
      <skos:prefLabel xml:lang="en">Ship: Solander</skos:prefLabel>
      <skos:inScheme rdf:resource="urn:marlin.csiro.au:sourceregister:conceptscheme:1.0"/>
      <skos:definition xml:lang="en">Type: Ship Description: The RV Solander is a research vessel operated by AIMS. It was built by: Tenix Defence,Henderson, WA in 2007. 

SPECIFICATIONS:
Hull:               Steel
Classification:     ABS A1 AMS
Length (oa):        34.9m
Beam:               8.6m
Draft:              2.8m
Displacement:       415 tonnes
Service speed:      11 knots
Range:              2,700 nm

Main engines:       2 x Cummins KTA19 M3
Auxiliary engines:  2 x Cummins 6C-CP
Propulsion:         2 x controllable pitch prop
Radars:             2 x Furuno 1964C-BB
Sounder:            Furuno ETR-30N
Sonar:              Furuno CH 250
Satellite Comms:    Inmarsat C, Fleet 77, Fleet 33

Work winch:         4 tonne capacity
A-frame:            8 tonne capacity
Hydrographic winch: 350 kilogram capacity
CTD winch:          Livewire - carousel
Deck crane:         Palfinger PKM 120

Moon pool; Fume hood: Dynaflow 1000; Dry lab area: 20.6 m2; Wet lab area: 12.5 m2; Scientific freezer: 6.5 m3; Scientific office: 9.4 m2; Back deck area 70 m2(provision for half shipping container)</skos:definition>
      <skos:scopeNote xml:lang="en">Ship: Solander: Type: Ship Description: The RV Solander is a research vessel operated by AIMS. It was built by: Tenix Defence,Henderson, WA in 2007. 

SPECIFICATIONS:
Hull:               Steel
Classification:     ABS A1 AMS
Length (oa):        34.9m
Beam:               8.6m
Draft:              2.8m
Displacement:       415 tonnes
Service speed:      11 knots
Range:              2,700 nm

Main engines:       2 x Cummins KTA19 M3
Auxiliary engines:  2 x Cummins 6C-CP
Propulsion:         2 x controllable pitch prop
Radars:             2 x Furuno 1964C-BB
Sounder:            Furuno ETR-30N
Sonar:              Furuno CH 250
Satellite Comms:    Inmarsat C, Fleet 77, Fleet 33

Work winch:         4 tonne capacity
A-frame:            8 tonne capacity
Hydrographic winch: 350 kilogram capacity
CTD winch:          Livewire - carousel
Deck crane:         Palfinger PKM 120

Moon pool; Fume hood: Dynaflow 1000; Dry lab area: 20.6 m2; Wet lab area: 12.5 m2; Scientific freezer: 6.5 m3; Scientific office: 9.4 m2; Back deck area 70 m2(provision for half shipping container)</skos:scopeNote>
   </skos:Concept>
   <skos:Concept rdf:about="urn:marlin.csiro.au:sourceregister:concept:309">
      <skos:prefLabel xml:lang="en">Ship: Investigator (RV)</skos:prefLabel>
      <skos:inScheme rdf:resource="urn:marlin.csiro.au:sourceregister:conceptscheme:1.0"/>
      <skos:definition xml:lang="en">Type: Ship Description: RV Investigator ("Investigator" to be in italics)

Built for the Marine National Facility to replace the Southern Surveyor. In the May 2009 Federal Budget the Australian Government committed A$120 million to the purchase of a new ocean-going research vessel for the Marine National Facility.

Build completed in 2014.

Length: 94 metres, 
Days at sea: Up to 300, 
Scientific berths: 40, 
Endurance: 60 days,
Cruising speed: 12 knots,
Range: ~10,000 nm,
Extent of operating area: Ice edge.
O.N. 860820. IMO 9616888. Call sign VLMJ</skos:definition>
      <skos:scopeNote xml:lang="en">Ship: Investigator (RV): Type: Ship Description: RV Investigator ("Investigator" to be in italics)

Built for the Marine National Facility to replace the Southern Surveyor. In the May 2009 Federal Budget the Australian Government committed A$120 million to the purchase of a new ocean-going research vessel for the Marine National Facility.

Build completed in 2014.

Length: 94 metres, 
Days at sea: Up to 300, 
Scientific berths: 40, 
Endurance: 60 days,
Cruising speed: 12 knots,
Range: ~10,000 nm,
Extent of operating area: Ice edge.
O.N. 860820. IMO 9616888. Call sign VLMJ</skos:scopeNote>
   </skos:Concept>
   <skos:Concept rdf:about="urn:marlin.csiro.au:sourceregister:concept:310">
      <skos:prefLabel xml:lang="en">Coastal Station: IMOS NRS Field sampling</skos:prefLabel>
      <skos:inScheme rdf:resource="urn:marlin.csiro.au:sourceregister:conceptscheme:1.0"/>
      <skos:definition xml:lang="en">Type: Coastal Station Description: 9 Sites are included in the IMOS NRS Field Sampling stations.
Maria Island* (TAS)
Kangaroo Island (SA)
Esperance (WA)
Rottnest Island* (WA)
Ningaloo (WA)
Darwin (NT)
Yongala (QLD)
North Stradbroke Island (QLD)
Port Hacking 100* (NSW)

*Denotes long term stations already sampled and analysed historically by CMAR – some dating back to the 1940’s.

Sampling at these sites as part of the IMOS NRS Biogeochemical project began between  29/9/2008 and 8/11/2010 as is currently ongoing.</skos:definition>
      <skos:scopeNote xml:lang="en">Coastal Station: IMOS NRS Field sampling: Type: Coastal Station Description: 9 Sites are included in the IMOS NRS Field Sampling stations.
Maria Island* (TAS)
Kangaroo Island (SA)
Esperance (WA)
Rottnest Island* (WA)
Ningaloo (WA)
Darwin (NT)
Yongala (QLD)
North Stradbroke Island (QLD)
Port Hacking 100* (NSW)

*Denotes long term stations already sampled and analysed historically by CMAR – some dating back to the 1940’s.

Sampling at these sites as part of the IMOS NRS Biogeochemical project began between  29/9/2008 and 8/11/2010 as is currently ongoing.</skos:scopeNote>
   </skos:Concept>
   <skos:Concept rdf:about="urn:marlin.csiro.au:sourceregister:concept:312">
      <skos:prefLabel xml:lang="en">Ship: Tom Marshall</skos:prefLabel>
      <skos:inScheme rdf:resource="urn:marlin.csiro.au:sourceregister:conceptscheme:1.0"/>
      <skos:definition xml:lang="en">Type: Ship Description: Details:  Fisheries research vessel, length 14m
see http://www.vesselfinder.com/vessels/TOM-MARSHALL-IMO-0-MMSI-503448600
    http://www.daff.qld.gov.au/fisheries/research/scientific-capabilities

Vessel Details
--------------
Size:       14x6m
Year built: unknown
Ship type:  Fishing vessel
Flag:       Flag of Australia Australia
IMO number: N/A
MMSI:       503448600
Callsign    VLQ2940</skos:definition>
      <skos:scopeNote xml:lang="en">Ship: Tom Marshall: Type: Ship Description: Details:  Fisheries research vessel, length 14m
see http://www.vesselfinder.com/vessels/TOM-MARSHALL-IMO-0-MMSI-503448600
    http://www.daff.qld.gov.au/fisheries/research/scientific-capabilities

Vessel Details
--------------
Size:       14x6m
Year built: unknown
Ship type:  Fishing vessel
Flag:       Flag of Australia Australia
IMO number: N/A
MMSI:       503448600
Callsign    VLQ2940</skos:scopeNote>
   </skos:Concept>
   <skos:Concept rdf:about="urn:marlin.csiro.au:sourceregister:concept:313">
      <skos:prefLabel xml:lang="en">Ship: Morona</skos:prefLabel>
      <skos:inScheme rdf:resource="urn:marlin.csiro.au:sourceregister:conceptscheme:1.0"/>
      <skos:definition xml:lang="en">Type: Ship Description: Name: Morona
Owner: IMAS
Details: smallish!

Specifications:</skos:definition>
      <skos:scopeNote xml:lang="en">Ship: Morona: Type: Ship Description: Name: Morona
Owner: IMAS
Details: smallish!

Specifications:</skos:scopeNote>
   </skos:Concept>
   <skos:Concept rdf:about="urn:marlin.csiro.au:sourceregister:concept:314">
      <skos:prefLabel xml:lang="en">Ship: Margaret Philippa</skos:prefLabel>
      <skos:inScheme rdf:resource="urn:marlin.csiro.au:sourceregister:conceptscheme:1.0"/>
      <skos:definition xml:lang="en">Type: Ship Description: Trawler 206 tons, built 1978  IMO 7816848 </skos:definition>
      <skos:scopeNote xml:lang="en">Ship: Margaret Philippa: Type: Ship Description: Trawler 206 tons, built 1978  IMO 7816848 </skos:scopeNote>
   </skos:Concept>
   <skos:Concept rdf:about="urn:marlin.csiro.au:sourceregister:concept:316">
      <skos:prefLabel xml:lang="en">Ship: Zeehaan</skos:prefLabel>
      <skos:inScheme rdf:resource="urn:marlin.csiro.au:sourceregister:conceptscheme:1.0"/>
      <skos:definition xml:lang="en">Type: Ship Description: 23 m stern trawler - details in http://eprints.utas.edu.au/14145/1/1981_Last_locality_records.df.pdf</skos:definition>
      <skos:scopeNote xml:lang="en">Ship: Zeehaan: Type: Ship Description: 23 m stern trawler - details in http://eprints.utas.edu.au/14145/1/1981_Last_locality_records.df.pdf</skos:scopeNote>
   </skos:Concept>
   <skos:Concept rdf:about="urn:marlin.csiro.au:sourceregister:concept:315">
      <skos:prefLabel xml:lang="en">Ship: S.Y. Endeavour</skos:prefLabel>
      <skos:inScheme rdf:resource="urn:marlin.csiro.au:sourceregister:conceptscheme:1.0"/>
      <skos:definition xml:lang="en">Type: Ship Description: fisheries investigations ship. 331 tons. lost at sea 3 December 1914  near Macquarie island. See http://www.parks.tas.gov.au/fahan_mi_shipwrecks/journals/Shipwrecks/sweandeavour13.pdf </skos:definition>
      <skos:scopeNote xml:lang="en">Ship: S.Y. Endeavour: Type: Ship Description: fisheries investigations ship. 331 tons. lost at sea 3 December 1914  near Macquarie island. See http://www.parks.tas.gov.au/fahan_mi_shipwrecks/journals/Shipwrecks/sweandeavour13.pdf </skos:scopeNote>
   </skos:Concept>
</rdf:RDF>