<?xml version="1.0" encoding="UTF-8"?>
<rdf:RDF xmlns:dc="http://purl.org/dc/elements/1.1/" xmlns:dct="http://purl.org/dc/terms/"
         xmlns:foaf="http://xmlns.com/foaf/0.1/"
         xmlns:gml="http://www.opengis.net/gml#"
         xmlns:rdf="http://www.w3.org/1999/02/22-rdf-syntax-ns#"
         xmlns:skos="http://www.w3.org/2004/02/skos/core#">
   <skos:ConceptScheme rdf:about="urn:aodn.org.au:geographicextents:conceptscheme:1.0">
      <dc:identifier>urn:aodn.org.au:geographicextents</dc:identifier>
      <dc:title>AODN Geographic Extent Names</dc:title>
      <dc:description>Australian Oceans Data Network List of Geographic Extent Names with Bounding Box</dc:description>
      <dc:URI>http://marlin.csiro.au/geonetwork/srv/eng/xml.metadata.get?uuid=urn:aodn.org.au:geographicextents</dc:URI>
      <dct:modified>2012-06-30</dct:modified>
      <dc:creator>
         <foaf:Organization>
            <foaf:name>CSIRO Oceans and Atmosphere Data Centre</foaf:name>
         </foaf:Organization>
      </dc:creator>
      <dc:publisher/>
      <dct:issued>2017-02-17T10:12:36</dct:issued>
      <skos:hasTopConcept rdf:resource="urn:aodn.org.au:geographicextents:concept:10009"/>
      <skos:hasTopConcept rdf:resource="urn:aodn.org.au:geographicextents:concept:10002"/>
      <skos:hasTopConcept rdf:resource="urn:aodn.org.au:geographicextents:concept:10001"/>
      <skos:hasTopConcept rdf:resource="urn:aodn.org.au:geographicextents:concept:10006"/>
      <skos:hasTopConcept rdf:resource="urn:aodn.org.au:geographicextents:concept:10007"/>
      <skos:hasTopConcept rdf:resource="urn:aodn.org.au:geographicextents:concept:10008"/>
      <skos:hasTopConcept rdf:resource="urn:aodn.org.au:geographicextents:concept:10004"/>
      <skos:hasTopConcept rdf:resource="urn:aodn.org.au:geographicextents:concept:10010"/>
      <skos:hasTopConcept rdf:resource="urn:aodn.org.au:geographicextents:concept:10011"/>
      <skos:hasTopConcept rdf:resource="urn:aodn.org.au:geographicextents:concept:10005"/>
      <skos:hasTopConcept rdf:resource="urn:aodn.org.au:geographicextents:concept:10000"/>
      <skos:hasTopConcept rdf:resource="urn:aodn.org.au:geographicextents:concept:10003"/>
   </skos:ConceptScheme>
   <skos:Concept rdf:about="urn:aodn.org.au:geographicextents:concept:10009">
      <skos:prefLabel xml:lang="en">Coastal Cities / Towns (Australia)</skos:prefLabel>
      <skos:inScheme rdf:resource="urn:aodn.org.au:geographicextents:conceptscheme:1.0"/>
      <gml:BoundedBy>
         <gml:Envelope gml:srsName="http://www.opengis.net/gml/srs/epsg.xml#epsg:4326">
            <gml:lowerCorner>-180 -90</gml:lowerCorner>
            <gml:upperCorner>180 90</gml:upperCorner>
         </gml:Envelope>
      </gml:BoundedBy>
      <skos:definition xml:lang="en">Coastal Cities / Towns (Australia)</skos:definition>
      <skos:scopeNote xml:lang="en">Coastal Cities / Towns (Australia): Coastal Cities / Towns (Australia)</skos:scopeNote>
      <skos:topConceptOf rdf:resource="urn:aodn.org.au:geographicextents:conceptscheme:1.0"/>
   </skos:Concept>
   <skos:Concept rdf:about="urn:aodn.org.au:geographicextents:concept:10002">
      <skos:prefLabel xml:lang="en">Coastal Waters (Australia)</skos:prefLabel>
      <skos:inScheme rdf:resource="urn:aodn.org.au:geographicextents:conceptscheme:1.0"/>
      <gml:BoundedBy>
         <gml:Envelope gml:srsName="http://www.opengis.net/gml/srs/epsg.xml#epsg:4326">
            <gml:lowerCorner>-180 -90</gml:lowerCorner>
            <gml:upperCorner>180 90</gml:upperCorner>
         </gml:Envelope>
      </gml:BoundedBy>
      <skos:definition xml:lang="en">Coastal Waters (Australia)</skos:definition>
      <skos:scopeNote xml:lang="en">Coastal Waters (Australia): Coastal Waters (Australia)</skos:scopeNote>
      <skos:topConceptOf rdf:resource="urn:aodn.org.au:geographicextents:conceptscheme:1.0"/>
   </skos:Concept>
   <skos:Concept rdf:about="urn:aodn.org.au:geographicextents:concept:10001">
      <skos:prefLabel xml:lang="en">Coastal Waters (Global)</skos:prefLabel>
      <skos:inScheme rdf:resource="urn:aodn.org.au:geographicextents:conceptscheme:1.0"/>
      <gml:BoundedBy>
         <gml:Envelope gml:srsName="http://www.opengis.net/gml/srs/epsg.xml#epsg:4326">
            <gml:lowerCorner>-180 -90</gml:lowerCorner>
            <gml:upperCorner>180 90</gml:upperCorner>
         </gml:Envelope>
      </gml:BoundedBy>
      <skos:definition xml:lang="en">Coastal Waters (Global)</skos:definition>
      <skos:scopeNote xml:lang="en">Coastal Waters (Global): Coastal Waters (Global)</skos:scopeNote>
      <skos:topConceptOf rdf:resource="urn:aodn.org.au:geographicextents:conceptscheme:1.0"/>
   </skos:Concept>
   <skos:Concept rdf:about="urn:aodn.org.au:geographicextents:concept:10006">
      <skos:prefLabel xml:lang="en">Continents</skos:prefLabel>
      <skos:inScheme rdf:resource="urn:aodn.org.au:geographicextents:conceptscheme:1.0"/>
      <gml:BoundedBy>
         <gml:Envelope gml:srsName="http://www.opengis.net/gml/srs/epsg.xml#epsg:4326">
            <gml:lowerCorner>-180 -90</gml:lowerCorner>
            <gml:upperCorner>180 90</gml:upperCorner>
         </gml:Envelope>
      </gml:BoundedBy>
      <skos:definition xml:lang="en">Continents</skos:definition>
      <skos:scopeNote xml:lang="en">Continents: Continents</skos:scopeNote>
      <skos:topConceptOf rdf:resource="urn:aodn.org.au:geographicextents:conceptscheme:1.0"/>
   </skos:Concept>
   <skos:Concept rdf:about="urn:aodn.org.au:geographicextents:concept:10007">
      <skos:prefLabel xml:lang="en">Countries</skos:prefLabel>
      <skos:inScheme rdf:resource="urn:aodn.org.au:geographicextents:conceptscheme:1.0"/>
      <gml:BoundedBy>
         <gml:Envelope gml:srsName="http://www.opengis.net/gml/srs/epsg.xml#epsg:4326">
            <gml:lowerCorner>-180 -90</gml:lowerCorner>
            <gml:upperCorner>180 90</gml:upperCorner>
         </gml:Envelope>
      </gml:BoundedBy>
      <skos:definition xml:lang="en">Countries</skos:definition>
      <skos:scopeNote xml:lang="en">Countries: Countries</skos:scopeNote>
      <skos:topConceptOf rdf:resource="urn:aodn.org.au:geographicextents:conceptscheme:1.0"/>
   </skos:Concept>
   <skos:Concept rdf:about="urn:aodn.org.au:geographicextents:concept:10008">
      <skos:prefLabel xml:lang="en">Global / Oceans</skos:prefLabel>
      <skos:inScheme rdf:resource="urn:aodn.org.au:geographicextents:conceptscheme:1.0"/>
      <gml:BoundedBy>
         <gml:Envelope gml:srsName="http://www.opengis.net/gml/srs/epsg.xml#epsg:4326">
            <gml:lowerCorner>-180 -90</gml:lowerCorner>
            <gml:upperCorner>180 90</gml:upperCorner>
         </gml:Envelope>
      </gml:BoundedBy>
      <skos:definition xml:lang="en">Global / Oceans</skos:definition>
      <skos:scopeNote xml:lang="en">Global / Oceans: Global / Oceans</skos:scopeNote>
      <skos:topConceptOf rdf:resource="urn:aodn.org.au:geographicextents:conceptscheme:1.0"/>
   </skos:Concept>
   <skos:Concept rdf:about="urn:aodn.org.au:geographicextents:concept:10004">
      <skos:prefLabel xml:lang="en">Marine Features (Australia)</skos:prefLabel>
      <skos:inScheme rdf:resource="urn:aodn.org.au:geographicextents:conceptscheme:1.0"/>
      <gml:BoundedBy>
         <gml:Envelope gml:srsName="http://www.opengis.net/gml/srs/epsg.xml#epsg:4326">
            <gml:lowerCorner>-180 -90</gml:lowerCorner>
            <gml:upperCorner>180 90</gml:upperCorner>
         </gml:Envelope>
      </gml:BoundedBy>
      <skos:definition xml:lang="en">Marine Features (Australia)</skos:definition>
      <skos:scopeNote xml:lang="en">Marine Features (Australia): Marine Features (Australia)</skos:scopeNote>
      <skos:topConceptOf rdf:resource="urn:aodn.org.au:geographicextents:conceptscheme:1.0"/>
   </skos:Concept>
   <skos:Concept rdf:about="urn:aodn.org.au:geographicextents:concept:10010">
      <skos:prefLabel xml:lang="en">Marine Planning Regions (Australia)</skos:prefLabel>
      <skos:inScheme rdf:resource="urn:aodn.org.au:geographicextents:conceptscheme:1.0"/>
      <gml:BoundedBy>
         <gml:Envelope gml:srsName="http://www.opengis.net/gml/srs/epsg.xml#epsg:4326">
            <gml:lowerCorner>-180 -90</gml:lowerCorner>
            <gml:upperCorner>180 90</gml:upperCorner>
         </gml:Envelope>
      </gml:BoundedBy>
      <skos:definition xml:lang="en">Marine Planning Regions (Australia)</skos:definition>
      <skos:scopeNote xml:lang="en">Marine Planning Regions (Australia): Marine Planning Regions (Australia)</skos:scopeNote>
      <skos:topConceptOf rdf:resource="urn:aodn.org.au:geographicextents:conceptscheme:1.0"/>
   </skos:Concept>
   <skos:Concept rdf:about="urn:aodn.org.au:geographicextents:concept:10011">
      <skos:prefLabel xml:lang="en">Named Locations (Antarctica)</skos:prefLabel>
      <skos:inScheme rdf:resource="urn:aodn.org.au:geographicextents:conceptscheme:1.0"/>
      <gml:BoundedBy>
         <gml:Envelope gml:srsName="http://www.opengis.net/gml/srs/epsg.xml#epsg:4326">
            <gml:lowerCorner>-180 -90</gml:lowerCorner>
            <gml:upperCorner>180 90</gml:upperCorner>
         </gml:Envelope>
      </gml:BoundedBy>
      <skos:definition xml:lang="en">Named Locations (Antarctica)</skos:definition>
      <skos:scopeNote xml:lang="en">Named Locations (Antarctica): Named Locations (Antarctica)</skos:scopeNote>
      <skos:topConceptOf rdf:resource="urn:aodn.org.au:geographicextents:conceptscheme:1.0"/>
   </skos:Concept>
   <skos:Concept rdf:about="urn:aodn.org.au:geographicextents:concept:10005">
      <skos:prefLabel xml:lang="en">Offshore Islands (Australia)</skos:prefLabel>
      <skos:inScheme rdf:resource="urn:aodn.org.au:geographicextents:conceptscheme:1.0"/>
      <gml:BoundedBy>
         <gml:Envelope gml:srsName="http://www.opengis.net/gml/srs/epsg.xml#epsg:4326">
            <gml:lowerCorner>-180 -90</gml:lowerCorner>
            <gml:upperCorner>180 90</gml:upperCorner>
         </gml:Envelope>
      </gml:BoundedBy>
      <skos:definition xml:lang="en">Offshore Islands (Australia)</skos:definition>
      <skos:scopeNote xml:lang="en">Offshore Islands (Australia): Offshore Islands (Australia)</skos:scopeNote>
      <skos:topConceptOf rdf:resource="urn:aodn.org.au:geographicextents:conceptscheme:1.0"/>
   </skos:Concept>
   <skos:Concept rdf:about="urn:aodn.org.au:geographicextents:concept:10000">
      <skos:prefLabel xml:lang="en">Regional Seas</skos:prefLabel>
      <skos:inScheme rdf:resource="urn:aodn.org.au:geographicextents:conceptscheme:1.0"/>
      <gml:BoundedBy>
         <gml:Envelope gml:srsName="http://www.opengis.net/gml/srs/epsg.xml#epsg:4326">
            <gml:lowerCorner>-180 -90</gml:lowerCorner>
            <gml:upperCorner>180 90</gml:upperCorner>
         </gml:Envelope>
      </gml:BoundedBy>
      <skos:definition xml:lang="en">Regional Seas</skos:definition>
      <skos:scopeNote xml:lang="en">Regional Seas: Regional Seas</skos:scopeNote>
      <skos:topConceptOf rdf:resource="urn:aodn.org.au:geographicextents:conceptscheme:1.0"/>
   </skos:Concept>
   <skos:Concept rdf:about="urn:aodn.org.au:geographicextents:concept:10003">
      <skos:prefLabel xml:lang="en">States, Territories (Australia)</skos:prefLabel>
      <skos:inScheme rdf:resource="urn:aodn.org.au:geographicextents:conceptscheme:1.0"/>
      <gml:BoundedBy>
         <gml:Envelope gml:srsName="http://www.opengis.net/gml/srs/epsg.xml#epsg:4326">
            <gml:lowerCorner>-180 -90</gml:lowerCorner>
            <gml:upperCorner>180 90</gml:upperCorner>
         </gml:Envelope>
      </gml:BoundedBy>
      <skos:definition xml:lang="en">States, Territories (Australia)</skos:definition>
      <skos:scopeNote xml:lang="en">States, Territories (Australia): States, Territories (Australia)</skos:scopeNote>
      <skos:topConceptOf rdf:resource="urn:aodn.org.au:geographicextents:conceptscheme:1.0"/>
   </skos:Concept>
   <skos:Concept rdf:about="urn:aodn.org.au:geographicextents:concept:102">
      <skos:prefLabel xml:lang="en">Coastal Cities / Towns (Australia) | Adelaide, SA</skos:prefLabel>
      <skos:inScheme rdf:resource="urn:aodn.org.au:geographicextents:conceptscheme:1.0"/>
      <gml:BoundedBy>
         <gml:Envelope gml:srsName="http://www.opengis.net/gml/srs/epsg.xml#epsg:4326">
            <gml:lowerCorner>138.44 -35.35</gml:lowerCorner>
            <gml:upperCorner>138.79 -34.65</gml:upperCorner>
         </gml:Envelope>
      </gml:BoundedBy>
      <skos:broader rdf:resource="urn:aodn.org.au:geographicextents:concept:10009"/>
      <skos:definition xml:lang="en">Coastal Cities / Towns (Australia) | Adelaide, SA</skos:definition>
      <skos:scopeNote xml:lang="en">Coastal Cities / Towns (Australia) | Adelaide, SA: Coastal Cities / Towns (Australia) | Adelaide, SA</skos:scopeNote>
   </skos:Concept>
   <skos:Concept rdf:about="urn:aodn.org.au:geographicextents:concept:103">
      <skos:prefLabel xml:lang="en">Coastal Cities / Towns (Australia) | Albany, WA</skos:prefLabel>
      <skos:inScheme rdf:resource="urn:aodn.org.au:geographicextents:conceptscheme:1.0"/>
      <gml:BoundedBy>
         <gml:Envelope gml:srsName="http://www.opengis.net/gml/srs/epsg.xml#epsg:4326">
            <gml:lowerCorner>117.87 -35.04</gml:lowerCorner>
            <gml:upperCorner>117.9 -35.01</gml:upperCorner>
         </gml:Envelope>
      </gml:BoundedBy>
      <skos:broader rdf:resource="urn:aodn.org.au:geographicextents:concept:10009"/>
      <skos:definition xml:lang="en">Coastal Cities / Towns (Australia) | Albany, WA</skos:definition>
      <skos:scopeNote xml:lang="en">Coastal Cities / Towns (Australia) | Albany, WA: Coastal Cities / Towns (Australia) | Albany, WA</skos:scopeNote>
   </skos:Concept>
   <skos:Concept rdf:about="urn:aodn.org.au:geographicextents:concept:104">
      <skos:prefLabel xml:lang="en">Coastal Cities / Towns (Australia) | Brisbane, QLD</skos:prefLabel>
      <skos:inScheme rdf:resource="urn:aodn.org.au:geographicextents:conceptscheme:1.0"/>
      <gml:BoundedBy>
         <gml:Envelope gml:srsName="http://www.opengis.net/gml/srs/epsg.xml#epsg:4326">
            <gml:lowerCorner>152.66 -27.77</gml:lowerCorner>
            <gml:upperCorner>153.32 -26.99</gml:upperCorner>
         </gml:Envelope>
      </gml:BoundedBy>
      <skos:broader rdf:resource="urn:aodn.org.au:geographicextents:concept:10009"/>
      <skos:definition xml:lang="en">Coastal Cities / Towns (Australia) | Brisbane, QLD</skos:definition>
      <skos:scopeNote xml:lang="en">Coastal Cities / Towns (Australia) | Brisbane, QLD: Coastal Cities / Towns (Australia) | Brisbane, QLD</skos:scopeNote>
   </skos:Concept>
   <skos:Concept rdf:about="urn:aodn.org.au:geographicextents:concept:105">
      <skos:prefLabel xml:lang="en">Coastal Cities / Towns (Australia) | Broome, WA</skos:prefLabel>
      <skos:inScheme rdf:resource="urn:aodn.org.au:geographicextents:conceptscheme:1.0"/>
      <gml:BoundedBy>
         <gml:Envelope gml:srsName="http://www.opengis.net/gml/srs/epsg.xml#epsg:4326">
            <gml:lowerCorner>122.21 -17.98</gml:lowerCorner>
            <gml:upperCorner>122.26 -17.94</gml:upperCorner>
         </gml:Envelope>
      </gml:BoundedBy>
      <skos:broader rdf:resource="urn:aodn.org.au:geographicextents:concept:10009"/>
      <skos:definition xml:lang="en">Coastal Cities / Towns (Australia) | Broome, WA</skos:definition>
      <skos:scopeNote xml:lang="en">Coastal Cities / Towns (Australia) | Broome, WA: Coastal Cities / Towns (Australia) | Broome, WA</skos:scopeNote>
   </skos:Concept>
   <skos:Concept rdf:about="urn:aodn.org.au:geographicextents:concept:106">
      <skos:prefLabel xml:lang="en">Coastal Cities / Towns (Australia) | Bunbury, WA</skos:prefLabel>
      <skos:inScheme rdf:resource="urn:aodn.org.au:geographicextents:conceptscheme:1.0"/>
      <gml:BoundedBy>
         <gml:Envelope gml:srsName="http://www.opengis.net/gml/srs/epsg.xml#epsg:4326">
            <gml:lowerCorner>115.6 -33.34</gml:lowerCorner>
            <gml:upperCorner>115.66 -33.3</gml:upperCorner>
         </gml:Envelope>
      </gml:BoundedBy>
      <skos:broader rdf:resource="urn:aodn.org.au:geographicextents:concept:10009"/>
      <skos:definition xml:lang="en">Coastal Cities / Towns (Australia) | Bunbury, WA</skos:definition>
      <skos:scopeNote xml:lang="en">Coastal Cities / Towns (Australia) | Bunbury, WA: Coastal Cities / Towns (Australia) | Bunbury, WA</skos:scopeNote>
   </skos:Concept>
   <skos:Concept rdf:about="urn:aodn.org.au:geographicextents:concept:107">
      <skos:prefLabel xml:lang="en">Coastal Cities / Towns (Australia) | Bundaberg, QLD</skos:prefLabel>
      <skos:inScheme rdf:resource="urn:aodn.org.au:geographicextents:conceptscheme:1.0"/>
      <gml:BoundedBy>
         <gml:Envelope gml:srsName="http://www.opengis.net/gml/srs/epsg.xml#epsg:4326">
            <gml:lowerCorner>152.34 -24.88</gml:lowerCorner>
            <gml:upperCorner>152.36 -24.86</gml:upperCorner>
         </gml:Envelope>
      </gml:BoundedBy>
      <skos:broader rdf:resource="urn:aodn.org.au:geographicextents:concept:10009"/>
      <skos:definition xml:lang="en">Coastal Cities / Towns (Australia) | Bundaberg, QLD</skos:definition>
      <skos:scopeNote xml:lang="en">Coastal Cities / Towns (Australia) | Bundaberg, QLD: Coastal Cities / Towns (Australia) | Bundaberg, QLD</skos:scopeNote>
   </skos:Concept>
   <skos:Concept rdf:about="urn:aodn.org.au:geographicextents:concept:108">
      <skos:prefLabel xml:lang="en">Coastal Cities / Towns (Australia) | Burnie, TAS</skos:prefLabel>
      <skos:inScheme rdf:resource="urn:aodn.org.au:geographicextents:conceptscheme:1.0"/>
      <gml:BoundedBy>
         <gml:Envelope gml:srsName="http://www.opengis.net/gml/srs/epsg.xml#epsg:4326">
            <gml:lowerCorner>145.89 -41.07</gml:lowerCorner>
            <gml:upperCorner>145.93 -41.04</gml:upperCorner>
         </gml:Envelope>
      </gml:BoundedBy>
      <skos:broader rdf:resource="urn:aodn.org.au:geographicextents:concept:10009"/>
      <skos:definition xml:lang="en">Coastal Cities / Towns (Australia) | Burnie, TAS</skos:definition>
      <skos:scopeNote xml:lang="en">Coastal Cities / Towns (Australia) | Burnie, TAS: Coastal Cities / Towns (Australia) | Burnie, TAS</skos:scopeNote>
   </skos:Concept>
   <skos:Concept rdf:about="urn:aodn.org.au:geographicextents:concept:109">
      <skos:prefLabel xml:lang="en">Coastal Cities / Towns (Australia) | Cairns, QLD</skos:prefLabel>
      <skos:inScheme rdf:resource="urn:aodn.org.au:geographicextents:conceptscheme:1.0"/>
      <gml:BoundedBy>
         <gml:Envelope gml:srsName="http://www.opengis.net/gml/srs/epsg.xml#epsg:4326">
            <gml:lowerCorner>145.65 -17.04</gml:lowerCorner>
            <gml:upperCorner>145.79 -16.72</gml:upperCorner>
         </gml:Envelope>
      </gml:BoundedBy>
      <skos:broader rdf:resource="urn:aodn.org.au:geographicextents:concept:10009"/>
      <skos:definition xml:lang="en">Coastal Cities / Towns (Australia) | Cairns, QLD</skos:definition>
      <skos:scopeNote xml:lang="en">Coastal Cities / Towns (Australia) | Cairns, QLD: Coastal Cities / Towns (Australia) | Cairns, QLD</skos:scopeNote>
   </skos:Concept>
   <skos:Concept rdf:about="urn:aodn.org.au:geographicextents:concept:1027">
      <skos:prefLabel xml:lang="en">Coastal Cities / Towns (Australia) | Coffs Harbour, NSW</skos:prefLabel>
      <skos:inScheme rdf:resource="urn:aodn.org.au:geographicextents:conceptscheme:1.0"/>
      <gml:BoundedBy>
         <gml:Envelope gml:srsName="http://www.opengis.net/gml/srs/epsg.xml#epsg:4326">
            <gml:lowerCorner>153.05 -30.36</gml:lowerCorner>
            <gml:upperCorner>153.16 -30.26</gml:upperCorner>
         </gml:Envelope>
      </gml:BoundedBy>
      <skos:broader rdf:resource="urn:aodn.org.au:geographicextents:concept:10009"/>
      <skos:definition xml:lang="en">Coastal Cities / Towns (Australia) | Coffs Harbour, NSW</skos:definition>
      <skos:scopeNote xml:lang="en">Coastal Cities / Towns (Australia) | Coffs Harbour, NSW: Coastal Cities / Towns (Australia) | Coffs Harbour, NSW</skos:scopeNote>
   </skos:Concept>
   <skos:Concept rdf:about="urn:aodn.org.au:geographicextents:concept:110">
      <skos:prefLabel xml:lang="en">Coastal Cities / Towns (Australia) | Darwin, NT</skos:prefLabel>
      <skos:inScheme rdf:resource="urn:aodn.org.au:geographicextents:conceptscheme:1.0"/>
      <gml:BoundedBy>
         <gml:Envelope gml:srsName="http://www.opengis.net/gml/srs/epsg.xml#epsg:4326">
            <gml:lowerCorner>130.82 12.53</gml:lowerCorner>
            <gml:upperCorner>131.06 -12.33</gml:upperCorner>
         </gml:Envelope>
      </gml:BoundedBy>
      <skos:broader rdf:resource="urn:aodn.org.au:geographicextents:concept:10009"/>
      <skos:definition xml:lang="en">Coastal Cities / Towns (Australia) | Darwin, NT</skos:definition>
      <skos:scopeNote xml:lang="en">Coastal Cities / Towns (Australia) | Darwin, NT: Coastal Cities / Towns (Australia) | Darwin, NT</skos:scopeNote>
   </skos:Concept>
   <skos:Concept rdf:about="urn:aodn.org.au:geographicextents:concept:111">
      <skos:prefLabel xml:lang="en">Coastal Cities / Towns (Australia) | Dampier, WA</skos:prefLabel>
      <skos:inScheme rdf:resource="urn:aodn.org.au:geographicextents:conceptscheme:1.0"/>
      <gml:BoundedBy>
         <gml:Envelope gml:srsName="http://www.opengis.net/gml/srs/epsg.xml#epsg:4326">
            <gml:lowerCorner>116.69 -20.68</gml:lowerCorner>
            <gml:upperCorner>116.87 -20.52</gml:upperCorner>
         </gml:Envelope>
      </gml:BoundedBy>
      <skos:broader rdf:resource="urn:aodn.org.au:geographicextents:concept:10009"/>
      <skos:definition xml:lang="en">Coastal Cities / Towns (Australia) | Dampier, WA</skos:definition>
      <skos:scopeNote xml:lang="en">Coastal Cities / Towns (Australia) | Dampier, WA: Coastal Cities / Towns (Australia) | Dampier, WA</skos:scopeNote>
   </skos:Concept>
   <skos:Concept rdf:about="urn:aodn.org.au:geographicextents:concept:112">
      <skos:prefLabel xml:lang="en">Coastal Cities / Towns (Australia) | Devonport, TAS</skos:prefLabel>
      <skos:inScheme rdf:resource="urn:aodn.org.au:geographicextents:conceptscheme:1.0"/>
      <gml:BoundedBy>
         <gml:Envelope gml:srsName="http://www.opengis.net/gml/srs/epsg.xml#epsg:4326">
            <gml:lowerCorner>146.32 -41.2</gml:lowerCorner>
            <gml:upperCorner>146.37 -41.15</gml:upperCorner>
         </gml:Envelope>
      </gml:BoundedBy>
      <skos:broader rdf:resource="urn:aodn.org.au:geographicextents:concept:10009"/>
      <skos:definition xml:lang="en">Coastal Cities / Towns (Australia) | Devonport, TAS</skos:definition>
      <skos:scopeNote xml:lang="en">Coastal Cities / Towns (Australia) | Devonport, TAS: Coastal Cities / Towns (Australia) | Devonport, TAS</skos:scopeNote>
   </skos:Concept>
   <skos:Concept rdf:about="urn:aodn.org.au:geographicextents:concept:113">
      <skos:prefLabel xml:lang="en">Coastal Cities / Towns (Australia) | Esperance, WA</skos:prefLabel>
      <skos:inScheme rdf:resource="urn:aodn.org.au:geographicextents:conceptscheme:1.0"/>
      <gml:BoundedBy>
         <gml:Envelope gml:srsName="http://www.opengis.net/gml/srs/epsg.xml#epsg:4326">
            <gml:lowerCorner>121.88 -33.87</gml:lowerCorner>
            <gml:upperCorner>121.91 -33.85</gml:upperCorner>
         </gml:Envelope>
      </gml:BoundedBy>
      <skos:broader rdf:resource="urn:aodn.org.au:geographicextents:concept:10009"/>
      <skos:definition xml:lang="en">Coastal Cities / Towns (Australia) | Esperance, WA</skos:definition>
      <skos:scopeNote xml:lang="en">Coastal Cities / Towns (Australia) | Esperance, WA: Coastal Cities / Towns (Australia) | Esperance, WA</skos:scopeNote>
   </skos:Concept>
   <skos:Concept rdf:about="urn:aodn.org.au:geographicextents:concept:114">
      <skos:prefLabel xml:lang="en">Coastal Cities / Towns (Australia) | Fremantle, WA</skos:prefLabel>
      <skos:inScheme rdf:resource="urn:aodn.org.au:geographicextents:conceptscheme:1.0"/>
      <gml:BoundedBy>
         <gml:Envelope gml:srsName="http://www.opengis.net/gml/srs/epsg.xml#epsg:4326">
            <gml:lowerCorner>115.73 -32.07</gml:lowerCorner>
            <gml:upperCorner>115.78 -32.04</gml:upperCorner>
         </gml:Envelope>
      </gml:BoundedBy>
      <skos:broader rdf:resource="urn:aodn.org.au:geographicextents:concept:10009"/>
      <skos:definition xml:lang="en">Coastal Cities / Towns (Australia) | Fremantle, WA</skos:definition>
      <skos:scopeNote xml:lang="en">Coastal Cities / Towns (Australia) | Fremantle, WA: Coastal Cities / Towns (Australia) | Fremantle, WA</skos:scopeNote>
   </skos:Concept>
   <skos:Concept rdf:about="urn:aodn.org.au:geographicextents:concept:115">
      <skos:prefLabel xml:lang="en">Coastal Cities / Towns (Australia) | Geraldton, WA</skos:prefLabel>
      <skos:inScheme rdf:resource="urn:aodn.org.au:geographicextents:conceptscheme:1.0"/>
      <gml:BoundedBy>
         <gml:Envelope gml:srsName="http://www.opengis.net/gml/srs/epsg.xml#epsg:4326">
            <gml:lowerCorner>114.59 -28.79</gml:lowerCorner>
            <gml:upperCorner>114.63 -28.76</gml:upperCorner>
         </gml:Envelope>
      </gml:BoundedBy>
      <skos:broader rdf:resource="urn:aodn.org.au:geographicextents:concept:10009"/>
      <skos:definition xml:lang="en">Coastal Cities / Towns (Australia) | Geraldton, WA</skos:definition>
      <skos:scopeNote xml:lang="en">Coastal Cities / Towns (Australia) | Geraldton, WA: Coastal Cities / Towns (Australia) | Geraldton, WA</skos:scopeNote>
   </skos:Concept>
   <skos:Concept rdf:about="urn:aodn.org.au:geographicextents:concept:116">
      <skos:prefLabel xml:lang="en">Coastal Cities / Towns (Australia) | Gladstone, QLD</skos:prefLabel>
      <skos:inScheme rdf:resource="urn:aodn.org.au:geographicextents:conceptscheme:1.0"/>
      <gml:BoundedBy>
         <gml:Envelope gml:srsName="http://www.opengis.net/gml/srs/epsg.xml#epsg:4326">
            <gml:lowerCorner>151.23 -23.86</gml:lowerCorner>
            <gml:upperCorner>151.27 -23.83</gml:upperCorner>
         </gml:Envelope>
      </gml:BoundedBy>
      <skos:broader rdf:resource="urn:aodn.org.au:geographicextents:concept:10009"/>
      <skos:definition xml:lang="en">Coastal Cities / Towns (Australia) | Gladstone, QLD</skos:definition>
      <skos:scopeNote xml:lang="en">Coastal Cities / Towns (Australia) | Gladstone, QLD: Coastal Cities / Towns (Australia) | Gladstone, QLD</skos:scopeNote>
   </skos:Concept>
   <skos:Concept rdf:about="urn:aodn.org.au:geographicextents:concept:117">
      <skos:prefLabel xml:lang="en">Coastal Cities / Towns (Australia) | Hobart, TAS</skos:prefLabel>
      <skos:inScheme rdf:resource="urn:aodn.org.au:geographicextents:conceptscheme:1.0"/>
      <gml:BoundedBy>
         <gml:Envelope gml:srsName="http://www.opengis.net/gml/srs/epsg.xml#epsg:4326">
            <gml:lowerCorner>147.31 -42.9</gml:lowerCorner>
            <gml:upperCorner>147.35 -42.88</gml:upperCorner>
         </gml:Envelope>
      </gml:BoundedBy>
      <skos:broader rdf:resource="urn:aodn.org.au:geographicextents:concept:10009"/>
      <skos:definition xml:lang="en">Coastal Cities / Towns (Australia) | Hobart, TAS</skos:definition>
      <skos:scopeNote xml:lang="en">Coastal Cities / Towns (Australia) | Hobart, TAS: Coastal Cities / Towns (Australia) | Hobart, TAS</skos:scopeNote>
   </skos:Concept>
   <skos:Concept rdf:about="urn:aodn.org.au:geographicextents:concept:118">
      <skos:prefLabel xml:lang="en">Coastal Cities / Towns (Australia) | Launceston, TAS</skos:prefLabel>
      <skos:inScheme rdf:resource="urn:aodn.org.au:geographicextents:conceptscheme:1.0"/>
      <gml:BoundedBy>
         <gml:Envelope gml:srsName="http://www.opengis.net/gml/srs/epsg.xml#epsg:4326">
            <gml:lowerCorner>147.12 -41.46</gml:lowerCorner>
            <gml:upperCorner>147.17 -41.41</gml:upperCorner>
         </gml:Envelope>
      </gml:BoundedBy>
      <skos:broader rdf:resource="urn:aodn.org.au:geographicextents:concept:10009"/>
      <skos:definition xml:lang="en">Coastal Cities / Towns (Australia) | Launceston, TAS</skos:definition>
      <skos:scopeNote xml:lang="en">Coastal Cities / Towns (Australia) | Launceston, TAS: Coastal Cities / Towns (Australia) | Launceston, TAS</skos:scopeNote>
   </skos:Concept>
   <skos:Concept rdf:about="urn:aodn.org.au:geographicextents:concept:119">
      <skos:prefLabel xml:lang="en">Coastal Cities / Towns (Australia) | Mackay, QLD</skos:prefLabel>
      <skos:inScheme rdf:resource="urn:aodn.org.au:geographicextents:conceptscheme:1.0"/>
      <gml:BoundedBy>
         <gml:Envelope gml:srsName="http://www.opengis.net/gml/srs/epsg.xml#epsg:4326">
            <gml:lowerCorner>149.16 -21.16</gml:lowerCorner>
            <gml:upperCorner>149.2 -21.13</gml:upperCorner>
         </gml:Envelope>
      </gml:BoundedBy>
      <skos:broader rdf:resource="urn:aodn.org.au:geographicextents:concept:10009"/>
      <skos:definition xml:lang="en">Coastal Cities / Towns (Australia) | Mackay, QLD</skos:definition>
      <skos:scopeNote xml:lang="en">Coastal Cities / Towns (Australia) | Mackay, QLD: Coastal Cities / Towns (Australia) | Mackay, QLD</skos:scopeNote>
   </skos:Concept>
   <skos:Concept rdf:about="urn:aodn.org.au:geographicextents:concept:120">
      <skos:prefLabel xml:lang="en">Coastal Cities / Towns (Australia) | Melbourne, VIC</skos:prefLabel>
      <skos:inScheme rdf:resource="urn:aodn.org.au:geographicextents:conceptscheme:1.0"/>
      <gml:BoundedBy>
         <gml:Envelope gml:srsName="http://www.opengis.net/gml/srs/epsg.xml#epsg:4326">
            <gml:lowerCorner>144.59 -38.44</gml:lowerCorner>
            <gml:upperCorner>145.52 -37.51</gml:upperCorner>
         </gml:Envelope>
      </gml:BoundedBy>
      <skos:broader rdf:resource="urn:aodn.org.au:geographicextents:concept:10009"/>
      <skos:definition xml:lang="en">Coastal Cities / Towns (Australia) | Melbourne, VIC</skos:definition>
      <skos:scopeNote xml:lang="en">Coastal Cities / Towns (Australia) | Melbourne, VIC: Coastal Cities / Towns (Australia) | Melbourne, VIC</skos:scopeNote>
   </skos:Concept>
   <skos:Concept rdf:about="urn:aodn.org.au:geographicextents:concept:121">
      <skos:prefLabel xml:lang="en">Coastal Cities / Towns (Australia) | Newcastle, NSW</skos:prefLabel>
      <skos:inScheme rdf:resource="urn:aodn.org.au:geographicextents:conceptscheme:1.0"/>
      <gml:BoundedBy>
         <gml:Envelope gml:srsName="http://www.opengis.net/gml/srs/epsg.xml#epsg:4326">
            <gml:lowerCorner>151.75 -32.94</gml:lowerCorner>
            <gml:upperCorner>151.81 -32.9</gml:upperCorner>
         </gml:Envelope>
      </gml:BoundedBy>
      <skos:broader rdf:resource="urn:aodn.org.au:geographicextents:concept:10009"/>
      <skos:definition xml:lang="en">Coastal Cities / Towns (Australia) | Newcastle, NSW</skos:definition>
      <skos:scopeNote xml:lang="en">Coastal Cities / Towns (Australia) | Newcastle, NSW: Coastal Cities / Towns (Australia) | Newcastle, NSW</skos:scopeNote>
   </skos:Concept>
   <skos:Concept rdf:about="urn:aodn.org.au:geographicextents:concept:1028">
      <skos:prefLabel xml:lang="en">Coastal Cities / Towns (Australia) | Onslow, WA</skos:prefLabel>
      <skos:inScheme rdf:resource="urn:aodn.org.au:geographicextents:conceptscheme:1.0"/>
      <gml:BoundedBy>
         <gml:Envelope gml:srsName="http://www.opengis.net/gml/srs/epsg.xml#epsg:4326">
            <gml:lowerCorner>115.03 -21.73</gml:lowerCorner>
            <gml:upperCorner>115.26 -21.62</gml:upperCorner>
         </gml:Envelope>
      </gml:BoundedBy>
      <skos:broader rdf:resource="urn:aodn.org.au:geographicextents:concept:10009"/>
      <skos:definition xml:lang="en">Coastal Cities / Towns (Australia) | Onslow, WA</skos:definition>
      <skos:scopeNote xml:lang="en">Coastal Cities / Towns (Australia) | Onslow, WA: Coastal Cities / Towns (Australia) | Onslow, WA</skos:scopeNote>
   </skos:Concept>
   <skos:Concept rdf:about="urn:aodn.org.au:geographicextents:concept:122">
      <skos:prefLabel xml:lang="en">Coastal Cities / Towns (Australia) | Perth, WA</skos:prefLabel>
      <skos:inScheme rdf:resource="urn:aodn.org.au:geographicextents:conceptscheme:1.0"/>
      <gml:BoundedBy>
         <gml:Envelope gml:srsName="http://www.opengis.net/gml/srs/epsg.xml#epsg:4326">
            <gml:lowerCorner>115.68 -32.46</gml:lowerCorner>
            <gml:upperCorner>116.24 -31.62</gml:upperCorner>
         </gml:Envelope>
      </gml:BoundedBy>
      <skos:broader rdf:resource="urn:aodn.org.au:geographicextents:concept:10009"/>
      <skos:definition xml:lang="en">Coastal Cities / Towns (Australia) | Perth, WA</skos:definition>
      <skos:scopeNote xml:lang="en">Coastal Cities / Towns (Australia) | Perth, WA: Coastal Cities / Towns (Australia) | Perth, WA</skos:scopeNote>
   </skos:Concept>
   <skos:Concept rdf:about="urn:aodn.org.au:geographicextents:concept:123">
      <skos:prefLabel xml:lang="en">Coastal Cities / Towns (Australia) | Port Hedland, WA</skos:prefLabel>
      <skos:inScheme rdf:resource="urn:aodn.org.au:geographicextents:conceptscheme:1.0"/>
      <gml:BoundedBy>
         <gml:Envelope gml:srsName="http://www.opengis.net/gml/srs/epsg.xml#epsg:4326">
            <gml:lowerCorner>118.57 -20.4</gml:lowerCorner>
            <gml:upperCorner>118.69 -20.27</gml:upperCorner>
         </gml:Envelope>
      </gml:BoundedBy>
      <skos:broader rdf:resource="urn:aodn.org.au:geographicextents:concept:10009"/>
      <skos:definition xml:lang="en">Coastal Cities / Towns (Australia) | Port Hedland, WA</skos:definition>
      <skos:scopeNote xml:lang="en">Coastal Cities / Towns (Australia) | Port Hedland, WA: Coastal Cities / Towns (Australia) | Port Hedland, WA</skos:scopeNote>
   </skos:Concept>
   <skos:Concept rdf:about="urn:aodn.org.au:geographicextents:concept:124">
      <skos:prefLabel xml:lang="en">Coastal Cities / Towns (Australia) | Portland, VIC</skos:prefLabel>
      <skos:inScheme rdf:resource="urn:aodn.org.au:geographicextents:conceptscheme:1.0"/>
      <gml:BoundedBy>
         <gml:Envelope gml:srsName="http://www.opengis.net/gml/srs/epsg.xml#epsg:4326">
            <gml:lowerCorner>141.56 -38.41</gml:lowerCorner>
            <gml:upperCorner>141.66 -38.32</gml:upperCorner>
         </gml:Envelope>
      </gml:BoundedBy>
      <skos:broader rdf:resource="urn:aodn.org.au:geographicextents:concept:10009"/>
      <skos:definition xml:lang="en">Coastal Cities / Towns (Australia) | Portland, VIC</skos:definition>
      <skos:scopeNote xml:lang="en">Coastal Cities / Towns (Australia) | Portland, VIC: Coastal Cities / Towns (Australia) | Portland, VIC</skos:scopeNote>
   </skos:Concept>
   <skos:Concept rdf:about="urn:aodn.org.au:geographicextents:concept:125">
      <skos:prefLabel xml:lang="en">Coastal Cities / Towns (Australia) | Rockhampton, QLD</skos:prefLabel>
      <skos:inScheme rdf:resource="urn:aodn.org.au:geographicextents:conceptscheme:1.0"/>
      <gml:BoundedBy>
         <gml:Envelope gml:srsName="http://www.opengis.net/gml/srs/epsg.xml#epsg:4326">
            <gml:lowerCorner>150.49 -23.4</gml:lowerCorner>
            <gml:upperCorner>150.53 -23.36</gml:upperCorner>
         </gml:Envelope>
      </gml:BoundedBy>
      <skos:broader rdf:resource="urn:aodn.org.au:geographicextents:concept:10009"/>
      <skos:definition xml:lang="en">Coastal Cities / Towns (Australia) | Rockhampton, QLD</skos:definition>
      <skos:scopeNote xml:lang="en">Coastal Cities / Towns (Australia) | Rockhampton, QLD: Coastal Cities / Towns (Australia) | Rockhampton, QLD</skos:scopeNote>
   </skos:Concept>
   <skos:Concept rdf:about="urn:aodn.org.au:geographicextents:concept:126">
      <skos:prefLabel xml:lang="en">Coastal Cities / Towns (Australia) | Sydney, NSW</skos:prefLabel>
      <skos:inScheme rdf:resource="urn:aodn.org.au:geographicextents:conceptscheme:1.0"/>
      <gml:BoundedBy>
         <gml:Envelope gml:srsName="http://www.opengis.net/gml/srs/epsg.xml#epsg:4326">
            <gml:lowerCorner>150.52 -34.12</gml:lowerCorner>
            <gml:upperCorner>151.35 -33.57</gml:upperCorner>
         </gml:Envelope>
      </gml:BoundedBy>
      <skos:broader rdf:resource="urn:aodn.org.au:geographicextents:concept:10009"/>
      <skos:definition xml:lang="en">Coastal Cities / Towns (Australia) | Sydney, NSW</skos:definition>
      <skos:scopeNote xml:lang="en">Coastal Cities / Towns (Australia) | Sydney, NSW: Coastal Cities / Towns (Australia) | Sydney, NSW</skos:scopeNote>
   </skos:Concept>
   <skos:Concept rdf:about="urn:aodn.org.au:geographicextents:concept:127">
      <skos:prefLabel xml:lang="en">Coastal Cities / Towns (Australia) | Townsville, QLD</skos:prefLabel>
      <skos:inScheme rdf:resource="urn:aodn.org.au:geographicextents:conceptscheme:1.0"/>
      <gml:BoundedBy>
         <gml:Envelope gml:srsName="http://www.opengis.net/gml/srs/epsg.xml#epsg:4326">
            <gml:lowerCorner>146.8 -19.28</gml:lowerCorner>
            <gml:upperCorner>146.83 -19.24</gml:upperCorner>
         </gml:Envelope>
      </gml:BoundedBy>
      <skos:broader rdf:resource="urn:aodn.org.au:geographicextents:concept:10009"/>
      <skos:definition xml:lang="en">Coastal Cities / Towns (Australia) | Townsville, QLD</skos:definition>
      <skos:scopeNote xml:lang="en">Coastal Cities / Towns (Australia) | Townsville, QLD: Coastal Cities / Towns (Australia) | Townsville, QLD</skos:scopeNote>
   </skos:Concept>
   <skos:Concept rdf:about="urn:aodn.org.au:geographicextents:concept:128">
      <skos:prefLabel xml:lang="en">Coastal Cities / Towns (Australia) | Wollongong, NSW</skos:prefLabel>
      <skos:inScheme rdf:resource="urn:aodn.org.au:geographicextents:conceptscheme:1.0"/>
      <gml:BoundedBy>
         <gml:Envelope gml:srsName="http://www.opengis.net/gml/srs/epsg.xml#epsg:4326">
            <gml:lowerCorner>150.87 -34.45</gml:lowerCorner>
            <gml:upperCorner>150.92 -34.41</gml:upperCorner>
         </gml:Envelope>
      </gml:BoundedBy>
      <skos:broader rdf:resource="urn:aodn.org.au:geographicextents:concept:10009"/>
      <skos:definition xml:lang="en">Coastal Cities / Towns (Australia) | Wollongong, NSW</skos:definition>
      <skos:scopeNote xml:lang="en">Coastal Cities / Towns (Australia) | Wollongong, NSW: Coastal Cities / Towns (Australia) | Wollongong, NSW</skos:scopeNote>
   </skos:Concept>
   <skos:Concept rdf:about="urn:aodn.org.au:geographicextents:concept:1002">
      <skos:prefLabel xml:lang="en">Coastal Waters (Australia) | New South Wales Coast, NSW</skos:prefLabel>
      <skos:inScheme rdf:resource="urn:aodn.org.au:geographicextents:conceptscheme:1.0"/>
      <gml:BoundedBy>
         <gml:Envelope gml:srsName="http://www.opengis.net/gml/srs/epsg.xml#epsg:4326">
            <gml:lowerCorner>150 -37.7</gml:lowerCorner>
            <gml:upperCorner>154 -28</gml:upperCorner>
         </gml:Envelope>
      </gml:BoundedBy>
      <skos:broader rdf:resource="urn:aodn.org.au:geographicextents:concept:10002"/>
      <skos:definition xml:lang="en">Coastal Waters (Australia) | New South Wales Coast, NSW</skos:definition>
      <skos:scopeNote xml:lang="en">Coastal Waters (Australia) | New South Wales Coast, NSW: Coastal Waters (Australia) | New South Wales Coast, NSW</skos:scopeNote>
   </skos:Concept>
   <skos:Concept rdf:about="urn:aodn.org.au:geographicextents:concept:1003">
      <skos:prefLabel xml:lang="en">Coastal Waters (Australia) | Northern Territory Coast, NT</skos:prefLabel>
      <skos:inScheme rdf:resource="urn:aodn.org.au:geographicextents:conceptscheme:1.0"/>
      <gml:BoundedBy>
         <gml:Envelope gml:srsName="http://www.opengis.net/gml/srs/epsg.xml#epsg:4326">
            <gml:lowerCorner>129 -15</gml:lowerCorner>
            <gml:upperCorner>138 -9</gml:upperCorner>
         </gml:Envelope>
      </gml:BoundedBy>
      <skos:broader rdf:resource="urn:aodn.org.au:geographicextents:concept:10002"/>
      <skos:definition xml:lang="en">Coastal Waters (Australia) | Northern Territory Coast, NT</skos:definition>
      <skos:scopeNote xml:lang="en">Coastal Waters (Australia) | Northern Territory Coast, NT: Coastal Waters (Australia) | Northern Territory Coast, NT</skos:scopeNote>
   </skos:Concept>
   <skos:Concept rdf:about="urn:aodn.org.au:geographicextents:concept:1005">
      <skos:prefLabel xml:lang="en">Coastal Waters (Australia) | Queensland Coast, QLD</skos:prefLabel>
      <skos:inScheme rdf:resource="urn:aodn.org.au:geographicextents:conceptscheme:1.0"/>
      <gml:BoundedBy>
         <gml:Envelope gml:srsName="http://www.opengis.net/gml/srs/epsg.xml#epsg:4326">
            <gml:lowerCorner>138 -29.5</gml:lowerCorner>
            <gml:upperCorner>155 -9</gml:upperCorner>
         </gml:Envelope>
      </gml:BoundedBy>
      <skos:broader rdf:resource="urn:aodn.org.au:geographicextents:concept:10002"/>
      <skos:definition xml:lang="en">Coastal Waters (Australia) | Queensland Coast, QLD</skos:definition>
      <skos:scopeNote xml:lang="en">Coastal Waters (Australia) | Queensland Coast, QLD: Coastal Waters (Australia) | Queensland Coast, QLD</skos:scopeNote>
   </skos:Concept>
   <skos:Concept rdf:about="urn:aodn.org.au:geographicextents:concept:1007">
      <skos:prefLabel xml:lang="en">Coastal Waters (Australia) | Queensland Coast Northwest, QLD</skos:prefLabel>
      <skos:inScheme rdf:resource="urn:aodn.org.au:geographicextents:conceptscheme:1.0"/>
      <gml:BoundedBy>
         <gml:Envelope gml:srsName="http://www.opengis.net/gml/srs/epsg.xml#epsg:4326">
            <gml:lowerCorner>138 -18</gml:lowerCorner>
            <gml:upperCorner>142.5 -11</gml:upperCorner>
         </gml:Envelope>
      </gml:BoundedBy>
      <skos:broader rdf:resource="urn:aodn.org.au:geographicextents:concept:10002"/>
      <skos:definition xml:lang="en">Coastal Waters (Australia) | Queensland Coast Northwest, QLD</skos:definition>
      <skos:scopeNote xml:lang="en">Coastal Waters (Australia) | Queensland Coast Northwest, QLD: Coastal Waters (Australia) | Queensland Coast Northwest, QLD</skos:scopeNote>
   </skos:Concept>
   <skos:Concept rdf:about="urn:aodn.org.au:geographicextents:concept:1008">
      <skos:prefLabel xml:lang="en">Coastal Waters (Australia) | Queensland Coast South, QLD</skos:prefLabel>
      <skos:inScheme rdf:resource="urn:aodn.org.au:geographicextents:conceptscheme:1.0"/>
      <gml:BoundedBy>
         <gml:Envelope gml:srsName="http://www.opengis.net/gml/srs/epsg.xml#epsg:4326">
            <gml:lowerCorner>152 -28</gml:lowerCorner>
            <gml:upperCorner>154 -24.5</gml:upperCorner>
         </gml:Envelope>
      </gml:BoundedBy>
      <skos:broader rdf:resource="urn:aodn.org.au:geographicextents:concept:10002"/>
      <skos:definition xml:lang="en">Coastal Waters (Australia) | Queensland Coast South, QLD</skos:definition>
      <skos:scopeNote xml:lang="en">Coastal Waters (Australia) | Queensland Coast South, QLD: Coastal Waters (Australia) | Queensland Coast South, QLD</skos:scopeNote>
   </skos:Concept>
   <skos:Concept rdf:about="urn:aodn.org.au:geographicextents:concept:1009">
      <skos:prefLabel xml:lang="en">Coastal Waters (Australia) | South Australia Coast, SA</skos:prefLabel>
      <skos:inScheme rdf:resource="urn:aodn.org.au:geographicextents:conceptscheme:1.0"/>
      <gml:BoundedBy>
         <gml:Envelope gml:srsName="http://www.opengis.net/gml/srs/epsg.xml#epsg:4326">
            <gml:lowerCorner>129 -38.5</gml:lowerCorner>
            <gml:upperCorner>141 -31.5</gml:upperCorner>
         </gml:Envelope>
      </gml:BoundedBy>
      <skos:broader rdf:resource="urn:aodn.org.au:geographicextents:concept:10002"/>
      <skos:definition xml:lang="en">Coastal Waters (Australia) | South Australia Coast, SA</skos:definition>
      <skos:scopeNote xml:lang="en">Coastal Waters (Australia) | South Australia Coast, SA: Coastal Waters (Australia) | South Australia Coast, SA</skos:scopeNote>
   </skos:Concept>
   <skos:Concept rdf:about="urn:aodn.org.au:geographicextents:concept:1010">
      <skos:prefLabel xml:lang="en">Coastal Waters (Australia) | Tasmania Coast, TAS</skos:prefLabel>
      <skos:inScheme rdf:resource="urn:aodn.org.au:geographicextents:conceptscheme:1.0"/>
      <gml:BoundedBy>
         <gml:Envelope gml:srsName="http://www.opengis.net/gml/srs/epsg.xml#epsg:4326">
            <gml:lowerCorner>143.5 -45</gml:lowerCorner>
            <gml:upperCorner>149 -39.5</gml:upperCorner>
         </gml:Envelope>
      </gml:BoundedBy>
      <skos:broader rdf:resource="urn:aodn.org.au:geographicextents:concept:10002"/>
      <skos:definition xml:lang="en">Coastal Waters (Australia) | Tasmania Coast, TAS</skos:definition>
      <skos:scopeNote xml:lang="en">Coastal Waters (Australia) | Tasmania Coast, TAS: Coastal Waters (Australia) | Tasmania Coast, TAS</skos:scopeNote>
   </skos:Concept>
   <skos:Concept rdf:about="urn:aodn.org.au:geographicextents:concept:1011">
      <skos:prefLabel xml:lang="en">Coastal Waters (Australia) | Tasmania Coast East and Southeast, TAS</skos:prefLabel>
      <skos:inScheme rdf:resource="urn:aodn.org.au:geographicextents:conceptscheme:1.0"/>
      <gml:BoundedBy>
         <gml:Envelope gml:srsName="http://www.opengis.net/gml/srs/epsg.xml#epsg:4326">
            <gml:lowerCorner>146.5 -45</gml:lowerCorner>
            <gml:upperCorner>149 -39.5</gml:upperCorner>
         </gml:Envelope>
      </gml:BoundedBy>
      <skos:broader rdf:resource="urn:aodn.org.au:geographicextents:concept:10002"/>
      <skos:definition xml:lang="en">Coastal Waters (Australia) | Tasmania Coast East and Southeast, TAS</skos:definition>
      <skos:scopeNote xml:lang="en">Coastal Waters (Australia) | Tasmania Coast East and Southeast, TAS: Coastal Waters (Australia) | Tasmania Coast East and Southeast, TAS</skos:scopeNote>
   </skos:Concept>
   <skos:Concept rdf:about="urn:aodn.org.au:geographicextents:concept:1012">
      <skos:prefLabel xml:lang="en">Coastal Waters (Australia) | Tasmania Coast North, TAS</skos:prefLabel>
      <skos:inScheme rdf:resource="urn:aodn.org.au:geographicextents:conceptscheme:1.0"/>
      <gml:BoundedBy>
         <gml:Envelope gml:srsName="http://www.opengis.net/gml/srs/epsg.xml#epsg:4326">
            <gml:lowerCorner>144 -41.5</gml:lowerCorner>
            <gml:upperCorner>148.5 -39</gml:upperCorner>
         </gml:Envelope>
      </gml:BoundedBy>
      <skos:broader rdf:resource="urn:aodn.org.au:geographicextents:concept:10002"/>
      <skos:definition xml:lang="en">Coastal Waters (Australia) | Tasmania Coast North, TAS</skos:definition>
      <skos:scopeNote xml:lang="en">Coastal Waters (Australia) | Tasmania Coast North, TAS: Coastal Waters (Australia) | Tasmania Coast North, TAS</skos:scopeNote>
   </skos:Concept>
   <skos:Concept rdf:about="urn:aodn.org.au:geographicextents:concept:1013">
      <skos:prefLabel xml:lang="en">Coastal Waters (Australia) | Tasmania Coast West, TAS</skos:prefLabel>
      <skos:inScheme rdf:resource="urn:aodn.org.au:geographicextents:conceptscheme:1.0"/>
      <gml:BoundedBy>
         <gml:Envelope gml:srsName="http://www.opengis.net/gml/srs/epsg.xml#epsg:4326">
            <gml:lowerCorner>143.5 -44.5</gml:lowerCorner>
            <gml:upperCorner>146.5 -39.5</gml:upperCorner>
         </gml:Envelope>
      </gml:BoundedBy>
      <skos:broader rdf:resource="urn:aodn.org.au:geographicextents:concept:10002"/>
      <skos:definition xml:lang="en">Coastal Waters (Australia) | Tasmania Coast West, TAS</skos:definition>
      <skos:scopeNote xml:lang="en">Coastal Waters (Australia) | Tasmania Coast West, TAS: Coastal Waters (Australia) | Tasmania Coast West, TAS</skos:scopeNote>
   </skos:Concept>
   <skos:Concept rdf:about="urn:aodn.org.au:geographicextents:concept:1014">
      <skos:prefLabel xml:lang="en">Coastal Waters (Australia) | Victoria Coast, VIC</skos:prefLabel>
      <skos:inScheme rdf:resource="urn:aodn.org.au:geographicextents:conceptscheme:1.0"/>
      <gml:BoundedBy>
         <gml:Envelope gml:srsName="http://www.opengis.net/gml/srs/epsg.xml#epsg:4326">
            <gml:lowerCorner>141 -40</gml:lowerCorner>
            <gml:upperCorner>150 -37.5</gml:upperCorner>
         </gml:Envelope>
      </gml:BoundedBy>
      <skos:broader rdf:resource="urn:aodn.org.au:geographicextents:concept:10002"/>
      <skos:definition xml:lang="en">Coastal Waters (Australia) | Victoria Coast, VIC</skos:definition>
      <skos:scopeNote xml:lang="en">Coastal Waters (Australia) | Victoria Coast, VIC: Coastal Waters (Australia) | Victoria Coast, VIC</skos:scopeNote>
   </skos:Concept>
   <skos:Concept rdf:about="urn:aodn.org.au:geographicextents:concept:1015">
      <skos:prefLabel xml:lang="en">Coastal Waters (Australia) | West Australia Coast, WA</skos:prefLabel>
      <skos:inScheme rdf:resource="urn:aodn.org.au:geographicextents:conceptscheme:1.0"/>
      <gml:BoundedBy>
         <gml:Envelope gml:srsName="http://www.opengis.net/gml/srs/epsg.xml#epsg:4326">
            <gml:lowerCorner>109 -38</gml:lowerCorner>
            <gml:upperCorner>129 -12</gml:upperCorner>
         </gml:Envelope>
      </gml:BoundedBy>
      <skos:broader rdf:resource="urn:aodn.org.au:geographicextents:concept:10002"/>
      <skos:definition xml:lang="en">Coastal Waters (Australia) | West Australia Coast, WA</skos:definition>
      <skos:scopeNote xml:lang="en">Coastal Waters (Australia) | West Australia Coast, WA: Coastal Waters (Australia) | West Australia Coast, WA</skos:scopeNote>
   </skos:Concept>
   <skos:Concept rdf:about="urn:aodn.org.au:geographicextents:concept:1016">
      <skos:prefLabel xml:lang="en">Coastal Waters (Australia) | West Australia Coast North, WA</skos:prefLabel>
      <skos:inScheme rdf:resource="urn:aodn.org.au:geographicextents:conceptscheme:1.0"/>
      <gml:BoundedBy>
         <gml:Envelope gml:srsName="http://www.opengis.net/gml/srs/epsg.xml#epsg:4326">
            <gml:lowerCorner>113.5 -22</gml:lowerCorner>
            <gml:upperCorner>129 -10</gml:upperCorner>
         </gml:Envelope>
      </gml:BoundedBy>
      <skos:broader rdf:resource="urn:aodn.org.au:geographicextents:concept:10002"/>
      <skos:definition xml:lang="en">Coastal Waters (Australia) | West Australia Coast North, WA</skos:definition>
      <skos:scopeNote xml:lang="en">Coastal Waters (Australia) | West Australia Coast North, WA: Coastal Waters (Australia) | West Australia Coast North, WA</skos:scopeNote>
   </skos:Concept>
   <skos:Concept rdf:about="urn:aodn.org.au:geographicextents:concept:1017">
      <skos:prefLabel xml:lang="en">Coastal Waters (Australia) | West Australia Coast South, WA</skos:prefLabel>
      <skos:inScheme rdf:resource="urn:aodn.org.au:geographicextents:conceptscheme:1.0"/>
      <gml:BoundedBy>
         <gml:Envelope gml:srsName="http://www.opengis.net/gml/srs/epsg.xml#epsg:4326">
            <gml:lowerCorner>114 -36</gml:lowerCorner>
            <gml:upperCorner>129 -31.5</gml:upperCorner>
         </gml:Envelope>
      </gml:BoundedBy>
      <skos:broader rdf:resource="urn:aodn.org.au:geographicextents:concept:10002"/>
      <skos:definition xml:lang="en">Coastal Waters (Australia) | West Australia Coast South, WA</skos:definition>
      <skos:scopeNote xml:lang="en">Coastal Waters (Australia) | West Australia Coast South, WA: Coastal Waters (Australia) | West Australia Coast South, WA</skos:scopeNote>
   </skos:Concept>
   <skos:Concept rdf:about="urn:aodn.org.au:geographicextents:concept:1018">
      <skos:prefLabel xml:lang="en">Coastal Waters (Australia) | West Australia Coast West, WA</skos:prefLabel>
      <skos:inScheme rdf:resource="urn:aodn.org.au:geographicextents:conceptscheme:1.0"/>
      <gml:BoundedBy>
         <gml:Envelope gml:srsName="http://www.opengis.net/gml/srs/epsg.xml#epsg:4326">
            <gml:lowerCorner>112 -35</gml:lowerCorner>
            <gml:upperCorner>116 -22</gml:upperCorner>
         </gml:Envelope>
      </gml:BoundedBy>
      <skos:broader rdf:resource="urn:aodn.org.au:geographicextents:concept:10002"/>
      <skos:definition xml:lang="en">Coastal Waters (Australia) | West Australia Coast West, WA</skos:definition>
      <skos:scopeNote xml:lang="en">Coastal Waters (Australia) | West Australia Coast West, WA: Coastal Waters (Australia) | West Australia Coast West, WA</skos:scopeNote>
   </skos:Concept>
   <skos:Concept rdf:about="urn:aodn.org.au:geographicextents:concept:1022">
      <skos:prefLabel xml:lang="en">Coastal Waters (Global) | Indonesia Coast</skos:prefLabel>
      <skos:inScheme rdf:resource="urn:aodn.org.au:geographicextents:conceptscheme:1.0"/>
      <gml:BoundedBy>
         <gml:Envelope gml:srsName="http://www.opengis.net/gml/srs/epsg.xml#epsg:4326">
            <gml:lowerCorner>100 -12</gml:lowerCorner>
            <gml:upperCorner>141 2</gml:upperCorner>
         </gml:Envelope>
      </gml:BoundedBy>
      <skos:broader rdf:resource="urn:aodn.org.au:geographicextents:concept:10001"/>
      <skos:definition xml:lang="en">Coastal Waters (Global) | Indonesia Coast</skos:definition>
      <skos:scopeNote xml:lang="en">Coastal Waters (Global) | Indonesia Coast: Coastal Waters (Global) | Indonesia Coast</skos:scopeNote>
   </skos:Concept>
   <skos:Concept rdf:about="urn:aodn.org.au:geographicextents:concept:1023">
      <skos:prefLabel xml:lang="en">Coastal Waters (Global) | New Zealand Coast</skos:prefLabel>
      <skos:inScheme rdf:resource="urn:aodn.org.au:geographicextents:conceptscheme:1.0"/>
      <gml:BoundedBy>
         <gml:Envelope gml:srsName="http://www.opengis.net/gml/srs/epsg.xml#epsg:4326">
            <gml:lowerCorner>164 -48</gml:lowerCorner>
            <gml:upperCorner>180 -32</gml:upperCorner>
         </gml:Envelope>
      </gml:BoundedBy>
      <skos:broader rdf:resource="urn:aodn.org.au:geographicextents:concept:10001"/>
      <skos:definition xml:lang="en">Coastal Waters (Global) | New Zealand Coast</skos:definition>
      <skos:scopeNote xml:lang="en">Coastal Waters (Global) | New Zealand Coast: Coastal Waters (Global) | New Zealand Coast</skos:scopeNote>
   </skos:Concept>
   <skos:Concept rdf:about="urn:aodn.org.au:geographicextents:concept:1024">
      <skos:prefLabel xml:lang="en">Coastal Waters (Global) | Papua New Guinea Coast</skos:prefLabel>
      <skos:inScheme rdf:resource="urn:aodn.org.au:geographicextents:conceptscheme:1.0"/>
      <gml:BoundedBy>
         <gml:Envelope gml:srsName="http://www.opengis.net/gml/srs/epsg.xml#epsg:4326">
            <gml:lowerCorner>141 -12</gml:lowerCorner>
            <gml:upperCorner>156 -2</gml:upperCorner>
         </gml:Envelope>
      </gml:BoundedBy>
      <skos:broader rdf:resource="urn:aodn.org.au:geographicextents:concept:10001"/>
      <skos:definition xml:lang="en">Coastal Waters (Global) | Papua New Guinea Coast</skos:definition>
      <skos:scopeNote xml:lang="en">Coastal Waters (Global) | Papua New Guinea Coast: Coastal Waters (Global) | Papua New Guinea Coast</skos:scopeNote>
   </skos:Concept>
   <skos:Concept rdf:about="urn:aodn.org.au:geographicextents:concept:25">
      <skos:prefLabel xml:lang="en">Continents | Antarctica</skos:prefLabel>
      <skos:inScheme rdf:resource="urn:aodn.org.au:geographicextents:conceptscheme:1.0"/>
      <gml:BoundedBy>
         <gml:Envelope gml:srsName="http://www.opengis.net/gml/srs/epsg.xml#epsg:4326">
            <gml:lowerCorner>-180 -90</gml:lowerCorner>
            <gml:upperCorner>180 -60</gml:upperCorner>
         </gml:Envelope>
      </gml:BoundedBy>
      <skos:broader rdf:resource="urn:aodn.org.au:geographicextents:concept:10006"/>
      <skos:definition xml:lang="en">Continents | Antarctica</skos:definition>
      <skos:scopeNote xml:lang="en">Continents | Antarctica: Continents | Antarctica</skos:scopeNote>
   </skos:Concept>
   <skos:Concept rdf:about="urn:aodn.org.au:geographicextents:concept:26">
      <skos:prefLabel xml:lang="en">Countries | Australia</skos:prefLabel>
      <skos:inScheme rdf:resource="urn:aodn.org.au:geographicextents:conceptscheme:1.0"/>
      <gml:BoundedBy>
         <gml:Envelope gml:srsName="http://www.opengis.net/gml/srs/epsg.xml#epsg:4326">
            <gml:lowerCorner>112 -44</gml:lowerCorner>
            <gml:upperCorner>154 -9</gml:upperCorner>
         </gml:Envelope>
      </gml:BoundedBy>
      <skos:broader rdf:resource="urn:aodn.org.au:geographicextents:concept:10007"/>
      <skos:definition xml:lang="en">Countries | Australia</skos:definition>
      <skos:scopeNote xml:lang="en">Countries | Australia: Countries | Australia</skos:scopeNote>
   </skos:Concept>
   <skos:Concept rdf:about="urn:aodn.org.au:geographicextents:concept:1019">
      <skos:prefLabel xml:lang="en">Countries | Australia (including external territories)</skos:prefLabel>
      <skos:inScheme rdf:resource="urn:aodn.org.au:geographicextents:conceptscheme:1.0"/>
      <gml:BoundedBy>
         <gml:Envelope gml:srsName="http://www.opengis.net/gml/srs/epsg.xml#epsg:4326">
            <gml:lowerCorner>72.7 -53.5</gml:lowerCorner>
            <gml:upperCorner>168.2 -9.5</gml:upperCorner>
         </gml:Envelope>
      </gml:BoundedBy>
      <skos:broader rdf:resource="urn:aodn.org.au:geographicextents:concept:10007"/>
      <skos:definition xml:lang="en">Countries | Australia (including external territories)</skos:definition>
      <skos:scopeNote xml:lang="en">Countries | Australia (including external territories): Countries | Australia (including external territories)</skos:scopeNote>
   </skos:Concept>
   <skos:Concept rdf:about="urn:aodn.org.au:geographicextents:concept:1029">
      <skos:prefLabel xml:lang="en">Countries | Fiji</skos:prefLabel>
      <skos:inScheme rdf:resource="urn:aodn.org.au:geographicextents:conceptscheme:1.0"/>
      <gml:BoundedBy>
         <gml:Envelope gml:srsName="http://www.opengis.net/gml/srs/epsg.xml#epsg:4326">
            <gml:lowerCorner>176.79 -20.9</gml:lowerCorner>
            <gml:upperCorner>-177.86 -12.2</gml:upperCorner>
         </gml:Envelope>
      </gml:BoundedBy>
      <skos:broader rdf:resource="urn:aodn.org.au:geographicextents:concept:10007"/>
      <skos:definition xml:lang="en">Countries | Fiji</skos:definition>
      <skos:scopeNote xml:lang="en">Countries | Fiji: Countries | Fiji</skos:scopeNote>
   </skos:Concept>
   <skos:Concept rdf:about="urn:aodn.org.au:geographicextents:concept:28">
      <skos:prefLabel xml:lang="en">Countries | Indonesia</skos:prefLabel>
      <skos:inScheme rdf:resource="urn:aodn.org.au:geographicextents:conceptscheme:1.0"/>
      <gml:BoundedBy>
         <gml:Envelope gml:srsName="http://www.opengis.net/gml/srs/epsg.xml#epsg:4326">
            <gml:lowerCorner>94.73 -11.11</gml:lowerCorner>
            <gml:upperCorner>141.05 6.2</gml:upperCorner>
         </gml:Envelope>
      </gml:BoundedBy>
      <skos:broader rdf:resource="urn:aodn.org.au:geographicextents:concept:10007"/>
      <skos:definition xml:lang="en">Countries | Indonesia</skos:definition>
      <skos:scopeNote xml:lang="en">Countries | Indonesia: Countries | Indonesia</skos:scopeNote>
   </skos:Concept>
   <skos:Concept rdf:about="urn:aodn.org.au:geographicextents:concept:1030">
      <skos:prefLabel xml:lang="en">Countries | Japan</skos:prefLabel>
      <skos:inScheme rdf:resource="urn:aodn.org.au:geographicextents:conceptscheme:1.0"/>
      <gml:BoundedBy>
         <gml:Envelope gml:srsName="http://www.opengis.net/gml/srs/epsg.xml#epsg:4326">
            <gml:lowerCorner>122.85 20.35</gml:lowerCorner>
            <gml:upperCorner>154.01 45.65</gml:upperCorner>
         </gml:Envelope>
      </gml:BoundedBy>
      <skos:broader rdf:resource="urn:aodn.org.au:geographicextents:concept:10007"/>
      <skos:definition xml:lang="en">Countries | Japan</skos:definition>
      <skos:scopeNote xml:lang="en">Countries | Japan: Countries | Japan</skos:scopeNote>
   </skos:Concept>
   <skos:Concept rdf:about="urn:aodn.org.au:geographicextents:concept:1031">
      <skos:prefLabel xml:lang="en">Countries | Mauritius</skos:prefLabel>
      <skos:inScheme rdf:resource="urn:aodn.org.au:geographicextents:conceptscheme:1.0"/>
      <gml:BoundedBy>
         <gml:Envelope gml:srsName="http://www.opengis.net/gml/srs/epsg.xml#epsg:4326">
            <gml:lowerCorner>56.31 -20.75</gml:lowerCorner>
            <gml:upperCorner>63.81 -10.08</gml:upperCorner>
         </gml:Envelope>
      </gml:BoundedBy>
      <skos:broader rdf:resource="urn:aodn.org.au:geographicextents:concept:10007"/>
      <skos:definition xml:lang="en">Countries | Mauritius</skos:definition>
      <skos:scopeNote xml:lang="en">Countries | Mauritius: Countries | Mauritius</skos:scopeNote>
   </skos:Concept>
   <skos:Concept rdf:about="urn:aodn.org.au:geographicextents:concept:29">
      <skos:prefLabel xml:lang="en">Countries | New Caledonia</skos:prefLabel>
      <skos:inScheme rdf:resource="urn:aodn.org.au:geographicextents:conceptscheme:1.0"/>
      <gml:BoundedBy>
         <gml:Envelope gml:srsName="http://www.opengis.net/gml/srs/epsg.xml#epsg:4326">
            <gml:lowerCorner>163.35 -23.26</gml:lowerCorner>
            <gml:upperCorner>168.34 -19.16</gml:upperCorner>
         </gml:Envelope>
      </gml:BoundedBy>
      <skos:broader rdf:resource="urn:aodn.org.au:geographicextents:concept:10007"/>
      <skos:definition xml:lang="en">Countries | New Caledonia</skos:definition>
      <skos:scopeNote xml:lang="en">Countries | New Caledonia: Countries | New Caledonia</skos:scopeNote>
   </skos:Concept>
   <skos:Concept rdf:about="urn:aodn.org.au:geographicextents:concept:30">
      <skos:prefLabel xml:lang="en">Countries | New Zealand</skos:prefLabel>
      <skos:inScheme rdf:resource="urn:aodn.org.au:geographicextents:conceptscheme:1.0"/>
      <gml:BoundedBy>
         <gml:Envelope gml:srsName="http://www.opengis.net/gml/srs/epsg.xml#epsg:4326">
            <gml:lowerCorner>165.74 -52.73</gml:lowerCorner>
            <gml:upperCorner>-175.12 -28.87</gml:upperCorner>
         </gml:Envelope>
      </gml:BoundedBy>
      <skos:broader rdf:resource="urn:aodn.org.au:geographicextents:concept:10007"/>
      <skos:definition xml:lang="en">Countries | New Zealand</skos:definition>
      <skos:scopeNote xml:lang="en">Countries | New Zealand: Countries | New Zealand</skos:scopeNote>
   </skos:Concept>
   <skos:Concept rdf:about="urn:aodn.org.au:geographicextents:concept:31">
      <skos:prefLabel xml:lang="en">Countries | Papua New Guinea</skos:prefLabel>
      <skos:inScheme rdf:resource="urn:aodn.org.au:geographicextents:conceptscheme:1.0"/>
      <gml:BoundedBy>
         <gml:Envelope gml:srsName="http://www.opengis.net/gml/srs/epsg.xml#epsg:4326">
            <gml:lowerCorner>140.84 -12.09</gml:lowerCorner>
            <gml:upperCorner>159.97 -0.67</gml:upperCorner>
         </gml:Envelope>
      </gml:BoundedBy>
      <skos:broader rdf:resource="urn:aodn.org.au:geographicextents:concept:10007"/>
      <skos:definition xml:lang="en">Countries | Papua New Guinea</skos:definition>
      <skos:scopeNote xml:lang="en">Countries | Papua New Guinea: Countries | Papua New Guinea</skos:scopeNote>
   </skos:Concept>
   <skos:Concept rdf:about="urn:aodn.org.au:geographicextents:concept:32">
      <skos:prefLabel xml:lang="en">Countries | Solomon Islands</skos:prefLabel>
      <skos:inScheme rdf:resource="urn:aodn.org.au:geographicextents:conceptscheme:1.0"/>
      <gml:BoundedBy>
         <gml:Envelope gml:srsName="http://www.opengis.net/gml/srs/epsg.xml#epsg:4326">
            <gml:lowerCorner>155.11 -12.69</gml:lowerCorner>
            <gml:upperCorner>168.03 -6.07</gml:upperCorner>
         </gml:Envelope>
      </gml:BoundedBy>
      <skos:broader rdf:resource="urn:aodn.org.au:geographicextents:concept:10007"/>
      <skos:definition xml:lang="en">Countries | Solomon Islands</skos:definition>
      <skos:scopeNote xml:lang="en">Countries | Solomon Islands: Countries | Solomon Islands</skos:scopeNote>
   </skos:Concept>
   <skos:Concept rdf:about="urn:aodn.org.au:geographicextents:concept:27">
      <skos:prefLabel xml:lang="en">Countries | Timor-Leste</skos:prefLabel>
      <skos:inScheme rdf:resource="urn:aodn.org.au:geographicextents:conceptscheme:1.0"/>
      <gml:BoundedBy>
         <gml:Envelope gml:srsName="http://www.opengis.net/gml/srs/epsg.xml#epsg:4326">
            <gml:lowerCorner>124.03 -9.54</gml:lowerCorner>
            <gml:upperCorner>127.43 -8.04</gml:upperCorner>
         </gml:Envelope>
      </gml:BoundedBy>
      <skos:broader rdf:resource="urn:aodn.org.au:geographicextents:concept:10007"/>
      <skos:definition xml:lang="en">Countries | Timor-Leste</skos:definition>
      <skos:scopeNote xml:lang="en">Countries | Timor-Leste: Countries | Timor-Leste</skos:scopeNote>
   </skos:Concept>
   <skos:Concept rdf:about="urn:aodn.org.au:geographicextents:concept:1032">
      <skos:prefLabel xml:lang="en">Countries | Tonga</skos:prefLabel>
      <skos:inScheme rdf:resource="urn:aodn.org.au:geographicextents:conceptscheme:1.0"/>
      <gml:BoundedBy>
         <gml:Envelope gml:srsName="http://www.opengis.net/gml/srs/epsg.xml#epsg:4326">
            <gml:lowerCorner>-175.96 -21.84</gml:lowerCorner>
            <gml:upperCorner>-173.25 -15.4</gml:upperCorner>
         </gml:Envelope>
      </gml:BoundedBy>
      <skos:broader rdf:resource="urn:aodn.org.au:geographicextents:concept:10007"/>
      <skos:definition xml:lang="en">Countries | Tonga</skos:definition>
      <skos:scopeNote xml:lang="en">Countries | Tonga: Countries | Tonga</skos:scopeNote>
   </skos:Concept>
   <skos:Concept rdf:about="urn:aodn.org.au:geographicextents:concept:33">
      <skos:prefLabel xml:lang="en">Countries | Vanuatu</skos:prefLabel>
      <skos:inScheme rdf:resource="urn:aodn.org.au:geographicextents:conceptscheme:1.0"/>
      <gml:BoundedBy>
         <gml:Envelope gml:srsName="http://www.opengis.net/gml/srs/epsg.xml#epsg:4326">
            <gml:lowerCorner>166.05 -20.54</gml:lowerCorner>
            <gml:upperCorner>170.51 -12.8</gml:upperCorner>
         </gml:Envelope>
      </gml:BoundedBy>
      <skos:broader rdf:resource="urn:aodn.org.au:geographicextents:concept:10007"/>
      <skos:definition xml:lang="en">Countries | Vanuatu</skos:definition>
      <skos:scopeNote xml:lang="en">Countries | Vanuatu: Countries | Vanuatu</skos:scopeNote>
   </skos:Concept>
   <skos:Concept rdf:about="urn:aodn.org.au:geographicextents:concept:3">
      <skos:prefLabel xml:lang="en">Global / Oceans | Atlantic Ocean</skos:prefLabel>
      <skos:inScheme rdf:resource="urn:aodn.org.au:geographicextents:conceptscheme:1.0"/>
      <gml:BoundedBy>
         <gml:Envelope gml:srsName="http://www.opengis.net/gml/srs/epsg.xml#epsg:4326">
            <gml:lowerCorner>-80 -60</gml:lowerCorner>
            <gml:upperCorner>20 67</gml:upperCorner>
         </gml:Envelope>
      </gml:BoundedBy>
      <skos:broader rdf:resource="urn:aodn.org.au:geographicextents:concept:10008"/>
      <skos:definition xml:lang="en">Global / Oceans | Atlantic Ocean</skos:definition>
      <skos:scopeNote xml:lang="en">Global / Oceans | Atlantic Ocean: Global / Oceans | Atlantic Ocean</skos:scopeNote>
   </skos:Concept>
   <skos:Concept rdf:about="urn:aodn.org.au:geographicextents:concept:1000">
      <skos:prefLabel xml:lang="en">Global / Oceans | Australasia</skos:prefLabel>
      <skos:inScheme rdf:resource="urn:aodn.org.au:geographicextents:conceptscheme:1.0"/>
      <gml:BoundedBy>
         <gml:Envelope gml:srsName="http://www.opengis.net/gml/srs/epsg.xml#epsg:4326">
            <gml:lowerCorner>112 -60</gml:lowerCorner>
            <gml:upperCorner>180 0</gml:upperCorner>
         </gml:Envelope>
      </gml:BoundedBy>
      <skos:broader rdf:resource="urn:aodn.org.au:geographicextents:concept:10008"/>
      <skos:definition xml:lang="en">Global / Oceans | Australasia</skos:definition>
      <skos:scopeNote xml:lang="en">Global / Oceans | Australasia: Global / Oceans | Australasia</skos:scopeNote>
   </skos:Concept>
   <skos:Concept rdf:about="urn:aodn.org.au:geographicextents:concept:1020">
      <skos:prefLabel xml:lang="en">Global / Oceans | East Indian Ocean</skos:prefLabel>
      <skos:inScheme rdf:resource="urn:aodn.org.au:geographicextents:conceptscheme:1.0"/>
      <gml:BoundedBy>
         <gml:Envelope gml:srsName="http://www.opengis.net/gml/srs/epsg.xml#epsg:4326">
            <gml:lowerCorner>75 -70</gml:lowerCorner>
            <gml:upperCorner>120 28</gml:upperCorner>
         </gml:Envelope>
      </gml:BoundedBy>
      <skos:broader rdf:resource="urn:aodn.org.au:geographicextents:concept:10008"/>
      <skos:definition xml:lang="en">Global / Oceans | East Indian Ocean</skos:definition>
      <skos:scopeNote xml:lang="en">Global / Oceans | East Indian Ocean: Global / Oceans | East Indian Ocean</skos:scopeNote>
   </skos:Concept>
   <skos:Concept rdf:about="urn:aodn.org.au:geographicextents:concept:4">
      <skos:prefLabel xml:lang="en">Global / Oceans | Indian Ocean</skos:prefLabel>
      <skos:inScheme rdf:resource="urn:aodn.org.au:geographicextents:conceptscheme:1.0"/>
      <gml:BoundedBy>
         <gml:Envelope gml:srsName="http://www.opengis.net/gml/srs/epsg.xml#epsg:4326">
            <gml:lowerCorner>20 -70</gml:lowerCorner>
            <gml:upperCorner>127 28</gml:upperCorner>
         </gml:Envelope>
      </gml:BoundedBy>
      <skos:broader rdf:resource="urn:aodn.org.au:geographicextents:concept:10008"/>
      <skos:definition xml:lang="en">Global / Oceans | Indian Ocean</skos:definition>
      <skos:scopeNote xml:lang="en">Global / Oceans | Indian Ocean: Global / Oceans | Indian Ocean</skos:scopeNote>
   </skos:Concept>
   <skos:Concept rdf:about="urn:aodn.org.au:geographicextents:concept:5">
      <skos:prefLabel xml:lang="en">Global / Oceans | Pacific Ocean</skos:prefLabel>
      <skos:inScheme rdf:resource="urn:aodn.org.au:geographicextents:conceptscheme:1.0"/>
      <gml:BoundedBy>
         <gml:Envelope gml:srsName="http://www.opengis.net/gml/srs/epsg.xml#epsg:4326">
            <gml:lowerCorner>120 -70</gml:lowerCorner>
            <gml:upperCorner>-70 90</gml:upperCorner>
         </gml:Envelope>
      </gml:BoundedBy>
      <skos:broader rdf:resource="urn:aodn.org.au:geographicextents:concept:10008"/>
      <skos:definition xml:lang="en">Global / Oceans | Pacific Ocean</skos:definition>
      <skos:scopeNote xml:lang="en">Global / Oceans | Pacific Ocean: Global / Oceans | Pacific Ocean</skos:scopeNote>
   </skos:Concept>
   <skos:Concept rdf:about="urn:aodn.org.au:geographicextents:concept:6">
      <skos:prefLabel xml:lang="en">Global / Oceans | Southern Ocean</skos:prefLabel>
      <skos:inScheme rdf:resource="urn:aodn.org.au:geographicextents:conceptscheme:1.0"/>
      <gml:BoundedBy>
         <gml:Envelope gml:srsName="http://www.opengis.net/gml/srs/epsg.xml#epsg:4326">
            <gml:lowerCorner>-180 -85</gml:lowerCorner>
            <gml:upperCorner>180 -33</gml:upperCorner>
         </gml:Envelope>
      </gml:BoundedBy>
      <skos:broader rdf:resource="urn:aodn.org.au:geographicextents:concept:10008"/>
      <skos:definition xml:lang="en">Global / Oceans | Southern Ocean</skos:definition>
      <skos:scopeNote xml:lang="en">Global / Oceans | Southern Ocean: Global / Oceans | Southern Ocean</skos:scopeNote>
   </skos:Concept>
   <skos:Concept rdf:about="urn:aodn.org.au:geographicextents:concept:142">
      <skos:prefLabel xml:lang="en">Global / Oceans | Southern Ocean/ Australia extension</skos:prefLabel>
      <skos:inScheme rdf:resource="urn:aodn.org.au:geographicextents:conceptscheme:1.0"/>
      <gml:BoundedBy>
         <gml:Envelope gml:srsName="http://www.opengis.net/gml/srs/epsg.xml#epsg:4326">
            <gml:lowerCorner>71 -85</gml:lowerCorner>
            <gml:upperCorner>155 -33</gml:upperCorner>
         </gml:Envelope>
      </gml:BoundedBy>
      <skos:broader rdf:resource="urn:aodn.org.au:geographicextents:concept:10008"/>
      <skos:definition xml:lang="en">Global / Oceans | Southern Ocean/ Australia extension</skos:definition>
      <skos:scopeNote xml:lang="en">Global / Oceans | Southern Ocean/ Australia extension: Global / Oceans | Southern Ocean/ Australia extension</skos:scopeNote>
   </skos:Concept>
   <skos:Concept rdf:about="urn:aodn.org.au:geographicextents:concept:1025">
      <skos:prefLabel xml:lang="en">Global / Oceans | South West Pacific Ocean</skos:prefLabel>
      <skos:inScheme rdf:resource="urn:aodn.org.au:geographicextents:conceptscheme:1.0"/>
      <gml:BoundedBy>
         <gml:Envelope gml:srsName="http://www.opengis.net/gml/srs/epsg.xml#epsg:4326">
            <gml:lowerCorner>130 -84</gml:lowerCorner>
            <gml:upperCorner>180 0</gml:upperCorner>
         </gml:Envelope>
      </gml:BoundedBy>
      <skos:broader rdf:resource="urn:aodn.org.au:geographicextents:concept:10008"/>
      <skos:definition xml:lang="en">Global / Oceans | South West Pacific Ocean</skos:definition>
      <skos:scopeNote xml:lang="en">Global / Oceans | South West Pacific Ocean: Global / Oceans | South West Pacific Ocean</skos:scopeNote>
   </skos:Concept>
   <skos:Concept rdf:about="urn:aodn.org.au:geographicextents:concept:1021">
      <skos:prefLabel xml:lang="en">Global / Oceans | West Equatorial Pacific Ocean</skos:prefLabel>
      <skos:inScheme rdf:resource="urn:aodn.org.au:geographicextents:conceptscheme:1.0"/>
      <gml:BoundedBy>
         <gml:Envelope gml:srsName="http://www.opengis.net/gml/srs/epsg.xml#epsg:4326">
            <gml:lowerCorner>129 -5</gml:lowerCorner>
            <gml:upperCorner>180 5</gml:upperCorner>
         </gml:Envelope>
      </gml:BoundedBy>
      <skos:broader rdf:resource="urn:aodn.org.au:geographicextents:concept:10008"/>
      <skos:definition xml:lang="en">Global / Oceans | West Equatorial Pacific Ocean</skos:definition>
      <skos:scopeNote xml:lang="en">Global / Oceans | West Equatorial Pacific Ocean: Global / Oceans | West Equatorial Pacific Ocean</skos:scopeNote>
   </skos:Concept>
   <skos:Concept rdf:about="urn:aodn.org.au:geographicextents:concept:1">
      <skos:prefLabel xml:lang="en">Global / Oceans | World</skos:prefLabel>
      <skos:inScheme rdf:resource="urn:aodn.org.au:geographicextents:conceptscheme:1.0"/>
      <gml:BoundedBy>
         <gml:Envelope gml:srsName="http://www.opengis.net/gml/srs/epsg.xml#epsg:4326">
            <gml:lowerCorner>-180 -90</gml:lowerCorner>
            <gml:upperCorner>180 90</gml:upperCorner>
         </gml:Envelope>
      </gml:BoundedBy>
      <skos:broader rdf:resource="urn:aodn.org.au:geographicextents:concept:10008"/>
      <skos:definition xml:lang="en">Global / Oceans | World</skos:definition>
      <skos:scopeNote xml:lang="en">Global / Oceans | World: Global / Oceans | World</skos:scopeNote>
   </skos:Concept>
   <skos:Concept rdf:about="urn:aodn.org.au:geographicextents:concept:2">
      <skos:prefLabel xml:lang="en">Global / Oceans | World Ocean</skos:prefLabel>
      <skos:inScheme rdf:resource="urn:aodn.org.au:geographicextents:conceptscheme:1.0"/>
      <gml:BoundedBy>
         <gml:Envelope gml:srsName="http://www.opengis.net/gml/srs/epsg.xml#epsg:4326">
            <gml:lowerCorner>-180 -90</gml:lowerCorner>
            <gml:upperCorner>180 90</gml:upperCorner>
         </gml:Envelope>
      </gml:BoundedBy>
      <skos:broader rdf:resource="urn:aodn.org.au:geographicextents:concept:10008"/>
      <skos:definition xml:lang="en">Global / Oceans | World Ocean</skos:definition>
      <skos:scopeNote xml:lang="en">Global / Oceans | World Ocean: Global / Oceans | World Ocean</skos:scopeNote>
   </skos:Concept>
   <skos:Concept rdf:about="urn:aodn.org.au:geographicextents:concept:1033">
      <skos:prefLabel xml:lang="en">Marine Features (Australia) | Abrolhos Islands, WA</skos:prefLabel>
      <skos:inScheme rdf:resource="urn:aodn.org.au:geographicextents:conceptscheme:1.0"/>
      <gml:BoundedBy>
         <gml:Envelope gml:srsName="http://www.opengis.net/gml/srs/epsg.xml#epsg:4326">
            <gml:lowerCorner>113.55 -29.01</gml:lowerCorner>
            <gml:upperCorner>114.05 -28.25</gml:upperCorner>
         </gml:Envelope>
      </gml:BoundedBy>
      <skos:broader rdf:resource="urn:aodn.org.au:geographicextents:concept:10004"/>
      <skos:definition xml:lang="en">Marine Features (Australia) | Abrolhos Islands, WA</skos:definition>
      <skos:scopeNote xml:lang="en">Marine Features (Australia) | Abrolhos Islands, WA: Marine Features (Australia) | Abrolhos Islands, WA</skos:scopeNote>
   </skos:Concept>
   <skos:Concept rdf:about="urn:aodn.org.au:geographicextents:concept:1034">
      <skos:prefLabel xml:lang="en">Marine Features (Australia) | Admiralty Gulf, WA</skos:prefLabel>
      <skos:inScheme rdf:resource="urn:aodn.org.au:geographicextents:conceptscheme:1.0"/>
      <gml:BoundedBy>
         <gml:Envelope gml:srsName="http://www.opengis.net/gml/srs/epsg.xml#epsg:4326">
            <gml:lowerCorner>125.6 -14.7</gml:lowerCorner>
            <gml:upperCorner>126.15 -14</gml:upperCorner>
         </gml:Envelope>
      </gml:BoundedBy>
      <skos:broader rdf:resource="urn:aodn.org.au:geographicextents:concept:10004"/>
      <skos:definition xml:lang="en">Marine Features (Australia) | Admiralty Gulf, WA</skos:definition>
      <skos:scopeNote xml:lang="en">Marine Features (Australia) | Admiralty Gulf, WA: Marine Features (Australia) | Admiralty Gulf, WA</skos:scopeNote>
   </skos:Concept>
   <skos:Concept rdf:about="urn:aodn.org.au:geographicextents:concept:64">
      <skos:prefLabel xml:lang="en">Marine Features (Australia) | Albatross Bay, QLD</skos:prefLabel>
      <skos:inScheme rdf:resource="urn:aodn.org.au:geographicextents:conceptscheme:1.0"/>
      <gml:BoundedBy>
         <gml:Envelope gml:srsName="http://www.opengis.net/gml/srs/epsg.xml#epsg:4326">
            <gml:lowerCorner>141.5 -13</gml:lowerCorner>
            <gml:upperCorner>142 -12.5</gml:upperCorner>
         </gml:Envelope>
      </gml:BoundedBy>
      <skos:broader rdf:resource="urn:aodn.org.au:geographicextents:concept:10004"/>
      <skos:definition xml:lang="en">Marine Features (Australia) | Albatross Bay, QLD</skos:definition>
      <skos:scopeNote xml:lang="en">Marine Features (Australia) | Albatross Bay, QLD: Marine Features (Australia) | Albatross Bay, QLD</skos:scopeNote>
   </skos:Concept>
   <skos:Concept rdf:about="urn:aodn.org.au:geographicextents:concept:1035">
      <skos:prefLabel xml:lang="en">Marine Features (Australia) | Ashmore Reef, WA</skos:prefLabel>
      <skos:inScheme rdf:resource="urn:aodn.org.au:geographicextents:conceptscheme:1.0"/>
      <gml:BoundedBy>
         <gml:Envelope gml:srsName="http://www.opengis.net/gml/srs/epsg.xml#epsg:4326">
            <gml:lowerCorner>122.8 -12.61</gml:lowerCorner>
            <gml:upperCorner>123.71 -12.08</gml:upperCorner>
         </gml:Envelope>
      </gml:BoundedBy>
      <skos:broader rdf:resource="urn:aodn.org.au:geographicextents:concept:10004"/>
      <skos:definition xml:lang="en">Marine Features (Australia) | Ashmore Reef, WA</skos:definition>
      <skos:scopeNote xml:lang="en">Marine Features (Australia) | Ashmore Reef, WA: Marine Features (Australia) | Ashmore Reef, WA</skos:scopeNote>
   </skos:Concept>
   <skos:Concept rdf:about="urn:aodn.org.au:geographicextents:concept:1001">
      <skos:prefLabel xml:lang="en">Marine Features (Australia) | Australian EEZ</skos:prefLabel>
      <skos:inScheme rdf:resource="urn:aodn.org.au:geographicextents:conceptscheme:1.0"/>
      <gml:BoundedBy>
         <gml:Envelope gml:srsName="http://www.opengis.net/gml/srs/epsg.xml#epsg:4326">
            <gml:lowerCorner>65 -60</gml:lowerCorner>
            <gml:upperCorner>175 -8.5</gml:upperCorner>
         </gml:Envelope>
      </gml:BoundedBy>
      <skos:broader rdf:resource="urn:aodn.org.au:geographicextents:concept:10004"/>
      <skos:definition xml:lang="en">Marine Features (Australia) | Australian EEZ</skos:definition>
      <skos:scopeNote xml:lang="en">Marine Features (Australia) | Australian EEZ: Marine Features (Australia) | Australian EEZ</skos:scopeNote>
   </skos:Concept>
   <skos:Concept rdf:about="urn:aodn.org.au:geographicextents:concept:65">
      <skos:prefLabel xml:lang="en">Marine Features (Australia) | Australian North West Shelf, WA</skos:prefLabel>
      <skos:inScheme rdf:resource="urn:aodn.org.au:geographicextents:conceptscheme:1.0"/>
      <gml:BoundedBy>
         <gml:Envelope gml:srsName="http://www.opengis.net/gml/srs/epsg.xml#epsg:4326">
            <gml:lowerCorner>114 -24</gml:lowerCorner>
            <gml:upperCorner>122 -17</gml:upperCorner>
         </gml:Envelope>
      </gml:BoundedBy>
      <skos:broader rdf:resource="urn:aodn.org.au:geographicextents:concept:10004"/>
      <skos:definition xml:lang="en">Marine Features (Australia) | Australian North West Shelf, WA</skos:definition>
      <skos:scopeNote xml:lang="en">Marine Features (Australia) | Australian North West Shelf, WA: Marine Features (Australia) | Australian North West Shelf, WA</skos:scopeNote>
   </skos:Concept>
   <skos:Concept rdf:about="urn:aodn.org.au:geographicextents:concept:1036">
      <skos:prefLabel xml:lang="en">Marine Features (Australia) | Barker Inlet-Port River estuary, SA</skos:prefLabel>
      <skos:inScheme rdf:resource="urn:aodn.org.au:geographicextents:conceptscheme:1.0"/>
      <gml:BoundedBy>
         <gml:Envelope gml:srsName="http://www.opengis.net/gml/srs/epsg.xml#epsg:4326">
            <gml:lowerCorner>138.52 -34.81</gml:lowerCorner>
            <gml:upperCorner>138.55 -34.74</gml:upperCorner>
         </gml:Envelope>
      </gml:BoundedBy>
      <skos:broader rdf:resource="urn:aodn.org.au:geographicextents:concept:10004"/>
      <skos:definition xml:lang="en">Marine Features (Australia) | Barker Inlet-Port River estuary, SA</skos:definition>
      <skos:scopeNote xml:lang="en">Marine Features (Australia) | Barker Inlet-Port River estuary, SA: Marine Features (Australia) | Barker Inlet-Port River estuary, SA</skos:scopeNote>
   </skos:Concept>
   <skos:Concept rdf:about="urn:aodn.org.au:geographicextents:concept:1037">
      <skos:prefLabel xml:lang="en">Marine Features (Australia) | Barrow Island, WA</skos:prefLabel>
      <skos:inScheme rdf:resource="urn:aodn.org.au:geographicextents:conceptscheme:1.0"/>
      <gml:BoundedBy>
         <gml:Envelope gml:srsName="http://www.opengis.net/gml/srs/epsg.xml#epsg:4326">
            <gml:lowerCorner>115.23 -21</gml:lowerCorner>
            <gml:upperCorner>115.53 -20.63</gml:upperCorner>
         </gml:Envelope>
      </gml:BoundedBy>
      <skos:broader rdf:resource="urn:aodn.org.au:geographicextents:concept:10004"/>
      <skos:definition xml:lang="en">Marine Features (Australia) | Barrow Island, WA</skos:definition>
      <skos:scopeNote xml:lang="en">Marine Features (Australia) | Barrow Island, WA: Marine Features (Australia) | Barrow Island, WA</skos:scopeNote>
   </skos:Concept>
   <skos:Concept rdf:about="urn:aodn.org.au:geographicextents:concept:66">
      <skos:prefLabel xml:lang="en">Marine Features (Australia) | Bass Strait, TAS/VIC</skos:prefLabel>
      <skos:inScheme rdf:resource="urn:aodn.org.au:geographicextents:conceptscheme:1.0"/>
      <gml:BoundedBy>
         <gml:Envelope gml:srsName="http://www.opengis.net/gml/srs/epsg.xml#epsg:4326">
            <gml:lowerCorner>144 -41</gml:lowerCorner>
            <gml:upperCorner>150 -37</gml:upperCorner>
         </gml:Envelope>
      </gml:BoundedBy>
      <skos:broader rdf:resource="urn:aodn.org.au:geographicextents:concept:10004"/>
      <skos:definition xml:lang="en">Marine Features (Australia) | Bass Strait, TAS/VIC</skos:definition>
      <skos:scopeNote xml:lang="en">Marine Features (Australia) | Bass Strait, TAS/VIC: Marine Features (Australia) | Bass Strait, TAS/VIC</skos:scopeNote>
   </skos:Concept>
   <skos:Concept rdf:about="urn:aodn.org.au:geographicextents:concept:1038">
      <skos:prefLabel xml:lang="en">Marine Features (Australia) | Batemans Bay, NSW</skos:prefLabel>
      <skos:inScheme rdf:resource="urn:aodn.org.au:geographicextents:conceptscheme:1.0"/>
      <gml:BoundedBy>
         <gml:Envelope gml:srsName="http://www.opengis.net/gml/srs/epsg.xml#epsg:4326">
            <gml:lowerCorner>150.16 -35.78</gml:lowerCorner>
            <gml:upperCorner>150.28 -35.7</gml:upperCorner>
         </gml:Envelope>
      </gml:BoundedBy>
      <skos:broader rdf:resource="urn:aodn.org.au:geographicextents:concept:10004"/>
      <skos:definition xml:lang="en">Marine Features (Australia) | Batemans Bay, NSW</skos:definition>
      <skos:scopeNote xml:lang="en">Marine Features (Australia) | Batemans Bay, NSW: Marine Features (Australia) | Batemans Bay, NSW</skos:scopeNote>
   </skos:Concept>
   <skos:Concept rdf:about="urn:aodn.org.au:geographicextents:concept:1039">
      <skos:prefLabel xml:lang="en">Marine Features (Australia) | Bay of Rest, WA</skos:prefLabel>
      <skos:inScheme rdf:resource="urn:aodn.org.au:geographicextents:conceptscheme:1.0"/>
      <gml:BoundedBy>
         <gml:Envelope gml:srsName="http://www.opengis.net/gml/srs/epsg.xml#epsg:4326">
            <gml:lowerCorner>114.11 -22.34</gml:lowerCorner>
            <gml:upperCorner>114.15 -22.3</gml:upperCorner>
         </gml:Envelope>
      </gml:BoundedBy>
      <skos:broader rdf:resource="urn:aodn.org.au:geographicextents:concept:10004"/>
      <skos:definition xml:lang="en">Marine Features (Australia) | Bay of Rest, WA</skos:definition>
      <skos:scopeNote xml:lang="en">Marine Features (Australia) | Bay of Rest, WA: Marine Features (Australia) | Bay of Rest, WA</skos:scopeNote>
   </skos:Concept>
   <skos:Concept rdf:about="urn:aodn.org.au:geographicextents:concept:1040">
      <skos:prefLabel xml:lang="en">Marine Features (Australia) | Beagle Bay, WA</skos:prefLabel>
      <skos:inScheme rdf:resource="urn:aodn.org.au:geographicextents:conceptscheme:1.0"/>
      <gml:BoundedBy>
         <gml:Envelope gml:srsName="http://www.opengis.net/gml/srs/epsg.xml#epsg:4326">
            <gml:lowerCorner>122.48 -16.97</gml:lowerCorner>
            <gml:upperCorner>122.59 -16.85</gml:upperCorner>
         </gml:Envelope>
      </gml:BoundedBy>
      <skos:broader rdf:resource="urn:aodn.org.au:geographicextents:concept:10004"/>
      <skos:definition xml:lang="en">Marine Features (Australia) | Beagle Bay, WA</skos:definition>
      <skos:scopeNote xml:lang="en">Marine Features (Australia) | Beagle Bay, WA: Marine Features (Australia) | Beagle Bay, WA</skos:scopeNote>
   </skos:Concept>
   <skos:Concept rdf:about="urn:aodn.org.au:geographicextents:concept:1041">
      <skos:prefLabel xml:lang="en">Marine Features (Australia) | Bonney Coast, SA</skos:prefLabel>
      <skos:inScheme rdf:resource="urn:aodn.org.au:geographicextents:conceptscheme:1.0"/>
      <gml:BoundedBy>
         <gml:Envelope gml:srsName="http://www.opengis.net/gml/srs/epsg.xml#epsg:4326">
            <gml:lowerCorner>139.41 -38.42</gml:lowerCorner>
            <gml:upperCorner>141.6 -36.93</gml:upperCorner>
         </gml:Envelope>
      </gml:BoundedBy>
      <skos:broader rdf:resource="urn:aodn.org.au:geographicextents:concept:10004"/>
      <skos:definition xml:lang="en">Marine Features (Australia) | Bonney Coast, SA</skos:definition>
      <skos:scopeNote xml:lang="en">Marine Features (Australia) | Bonney Coast, SA: Marine Features (Australia) | Bonney Coast, SA</skos:scopeNote>
   </skos:Concept>
   <skos:Concept rdf:about="urn:aodn.org.au:geographicextents:concept:67">
      <skos:prefLabel xml:lang="en">Marine Features (Australia) | Botany Bay, NSW</skos:prefLabel>
      <skos:inScheme rdf:resource="urn:aodn.org.au:geographicextents:conceptscheme:1.0"/>
      <gml:BoundedBy>
         <gml:Envelope gml:srsName="http://www.opengis.net/gml/srs/epsg.xml#epsg:4326">
            <gml:lowerCorner>151.14 -34</gml:lowerCorner>
            <gml:upperCorner>151.24 -33.95</gml:upperCorner>
         </gml:Envelope>
      </gml:BoundedBy>
      <skos:broader rdf:resource="urn:aodn.org.au:geographicextents:concept:10004"/>
      <skos:definition xml:lang="en">Marine Features (Australia) | Botany Bay, NSW</skos:definition>
      <skos:scopeNote xml:lang="en">Marine Features (Australia) | Botany Bay, NSW: Marine Features (Australia) | Botany Bay, NSW</skos:scopeNote>
   </skos:Concept>
   <skos:Concept rdf:about="urn:aodn.org.au:geographicextents:concept:68">
      <skos:prefLabel xml:lang="en">Marine Features (Australia) | Broken Bay, NSW</skos:prefLabel>
      <skos:inScheme rdf:resource="urn:aodn.org.au:geographicextents:conceptscheme:1.0"/>
      <gml:BoundedBy>
         <gml:Envelope gml:srsName="http://www.opengis.net/gml/srs/epsg.xml#epsg:4326">
            <gml:lowerCorner>151.2 -33.7</gml:lowerCorner>
            <gml:upperCorner>151.4 -33.5</gml:upperCorner>
         </gml:Envelope>
      </gml:BoundedBy>
      <skos:broader rdf:resource="urn:aodn.org.au:geographicextents:concept:10004"/>
      <skos:definition xml:lang="en">Marine Features (Australia) | Broken Bay, NSW</skos:definition>
      <skos:scopeNote xml:lang="en">Marine Features (Australia) | Broken Bay, NSW: Marine Features (Australia) | Broken Bay, NSW</skos:scopeNote>
   </skos:Concept>
   <skos:Concept rdf:about="urn:aodn.org.au:geographicextents:concept:1042">
      <skos:prefLabel xml:lang="en">Marine Features (Australia) | Burrup Peninsula, WA</skos:prefLabel>
      <skos:inScheme rdf:resource="urn:aodn.org.au:geographicextents:conceptscheme:1.0"/>
      <gml:BoundedBy>
         <gml:Envelope gml:srsName="http://www.opengis.net/gml/srs/epsg.xml#epsg:4326">
            <gml:lowerCorner>116.64 -20.72</gml:lowerCorner>
            <gml:upperCorner>116.88 -20.51</gml:upperCorner>
         </gml:Envelope>
      </gml:BoundedBy>
      <skos:broader rdf:resource="urn:aodn.org.au:geographicextents:concept:10004"/>
      <skos:definition xml:lang="en">Marine Features (Australia) | Burrup Peninsula, WA</skos:definition>
      <skos:scopeNote xml:lang="en">Marine Features (Australia) | Burrup Peninsula, WA: Marine Features (Australia) | Burrup Peninsula, WA</skos:scopeNote>
   </skos:Concept>
   <skos:Concept rdf:about="urn:aodn.org.au:geographicextents:concept:1043">
      <skos:prefLabel xml:lang="en">Marine Features (Australia) | Cape Naturaliste, WA</skos:prefLabel>
      <skos:inScheme rdf:resource="urn:aodn.org.au:geographicextents:conceptscheme:1.0"/>
      <gml:BoundedBy>
         <gml:Envelope gml:srsName="http://www.opengis.net/gml/srs/epsg.xml#epsg:4326">
            <gml:lowerCorner>115.02 -33.63</gml:lowerCorner>
            <gml:upperCorner>115.12 -33.52</gml:upperCorner>
         </gml:Envelope>
      </gml:BoundedBy>
      <skos:broader rdf:resource="urn:aodn.org.au:geographicextents:concept:10004"/>
      <skos:definition xml:lang="en">Marine Features (Australia) | Cape Naturaliste, WA</skos:definition>
      <skos:scopeNote xml:lang="en">Marine Features (Australia) | Cape Naturaliste, WA: Marine Features (Australia) | Cape Naturaliste, WA</skos:scopeNote>
   </skos:Concept>
   <skos:Concept rdf:about="urn:aodn.org.au:geographicextents:concept:1044">
      <skos:prefLabel xml:lang="en">Marine Features (Australia) | Cockatoo Island, WA</skos:prefLabel>
      <skos:inScheme rdf:resource="urn:aodn.org.au:geographicextents:conceptscheme:1.0"/>
      <gml:BoundedBy>
         <gml:Envelope gml:srsName="http://www.opengis.net/gml/srs/epsg.xml#epsg:4326">
            <gml:lowerCorner>123.57 -16.12</gml:lowerCorner>
            <gml:upperCorner>123.66 -16.07</gml:upperCorner>
         </gml:Envelope>
      </gml:BoundedBy>
      <skos:broader rdf:resource="urn:aodn.org.au:geographicextents:concept:10004"/>
      <skos:definition xml:lang="en">Marine Features (Australia) | Cockatoo Island, WA</skos:definition>
      <skos:scopeNote xml:lang="en">Marine Features (Australia) | Cockatoo Island, WA: Marine Features (Australia) | Cockatoo Island, WA</skos:scopeNote>
   </skos:Concept>
   <skos:Concept rdf:about="urn:aodn.org.au:geographicextents:concept:1045">
      <skos:prefLabel xml:lang="en">Marine Features (Australia) | Cockburn Sound, WA</skos:prefLabel>
      <skos:inScheme rdf:resource="urn:aodn.org.au:geographicextents:conceptscheme:1.0"/>
      <gml:BoundedBy>
         <gml:Envelope gml:srsName="http://www.opengis.net/gml/srs/epsg.xml#epsg:4326">
            <gml:lowerCorner>115.66 -32.28</gml:lowerCorner>
            <gml:upperCorner>115.79 -32.11</gml:upperCorner>
         </gml:Envelope>
      </gml:BoundedBy>
      <skos:broader rdf:resource="urn:aodn.org.au:geographicextents:concept:10004"/>
      <skos:definition xml:lang="en">Marine Features (Australia) | Cockburn Sound, WA</skos:definition>
      <skos:scopeNote xml:lang="en">Marine Features (Australia) | Cockburn Sound, WA: Marine Features (Australia) | Cockburn Sound, WA</skos:scopeNote>
   </skos:Concept>
   <skos:Concept rdf:about="urn:aodn.org.au:geographicextents:concept:1046">
      <skos:prefLabel xml:lang="en">Marine Features (Australia) | Coral Bay, WA</skos:prefLabel>
      <skos:inScheme rdf:resource="urn:aodn.org.au:geographicextents:conceptscheme:1.0"/>
      <gml:BoundedBy>
         <gml:Envelope gml:srsName="http://www.opengis.net/gml/srs/epsg.xml#epsg:4326">
            <gml:lowerCorner>113.76 -23.15</gml:lowerCorner>
            <gml:upperCorner>113.78 -23.13</gml:upperCorner>
         </gml:Envelope>
      </gml:BoundedBy>
      <skos:broader rdf:resource="urn:aodn.org.au:geographicextents:concept:10004"/>
      <skos:definition xml:lang="en">Marine Features (Australia) | Coral Bay, WA</skos:definition>
      <skos:scopeNote xml:lang="en">Marine Features (Australia) | Coral Bay, WA: Marine Features (Australia) | Coral Bay, WA</skos:scopeNote>
   </skos:Concept>
   <skos:Concept rdf:about="urn:aodn.org.au:geographicextents:concept:1047">
      <skos:prefLabel xml:lang="en">Marine Features (Australia) | Dampier Archipelago, WA</skos:prefLabel>
      <skos:inScheme rdf:resource="urn:aodn.org.au:geographicextents:conceptscheme:1.0"/>
      <gml:BoundedBy>
         <gml:Envelope gml:srsName="http://www.opengis.net/gml/srs/epsg.xml#epsg:4326">
            <gml:lowerCorner>116.33 -20.85</gml:lowerCorner>
            <gml:upperCorner>117.22 -20.3</gml:upperCorner>
         </gml:Envelope>
      </gml:BoundedBy>
      <skos:broader rdf:resource="urn:aodn.org.au:geographicextents:concept:10004"/>
      <skos:definition xml:lang="en">Marine Features (Australia) | Dampier Archipelago, WA</skos:definition>
      <skos:scopeNote xml:lang="en">Marine Features (Australia) | Dampier Archipelago, WA: Marine Features (Australia) | Dampier Archipelago, WA</skos:scopeNote>
   </skos:Concept>
   <skos:Concept rdf:about="urn:aodn.org.au:geographicextents:concept:69">
      <skos:prefLabel xml:lang="en">Marine Features (Australia) | Derwent Estuary, TAS</skos:prefLabel>
      <skos:inScheme rdf:resource="urn:aodn.org.au:geographicextents:conceptscheme:1.0"/>
      <gml:BoundedBy>
         <gml:Envelope gml:srsName="http://www.opengis.net/gml/srs/epsg.xml#epsg:4326">
            <gml:lowerCorner>147.2 -43.1</gml:lowerCorner>
            <gml:upperCorner>147.5 -42.7</gml:upperCorner>
         </gml:Envelope>
      </gml:BoundedBy>
      <skos:broader rdf:resource="urn:aodn.org.au:geographicextents:concept:10004"/>
      <skos:definition xml:lang="en">Marine Features (Australia) | Derwent Estuary, TAS</skos:definition>
      <skos:scopeNote xml:lang="en">Marine Features (Australia) | Derwent Estuary, TAS: Marine Features (Australia) | Derwent Estuary, TAS</skos:scopeNote>
   </skos:Concept>
   <skos:Concept rdf:about="urn:aodn.org.au:geographicextents:concept:1048">
      <skos:prefLabel xml:lang="en">Marine Features (Australia) | Dirk Hartog Island, WA</skos:prefLabel>
      <skos:inScheme rdf:resource="urn:aodn.org.au:geographicextents:conceptscheme:1.0"/>
      <gml:BoundedBy>
         <gml:Envelope gml:srsName="http://www.opengis.net/gml/srs/epsg.xml#epsg:4326">
            <gml:lowerCorner>112.92 -26.17</gml:lowerCorner>
            <gml:upperCorner>113.24 -25.48</gml:upperCorner>
         </gml:Envelope>
      </gml:BoundedBy>
      <skos:broader rdf:resource="urn:aodn.org.au:geographicextents:concept:10004"/>
      <skos:definition xml:lang="en">Marine Features (Australia) | Dirk Hartog Island, WA</skos:definition>
      <skos:scopeNote xml:lang="en">Marine Features (Australia) | Dirk Hartog Island, WA: Marine Features (Australia) | Dirk Hartog Island, WA</skos:scopeNote>
   </skos:Concept>
   <skos:Concept rdf:about="urn:aodn.org.au:geographicextents:concept:1049">
      <skos:prefLabel xml:lang="en">Marine Features (Australia) | East Australian Current</skos:prefLabel>
      <skos:inScheme rdf:resource="urn:aodn.org.au:geographicextents:conceptscheme:1.0"/>
      <gml:BoundedBy>
         <gml:Envelope gml:srsName="http://www.opengis.net/gml/srs/epsg.xml#epsg:4326">
            <gml:lowerCorner>148.5 -43.4</gml:lowerCorner>
            <gml:upperCorner>157.9 -19.8</gml:upperCorner>
         </gml:Envelope>
      </gml:BoundedBy>
      <skos:broader rdf:resource="urn:aodn.org.au:geographicextents:concept:10004"/>
      <skos:definition xml:lang="en">Marine Features (Australia) | East Australian Current</skos:definition>
      <skos:scopeNote xml:lang="en">Marine Features (Australia) | East Australian Current: Marine Features (Australia) | East Australian Current</skos:scopeNote>
   </skos:Concept>
   <skos:Concept rdf:about="urn:aodn.org.au:geographicextents:concept:1050">
      <skos:prefLabel xml:lang="en">Marine Features (Australia) | Eighty Mile Beach, WA</skos:prefLabel>
      <skos:inScheme rdf:resource="urn:aodn.org.au:geographicextents:conceptscheme:1.0"/>
      <gml:BoundedBy>
         <gml:Envelope gml:srsName="http://www.opengis.net/gml/srs/epsg.xml#epsg:4326">
            <gml:lowerCorner>120.05 -19.98</gml:lowerCorner>
            <gml:upperCorner>121.62 -18.92</gml:upperCorner>
         </gml:Envelope>
      </gml:BoundedBy>
      <skos:broader rdf:resource="urn:aodn.org.au:geographicextents:concept:10004"/>
      <skos:definition xml:lang="en">Marine Features (Australia) | Eighty Mile Beach, WA</skos:definition>
      <skos:scopeNote xml:lang="en">Marine Features (Australia) | Eighty Mile Beach, WA: Marine Features (Australia) | Eighty Mile Beach, WA</skos:scopeNote>
   </skos:Concept>
   <skos:Concept rdf:about="urn:aodn.org.au:geographicextents:concept:70">
      <skos:prefLabel xml:lang="en">Marine Features (Australia) | Exmouth Gulf, WA</skos:prefLabel>
      <skos:inScheme rdf:resource="urn:aodn.org.au:geographicextents:conceptscheme:1.0"/>
      <gml:BoundedBy>
         <gml:Envelope gml:srsName="http://www.opengis.net/gml/srs/epsg.xml#epsg:4326">
            <gml:lowerCorner>114 -23</gml:lowerCorner>
            <gml:upperCorner>115 -21</gml:upperCorner>
         </gml:Envelope>
      </gml:BoundedBy>
      <skos:broader rdf:resource="urn:aodn.org.au:geographicextents:concept:10004"/>
      <skos:definition xml:lang="en">Marine Features (Australia) | Exmouth Gulf, WA</skos:definition>
      <skos:scopeNote xml:lang="en">Marine Features (Australia) | Exmouth Gulf, WA: Marine Features (Australia) | Exmouth Gulf, WA</skos:scopeNote>
   </skos:Concept>
   <skos:Concept rdf:about="urn:aodn.org.au:geographicextents:concept:1004">
      <skos:prefLabel xml:lang="en">Marine Features (Australia) | Fitzroy River, QLD</skos:prefLabel>
      <skos:inScheme rdf:resource="urn:aodn.org.au:geographicextents:conceptscheme:1.0"/>
      <gml:BoundedBy>
         <gml:Envelope gml:srsName="http://www.opengis.net/gml/srs/epsg.xml#epsg:4326">
            <gml:lowerCorner>150.5 -24</gml:lowerCorner>
            <gml:upperCorner>151.8 -23</gml:upperCorner>
         </gml:Envelope>
      </gml:BoundedBy>
      <skos:broader rdf:resource="urn:aodn.org.au:geographicextents:concept:10004"/>
      <skos:definition xml:lang="en">Marine Features (Australia) | Fitzroy River, QLD</skos:definition>
      <skos:scopeNote xml:lang="en">Marine Features (Australia) | Fitzroy River, QLD: Marine Features (Australia) | Fitzroy River, QLD</skos:scopeNote>
   </skos:Concept>
   <skos:Concept rdf:about="urn:aodn.org.au:geographicextents:concept:71">
      <skos:prefLabel xml:lang="en">Marine Features (Australia) | Flinders Bay, WA</skos:prefLabel>
      <skos:inScheme rdf:resource="urn:aodn.org.au:geographicextents:conceptscheme:1.0"/>
      <gml:BoundedBy>
         <gml:Envelope gml:srsName="http://www.opengis.net/gml/srs/epsg.xml#epsg:4326">
            <gml:lowerCorner>115.1 -34.45</gml:lowerCorner>
            <gml:upperCorner>115.55 -34.3</gml:upperCorner>
         </gml:Envelope>
      </gml:BoundedBy>
      <skos:broader rdf:resource="urn:aodn.org.au:geographicextents:concept:10004"/>
      <skos:definition xml:lang="en">Marine Features (Australia) | Flinders Bay, WA</skos:definition>
      <skos:scopeNote xml:lang="en">Marine Features (Australia) | Flinders Bay, WA: Marine Features (Australia) | Flinders Bay, WA</skos:scopeNote>
   </skos:Concept>
   <skos:Concept rdf:about="urn:aodn.org.au:geographicextents:concept:72">
      <skos:prefLabel xml:lang="en">Marine Features (Australia) | Flinders Island, TAS</skos:prefLabel>
      <skos:inScheme rdf:resource="urn:aodn.org.au:geographicextents:conceptscheme:1.0"/>
      <gml:BoundedBy>
         <gml:Envelope gml:srsName="http://www.opengis.net/gml/srs/epsg.xml#epsg:4326">
            <gml:lowerCorner>147.74 -40.28</gml:lowerCorner>
            <gml:upperCorner>148.34 -39.71</gml:upperCorner>
         </gml:Envelope>
      </gml:BoundedBy>
      <skos:broader rdf:resource="urn:aodn.org.au:geographicextents:concept:10004"/>
      <skos:definition xml:lang="en">Marine Features (Australia) | Flinders Island, TAS</skos:definition>
      <skos:scopeNote xml:lang="en">Marine Features (Australia) | Flinders Island, TAS: Marine Features (Australia) | Flinders Island, TAS</skos:scopeNote>
   </skos:Concept>
   <skos:Concept rdf:about="urn:aodn.org.au:geographicextents:concept:73">
      <skos:prefLabel xml:lang="en">Marine Features (Australia) | Fraser Island, QLD</skos:prefLabel>
      <skos:inScheme rdf:resource="urn:aodn.org.au:geographicextents:conceptscheme:1.0"/>
      <gml:BoundedBy>
         <gml:Envelope gml:srsName="http://www.opengis.net/gml/srs/epsg.xml#epsg:4326">
            <gml:lowerCorner>152.94 -25.8</gml:lowerCorner>
            <gml:upperCorner>153.37 -24.69</gml:upperCorner>
         </gml:Envelope>
      </gml:BoundedBy>
      <skos:broader rdf:resource="urn:aodn.org.au:geographicextents:concept:10004"/>
      <skos:definition xml:lang="en">Marine Features (Australia) | Fraser Island, QLD</skos:definition>
      <skos:scopeNote xml:lang="en">Marine Features (Australia) | Fraser Island, QLD: Marine Features (Australia) | Fraser Island, QLD</skos:scopeNote>
   </skos:Concept>
   <skos:Concept rdf:about="urn:aodn.org.au:geographicextents:concept:74">
      <skos:prefLabel xml:lang="en">Marine Features (Australia) | Geographe Bay, WA</skos:prefLabel>
      <skos:inScheme rdf:resource="urn:aodn.org.au:geographicextents:conceptscheme:1.0"/>
      <gml:BoundedBy>
         <gml:Envelope gml:srsName="http://www.opengis.net/gml/srs/epsg.xml#epsg:4326">
            <gml:lowerCorner>115 -33.7</gml:lowerCorner>
            <gml:upperCorner>115.7 -32.7</gml:upperCorner>
         </gml:Envelope>
      </gml:BoundedBy>
      <skos:broader rdf:resource="urn:aodn.org.au:geographicextents:concept:10004"/>
      <skos:definition xml:lang="en">Marine Features (Australia) | Geographe Bay, WA</skos:definition>
      <skos:scopeNote xml:lang="en">Marine Features (Australia) | Geographe Bay, WA: Marine Features (Australia) | Geographe Bay, WA</skos:scopeNote>
   </skos:Concept>
   <skos:Concept rdf:about="urn:aodn.org.au:geographicextents:concept:1051">
      <skos:prefLabel xml:lang="en">Marine Features (Australia) | Gippsland Lakes, VIC</skos:prefLabel>
      <skos:inScheme rdf:resource="urn:aodn.org.au:geographicextents:conceptscheme:1.0"/>
      <gml:BoundedBy>
         <gml:Envelope gml:srsName="http://www.opengis.net/gml/srs/epsg.xml#epsg:4326">
            <gml:lowerCorner>147.2 -38.36</gml:lowerCorner>
            <gml:upperCorner>148.15 -37.77</gml:upperCorner>
         </gml:Envelope>
      </gml:BoundedBy>
      <skos:broader rdf:resource="urn:aodn.org.au:geographicextents:concept:10004"/>
      <skos:definition xml:lang="en">Marine Features (Australia) | Gippsland Lakes, VIC</skos:definition>
      <skos:scopeNote xml:lang="en">Marine Features (Australia) | Gippsland Lakes, VIC: Marine Features (Australia) | Gippsland Lakes, VIC</skos:scopeNote>
   </skos:Concept>
   <skos:Concept rdf:about="urn:aodn.org.au:geographicextents:concept:75">
      <skos:prefLabel xml:lang="en">Marine Features (Australia) | Great Australian Bight, SA/WA</skos:prefLabel>
      <skos:inScheme rdf:resource="urn:aodn.org.au:geographicextents:conceptscheme:1.0"/>
      <gml:BoundedBy>
         <gml:Envelope gml:srsName="http://www.opengis.net/gml/srs/epsg.xml#epsg:4326">
            <gml:lowerCorner>118 -35</gml:lowerCorner>
            <gml:upperCorner>136 -31</gml:upperCorner>
         </gml:Envelope>
      </gml:BoundedBy>
      <skos:broader rdf:resource="urn:aodn.org.au:geographicextents:concept:10004"/>
      <skos:definition xml:lang="en">Marine Features (Australia) | Great Australian Bight, SA/WA</skos:definition>
      <skos:scopeNote xml:lang="en">Marine Features (Australia) | Great Australian Bight, SA/WA: Marine Features (Australia) | Great Australian Bight, SA/WA</skos:scopeNote>
   </skos:Concept>
   <skos:Concept rdf:about="urn:aodn.org.au:geographicextents:concept:1006">
      <skos:prefLabel xml:lang="en">Marine Features (Australia) | Great Barrier Reef, QLD</skos:prefLabel>
      <skos:inScheme rdf:resource="urn:aodn.org.au:geographicextents:conceptscheme:1.0"/>
      <gml:BoundedBy>
         <gml:Envelope gml:srsName="http://www.opengis.net/gml/srs/epsg.xml#epsg:4326">
            <gml:lowerCorner>141 -24</gml:lowerCorner>
            <gml:upperCorner>153 -9</gml:upperCorner>
         </gml:Envelope>
      </gml:BoundedBy>
      <skos:broader rdf:resource="urn:aodn.org.au:geographicextents:concept:10004"/>
      <skos:definition xml:lang="en">Marine Features (Australia) | Great Barrier Reef, QLD</skos:definition>
      <skos:scopeNote xml:lang="en">Marine Features (Australia) | Great Barrier Reef, QLD: Marine Features (Australia) | Great Barrier Reef, QLD</skos:scopeNote>
   </skos:Concept>
   <skos:Concept rdf:about="urn:aodn.org.au:geographicextents:concept:77">
      <skos:prefLabel xml:lang="en">Marine Features (Australia) | Great Barrier Reef Cairns Section, QLD</skos:prefLabel>
      <skos:inScheme rdf:resource="urn:aodn.org.au:geographicextents:conceptscheme:1.0"/>
      <gml:BoundedBy>
         <gml:Envelope gml:srsName="http://www.opengis.net/gml/srs/epsg.xml#epsg:4326">
            <gml:lowerCorner>145 -18</gml:lowerCorner>
            <gml:upperCorner>147 -15</gml:upperCorner>
         </gml:Envelope>
      </gml:BoundedBy>
      <skos:broader rdf:resource="urn:aodn.org.au:geographicextents:concept:10004"/>
      <skos:definition xml:lang="en">Marine Features (Australia) | Great Barrier Reef Cairns Section, QLD</skos:definition>
      <skos:scopeNote xml:lang="en">Marine Features (Australia) | Great Barrier Reef Cairns Section, QLD: Marine Features (Australia) | Great Barrier Reef Cairns Section, QLD</skos:scopeNote>
   </skos:Concept>
   <skos:Concept rdf:about="urn:aodn.org.au:geographicextents:concept:78">
      <skos:prefLabel xml:lang="en">Marine Features (Australia) | Great Barrier Reef Capricorn/Bunker Section, QLD</skos:prefLabel>
      <skos:inScheme rdf:resource="urn:aodn.org.au:geographicextents:conceptscheme:1.0"/>
      <gml:BoundedBy>
         <gml:Envelope gml:srsName="http://www.opengis.net/gml/srs/epsg.xml#epsg:4326">
            <gml:lowerCorner>151.5 -24.5</gml:lowerCorner>
            <gml:upperCorner>153 -23</gml:upperCorner>
         </gml:Envelope>
      </gml:BoundedBy>
      <skos:broader rdf:resource="urn:aodn.org.au:geographicextents:concept:10004"/>
      <skos:definition xml:lang="en">Marine Features (Australia) | Great Barrier Reef Capricorn/Bunker Section, QLD</skos:definition>
      <skos:scopeNote xml:lang="en">Marine Features (Australia) | Great Barrier Reef Capricorn/Bunker Section, QLD: Marine Features (Australia) | Great Barrier Reef Capricorn/Bunker Section, QLD</skos:scopeNote>
   </skos:Concept>
   <skos:Concept rdf:about="urn:aodn.org.au:geographicextents:concept:79">
      <skos:prefLabel xml:lang="en">Marine Features (Australia) | Great Barrier Reef Central Section, QLD</skos:prefLabel>
      <skos:inScheme rdf:resource="urn:aodn.org.au:geographicextents:conceptscheme:1.0"/>
      <gml:BoundedBy>
         <gml:Envelope gml:srsName="http://www.opengis.net/gml/srs/epsg.xml#epsg:4326">
            <gml:lowerCorner>146 -21</gml:lowerCorner>
            <gml:upperCorner>150.5 -18</gml:upperCorner>
         </gml:Envelope>
      </gml:BoundedBy>
      <skos:broader rdf:resource="urn:aodn.org.au:geographicextents:concept:10004"/>
      <skos:definition xml:lang="en">Marine Features (Australia) | Great Barrier Reef Central Section, QLD</skos:definition>
      <skos:scopeNote xml:lang="en">Marine Features (Australia) | Great Barrier Reef Central Section, QLD: Marine Features (Australia) | Great Barrier Reef Central Section, QLD</skos:scopeNote>
   </skos:Concept>
   <skos:Concept rdf:about="urn:aodn.org.au:geographicextents:concept:80">
      <skos:prefLabel xml:lang="en">Marine Features (Australia) | Great Barrier Reef Far North Section, QLD</skos:prefLabel>
      <skos:inScheme rdf:resource="urn:aodn.org.au:geographicextents:conceptscheme:1.0"/>
      <gml:BoundedBy>
         <gml:Envelope gml:srsName="http://www.opengis.net/gml/srs/epsg.xml#epsg:4326">
            <gml:lowerCorner>143 -15</gml:lowerCorner>
            <gml:upperCorner>145.5 -11</gml:upperCorner>
         </gml:Envelope>
      </gml:BoundedBy>
      <skos:broader rdf:resource="urn:aodn.org.au:geographicextents:concept:10004"/>
      <skos:definition xml:lang="en">Marine Features (Australia) | Great Barrier Reef Far North Section, QLD</skos:definition>
      <skos:scopeNote xml:lang="en">Marine Features (Australia) | Great Barrier Reef Far North Section, QLD: Marine Features (Australia) | Great Barrier Reef Far North Section, QLD</skos:scopeNote>
   </skos:Concept>
   <skos:Concept rdf:about="urn:aodn.org.au:geographicextents:concept:81">
      <skos:prefLabel xml:lang="en">Marine Features (Australia) | Great Barrier Reef Mackay Section, QLD</skos:prefLabel>
      <skos:inScheme rdf:resource="urn:aodn.org.au:geographicextents:conceptscheme:1.0"/>
      <gml:BoundedBy>
         <gml:Envelope gml:srsName="http://www.opengis.net/gml/srs/epsg.xml#epsg:4326">
            <gml:lowerCorner>149 -23</gml:lowerCorner>
            <gml:upperCorner>153 -21</gml:upperCorner>
         </gml:Envelope>
      </gml:BoundedBy>
      <skos:broader rdf:resource="urn:aodn.org.au:geographicextents:concept:10004"/>
      <skos:definition xml:lang="en">Marine Features (Australia) | Great Barrier Reef Mackay Section, QLD</skos:definition>
      <skos:scopeNote xml:lang="en">Marine Features (Australia) | Great Barrier Reef Mackay Section, QLD: Marine Features (Australia) | Great Barrier Reef Mackay Section, QLD</skos:scopeNote>
   </skos:Concept>
   <skos:Concept rdf:about="urn:aodn.org.au:geographicextents:concept:82">
      <skos:prefLabel xml:lang="en">Marine Features (Australia) | Groote Eylandt, NT</skos:prefLabel>
      <skos:inScheme rdf:resource="urn:aodn.org.au:geographicextents:conceptscheme:1.0"/>
      <gml:BoundedBy>
         <gml:Envelope gml:srsName="http://www.opengis.net/gml/srs/epsg.xml#epsg:4326">
            <gml:lowerCorner>136 -14.5</gml:lowerCorner>
            <gml:upperCorner>137 -13.5</gml:upperCorner>
         </gml:Envelope>
      </gml:BoundedBy>
      <skos:broader rdf:resource="urn:aodn.org.au:geographicextents:concept:10004"/>
      <skos:definition xml:lang="en">Marine Features (Australia) | Groote Eylandt, NT</skos:definition>
      <skos:scopeNote xml:lang="en">Marine Features (Australia) | Groote Eylandt, NT: Marine Features (Australia) | Groote Eylandt, NT</skos:scopeNote>
   </skos:Concept>
   <skos:Concept rdf:about="urn:aodn.org.au:geographicextents:concept:83">
      <skos:prefLabel xml:lang="en">Marine Features (Australia) | Gulf of Carpentaria, NT/QLD</skos:prefLabel>
      <skos:inScheme rdf:resource="urn:aodn.org.au:geographicextents:conceptscheme:1.0"/>
      <gml:BoundedBy>
         <gml:Envelope gml:srsName="http://www.opengis.net/gml/srs/epsg.xml#epsg:4326">
            <gml:lowerCorner>136 -18</gml:lowerCorner>
            <gml:upperCorner>142 -11</gml:upperCorner>
         </gml:Envelope>
      </gml:BoundedBy>
      <skos:broader rdf:resource="urn:aodn.org.au:geographicextents:concept:10004"/>
      <skos:definition xml:lang="en">Marine Features (Australia) | Gulf of Carpentaria, NT/QLD</skos:definition>
      <skos:scopeNote xml:lang="en">Marine Features (Australia) | Gulf of Carpentaria, NT/QLD: Marine Features (Australia) | Gulf of Carpentaria, NT/QLD</skos:scopeNote>
   </skos:Concept>
   <skos:Concept rdf:about="urn:aodn.org.au:geographicextents:concept:84">
      <skos:prefLabel xml:lang="en">Marine Features (Australia) | Gulf St. Vincent, SA</skos:prefLabel>
      <skos:inScheme rdf:resource="urn:aodn.org.au:geographicextents:conceptscheme:1.0"/>
      <gml:BoundedBy>
         <gml:Envelope gml:srsName="http://www.opengis.net/gml/srs/epsg.xml#epsg:4326">
            <gml:lowerCorner>137.2 -35.75</gml:lowerCorner>
            <gml:upperCorner>138.6 -34</gml:upperCorner>
         </gml:Envelope>
      </gml:BoundedBy>
      <skos:broader rdf:resource="urn:aodn.org.au:geographicextents:concept:10004"/>
      <skos:definition xml:lang="en">Marine Features (Australia) | Gulf St. Vincent, SA</skos:definition>
      <skos:scopeNote xml:lang="en">Marine Features (Australia) | Gulf St. Vincent, SA: Marine Features (Australia) | Gulf St. Vincent, SA</skos:scopeNote>
   </skos:Concept>
   <skos:Concept rdf:about="urn:aodn.org.au:geographicextents:concept:1052">
      <skos:prefLabel xml:lang="en">Marine Features (Australia) | Hardwicke Bay, SA</skos:prefLabel>
      <skos:inScheme rdf:resource="urn:aodn.org.au:geographicextents:conceptscheme:1.0"/>
      <gml:BoundedBy>
         <gml:Envelope gml:srsName="http://www.opengis.net/gml/srs/epsg.xml#epsg:4326">
            <gml:lowerCorner>137.28 -34.96</gml:lowerCorner>
            <gml:upperCorner>137.47 -34.86</gml:upperCorner>
         </gml:Envelope>
      </gml:BoundedBy>
      <skos:broader rdf:resource="urn:aodn.org.au:geographicextents:concept:10004"/>
      <skos:definition xml:lang="en">Marine Features (Australia) | Hardwicke Bay, SA</skos:definition>
      <skos:scopeNote xml:lang="en">Marine Features (Australia) | Hardwicke Bay, SA: Marine Features (Australia) | Hardwicke Bay, SA</skos:scopeNote>
   </skos:Concept>
   <skos:Concept rdf:about="urn:aodn.org.au:geographicextents:concept:1053">
      <skos:prefLabel xml:lang="en">Marine Features (Australia) | Heron Island, QLD</skos:prefLabel>
      <skos:inScheme rdf:resource="urn:aodn.org.au:geographicextents:conceptscheme:1.0"/>
      <gml:BoundedBy>
         <gml:Envelope gml:srsName="http://www.opengis.net/gml/srs/epsg.xml#epsg:4326">
            <gml:lowerCorner>151.91 -23.45</gml:lowerCorner>
            <gml:upperCorner>151.92 -23.44</gml:upperCorner>
         </gml:Envelope>
      </gml:BoundedBy>
      <skos:broader rdf:resource="urn:aodn.org.au:geographicextents:concept:10004"/>
      <skos:definition xml:lang="en">Marine Features (Australia) | Heron Island, QLD</skos:definition>
      <skos:scopeNote xml:lang="en">Marine Features (Australia) | Heron Island, QLD: Marine Features (Australia) | Heron Island, QLD</skos:scopeNote>
   </skos:Concept>
   <skos:Concept rdf:about="urn:aodn.org.au:geographicextents:concept:85">
      <skos:prefLabel xml:lang="en">Marine Features (Australia) | Hervey Bay, QLD</skos:prefLabel>
      <skos:inScheme rdf:resource="urn:aodn.org.au:geographicextents:conceptscheme:1.0"/>
      <gml:BoundedBy>
         <gml:Envelope gml:srsName="http://www.opengis.net/gml/srs/epsg.xml#epsg:4326">
            <gml:lowerCorner>152.4 -25.45</gml:lowerCorner>
            <gml:upperCorner>153.25 -24.74</gml:upperCorner>
         </gml:Envelope>
      </gml:BoundedBy>
      <skos:broader rdf:resource="urn:aodn.org.au:geographicextents:concept:10004"/>
      <skos:definition xml:lang="en">Marine Features (Australia) | Hervey Bay, QLD</skos:definition>
      <skos:scopeNote xml:lang="en">Marine Features (Australia) | Hervey Bay, QLD: Marine Features (Australia) | Hervey Bay, QLD</skos:scopeNote>
   </skos:Concept>
   <skos:Concept rdf:about="urn:aodn.org.au:geographicextents:concept:1054">
      <skos:prefLabel xml:lang="en">Marine Features (Australia) | Indonesian Throughflow</skos:prefLabel>
      <skos:inScheme rdf:resource="urn:aodn.org.au:geographicextents:conceptscheme:1.0"/>
      <gml:BoundedBy>
         <gml:Envelope gml:srsName="http://www.opengis.net/gml/srs/epsg.xml#epsg:4326">
            <gml:lowerCorner>105 -15</gml:lowerCorner>
            <gml:upperCorner>130 5</gml:upperCorner>
         </gml:Envelope>
      </gml:BoundedBy>
      <skos:broader rdf:resource="urn:aodn.org.au:geographicextents:concept:10004"/>
      <skos:definition xml:lang="en">Marine Features (Australia) | Indonesian Throughflow</skos:definition>
      <skos:scopeNote xml:lang="en">Marine Features (Australia) | Indonesian Throughflow: Marine Features (Australia) | Indonesian Throughflow</skos:scopeNote>
   </skos:Concept>
   <skos:Concept rdf:about="urn:aodn.org.au:geographicextents:concept:86">
      <skos:prefLabel xml:lang="en">Marine Features (Australia) | Jervis Bay, ACT</skos:prefLabel>
      <skos:inScheme rdf:resource="urn:aodn.org.au:geographicextents:conceptscheme:1.0"/>
      <gml:BoundedBy>
         <gml:Envelope gml:srsName="http://www.opengis.net/gml/srs/epsg.xml#epsg:4326">
            <gml:lowerCorner>150.67 -35.14</gml:lowerCorner>
            <gml:upperCorner>150.78 -34.99</gml:upperCorner>
         </gml:Envelope>
      </gml:BoundedBy>
      <skos:broader rdf:resource="urn:aodn.org.au:geographicextents:concept:10004"/>
      <skos:definition xml:lang="en">Marine Features (Australia) | Jervis Bay, ACT</skos:definition>
      <skos:scopeNote xml:lang="en">Marine Features (Australia) | Jervis Bay, ACT: Marine Features (Australia) | Jervis Bay, ACT</skos:scopeNote>
   </skos:Concept>
   <skos:Concept rdf:about="urn:aodn.org.au:geographicextents:concept:87">
      <skos:prefLabel xml:lang="en">Marine Features (Australia) | Joseph Bonaparte Gulf, NT/WA</skos:prefLabel>
      <skos:inScheme rdf:resource="urn:aodn.org.au:geographicextents:conceptscheme:1.0"/>
      <gml:BoundedBy>
         <gml:Envelope gml:srsName="http://www.opengis.net/gml/srs/epsg.xml#epsg:4326">
            <gml:lowerCorner>127 -15</gml:lowerCorner>
            <gml:upperCorner>130 -13</gml:upperCorner>
         </gml:Envelope>
      </gml:BoundedBy>
      <skos:broader rdf:resource="urn:aodn.org.au:geographicextents:concept:10004"/>
      <skos:definition xml:lang="en">Marine Features (Australia) | Joseph Bonaparte Gulf, NT/WA</skos:definition>
      <skos:scopeNote xml:lang="en">Marine Features (Australia) | Joseph Bonaparte Gulf, NT/WA: Marine Features (Australia) | Joseph Bonaparte Gulf, NT/WA</skos:scopeNote>
   </skos:Concept>
   <skos:Concept rdf:about="urn:aodn.org.au:geographicextents:concept:1055">
      <skos:prefLabel xml:lang="en">Marine Features (Australia) | Jurabi Coast Nature Reserve, WA</skos:prefLabel>
      <skos:inScheme rdf:resource="urn:aodn.org.au:geographicextents:conceptscheme:1.0"/>
      <gml:BoundedBy>
         <gml:Envelope gml:srsName="http://www.opengis.net/gml/srs/epsg.xml#epsg:4326">
            <gml:lowerCorner>113.7 -22.4</gml:lowerCorner>
            <gml:upperCorner>114.1 -21.8</gml:upperCorner>
         </gml:Envelope>
      </gml:BoundedBy>
      <skos:broader rdf:resource="urn:aodn.org.au:geographicextents:concept:10004"/>
      <skos:definition xml:lang="en">Marine Features (Australia) | Jurabi Coast Nature Reserve, WA</skos:definition>
      <skos:scopeNote xml:lang="en">Marine Features (Australia) | Jurabi Coast Nature Reserve, WA: Marine Features (Australia) | Jurabi Coast Nature Reserve, WA</skos:scopeNote>
   </skos:Concept>
   <skos:Concept rdf:about="urn:aodn.org.au:geographicextents:concept:88">
      <skos:prefLabel xml:lang="en">Marine Features (Australia) | Kangaroo Island, SA</skos:prefLabel>
      <skos:inScheme rdf:resource="urn:aodn.org.au:geographicextents:conceptscheme:1.0"/>
      <gml:BoundedBy>
         <gml:Envelope gml:srsName="http://www.opengis.net/gml/srs/epsg.xml#epsg:4326">
            <gml:lowerCorner>136.54 -36.14</gml:lowerCorner>
            <gml:upperCorner>138.14 -35.49</gml:upperCorner>
         </gml:Envelope>
      </gml:BoundedBy>
      <skos:broader rdf:resource="urn:aodn.org.au:geographicextents:concept:10004"/>
      <skos:definition xml:lang="en">Marine Features (Australia) | Kangaroo Island, SA</skos:definition>
      <skos:scopeNote xml:lang="en">Marine Features (Australia) | Kangaroo Island, SA: Marine Features (Australia) | Kangaroo Island, SA</skos:scopeNote>
   </skos:Concept>
   <skos:Concept rdf:about="urn:aodn.org.au:geographicextents:concept:1056">
      <skos:prefLabel xml:lang="en">Marine Features (Australia) | Kimberley Coast, WA</skos:prefLabel>
      <skos:inScheme rdf:resource="urn:aodn.org.au:geographicextents:conceptscheme:1.0"/>
      <gml:BoundedBy>
         <gml:Envelope gml:srsName="http://www.opengis.net/gml/srs/epsg.xml#epsg:4326">
            <gml:lowerCorner>119 -21</gml:lowerCorner>
            <gml:upperCorner>129 -13.5</gml:upperCorner>
         </gml:Envelope>
      </gml:BoundedBy>
      <skos:broader rdf:resource="urn:aodn.org.au:geographicextents:concept:10004"/>
      <skos:definition xml:lang="en">Marine Features (Australia) | Kimberley Coast, WA</skos:definition>
      <skos:scopeNote xml:lang="en">Marine Features (Australia) | Kimberley Coast, WA: Marine Features (Australia) | Kimberley Coast, WA</skos:scopeNote>
   </skos:Concept>
   <skos:Concept rdf:about="urn:aodn.org.au:geographicextents:concept:1057">
      <skos:prefLabel xml:lang="en">Marine Features (Australia) | Kimberley Islands, WA</skos:prefLabel>
      <skos:inScheme rdf:resource="urn:aodn.org.au:geographicextents:conceptscheme:1.0"/>
      <gml:BoundedBy>
         <gml:Envelope gml:srsName="http://www.opengis.net/gml/srs/epsg.xml#epsg:4326">
            <gml:lowerCorner>119 -21</gml:lowerCorner>
            <gml:upperCorner>129 -13.5</gml:upperCorner>
         </gml:Envelope>
      </gml:BoundedBy>
      <skos:broader rdf:resource="urn:aodn.org.au:geographicextents:concept:10004"/>
      <skos:definition xml:lang="en">Marine Features (Australia) | Kimberley Islands, WA</skos:definition>
      <skos:scopeNote xml:lang="en">Marine Features (Australia) | Kimberley Islands, WA: Marine Features (Australia) | Kimberley Islands, WA</skos:scopeNote>
   </skos:Concept>
   <skos:Concept rdf:about="urn:aodn.org.au:geographicextents:concept:89">
      <skos:prefLabel xml:lang="en">Marine Features (Australia) | King Island, TAS</skos:prefLabel>
      <skos:inScheme rdf:resource="urn:aodn.org.au:geographicextents:conceptscheme:1.0"/>
      <gml:BoundedBy>
         <gml:Envelope gml:srsName="http://www.opengis.net/gml/srs/epsg.xml#epsg:4326">
            <gml:lowerCorner>143.83 -40.16</gml:lowerCorner>
            <gml:upperCorner>144.14 -39.57</gml:upperCorner>
         </gml:Envelope>
      </gml:BoundedBy>
      <skos:broader rdf:resource="urn:aodn.org.au:geographicextents:concept:10004"/>
      <skos:definition xml:lang="en">Marine Features (Australia) | King Island, TAS</skos:definition>
      <skos:scopeNote xml:lang="en">Marine Features (Australia) | King Island, TAS: Marine Features (Australia) | King Island, TAS</skos:scopeNote>
   </skos:Concept>
   <skos:Concept rdf:about="urn:aodn.org.au:geographicextents:concept:90">
      <skos:prefLabel xml:lang="en">Marine Features (Australia) | King Sound, WA</skos:prefLabel>
      <skos:inScheme rdf:resource="urn:aodn.org.au:geographicextents:conceptscheme:1.0"/>
      <gml:BoundedBy>
         <gml:Envelope gml:srsName="http://www.opengis.net/gml/srs/epsg.xml#epsg:4326">
            <gml:lowerCorner>123 -18</gml:lowerCorner>
            <gml:upperCorner>124 -16</gml:upperCorner>
         </gml:Envelope>
      </gml:BoundedBy>
      <skos:broader rdf:resource="urn:aodn.org.au:geographicextents:concept:10004"/>
      <skos:definition xml:lang="en">Marine Features (Australia) | King Sound, WA</skos:definition>
      <skos:scopeNote xml:lang="en">Marine Features (Australia) | King Sound, WA: Marine Features (Australia) | King Sound, WA</skos:scopeNote>
   </skos:Concept>
   <skos:Concept rdf:about="urn:aodn.org.au:geographicextents:concept:1058">
      <skos:prefLabel xml:lang="en">Marine Features (Australia) | Koolan Island, WA</skos:prefLabel>
      <skos:inScheme rdf:resource="urn:aodn.org.au:geographicextents:conceptscheme:1.0"/>
      <gml:BoundedBy>
         <gml:Envelope gml:srsName="http://www.opengis.net/gml/srs/epsg.xml#epsg:4326">
            <gml:lowerCorner>123.68 -16.17</gml:lowerCorner>
            <gml:upperCorner>123.8 -16.1</gml:upperCorner>
         </gml:Envelope>
      </gml:BoundedBy>
      <skos:broader rdf:resource="urn:aodn.org.au:geographicextents:concept:10004"/>
      <skos:definition xml:lang="en">Marine Features (Australia) | Koolan Island, WA</skos:definition>
      <skos:scopeNote xml:lang="en">Marine Features (Australia) | Koolan Island, WA: Marine Features (Australia) | Koolan Island, WA</skos:scopeNote>
   </skos:Concept>
   <skos:Concept rdf:about="urn:aodn.org.au:geographicextents:concept:1059">
      <skos:prefLabel xml:lang="en">Marine Features (Australia) | Leeuwin Current</skos:prefLabel>
      <skos:inScheme rdf:resource="urn:aodn.org.au:geographicextents:conceptscheme:1.0"/>
      <gml:BoundedBy>
         <gml:Envelope gml:srsName="http://www.opengis.net/gml/srs/epsg.xml#epsg:4326">
            <gml:lowerCorner>110 -43</gml:lowerCorner>
            <gml:upperCorner>145 -21</gml:upperCorner>
         </gml:Envelope>
      </gml:BoundedBy>
      <skos:broader rdf:resource="urn:aodn.org.au:geographicextents:concept:10004"/>
      <skos:definition xml:lang="en">Marine Features (Australia) | Leeuwin Current</skos:definition>
      <skos:scopeNote xml:lang="en">Marine Features (Australia) | Leeuwin Current: Marine Features (Australia) | Leeuwin Current</skos:scopeNote>
   </skos:Concept>
   <skos:Concept rdf:about="urn:aodn.org.au:geographicextents:concept:91">
      <skos:prefLabel xml:lang="en">Marine Features (Australia) | Macquarie Harbour, TAS</skos:prefLabel>
      <skos:inScheme rdf:resource="urn:aodn.org.au:geographicextents:conceptscheme:1.0"/>
      <gml:BoundedBy>
         <gml:Envelope gml:srsName="http://www.opengis.net/gml/srs/epsg.xml#epsg:4326">
            <gml:lowerCorner>145.2 -42.5</gml:lowerCorner>
            <gml:upperCorner>145.6 -42.1</gml:upperCorner>
         </gml:Envelope>
      </gml:BoundedBy>
      <skos:broader rdf:resource="urn:aodn.org.au:geographicextents:concept:10004"/>
      <skos:definition xml:lang="en">Marine Features (Australia) | Macquarie Harbour, TAS</skos:definition>
      <skos:scopeNote xml:lang="en">Marine Features (Australia) | Macquarie Harbour, TAS: Marine Features (Australia) | Macquarie Harbour, TAS</skos:scopeNote>
   </skos:Concept>
   <skos:Concept rdf:about="urn:aodn.org.au:geographicextents:concept:92">
      <skos:prefLabel xml:lang="en">Marine Features (Australia) | Melville Island, NT</skos:prefLabel>
      <skos:inScheme rdf:resource="urn:aodn.org.au:geographicextents:conceptscheme:1.0"/>
      <gml:BoundedBy>
         <gml:Envelope gml:srsName="http://www.opengis.net/gml/srs/epsg.xml#epsg:4326">
            <gml:lowerCorner>130.36 -11.94</gml:lowerCorner>
            <gml:upperCorner>131.55 -11.16</gml:upperCorner>
         </gml:Envelope>
      </gml:BoundedBy>
      <skos:broader rdf:resource="urn:aodn.org.au:geographicextents:concept:10004"/>
      <skos:definition xml:lang="en">Marine Features (Australia) | Melville Island, NT</skos:definition>
      <skos:scopeNote xml:lang="en">Marine Features (Australia) | Melville Island, NT: Marine Features (Australia) | Melville Island, NT</skos:scopeNote>
   </skos:Concept>
   <skos:Concept rdf:about="urn:aodn.org.au:geographicextents:concept:1060">
      <skos:prefLabel xml:lang="en">Marine Features (Australia) | Mermaid Reef, WA</skos:prefLabel>
      <skos:inScheme rdf:resource="urn:aodn.org.au:geographicextents:conceptscheme:1.0"/>
      <gml:BoundedBy>
         <gml:Envelope gml:srsName="http://www.opengis.net/gml/srs/epsg.xml#epsg:4326">
            <gml:lowerCorner>119.42 -17.15</gml:lowerCorner>
            <gml:upperCorner>119.7 -16.92</gml:upperCorner>
         </gml:Envelope>
      </gml:BoundedBy>
      <skos:broader rdf:resource="urn:aodn.org.au:geographicextents:concept:10004"/>
      <skos:definition xml:lang="en">Marine Features (Australia) | Mermaid Reef, WA</skos:definition>
      <skos:scopeNote xml:lang="en">Marine Features (Australia) | Mermaid Reef, WA: Marine Features (Australia) | Mermaid Reef, WA</skos:scopeNote>
   </skos:Concept>
   <skos:Concept rdf:about="urn:aodn.org.au:geographicextents:concept:1061">
      <skos:prefLabel xml:lang="en">Marine Features (Australia) | Montebello Islands, WA</skos:prefLabel>
      <skos:inScheme rdf:resource="urn:aodn.org.au:geographicextents:conceptscheme:1.0"/>
      <gml:BoundedBy>
         <gml:Envelope gml:srsName="http://www.opengis.net/gml/srs/epsg.xml#epsg:4326">
            <gml:lowerCorner>115.48 -20.54</gml:lowerCorner>
            <gml:upperCorner>115.63 -20.34</gml:upperCorner>
         </gml:Envelope>
      </gml:BoundedBy>
      <skos:broader rdf:resource="urn:aodn.org.au:geographicextents:concept:10004"/>
      <skos:definition xml:lang="en">Marine Features (Australia) | Montebello Islands, WA</skos:definition>
      <skos:scopeNote xml:lang="en">Marine Features (Australia) | Montebello Islands, WA: Marine Features (Australia) | Montebello Islands, WA</skos:scopeNote>
   </skos:Concept>
   <skos:Concept rdf:about="urn:aodn.org.au:geographicextents:concept:93">
      <skos:prefLabel xml:lang="en">Marine Features (Australia) | Moreton Bay, QLD</skos:prefLabel>
      <skos:inScheme rdf:resource="urn:aodn.org.au:geographicextents:conceptscheme:1.0"/>
      <gml:BoundedBy>
         <gml:Envelope gml:srsName="http://www.opengis.net/gml/srs/epsg.xml#epsg:4326">
            <gml:lowerCorner>153 -28</gml:lowerCorner>
            <gml:upperCorner>154 -27</gml:upperCorner>
         </gml:Envelope>
      </gml:BoundedBy>
      <skos:broader rdf:resource="urn:aodn.org.au:geographicextents:concept:10004"/>
      <skos:definition xml:lang="en">Marine Features (Australia) | Moreton Bay, QLD</skos:definition>
      <skos:scopeNote xml:lang="en">Marine Features (Australia) | Moreton Bay, QLD: Marine Features (Australia) | Moreton Bay, QLD</skos:scopeNote>
   </skos:Concept>
   <skos:Concept rdf:about="urn:aodn.org.au:geographicextents:concept:94">
      <skos:prefLabel xml:lang="en">Marine Features (Australia) | Mornington Island, QLD</skos:prefLabel>
      <skos:inScheme rdf:resource="urn:aodn.org.au:geographicextents:conceptscheme:1.0"/>
      <gml:BoundedBy>
         <gml:Envelope gml:srsName="http://www.opengis.net/gml/srs/epsg.xml#epsg:4326">
            <gml:lowerCorner>139.11 -16.79</gml:lowerCorner>
            <gml:upperCorner>139.75 -16.35</gml:upperCorner>
         </gml:Envelope>
      </gml:BoundedBy>
      <skos:broader rdf:resource="urn:aodn.org.au:geographicextents:concept:10004"/>
      <skos:definition xml:lang="en">Marine Features (Australia) | Mornington Island, QLD</skos:definition>
      <skos:scopeNote xml:lang="en">Marine Features (Australia) | Mornington Island, QLD: Marine Features (Australia) | Mornington Island, QLD</skos:scopeNote>
   </skos:Concept>
   <skos:Concept rdf:about="urn:aodn.org.au:geographicextents:concept:1062">
      <skos:prefLabel xml:lang="en">Marine Features (Australia) | Ningaloo Marine Park, WA</skos:prefLabel>
      <skos:inScheme rdf:resource="urn:aodn.org.au:geographicextents:conceptscheme:1.0"/>
      <gml:BoundedBy>
         <gml:Envelope gml:srsName="http://www.opengis.net/gml/srs/epsg.xml#epsg:4326">
            <gml:lowerCorner>113.26 -24.13</gml:lowerCorner>
            <gml:upperCorner>114.22 -21.77</gml:upperCorner>
         </gml:Envelope>
      </gml:BoundedBy>
      <skos:broader rdf:resource="urn:aodn.org.au:geographicextents:concept:10004"/>
      <skos:definition xml:lang="en">Marine Features (Australia) | Ningaloo Marine Park, WA</skos:definition>
      <skos:scopeNote xml:lang="en">Marine Features (Australia) | Ningaloo Marine Park, WA: Marine Features (Australia) | Ningaloo Marine Park, WA</skos:scopeNote>
   </skos:Concept>
   <skos:Concept rdf:about="urn:aodn.org.au:geographicextents:concept:1063">
      <skos:prefLabel xml:lang="en">Marine Features (Australia) | North West Cape, WA</skos:prefLabel>
      <skos:inScheme rdf:resource="urn:aodn.org.au:geographicextents:conceptscheme:1.0"/>
      <gml:BoundedBy>
         <gml:Envelope gml:srsName="http://www.opengis.net/gml/srs/epsg.xml#epsg:4326">
            <gml:lowerCorner>113.96 -22.07</gml:lowerCorner>
            <gml:upperCorner>114.2 -21.78</gml:upperCorner>
         </gml:Envelope>
      </gml:BoundedBy>
      <skos:broader rdf:resource="urn:aodn.org.au:geographicextents:concept:10004"/>
      <skos:definition xml:lang="en">Marine Features (Australia) | North West Cape, WA</skos:definition>
      <skos:scopeNote xml:lang="en">Marine Features (Australia) | North West Cape, WA: Marine Features (Australia) | North West Cape, WA</skos:scopeNote>
   </skos:Concept>
   <skos:Concept rdf:about="urn:aodn.org.au:geographicextents:concept:1064">
      <skos:prefLabel xml:lang="en">Marine Features (Australia) | One Tree Island, QLD</skos:prefLabel>
      <skos:inScheme rdf:resource="urn:aodn.org.au:geographicextents:conceptscheme:1.0"/>
      <gml:BoundedBy>
         <gml:Envelope gml:srsName="http://www.opengis.net/gml/srs/epsg.xml#epsg:4326">
            <gml:lowerCorner>152.08 -23.51</gml:lowerCorner>
            <gml:upperCorner>152.1 -23.5</gml:upperCorner>
         </gml:Envelope>
      </gml:BoundedBy>
      <skos:broader rdf:resource="urn:aodn.org.au:geographicextents:concept:10004"/>
      <skos:definition xml:lang="en">Marine Features (Australia) | One Tree Island, QLD</skos:definition>
      <skos:scopeNote xml:lang="en">Marine Features (Australia) | One Tree Island, QLD: Marine Features (Australia) | One Tree Island, QLD</skos:scopeNote>
   </skos:Concept>
   <skos:Concept rdf:about="urn:aodn.org.au:geographicextents:concept:1065">
      <skos:prefLabel xml:lang="en">Marine Features (Australia) | Owen Anchorage, WA</skos:prefLabel>
      <skos:inScheme rdf:resource="urn:aodn.org.au:geographicextents:conceptscheme:1.0"/>
      <gml:BoundedBy>
         <gml:Envelope gml:srsName="http://www.opengis.net/gml/srs/epsg.xml#epsg:4326">
            <gml:lowerCorner>115.73 -32.12</gml:lowerCorner>
            <gml:upperCorner>115.76 -32.08</gml:upperCorner>
         </gml:Envelope>
      </gml:BoundedBy>
      <skos:broader rdf:resource="urn:aodn.org.au:geographicextents:concept:10004"/>
      <skos:definition xml:lang="en">Marine Features (Australia) | Owen Anchorage, WA</skos:definition>
      <skos:scopeNote xml:lang="en">Marine Features (Australia) | Owen Anchorage, WA: Marine Features (Australia) | Owen Anchorage, WA</skos:scopeNote>
   </skos:Concept>
   <skos:Concept rdf:about="urn:aodn.org.au:geographicextents:concept:1066">
      <skos:prefLabel xml:lang="en">Marine Features (Australia) | Perth Canyon, WA</skos:prefLabel>
      <skos:inScheme rdf:resource="urn:aodn.org.au:geographicextents:conceptscheme:1.0"/>
      <gml:BoundedBy>
         <gml:Envelope gml:srsName="http://www.opengis.net/gml/srs/epsg.xml#epsg:4326">
            <gml:lowerCorner>114 -32</gml:lowerCorner>
            <gml:upperCorner>115 -31.5</gml:upperCorner>
         </gml:Envelope>
      </gml:BoundedBy>
      <skos:broader rdf:resource="urn:aodn.org.au:geographicextents:concept:10004"/>
      <skos:definition xml:lang="en">Marine Features (Australia) | Perth Canyon, WA</skos:definition>
      <skos:scopeNote xml:lang="en">Marine Features (Australia) | Perth Canyon, WA: Marine Features (Australia) | Perth Canyon, WA</skos:scopeNote>
   </skos:Concept>
   <skos:Concept rdf:about="urn:aodn.org.au:geographicextents:concept:1067">
      <skos:prefLabel xml:lang="en">Marine Features (Australia) | Pilbara Coast, WA</skos:prefLabel>
      <skos:inScheme rdf:resource="urn:aodn.org.au:geographicextents:conceptscheme:1.0"/>
      <gml:BoundedBy>
         <gml:Envelope gml:srsName="http://www.opengis.net/gml/srs/epsg.xml#epsg:4326">
            <gml:lowerCorner>117.1 -20.7</gml:lowerCorner>
            <gml:upperCorner>120.5 -18.5</gml:upperCorner>
         </gml:Envelope>
      </gml:BoundedBy>
      <skos:broader rdf:resource="urn:aodn.org.au:geographicextents:concept:10004"/>
      <skos:definition xml:lang="en">Marine Features (Australia) | Pilbara Coast, WA</skos:definition>
      <skos:scopeNote xml:lang="en">Marine Features (Australia) | Pilbara Coast, WA: Marine Features (Australia) | Pilbara Coast, WA</skos:scopeNote>
   </skos:Concept>
   <skos:Concept rdf:about="urn:aodn.org.au:geographicextents:concept:1068">
      <skos:prefLabel xml:lang="en">Marine Features (Australia) | Port Broughton, SA</skos:prefLabel>
      <skos:inScheme rdf:resource="urn:aodn.org.au:geographicextents:conceptscheme:1.0"/>
      <gml:BoundedBy>
         <gml:Envelope gml:srsName="http://www.opengis.net/gml/srs/epsg.xml#epsg:4326">
            <gml:lowerCorner>137.88 -33.63</gml:lowerCorner>
            <gml:upperCorner>137.98 -33.54</gml:upperCorner>
         </gml:Envelope>
      </gml:BoundedBy>
      <skos:broader rdf:resource="urn:aodn.org.au:geographicextents:concept:10004"/>
      <skos:definition xml:lang="en">Marine Features (Australia) | Port Broughton, SA</skos:definition>
      <skos:scopeNote xml:lang="en">Marine Features (Australia) | Port Broughton, SA: Marine Features (Australia) | Port Broughton, SA</skos:scopeNote>
   </skos:Concept>
   <skos:Concept rdf:about="urn:aodn.org.au:geographicextents:concept:95">
      <skos:prefLabel xml:lang="en">Marine Features (Australia) | Port Hacking, NSW</skos:prefLabel>
      <skos:inScheme rdf:resource="urn:aodn.org.au:geographicextents:conceptscheme:1.0"/>
      <gml:BoundedBy>
         <gml:Envelope gml:srsName="http://www.opengis.net/gml/srs/epsg.xml#epsg:4326">
            <gml:lowerCorner>151.11 -34.08</gml:lowerCorner>
            <gml:upperCorner>151.15 -34.07</gml:upperCorner>
         </gml:Envelope>
      </gml:BoundedBy>
      <skos:broader rdf:resource="urn:aodn.org.au:geographicextents:concept:10004"/>
      <skos:definition xml:lang="en">Marine Features (Australia) | Port Hacking, NSW</skos:definition>
      <skos:scopeNote xml:lang="en">Marine Features (Australia) | Port Hacking, NSW: Marine Features (Australia) | Port Hacking, NSW</skos:scopeNote>
   </skos:Concept>
   <skos:Concept rdf:about="urn:aodn.org.au:geographicextents:concept:96">
      <skos:prefLabel xml:lang="en">Marine Features (Australia) | Port Phillip Bay, VIC</skos:prefLabel>
      <skos:inScheme rdf:resource="urn:aodn.org.au:geographicextents:conceptscheme:1.0"/>
      <gml:BoundedBy>
         <gml:Envelope gml:srsName="http://www.opengis.net/gml/srs/epsg.xml#epsg:4326">
            <gml:lowerCorner>144.3 -38.3</gml:lowerCorner>
            <gml:upperCorner>145.2 -37.8</gml:upperCorner>
         </gml:Envelope>
      </gml:BoundedBy>
      <skos:broader rdf:resource="urn:aodn.org.au:geographicextents:concept:10004"/>
      <skos:definition xml:lang="en">Marine Features (Australia) | Port Phillip Bay, VIC</skos:definition>
      <skos:scopeNote xml:lang="en">Marine Features (Australia) | Port Phillip Bay, VIC: Marine Features (Australia) | Port Phillip Bay, VIC</skos:scopeNote>
   </skos:Concept>
   <skos:Concept rdf:about="urn:aodn.org.au:geographicextents:concept:1069">
      <skos:prefLabel xml:lang="en">Marine Features (Australia) | Port Pirie, SA</skos:prefLabel>
      <skos:inScheme rdf:resource="urn:aodn.org.au:geographicextents:conceptscheme:1.0"/>
      <gml:BoundedBy>
         <gml:Envelope gml:srsName="http://www.opengis.net/gml/srs/epsg.xml#epsg:4326">
            <gml:lowerCorner>137.99 -33.19</gml:lowerCorner>
            <gml:upperCorner>138.15 -33.14</gml:upperCorner>
         </gml:Envelope>
      </gml:BoundedBy>
      <skos:broader rdf:resource="urn:aodn.org.au:geographicextents:concept:10004"/>
      <skos:definition xml:lang="en">Marine Features (Australia) | Port Pirie, SA</skos:definition>
      <skos:scopeNote xml:lang="en">Marine Features (Australia) | Port Pirie, SA: Marine Features (Australia) | Port Pirie, SA</skos:scopeNote>
   </skos:Concept>
   <skos:Concept rdf:about="urn:aodn.org.au:geographicextents:concept:1070">
      <skos:prefLabel xml:lang="en">Marine Features (Australia) | Port Wakefield, SA</skos:prefLabel>
      <skos:inScheme rdf:resource="urn:aodn.org.au:geographicextents:conceptscheme:1.0"/>
      <gml:BoundedBy>
         <gml:Envelope gml:srsName="http://www.opengis.net/gml/srs/epsg.xml#epsg:4326">
            <gml:lowerCorner>138.11 -34.23</gml:lowerCorner>
            <gml:upperCorner>138.16 -34.15</gml:upperCorner>
         </gml:Envelope>
      </gml:BoundedBy>
      <skos:broader rdf:resource="urn:aodn.org.au:geographicextents:concept:10004"/>
      <skos:definition xml:lang="en">Marine Features (Australia) | Port Wakefield, SA</skos:definition>
      <skos:scopeNote xml:lang="en">Marine Features (Australia) | Port Wakefield, SA: Marine Features (Australia) | Port Wakefield, SA</skos:scopeNote>
   </skos:Concept>
   <skos:Concept rdf:about="urn:aodn.org.au:geographicextents:concept:1071">
      <skos:prefLabel xml:lang="en">Marine Features (Australia) | Port Victoria, SA</skos:prefLabel>
      <skos:inScheme rdf:resource="urn:aodn.org.au:geographicextents:conceptscheme:1.0"/>
      <gml:BoundedBy>
         <gml:Envelope gml:srsName="http://www.opengis.net/gml/srs/epsg.xml#epsg:4326">
            <gml:lowerCorner>137.46 -34.52</gml:lowerCorner>
            <gml:upperCorner>137.49 -34.48</gml:upperCorner>
         </gml:Envelope>
      </gml:BoundedBy>
      <skos:broader rdf:resource="urn:aodn.org.au:geographicextents:concept:10004"/>
      <skos:definition xml:lang="en">Marine Features (Australia) | Port Victoria, SA</skos:definition>
      <skos:scopeNote xml:lang="en">Marine Features (Australia) | Port Victoria, SA: Marine Features (Australia) | Port Victoria, SA</skos:scopeNote>
   </skos:Concept>
   <skos:Concept rdf:about="urn:aodn.org.au:geographicextents:concept:1072">
      <skos:prefLabel xml:lang="en">Marine Features (Australia) | Roebuck Bay, WA</skos:prefLabel>
      <skos:inScheme rdf:resource="urn:aodn.org.au:geographicextents:conceptscheme:1.0"/>
      <gml:BoundedBy>
         <gml:Envelope gml:srsName="http://www.opengis.net/gml/srs/epsg.xml#epsg:4326">
            <gml:lowerCorner>122.18 -18.24</gml:lowerCorner>
            <gml:upperCorner>122.39 -17.91</gml:upperCorner>
         </gml:Envelope>
      </gml:BoundedBy>
      <skos:broader rdf:resource="urn:aodn.org.au:geographicextents:concept:10004"/>
      <skos:definition xml:lang="en">Marine Features (Australia) | Roebuck Bay, WA</skos:definition>
      <skos:scopeNote xml:lang="en">Marine Features (Australia) | Roebuck Bay, WA: Marine Features (Australia) | Roebuck Bay, WA</skos:scopeNote>
   </skos:Concept>
   <skos:Concept rdf:about="urn:aodn.org.au:geographicextents:concept:1073">
      <skos:prefLabel xml:lang="en">Marine Features (Australia) | Rosemary Island, WA</skos:prefLabel>
      <skos:inScheme rdf:resource="urn:aodn.org.au:geographicextents:conceptscheme:1.0"/>
      <gml:BoundedBy>
         <gml:Envelope gml:srsName="http://www.opengis.net/gml/srs/epsg.xml#epsg:4326">
            <gml:lowerCorner>116.56 -20.51</gml:lowerCorner>
            <gml:upperCorner>116.62 -20.45</gml:upperCorner>
         </gml:Envelope>
      </gml:BoundedBy>
      <skos:broader rdf:resource="urn:aodn.org.au:geographicextents:concept:10004"/>
      <skos:definition xml:lang="en">Marine Features (Australia) | Rosemary Island, WA</skos:definition>
      <skos:scopeNote xml:lang="en">Marine Features (Australia) | Rosemary Island, WA: Marine Features (Australia) | Rosemary Island, WA</skos:scopeNote>
   </skos:Concept>
   <skos:Concept rdf:about="urn:aodn.org.au:geographicextents:concept:1074">
      <skos:prefLabel xml:lang="en">Marine Features (Australia) | Rottnest Island, WA</skos:prefLabel>
      <skos:inScheme rdf:resource="urn:aodn.org.au:geographicextents:conceptscheme:1.0"/>
      <gml:BoundedBy>
         <gml:Envelope gml:srsName="http://www.opengis.net/gml/srs/epsg.xml#epsg:4326">
            <gml:lowerCorner>115.44 -32.03</gml:lowerCorner>
            <gml:upperCorner>115.56 -31.987</gml:upperCorner>
         </gml:Envelope>
      </gml:BoundedBy>
      <skos:broader rdf:resource="urn:aodn.org.au:geographicextents:concept:10004"/>
      <skos:definition xml:lang="en">Marine Features (Australia) | Rottnest Island, WA</skos:definition>
      <skos:scopeNote xml:lang="en">Marine Features (Australia) | Rottnest Island, WA: Marine Features (Australia) | Rottnest Island, WA</skos:scopeNote>
   </skos:Concept>
   <skos:Concept rdf:about="urn:aodn.org.au:geographicextents:concept:1075">
      <skos:prefLabel xml:lang="en">Marine Features (Australia) | Rowley Shoals, WA</skos:prefLabel>
      <skos:inScheme rdf:resource="urn:aodn.org.au:geographicextents:conceptscheme:1.0"/>
      <gml:BoundedBy>
         <gml:Envelope gml:srsName="http://www.opengis.net/gml/srs/epsg.xml#epsg:4326">
            <gml:lowerCorner>118.83 -17.71</gml:lowerCorner>
            <gml:upperCorner>119.91 -16.87</gml:upperCorner>
         </gml:Envelope>
      </gml:BoundedBy>
      <skos:broader rdf:resource="urn:aodn.org.au:geographicextents:concept:10004"/>
      <skos:definition xml:lang="en">Marine Features (Australia) | Rowley Shoals, WA</skos:definition>
      <skos:scopeNote xml:lang="en">Marine Features (Australia) | Rowley Shoals, WA: Marine Features (Australia) | Rowley Shoals, WA</skos:scopeNote>
   </skos:Concept>
   <skos:Concept rdf:about="urn:aodn.org.au:geographicextents:concept:1076">
      <skos:prefLabel xml:lang="en">Marine Features (Australia) | Scott Reef, WA</skos:prefLabel>
      <skos:inScheme rdf:resource="urn:aodn.org.au:geographicextents:conceptscheme:1.0"/>
      <gml:BoundedBy>
         <gml:Envelope gml:srsName="http://www.opengis.net/gml/srs/epsg.xml#epsg:4326">
            <gml:lowerCorner>121.5 -14.5</gml:lowerCorner>
            <gml:upperCorner>122.5 -13.5</gml:upperCorner>
         </gml:Envelope>
      </gml:BoundedBy>
      <skos:broader rdf:resource="urn:aodn.org.au:geographicextents:concept:10004"/>
      <skos:definition xml:lang="en">Marine Features (Australia) | Scott Reef, WA</skos:definition>
      <skos:scopeNote xml:lang="en">Marine Features (Australia) | Scott Reef, WA: Marine Features (Australia) | Scott Reef, WA</skos:scopeNote>
   </skos:Concept>
   <skos:Concept rdf:about="urn:aodn.org.au:geographicextents:concept:97">
      <skos:prefLabel xml:lang="en">Marine Features (Australia) | Shark Bay, WA</skos:prefLabel>
      <skos:inScheme rdf:resource="urn:aodn.org.au:geographicextents:conceptscheme:1.0"/>
      <gml:BoundedBy>
         <gml:Envelope gml:srsName="http://www.opengis.net/gml/srs/epsg.xml#epsg:4326">
            <gml:lowerCorner>113 -27</gml:lowerCorner>
            <gml:upperCorner>115 -25</gml:upperCorner>
         </gml:Envelope>
      </gml:BoundedBy>
      <skos:broader rdf:resource="urn:aodn.org.au:geographicextents:concept:10004"/>
      <skos:definition xml:lang="en">Marine Features (Australia) | Shark Bay, WA</skos:definition>
      <skos:scopeNote xml:lang="en">Marine Features (Australia) | Shark Bay, WA: Marine Features (Australia) | Shark Bay, WA</skos:scopeNote>
   </skos:Concept>
   <skos:Concept rdf:about="urn:aodn.org.au:geographicextents:concept:98">
      <skos:prefLabel xml:lang="en">Marine Features (Australia) | Spencer Gulf, SA</skos:prefLabel>
      <skos:inScheme rdf:resource="urn:aodn.org.au:geographicextents:conceptscheme:1.0"/>
      <gml:BoundedBy>
         <gml:Envelope gml:srsName="http://www.opengis.net/gml/srs/epsg.xml#epsg:4326">
            <gml:lowerCorner>136 -35</gml:lowerCorner>
            <gml:upperCorner>138 -32</gml:upperCorner>
         </gml:Envelope>
      </gml:BoundedBy>
      <skos:broader rdf:resource="urn:aodn.org.au:geographicextents:concept:10004"/>
      <skos:definition xml:lang="en">Marine Features (Australia) | Spencer Gulf, SA</skos:definition>
      <skos:scopeNote xml:lang="en">Marine Features (Australia) | Spencer Gulf, SA: Marine Features (Australia) | Spencer Gulf, SA</skos:scopeNote>
   </skos:Concept>
   <skos:Concept rdf:about="urn:aodn.org.au:geographicextents:concept:1077">
      <skos:prefLabel xml:lang="en">Marine Features (Australia) | Swan Estuary, WA</skos:prefLabel>
      <skos:inScheme rdf:resource="urn:aodn.org.au:geographicextents:conceptscheme:1.0"/>
      <gml:BoundedBy>
         <gml:Envelope gml:srsName="http://www.opengis.net/gml/srs/epsg.xml#epsg:4326">
            <gml:lowerCorner>115.72 -32.08</gml:lowerCorner>
            <gml:upperCorner>115.88 -31.95</gml:upperCorner>
         </gml:Envelope>
      </gml:BoundedBy>
      <skos:broader rdf:resource="urn:aodn.org.au:geographicextents:concept:10004"/>
      <skos:definition xml:lang="en">Marine Features (Australia) | Swan Estuary, WA</skos:definition>
      <skos:scopeNote xml:lang="en">Marine Features (Australia) | Swan Estuary, WA: Marine Features (Australia) | Swan Estuary, WA</skos:scopeNote>
   </skos:Concept>
   <skos:Concept rdf:about="urn:aodn.org.au:geographicextents:concept:99">
      <skos:prefLabel xml:lang="en">Marine Features (Australia) | Swan River, WA</skos:prefLabel>
      <skos:inScheme rdf:resource="urn:aodn.org.au:geographicextents:conceptscheme:1.0"/>
      <gml:BoundedBy>
         <gml:Envelope gml:srsName="http://www.opengis.net/gml/srs/epsg.xml#epsg:4326">
            <gml:lowerCorner>115.6 -32.1</gml:lowerCorner>
            <gml:upperCorner>116 -31.9</gml:upperCorner>
         </gml:Envelope>
      </gml:BoundedBy>
      <skos:broader rdf:resource="urn:aodn.org.au:geographicextents:concept:10004"/>
      <skos:definition xml:lang="en">Marine Features (Australia) | Swan River, WA</skos:definition>
      <skos:scopeNote xml:lang="en">Marine Features (Australia) | Swan River, WA: Marine Features (Australia) | Swan River, WA</skos:scopeNote>
   </skos:Concept>
   <skos:Concept rdf:about="urn:aodn.org.au:geographicextents:concept:1026">
      <skos:prefLabel xml:lang="en">Marine Features (Australia) | Sydney Harbour, NSW</skos:prefLabel>
      <skos:inScheme rdf:resource="urn:aodn.org.au:geographicextents:conceptscheme:1.0"/>
      <gml:BoundedBy>
         <gml:Envelope gml:srsName="http://www.opengis.net/gml/srs/epsg.xml#epsg:4326">
            <gml:lowerCorner>151.17 -33.88</gml:lowerCorner>
            <gml:upperCorner>151.3 -33.81</gml:upperCorner>
         </gml:Envelope>
      </gml:BoundedBy>
      <skos:broader rdf:resource="urn:aodn.org.au:geographicextents:concept:10004"/>
      <skos:definition xml:lang="en">Marine Features (Australia) | Sydney Harbour, NSW</skos:definition>
      <skos:scopeNote xml:lang="en">Marine Features (Australia) | Sydney Harbour, NSW: Marine Features (Australia) | Sydney Harbour, NSW</skos:scopeNote>
   </skos:Concept>
   <skos:Concept rdf:about="urn:aodn.org.au:geographicextents:concept:1078">
      <skos:prefLabel xml:lang="en">Marine Features (Australia) | Tiparra Reef, SA</skos:prefLabel>
      <skos:inScheme rdf:resource="urn:aodn.org.au:geographicextents:conceptscheme:1.0"/>
      <gml:BoundedBy>
         <gml:Envelope gml:srsName="http://www.opengis.net/gml/srs/epsg.xml#epsg:4326">
            <gml:lowerCorner>137.3 -34.09</gml:lowerCorner>
            <gml:upperCorner>137.47 -33.99</gml:upperCorner>
         </gml:Envelope>
      </gml:BoundedBy>
      <skos:broader rdf:resource="urn:aodn.org.au:geographicextents:concept:10004"/>
      <skos:definition xml:lang="en">Marine Features (Australia) | Tiparra Reef, SA</skos:definition>
      <skos:scopeNote xml:lang="en">Marine Features (Australia) | Tiparra Reef, SA: Marine Features (Australia) | Tiparra Reef, SA</skos:scopeNote>
   </skos:Concept>
   <skos:Concept rdf:about="urn:aodn.org.au:geographicextents:concept:100">
      <skos:prefLabel xml:lang="en">Marine Features (Australia) | Torres Strait, QLD</skos:prefLabel>
      <skos:inScheme rdf:resource="urn:aodn.org.au:geographicextents:conceptscheme:1.0"/>
      <gml:BoundedBy>
         <gml:Envelope gml:srsName="http://www.opengis.net/gml/srs/epsg.xml#epsg:4326">
            <gml:lowerCorner>142 -11</gml:lowerCorner>
            <gml:upperCorner>143 -9</gml:upperCorner>
         </gml:Envelope>
      </gml:BoundedBy>
      <skos:broader rdf:resource="urn:aodn.org.au:geographicextents:concept:10004"/>
      <skos:definition xml:lang="en">Marine Features (Australia) | Torres Strait, QLD</skos:definition>
      <skos:scopeNote xml:lang="en">Marine Features (Australia) | Torres Strait, QLD: Marine Features (Australia) | Torres Strait, QLD</skos:scopeNote>
   </skos:Concept>
   <skos:Concept rdf:about="urn:aodn.org.au:geographicextents:concept:1079">
      <skos:prefLabel xml:lang="en">Marine Features (Australia) | Turquoise Coast, WA</skos:prefLabel>
      <skos:inScheme rdf:resource="urn:aodn.org.au:geographicextents:conceptscheme:1.0"/>
      <gml:BoundedBy>
         <gml:Envelope gml:srsName="http://www.opengis.net/gml/srs/epsg.xml#epsg:4326">
            <gml:lowerCorner>114.9 -31.2</gml:lowerCorner>
            <gml:upperCorner>115.3 -29.1</gml:upperCorner>
         </gml:Envelope>
      </gml:BoundedBy>
      <skos:broader rdf:resource="urn:aodn.org.au:geographicextents:concept:10004"/>
      <skos:definition xml:lang="en">Marine Features (Australia) | Turquoise Coast, WA</skos:definition>
      <skos:scopeNote xml:lang="en">Marine Features (Australia) | Turquoise Coast, WA: Marine Features (Australia) | Turquoise Coast, WA</skos:scopeNote>
   </skos:Concept>
   <skos:Concept rdf:about="urn:aodn.org.au:geographicextents:concept:101">
      <skos:prefLabel xml:lang="en">Marine Features (Australia) | Van Diemen Gulf, NT</skos:prefLabel>
      <skos:inScheme rdf:resource="urn:aodn.org.au:geographicextents:conceptscheme:1.0"/>
      <gml:BoundedBy>
         <gml:Envelope gml:srsName="http://www.opengis.net/gml/srs/epsg.xml#epsg:4326">
            <gml:lowerCorner>131 -13</gml:lowerCorner>
            <gml:upperCorner>133 -11</gml:upperCorner>
         </gml:Envelope>
      </gml:BoundedBy>
      <skos:broader rdf:resource="urn:aodn.org.au:geographicextents:concept:10004"/>
      <skos:definition xml:lang="en">Marine Features (Australia) | Van Diemen Gulf, NT</skos:definition>
      <skos:scopeNote xml:lang="en">Marine Features (Australia) | Van Diemen Gulf, NT: Marine Features (Australia) | Van Diemen Gulf, NT</skos:scopeNote>
   </skos:Concept>
   <skos:Concept rdf:about="urn:aodn.org.au:geographicextents:concept:1080">
      <skos:prefLabel xml:lang="en">Marine Features (Australia) | Western Port, VIC</skos:prefLabel>
      <skos:inScheme rdf:resource="urn:aodn.org.au:geographicextents:conceptscheme:1.0"/>
      <gml:BoundedBy>
         <gml:Envelope gml:srsName="http://www.opengis.net/gml/srs/epsg.xml#epsg:4326">
            <gml:lowerCorner>145.2 -38.4</gml:lowerCorner>
            <gml:upperCorner>145.3 -38.2</gml:upperCorner>
         </gml:Envelope>
      </gml:BoundedBy>
      <skos:broader rdf:resource="urn:aodn.org.au:geographicextents:concept:10004"/>
      <skos:definition xml:lang="en">Marine Features (Australia) | Western Port, VIC</skos:definition>
      <skos:scopeNote xml:lang="en">Marine Features (Australia) | Western Port, VIC: Marine Features (Australia) | Western Port, VIC</skos:scopeNote>
   </skos:Concept>
   <skos:Concept rdf:about="urn:aodn.org.au:geographicextents:concept:1081">
      <skos:prefLabel xml:lang="en">Marine Features (Australia) | Yorke Peninsula, SA</skos:prefLabel>
      <skos:inScheme rdf:resource="urn:aodn.org.au:geographicextents:conceptscheme:1.0"/>
      <gml:BoundedBy>
         <gml:Envelope gml:srsName="http://www.opengis.net/gml/srs/epsg.xml#epsg:4326">
            <gml:lowerCorner>136.82 -35.31</gml:lowerCorner>
            <gml:upperCorner>138.13 -34.08</gml:upperCorner>
         </gml:Envelope>
      </gml:BoundedBy>
      <skos:broader rdf:resource="urn:aodn.org.au:geographicextents:concept:10004"/>
      <skos:definition xml:lang="en">Marine Features (Australia) | Yorke Peninsula, SA</skos:definition>
      <skos:scopeNote xml:lang="en">Marine Features (Australia) | Yorke Peninsula, SA: Marine Features (Australia) | Yorke Peninsula, SA</skos:scopeNote>
   </skos:Concept>
   <skos:Concept rdf:about="urn:aodn.org.au:geographicextents:concept:50">
      <skos:prefLabel xml:lang="en">Marine Planning Regions (Australia) | Australian Antarctic</skos:prefLabel>
      <skos:inScheme rdf:resource="urn:aodn.org.au:geographicextents:conceptscheme:1.0"/>
      <gml:BoundedBy>
         <gml:Envelope gml:srsName="http://www.opengis.net/gml/srs/epsg.xml#epsg:4326">
            <gml:lowerCorner>45 -73</gml:lowerCorner>
            <gml:upperCorner>160 -60</gml:upperCorner>
         </gml:Envelope>
      </gml:BoundedBy>
      <skos:broader rdf:resource="urn:aodn.org.au:geographicextents:concept:10010"/>
      <skos:definition xml:lang="en">Marine Planning Regions (Australia) | Australian Antarctic</skos:definition>
      <skos:scopeNote xml:lang="en">Marine Planning Regions (Australia) | Australian Antarctic: Marine Planning Regions (Australia) | Australian Antarctic</skos:scopeNote>
   </skos:Concept>
   <skos:Concept rdf:about="urn:aodn.org.au:geographicextents:concept:51">
      <skos:prefLabel xml:lang="en">Marine Planning Regions (Australia) | East</skos:prefLabel>
      <skos:inScheme rdf:resource="urn:aodn.org.au:geographicextents:conceptscheme:1.0"/>
      <gml:BoundedBy>
         <gml:Envelope gml:srsName="http://www.opengis.net/gml/srs/epsg.xml#epsg:4326">
            <gml:lowerCorner>149.9 -37.3</gml:lowerCorner>
            <gml:upperCorner>158.3 -22.4</gml:upperCorner>
         </gml:Envelope>
      </gml:BoundedBy>
      <skos:broader rdf:resource="urn:aodn.org.au:geographicextents:concept:10010"/>
      <skos:definition xml:lang="en">Marine Planning Regions (Australia) | East</skos:definition>
      <skos:scopeNote xml:lang="en">Marine Planning Regions (Australia) | East: Marine Planning Regions (Australia) | East</skos:scopeNote>
   </skos:Concept>
   <skos:Concept rdf:about="urn:aodn.org.au:geographicextents:concept:52">
      <skos:prefLabel xml:lang="en">Marine Planning Regions (Australia) | Kerguelen</skos:prefLabel>
      <skos:inScheme rdf:resource="urn:aodn.org.au:geographicextents:conceptscheme:1.0"/>
      <gml:BoundedBy>
         <gml:Envelope gml:srsName="http://www.opengis.net/gml/srs/epsg.xml#epsg:4326">
            <gml:lowerCorner>67 -57</gml:lowerCorner>
            <gml:upperCorner>79 -48</gml:upperCorner>
         </gml:Envelope>
      </gml:BoundedBy>
      <skos:broader rdf:resource="urn:aodn.org.au:geographicextents:concept:10010"/>
      <skos:definition xml:lang="en">Marine Planning Regions (Australia) | Kerguelen</skos:definition>
      <skos:scopeNote xml:lang="en">Marine Planning Regions (Australia) | Kerguelen: Marine Planning Regions (Australia) | Kerguelen</skos:scopeNote>
   </skos:Concept>
   <skos:Concept rdf:about="urn:aodn.org.au:geographicextents:concept:53">
      <skos:prefLabel xml:lang="en">Marine Planning Regions (Australia) | Lord Howe</skos:prefLabel>
      <skos:inScheme rdf:resource="urn:aodn.org.au:geographicextents:conceptscheme:1.0"/>
      <gml:BoundedBy>
         <gml:Envelope gml:srsName="http://www.opengis.net/gml/srs/epsg.xml#epsg:4326">
            <gml:lowerCorner>158 -32</gml:lowerCorner>
            <gml:upperCorner>160 -31</gml:upperCorner>
         </gml:Envelope>
      </gml:BoundedBy>
      <skos:broader rdf:resource="urn:aodn.org.au:geographicextents:concept:10010"/>
      <skos:definition xml:lang="en">Marine Planning Regions (Australia) | Lord Howe</skos:definition>
      <skos:scopeNote xml:lang="en">Marine Planning Regions (Australia) | Lord Howe: Marine Planning Regions (Australia) | Lord Howe</skos:scopeNote>
   </skos:Concept>
   <skos:Concept rdf:about="urn:aodn.org.au:geographicextents:concept:54">
      <skos:prefLabel xml:lang="en">Marine Planning Regions (Australia) | Macquarie</skos:prefLabel>
      <skos:inScheme rdf:resource="urn:aodn.org.au:geographicextents:conceptscheme:1.0"/>
      <gml:BoundedBy>
         <gml:Envelope gml:srsName="http://www.opengis.net/gml/srs/epsg.xml#epsg:4326">
            <gml:lowerCorner>157 -55</gml:lowerCorner>
            <gml:upperCorner>160 -53</gml:upperCorner>
         </gml:Envelope>
      </gml:BoundedBy>
      <skos:broader rdf:resource="urn:aodn.org.au:geographicextents:concept:10010"/>
      <skos:definition xml:lang="en">Marine Planning Regions (Australia) | Macquarie</skos:definition>
      <skos:scopeNote xml:lang="en">Marine Planning Regions (Australia) | Macquarie: Marine Planning Regions (Australia) | Macquarie</skos:scopeNote>
   </skos:Concept>
   <skos:Concept rdf:about="urn:aodn.org.au:geographicextents:concept:139">
      <skos:prefLabel xml:lang="en">Named Locations (Antarctica) | Vincennes Bay</skos:prefLabel>
      <skos:inScheme rdf:resource="urn:aodn.org.au:geographicextents:conceptscheme:1.0"/>
      <gml:BoundedBy>
         <gml:Envelope gml:srsName="http://www.opengis.net/gml/srs/epsg.xml#epsg:4326">
            <gml:lowerCorner>107.26 -67.02</gml:lowerCorner>
            <gml:upperCorner>110.78 -66.18</gml:upperCorner>
         </gml:Envelope>
      </gml:BoundedBy>
      <skos:broader rdf:resource="urn:aodn.org.au:geographicextents:concept:10011"/>
      <skos:definition xml:lang="en">Named Locations (Antarctica) | Vincennes Bay</skos:definition>
      <skos:scopeNote xml:lang="en">Named Locations (Antarctica) | Vincennes Bay: Named Locations (Antarctica) | Vincennes Bay</skos:scopeNote>
   </skos:Concept>
   <skos:Concept rdf:about="urn:aodn.org.au:geographicextents:concept:55">
      <skos:prefLabel xml:lang="en">Marine Planning Regions (Australia) | Norfolk</skos:prefLabel>
      <skos:inScheme rdf:resource="urn:aodn.org.au:geographicextents:conceptscheme:1.0"/>
      <gml:BoundedBy>
         <gml:Envelope gml:srsName="http://www.opengis.net/gml/srs/epsg.xml#epsg:4326">
            <gml:lowerCorner>166 -31</gml:lowerCorner>
            <gml:upperCorner>169 -28</gml:upperCorner>
         </gml:Envelope>
      </gml:BoundedBy>
      <skos:broader rdf:resource="urn:aodn.org.au:geographicextents:concept:10010"/>
      <skos:definition xml:lang="en">Marine Planning Regions (Australia) | Norfolk</skos:definition>
      <skos:scopeNote xml:lang="en">Marine Planning Regions (Australia) | Norfolk: Marine Planning Regions (Australia) | Norfolk</skos:scopeNote>
   </skos:Concept>
   <skos:Concept rdf:about="urn:aodn.org.au:geographicextents:concept:57">
      <skos:prefLabel xml:lang="en">Marine Planning Regions (Australia) | North</skos:prefLabel>
      <skos:inScheme rdf:resource="urn:aodn.org.au:geographicextents:conceptscheme:1.0"/>
      <gml:BoundedBy>
         <gml:Envelope gml:srsName="http://www.opengis.net/gml/srs/epsg.xml#epsg:4326">
            <gml:lowerCorner>133 -18</gml:lowerCorner>
            <gml:upperCorner>145 -9</gml:upperCorner>
         </gml:Envelope>
      </gml:BoundedBy>
      <skos:broader rdf:resource="urn:aodn.org.au:geographicextents:concept:10010"/>
      <skos:definition xml:lang="en">Marine Planning Regions (Australia) | North</skos:definition>
      <skos:scopeNote xml:lang="en">Marine Planning Regions (Australia) | North: Marine Planning Regions (Australia) | North</skos:scopeNote>
   </skos:Concept>
   <skos:Concept rdf:about="urn:aodn.org.au:geographicextents:concept:58">
      <skos:prefLabel xml:lang="en">Marine Planning Regions (Australia) | North-east</skos:prefLabel>
      <skos:inScheme rdf:resource="urn:aodn.org.au:geographicextents:conceptscheme:1.0"/>
      <gml:BoundedBy>
         <gml:Envelope gml:srsName="http://www.opengis.net/gml/srs/epsg.xml#epsg:4326">
            <gml:lowerCorner>143 -26</gml:lowerCorner>
            <gml:upperCorner>163 -11</gml:upperCorner>
         </gml:Envelope>
      </gml:BoundedBy>
      <skos:broader rdf:resource="urn:aodn.org.au:geographicextents:concept:10010"/>
      <skos:definition xml:lang="en">Marine Planning Regions (Australia) | North-east</skos:definition>
      <skos:scopeNote xml:lang="en">Marine Planning Regions (Australia) | North-east: Marine Planning Regions (Australia) | North-east</skos:scopeNote>
   </skos:Concept>
   <skos:Concept rdf:about="urn:aodn.org.au:geographicextents:concept:59">
      <skos:prefLabel xml:lang="en">Marine Planning Regions (Australia) | North-west</skos:prefLabel>
      <skos:inScheme rdf:resource="urn:aodn.org.au:geographicextents:conceptscheme:1.0"/>
      <gml:BoundedBy>
         <gml:Envelope gml:srsName="http://www.opengis.net/gml/srs/epsg.xml#epsg:4326">
            <gml:lowerCorner>109 -23</gml:lowerCorner>
            <gml:upperCorner>127 -10</gml:upperCorner>
         </gml:Envelope>
      </gml:BoundedBy>
      <skos:broader rdf:resource="urn:aodn.org.au:geographicextents:concept:10010"/>
      <skos:definition xml:lang="en">Marine Planning Regions (Australia) | North-west</skos:definition>
      <skos:scopeNote xml:lang="en">Marine Planning Regions (Australia) | North-west: Marine Planning Regions (Australia) | North-west</skos:scopeNote>
   </skos:Concept>
   <skos:Concept rdf:about="urn:aodn.org.au:geographicextents:concept:60">
      <skos:prefLabel xml:lang="en">Marine Planning Regions (Australia) | South-east</skos:prefLabel>
      <skos:inScheme rdf:resource="urn:aodn.org.au:geographicextents:conceptscheme:1.0"/>
      <gml:BoundedBy>
         <gml:Envelope gml:srsName="http://www.opengis.net/gml/srs/epsg.xml#epsg:4326">
            <gml:lowerCorner>133 -48</gml:lowerCorner>
            <gml:upperCorner>155 -35</gml:upperCorner>
         </gml:Envelope>
      </gml:BoundedBy>
      <skos:broader rdf:resource="urn:aodn.org.au:geographicextents:concept:10010"/>
      <skos:definition xml:lang="en">Marine Planning Regions (Australia) | South-east</skos:definition>
      <skos:scopeNote xml:lang="en">Marine Planning Regions (Australia) | South-east: Marine Planning Regions (Australia) | South-east</skos:scopeNote>
   </skos:Concept>
   <skos:Concept rdf:about="urn:aodn.org.au:geographicextents:concept:61">
      <skos:prefLabel xml:lang="en">Marine Planning Regions (Australia) | South-west</skos:prefLabel>
      <skos:inScheme rdf:resource="urn:aodn.org.au:geographicextents:conceptscheme:1.0"/>
      <gml:BoundedBy>
         <gml:Envelope gml:srsName="http://www.opengis.net/gml/srs/epsg.xml#epsg:4326">
            <gml:lowerCorner>113 -38</gml:lowerCorner>
            <gml:upperCorner>138 -31</gml:upperCorner>
         </gml:Envelope>
      </gml:BoundedBy>
      <skos:broader rdf:resource="urn:aodn.org.au:geographicextents:concept:10010"/>
      <skos:definition xml:lang="en">Marine Planning Regions (Australia) | South-west</skos:definition>
      <skos:scopeNote xml:lang="en">Marine Planning Regions (Australia) | South-west: Marine Planning Regions (Australia) | South-west</skos:scopeNote>
   </skos:Concept>
   <skos:Concept rdf:about="urn:aodn.org.au:geographicextents:concept:62">
      <skos:prefLabel xml:lang="en">Marine Planning Regions (Australia) | Sunda</skos:prefLabel>
      <skos:inScheme rdf:resource="urn:aodn.org.au:geographicextents:conceptscheme:1.0"/>
      <gml:BoundedBy>
         <gml:Envelope gml:srsName="http://www.opengis.net/gml/srs/epsg.xml#epsg:4326">
            <gml:lowerCorner>95 -14</gml:lowerCorner>
            <gml:upperCorner>107 -9</gml:upperCorner>
         </gml:Envelope>
      </gml:BoundedBy>
      <skos:broader rdf:resource="urn:aodn.org.au:geographicextents:concept:10010"/>
      <skos:definition xml:lang="en">Marine Planning Regions (Australia) | Sunda</skos:definition>
      <skos:scopeNote xml:lang="en">Marine Planning Regions (Australia) | Sunda: Marine Planning Regions (Australia) | Sunda</skos:scopeNote>
   </skos:Concept>
   <skos:Concept rdf:about="urn:aodn.org.au:geographicextents:concept:63">
      <skos:prefLabel xml:lang="en">Marine Planning Regions (Australia) | Western-central</skos:prefLabel>
      <skos:inScheme rdf:resource="urn:aodn.org.au:geographicextents:conceptscheme:1.0"/>
      <gml:BoundedBy>
         <gml:Envelope gml:srsName="http://www.opengis.net/gml/srs/epsg.xml#epsg:4326">
            <gml:lowerCorner>109 -34</gml:lowerCorner>
            <gml:upperCorner>116 -21</gml:upperCorner>
         </gml:Envelope>
      </gml:BoundedBy>
      <skos:broader rdf:resource="urn:aodn.org.au:geographicextents:concept:10010"/>
      <skos:definition xml:lang="en">Marine Planning Regions (Australia) | Western-central</skos:definition>
      <skos:scopeNote xml:lang="en">Marine Planning Regions (Australia) | Western-central: Marine Planning Regions (Australia) | Western-central</skos:scopeNote>
   </skos:Concept>
   <skos:Concept rdf:about="urn:aodn.org.au:geographicextents:concept:1082">
      <skos:prefLabel xml:lang="en">Named Locations (Antarctica) | Amanda Bay</skos:prefLabel>
      <skos:inScheme rdf:resource="urn:aodn.org.au:geographicextents:conceptscheme:1.0"/>
      <gml:BoundedBy>
         <gml:Envelope gml:srsName="http://www.opengis.net/gml/srs/epsg.xml#epsg:4326">
            <gml:lowerCorner>73 -70</gml:lowerCorner>
            <gml:upperCorner>78 -68</gml:upperCorner>
         </gml:Envelope>
      </gml:BoundedBy>
      <skos:broader rdf:resource="urn:aodn.org.au:geographicextents:concept:10011"/>
      <skos:definition xml:lang="en">Named Locations (Antarctica) | Amanda Bay</skos:definition>
      <skos:scopeNote xml:lang="en">Named Locations (Antarctica) | Amanda Bay: Named Locations (Antarctica) | Amanda Bay</skos:scopeNote>
   </skos:Concept>
   <skos:Concept rdf:about="urn:aodn.org.au:geographicextents:concept:129">
      <skos:prefLabel xml:lang="en">Named Locations (Antarctica) | Amery Ice Shelf</skos:prefLabel>
      <skos:inScheme rdf:resource="urn:aodn.org.au:geographicextents:conceptscheme:1.0"/>
      <gml:BoundedBy>
         <gml:Envelope gml:srsName="http://www.opengis.net/gml/srs/epsg.xml#epsg:4326">
            <gml:lowerCorner>59 -73</gml:lowerCorner>
            <gml:upperCorner>81 -65</gml:upperCorner>
         </gml:Envelope>
      </gml:BoundedBy>
      <skos:broader rdf:resource="urn:aodn.org.au:geographicextents:concept:10011"/>
      <skos:definition xml:lang="en">Named Locations (Antarctica) | Amery Ice Shelf</skos:definition>
      <skos:scopeNote xml:lang="en">Named Locations (Antarctica) | Amery Ice Shelf: Named Locations (Antarctica) | Amery Ice Shelf</skos:scopeNote>
   </skos:Concept>
   <skos:Concept rdf:about="urn:aodn.org.au:geographicextents:concept:1083">
      <skos:prefLabel xml:lang="en">Named Locations (Antarctica) | Amery Oasis</skos:prefLabel>
      <skos:inScheme rdf:resource="urn:aodn.org.au:geographicextents:conceptscheme:1.0"/>
      <gml:BoundedBy>
         <gml:Envelope gml:srsName="http://www.opengis.net/gml/srs/epsg.xml#epsg:4326">
            <gml:lowerCorner>67 -72</gml:lowerCorner>
            <gml:upperCorner>74 -68</gml:upperCorner>
         </gml:Envelope>
      </gml:BoundedBy>
      <skos:broader rdf:resource="urn:aodn.org.au:geographicextents:concept:10011"/>
      <skos:definition xml:lang="en">Named Locations (Antarctica) | Amery Oasis</skos:definition>
      <skos:scopeNote xml:lang="en">Named Locations (Antarctica) | Amery Oasis: Named Locations (Antarctica) | Amery Oasis</skos:scopeNote>
   </skos:Concept>
   <skos:Concept rdf:about="urn:aodn.org.au:geographicextents:concept:1084">
      <skos:prefLabel xml:lang="en">Named Locations (Antarctica) | Antarctic Peninsula</skos:prefLabel>
      <skos:inScheme rdf:resource="urn:aodn.org.au:geographicextents:conceptscheme:1.0"/>
      <gml:BoundedBy>
         <gml:Envelope gml:srsName="http://www.opengis.net/gml/srs/epsg.xml#epsg:4326">
            <gml:lowerCorner>-80 -63</gml:lowerCorner>
            <gml:upperCorner>-52 -75</gml:upperCorner>
         </gml:Envelope>
      </gml:BoundedBy>
      <skos:broader rdf:resource="urn:aodn.org.au:geographicextents:concept:10011"/>
      <skos:definition xml:lang="en">Named Locations (Antarctica) | Antarctic Peninsula</skos:definition>
      <skos:scopeNote xml:lang="en">Named Locations (Antarctica) | Antarctic Peninsula: Named Locations (Antarctica) | Antarctic Peninsula</skos:scopeNote>
   </skos:Concept>
   <skos:Concept rdf:about="urn:aodn.org.au:geographicextents:concept:1085">
      <skos:prefLabel xml:lang="en">Named Locations (Antarctica) | Ardery Island</skos:prefLabel>
      <skos:inScheme rdf:resource="urn:aodn.org.au:geographicextents:conceptscheme:1.0"/>
      <gml:BoundedBy>
         <gml:Envelope gml:srsName="http://www.opengis.net/gml/srs/epsg.xml#epsg:4326">
            <gml:lowerCorner>110.44 -66.38</gml:lowerCorner>
            <gml:upperCorner>110.47 -66.36</gml:upperCorner>
         </gml:Envelope>
      </gml:BoundedBy>
      <skos:broader rdf:resource="urn:aodn.org.au:geographicextents:concept:10011"/>
      <skos:definition xml:lang="en">Named Locations (Antarctica) | Ardery Island</skos:definition>
      <skos:scopeNote xml:lang="en">Named Locations (Antarctica) | Ardery Island: Named Locations (Antarctica) | Ardery Island</skos:scopeNote>
   </skos:Concept>
   <skos:Concept rdf:about="urn:aodn.org.au:geographicextents:concept:1086">
      <skos:prefLabel xml:lang="en">Named Locations (Antarctica) | Auster Glacier</skos:prefLabel>
      <skos:inScheme rdf:resource="urn:aodn.org.au:geographicextents:conceptscheme:1.0"/>
      <gml:BoundedBy>
         <gml:Envelope gml:srsName="http://www.opengis.net/gml/srs/epsg.xml#epsg:4326">
            <gml:lowerCorner>47.79 -70.83</gml:lowerCorner>
            <gml:upperCorner>56.9 -65.41</gml:upperCorner>
         </gml:Envelope>
      </gml:BoundedBy>
      <skos:broader rdf:resource="urn:aodn.org.au:geographicextents:concept:10011"/>
      <skos:definition xml:lang="en">Named Locations (Antarctica) | Auster Glacier</skos:definition>
      <skos:scopeNote xml:lang="en">Named Locations (Antarctica) | Auster Glacier: Named Locations (Antarctica) | Auster Glacier</skos:scopeNote>
   </skos:Concept>
   <skos:Concept rdf:about="urn:aodn.org.au:geographicextents:concept:1088">
      <skos:prefLabel xml:lang="en">Named Locations (Antarctica) | Beall Island</skos:prefLabel>
      <skos:inScheme rdf:resource="urn:aodn.org.au:geographicextents:conceptscheme:1.0"/>
      <gml:BoundedBy>
         <gml:Envelope gml:srsName="http://www.opengis.net/gml/srs/epsg.xml#epsg:4326">
            <gml:lowerCorner>110.45 -66.32</gml:lowerCorner>
            <gml:upperCorner>110.5 -66.29</gml:upperCorner>
         </gml:Envelope>
      </gml:BoundedBy>
      <skos:broader rdf:resource="urn:aodn.org.au:geographicextents:concept:10011"/>
      <skos:definition xml:lang="en">Named Locations (Antarctica) | Beall Island</skos:definition>
      <skos:scopeNote xml:lang="en">Named Locations (Antarctica) | Beall Island: Named Locations (Antarctica) | Beall Island</skos:scopeNote>
   </skos:Concept>
   <skos:Concept rdf:about="urn:aodn.org.au:geographicextents:concept:1089">
      <skos:prefLabel xml:lang="en">Named Locations (Antarctica) | Beaver Lake</skos:prefLabel>
      <skos:inScheme rdf:resource="urn:aodn.org.au:geographicextents:conceptscheme:1.0"/>
      <gml:BoundedBy>
         <gml:Envelope gml:srsName="http://www.opengis.net/gml/srs/epsg.xml#epsg:4326">
            <gml:lowerCorner>68.1 -70.85</gml:lowerCorner>
            <gml:upperCorner>68.55 -70.72</gml:upperCorner>
         </gml:Envelope>
      </gml:BoundedBy>
      <skos:broader rdf:resource="urn:aodn.org.au:geographicextents:concept:10011"/>
      <skos:definition xml:lang="en">Named Locations (Antarctica) | Beaver Lake</skos:definition>
      <skos:scopeNote xml:lang="en">Named Locations (Antarctica) | Beaver Lake: Named Locations (Antarctica) | Beaver Lake</skos:scopeNote>
   </skos:Concept>
   <skos:Concept rdf:about="urn:aodn.org.au:geographicextents:concept:1090">
      <skos:prefLabel xml:lang="en">Named Locations (Antarctica) | Bechervaise Island</skos:prefLabel>
      <skos:inScheme rdf:resource="urn:aodn.org.au:geographicextents:conceptscheme:1.0"/>
      <gml:BoundedBy>
         <gml:Envelope gml:srsName="http://www.opengis.net/gml/srs/epsg.xml#epsg:4326">
            <gml:lowerCorner>62.8 -67.59</gml:lowerCorner>
            <gml:upperCorner>62.85 -67.57</gml:upperCorner>
         </gml:Envelope>
      </gml:BoundedBy>
      <skos:broader rdf:resource="urn:aodn.org.au:geographicextents:concept:10011"/>
      <skos:definition xml:lang="en">Named Locations (Antarctica) | Bechervaise Island</skos:definition>
      <skos:scopeNote xml:lang="en">Named Locations (Antarctica) | Bechervaise Island: Named Locations (Antarctica) | Bechervaise Island</skos:scopeNote>
   </skos:Concept>
   <skos:Concept rdf:about="urn:aodn.org.au:geographicextents:concept:1091">
      <skos:prefLabel xml:lang="en">Named Locations (Antarctica) | Bluff Island</skos:prefLabel>
      <skos:inScheme rdf:resource="urn:aodn.org.au:geographicextents:conceptscheme:1.0"/>
      <gml:BoundedBy>
         <gml:Envelope gml:srsName="http://www.opengis.net/gml/srs/epsg.xml#epsg:4326">
            <gml:lowerCorner>77.88 -68.56</gml:lowerCorner>
            <gml:upperCorner>77.93 -68.54</gml:upperCorner>
         </gml:Envelope>
      </gml:BoundedBy>
      <skos:broader rdf:resource="urn:aodn.org.au:geographicextents:concept:10011"/>
      <skos:definition xml:lang="en">Named Locations (Antarctica) | Bluff Island</skos:definition>
      <skos:scopeNote xml:lang="en">Named Locations (Antarctica) | Bluff Island: Named Locations (Antarctica) | Bluff Island</skos:scopeNote>
   </skos:Concept>
   <skos:Concept rdf:about="urn:aodn.org.au:geographicextents:concept:1092">
      <skos:prefLabel xml:lang="en">Named Locations (Antarctica) | Bolingen Islands</skos:prefLabel>
      <skos:inScheme rdf:resource="urn:aodn.org.au:geographicextents:conceptscheme:1.0"/>
      <gml:BoundedBy>
         <gml:Envelope gml:srsName="http://www.opengis.net/gml/srs/epsg.xml#epsg:4326">
            <gml:lowerCorner>75.7 -69.48</gml:lowerCorner>
            <gml:upperCorner>75.82 -69.44</gml:upperCorner>
         </gml:Envelope>
      </gml:BoundedBy>
      <skos:broader rdf:resource="urn:aodn.org.au:geographicextents:concept:10011"/>
      <skos:definition xml:lang="en">Named Locations (Antarctica) | Bolingen Islands</skos:definition>
      <skos:scopeNote xml:lang="en">Named Locations (Antarctica) | Bolingen Islands: Named Locations (Antarctica) | Bolingen Islands</skos:scopeNote>
   </skos:Concept>
   <skos:Concept rdf:about="urn:aodn.org.au:geographicextents:concept:1093">
      <skos:prefLabel xml:lang="en">Named Locations (Antarctica) | Brattstrand Bluff</skos:prefLabel>
      <skos:inScheme rdf:resource="urn:aodn.org.au:geographicextents:conceptscheme:1.0"/>
      <gml:BoundedBy>
         <gml:Envelope gml:srsName="http://www.opengis.net/gml/srs/epsg.xml#epsg:4326">
            <gml:lowerCorner>76.98 -69.23</gml:lowerCorner>
            <gml:upperCorner>77.05 -69.2</gml:upperCorner>
         </gml:Envelope>
      </gml:BoundedBy>
      <skos:broader rdf:resource="urn:aodn.org.au:geographicextents:concept:10011"/>
      <skos:definition xml:lang="en">Named Locations (Antarctica) | Brattstrand Bluff</skos:definition>
      <skos:scopeNote xml:lang="en">Named Locations (Antarctica) | Brattstrand Bluff: Named Locations (Antarctica) | Brattstrand Bluff</skos:scopeNote>
   </skos:Concept>
   <skos:Concept rdf:about="urn:aodn.org.au:geographicextents:concept:1094">
      <skos:prefLabel xml:lang="en">Named Locations (Antarctica) | Brown Bay</skos:prefLabel>
      <skos:inScheme rdf:resource="urn:aodn.org.au:geographicextents:conceptscheme:1.0"/>
      <gml:BoundedBy>
         <gml:Envelope gml:srsName="http://www.opengis.net/gml/srs/epsg.xml#epsg:4326">
            <gml:lowerCorner>110.5 -66.29</gml:lowerCorner>
            <gml:upperCorner>110.6 -66.25</gml:upperCorner>
         </gml:Envelope>
      </gml:BoundedBy>
      <skos:broader rdf:resource="urn:aodn.org.au:geographicextents:concept:10011"/>
      <skos:definition xml:lang="en">Named Locations (Antarctica) | Brown Bay</skos:definition>
      <skos:scopeNote xml:lang="en">Named Locations (Antarctica) | Brown Bay: Named Locations (Antarctica) | Brown Bay</skos:scopeNote>
   </skos:Concept>
   <skos:Concept rdf:about="urn:aodn.org.au:geographicextents:concept:1095">
      <skos:prefLabel xml:lang="en">Named Locations (Antarctica) | Bunger Hills</skos:prefLabel>
      <skos:inScheme rdf:resource="urn:aodn.org.au:geographicextents:conceptscheme:1.0"/>
      <gml:BoundedBy>
         <gml:Envelope gml:srsName="http://www.opengis.net/gml/srs/epsg.xml#epsg:4326">
            <gml:lowerCorner>100.2 -66.68</gml:lowerCorner>
            <gml:upperCorner>102.1 -65.9</gml:upperCorner>
         </gml:Envelope>
      </gml:BoundedBy>
      <skos:broader rdf:resource="urn:aodn.org.au:geographicextents:concept:10011"/>
      <skos:definition xml:lang="en">Named Locations (Antarctica) | Bunger Hills</skos:definition>
      <skos:scopeNote xml:lang="en">Named Locations (Antarctica) | Bunger Hills: Named Locations (Antarctica) | Bunger Hills</skos:scopeNote>
   </skos:Concept>
   <skos:Concept rdf:about="urn:aodn.org.au:geographicextents:concept:1096">
      <skos:prefLabel xml:lang="en">Named Locations (Antarctica) | Cape Denison</skos:prefLabel>
      <skos:inScheme rdf:resource="urn:aodn.org.au:geographicextents:conceptscheme:1.0"/>
      <gml:BoundedBy>
         <gml:Envelope gml:srsName="http://www.opengis.net/gml/srs/epsg.xml#epsg:4326">
            <gml:lowerCorner>142.65 -67.02</gml:lowerCorner>
            <gml:upperCorner>142.7 -67</gml:upperCorner>
         </gml:Envelope>
      </gml:BoundedBy>
      <skos:broader rdf:resource="urn:aodn.org.au:geographicextents:concept:10011"/>
      <skos:definition xml:lang="en">Named Locations (Antarctica) | Cape Denison</skos:definition>
      <skos:scopeNote xml:lang="en">Named Locations (Antarctica) | Cape Denison: Named Locations (Antarctica) | Cape Denison</skos:scopeNote>
   </skos:Concept>
   <skos:Concept rdf:about="urn:aodn.org.au:geographicextents:concept:1097">
      <skos:prefLabel xml:lang="en">Named Locations (Antarctica) | Cape Hallett</skos:prefLabel>
      <skos:inScheme rdf:resource="urn:aodn.org.au:geographicextents:conceptscheme:1.0"/>
      <gml:BoundedBy>
         <gml:Envelope gml:srsName="http://www.opengis.net/gml/srs/epsg.xml#epsg:4326">
            <gml:lowerCorner>170 -72.5</gml:lowerCorner>
            <gml:upperCorner>170.5 -72.3</gml:upperCorner>
         </gml:Envelope>
      </gml:BoundedBy>
      <skos:broader rdf:resource="urn:aodn.org.au:geographicextents:concept:10011"/>
      <skos:definition xml:lang="en">Named Locations (Antarctica) | Cape Hallett</skos:definition>
      <skos:scopeNote xml:lang="en">Named Locations (Antarctica) | Cape Hallett: Named Locations (Antarctica) | Cape Hallett</skos:scopeNote>
   </skos:Concept>
   <skos:Concept rdf:about="urn:aodn.org.au:geographicextents:concept:130">
      <skos:prefLabel xml:lang="en">Named Locations (Antarctica) | Casey Station (Australia)</skos:prefLabel>
      <skos:inScheme rdf:resource="urn:aodn.org.au:geographicextents:conceptscheme:1.0"/>
      <gml:BoundedBy>
         <gml:Envelope gml:srsName="http://www.opengis.net/gml/srs/epsg.xml#epsg:4326">
            <gml:lowerCorner>110.51 -66.29</gml:lowerCorner>
            <gml:upperCorner>110.28 -66.28</gml:upperCorner>
         </gml:Envelope>
      </gml:BoundedBy>
      <skos:broader rdf:resource="urn:aodn.org.au:geographicextents:concept:10011"/>
      <skos:definition xml:lang="en">Named Locations (Antarctica) | Casey Station (Australia)</skos:definition>
      <skos:scopeNote xml:lang="en">Named Locations (Antarctica) | Casey Station (Australia): Named Locations (Antarctica) | Casey Station (Australia)</skos:scopeNote>
   </skos:Concept>
   <skos:Concept rdf:about="urn:aodn.org.au:geographicextents:concept:1098">
      <skos:prefLabel xml:lang="en">Named Locations (Antarctica) | Casey Wharf</skos:prefLabel>
      <skos:inScheme rdf:resource="urn:aodn.org.au:geographicextents:conceptscheme:1.0"/>
      <gml:BoundedBy>
         <gml:Envelope gml:srsName="http://www.opengis.net/gml/srs/epsg.xml#epsg:4326">
            <gml:lowerCorner>110.53 -66.28</gml:lowerCorner>
            <gml:upperCorner>110.55 -66.27</gml:upperCorner>
         </gml:Envelope>
      </gml:BoundedBy>
      <skos:broader rdf:resource="urn:aodn.org.au:geographicextents:concept:10011"/>
      <skos:definition xml:lang="en">Named Locations (Antarctica) | Casey Wharf</skos:definition>
      <skos:scopeNote xml:lang="en">Named Locations (Antarctica) | Casey Wharf: Named Locations (Antarctica) | Casey Wharf</skos:scopeNote>
   </skos:Concept>
   <skos:Concept rdf:about="urn:aodn.org.au:geographicextents:concept:1099">
      <skos:prefLabel xml:lang="en">Named Locations (Antarctica) | Commonwealth Bay</skos:prefLabel>
      <skos:inScheme rdf:resource="urn:aodn.org.au:geographicextents:conceptscheme:1.0"/>
      <gml:BoundedBy>
         <gml:Envelope gml:srsName="http://www.opengis.net/gml/srs/epsg.xml#epsg:4326">
            <gml:lowerCorner>142.1 -67.04</gml:lowerCorner>
            <gml:upperCorner>143.45 -66.8</gml:upperCorner>
         </gml:Envelope>
      </gml:BoundedBy>
      <skos:broader rdf:resource="urn:aodn.org.au:geographicextents:concept:10011"/>
      <skos:definition xml:lang="en">Named Locations (Antarctica) | Commonwealth Bay</skos:definition>
      <skos:scopeNote xml:lang="en">Named Locations (Antarctica) | Commonwealth Bay: Named Locations (Antarctica) | Commonwealth Bay</skos:scopeNote>
   </skos:Concept>
   <skos:Concept rdf:about="urn:aodn.org.au:geographicextents:concept:131">
      <skos:prefLabel xml:lang="en">Named Locations (Antarctica) | Cook Ice Shelf</skos:prefLabel>
      <skos:inScheme rdf:resource="urn:aodn.org.au:geographicextents:conceptscheme:1.0"/>
      <gml:BoundedBy>
         <gml:Envelope gml:srsName="http://www.opengis.net/gml/srs/epsg.xml#epsg:4326">
            <gml:lowerCorner>150.88 -68.94</gml:lowerCorner>
            <gml:upperCorner>154.04 -68.22</gml:upperCorner>
         </gml:Envelope>
      </gml:BoundedBy>
      <skos:broader rdf:resource="urn:aodn.org.au:geographicextents:concept:10011"/>
      <skos:definition xml:lang="en">Named Locations (Antarctica) | Cook Ice Shelf</skos:definition>
      <skos:scopeNote xml:lang="en">Named Locations (Antarctica) | Cook Ice Shelf: Named Locations (Antarctica) | Cook Ice Shelf</skos:scopeNote>
   </skos:Concept>
   <skos:Concept rdf:about="urn:aodn.org.au:geographicextents:concept:132">
      <skos:prefLabel xml:lang="en">Named Locations (Antarctica) | Davis Sea</skos:prefLabel>
      <skos:inScheme rdf:resource="urn:aodn.org.au:geographicextents:conceptscheme:1.0"/>
      <gml:BoundedBy>
         <gml:Envelope gml:srsName="http://www.opengis.net/gml/srs/epsg.xml#epsg:4326">
            <gml:lowerCorner>90.35 -66.71</gml:lowerCorner>
            <gml:upperCorner>95.63 -65.06</gml:upperCorner>
         </gml:Envelope>
      </gml:BoundedBy>
      <skos:broader rdf:resource="urn:aodn.org.au:geographicextents:concept:10011"/>
      <skos:definition xml:lang="en">Named Locations (Antarctica) | Davis Sea</skos:definition>
      <skos:scopeNote xml:lang="en">Named Locations (Antarctica) | Davis Sea: Named Locations (Antarctica) | Davis Sea</skos:scopeNote>
   </skos:Concept>
   <skos:Concept rdf:about="urn:aodn.org.au:geographicextents:concept:133">
      <skos:prefLabel xml:lang="en">Named Locations (Antarctica) | Davis Station (Australia)</skos:prefLabel>
      <skos:inScheme rdf:resource="urn:aodn.org.au:geographicextents:conceptscheme:1.0"/>
      <gml:BoundedBy>
         <gml:Envelope gml:srsName="http://www.opengis.net/gml/srs/epsg.xml#epsg:4326">
            <gml:lowerCorner>77.96 -68.58</gml:lowerCorner>
            <gml:upperCorner>77.98 -68.57</gml:upperCorner>
         </gml:Envelope>
      </gml:BoundedBy>
      <skos:broader rdf:resource="urn:aodn.org.au:geographicextents:concept:10011"/>
      <skos:definition xml:lang="en">Named Locations (Antarctica) | Davis Station (Australia)</skos:definition>
      <skos:scopeNote xml:lang="en">Named Locations (Antarctica) | Davis Station (Australia): Named Locations (Antarctica) | Davis Station (Australia)</skos:scopeNote>
   </skos:Concept>
   <skos:Concept rdf:about="urn:aodn.org.au:geographicextents:concept:1100">
      <skos:prefLabel xml:lang="en">Named Locations (Antarctica) | Dry Valleys</skos:prefLabel>
      <skos:inScheme rdf:resource="urn:aodn.org.au:geographicextents:conceptscheme:1.0"/>
      <gml:BoundedBy>
         <gml:Envelope gml:srsName="http://www.opengis.net/gml/srs/epsg.xml#epsg:4326">
            <gml:lowerCorner>161 -77.8</gml:lowerCorner>
            <gml:upperCorner>164 -77.2</gml:upperCorner>
         </gml:Envelope>
      </gml:BoundedBy>
      <skos:broader rdf:resource="urn:aodn.org.au:geographicextents:concept:10011"/>
      <skos:definition xml:lang="en">Named Locations (Antarctica) | Dry Valleys</skos:definition>
      <skos:scopeNote xml:lang="en">Named Locations (Antarctica) | Dry Valleys: Named Locations (Antarctica) | Dry Valleys</skos:scopeNote>
   </skos:Concept>
   <skos:Concept rdf:about="urn:aodn.org.au:geographicextents:concept:134">
      <skos:prefLabel xml:lang="en">Named Locations (Antarctica) | Dumont D'Urville Sea (France)</skos:prefLabel>
      <skos:inScheme rdf:resource="urn:aodn.org.au:geographicextents:conceptscheme:1.0"/>
      <gml:BoundedBy>
         <gml:Envelope gml:srsName="http://www.opengis.net/gml/srs/epsg.xml#epsg:4326">
            <gml:lowerCorner>134 -68</gml:lowerCorner>
            <gml:upperCorner>146 -65</gml:upperCorner>
         </gml:Envelope>
      </gml:BoundedBy>
      <skos:broader rdf:resource="urn:aodn.org.au:geographicextents:concept:10011"/>
      <skos:definition xml:lang="en">Named Locations (Antarctica) | Dumont D'Urville Sea (France)</skos:definition>
      <skos:scopeNote xml:lang="en">Named Locations (Antarctica) | Dumont D'Urville Sea (France): Named Locations (Antarctica) | Dumont D'Urville Sea (France)</skos:scopeNote>
   </skos:Concept>
   <skos:Concept rdf:about="urn:aodn.org.au:geographicextents:concept:1101">
      <skos:prefLabel xml:lang="en">Named Locations (Antarctica) | East Antarctica</skos:prefLabel>
      <skos:inScheme rdf:resource="urn:aodn.org.au:geographicextents:conceptscheme:1.0"/>
      <gml:BoundedBy>
         <gml:Envelope gml:srsName="http://www.opengis.net/gml/srs/epsg.xml#epsg:4326">
            <gml:lowerCorner>170 -90</gml:lowerCorner>
            <gml:upperCorner>-40 -65</gml:upperCorner>
         </gml:Envelope>
      </gml:BoundedBy>
      <skos:broader rdf:resource="urn:aodn.org.au:geographicextents:concept:10011"/>
      <skos:definition xml:lang="en">Named Locations (Antarctica) | East Antarctica</skos:definition>
      <skos:scopeNote xml:lang="en">Named Locations (Antarctica) | East Antarctica: Named Locations (Antarctica) | East Antarctica</skos:scopeNote>
   </skos:Concept>
   <skos:Concept rdf:about="urn:aodn.org.au:geographicextents:concept:1102">
      <skos:prefLabel xml:lang="en">Named Locations (Antarctica) | Edmonson Point</skos:prefLabel>
      <skos:inScheme rdf:resource="urn:aodn.org.au:geographicextents:conceptscheme:1.0"/>
      <gml:BoundedBy>
         <gml:Envelope gml:srsName="http://www.opengis.net/gml/srs/epsg.xml#epsg:4326">
            <gml:lowerCorner>165.08 -74.34</gml:lowerCorner>
            <gml:upperCorner>165.15 -74.32</gml:upperCorner>
         </gml:Envelope>
      </gml:BoundedBy>
      <skos:broader rdf:resource="urn:aodn.org.au:geographicextents:concept:10011"/>
      <skos:definition xml:lang="en">Named Locations (Antarctica) | Edmonson Point</skos:definition>
      <skos:scopeNote xml:lang="en">Named Locations (Antarctica) | Edmonson Point: Named Locations (Antarctica) | Edmonson Point</skos:scopeNote>
   </skos:Concept>
   <skos:Concept rdf:about="urn:aodn.org.au:geographicextents:concept:1103">
      <skos:prefLabel xml:lang="en">Named Locations (Antarctica) | Ellis Fjord</skos:prefLabel>
      <skos:inScheme rdf:resource="urn:aodn.org.au:geographicextents:conceptscheme:1.0"/>
      <gml:BoundedBy>
         <gml:Envelope gml:srsName="http://www.opengis.net/gml/srs/epsg.xml#epsg:4326">
            <gml:lowerCorner>77.95 -68.63</gml:lowerCorner>
            <gml:upperCorner>78.22 -68.58</gml:upperCorner>
         </gml:Envelope>
      </gml:BoundedBy>
      <skos:broader rdf:resource="urn:aodn.org.au:geographicextents:concept:10011"/>
      <skos:definition xml:lang="en">Named Locations (Antarctica) | Ellis Fjord</skos:definition>
      <skos:scopeNote xml:lang="en">Named Locations (Antarctica) | Ellis Fjord: Named Locations (Antarctica) | Ellis Fjord</skos:scopeNote>
   </skos:Concept>
   <skos:Concept rdf:about="urn:aodn.org.au:geographicextents:concept:1104">
      <skos:prefLabel xml:lang="en">Named Locations (Antarctica) | Filla Island</skos:prefLabel>
      <skos:inScheme rdf:resource="urn:aodn.org.au:geographicextents:conceptscheme:1.0"/>
      <gml:BoundedBy>
         <gml:Envelope gml:srsName="http://www.opengis.net/gml/srs/epsg.xml#epsg:4326">
            <gml:lowerCorner>77.59 -68.87</gml:lowerCorner>
            <gml:upperCorner>78.02 -68.76</gml:upperCorner>
         </gml:Envelope>
      </gml:BoundedBy>
      <skos:broader rdf:resource="urn:aodn.org.au:geographicextents:concept:10011"/>
      <skos:definition xml:lang="en">Named Locations (Antarctica) | Filla Island</skos:definition>
      <skos:scopeNote xml:lang="en">Named Locations (Antarctica) | Filla Island: Named Locations (Antarctica) | Filla Island</skos:scopeNote>
   </skos:Concept>
   <skos:Concept rdf:about="urn:aodn.org.au:geographicextents:concept:1105">
      <skos:prefLabel xml:lang="en">Named Locations (Antarctica) | Gaussberg</skos:prefLabel>
      <skos:inScheme rdf:resource="urn:aodn.org.au:geographicextents:conceptscheme:1.0"/>
      <gml:BoundedBy>
         <gml:Envelope gml:srsName="http://www.opengis.net/gml/srs/epsg.xml#epsg:4326">
            <gml:lowerCorner>89.1 -66.85</gml:lowerCorner>
            <gml:upperCorner>89.26 -66.79</gml:upperCorner>
         </gml:Envelope>
      </gml:BoundedBy>
      <skos:broader rdf:resource="urn:aodn.org.au:geographicextents:concept:10011"/>
      <skos:definition xml:lang="en">Named Locations (Antarctica) | Gaussberg</skos:definition>
      <skos:scopeNote xml:lang="en">Named Locations (Antarctica) | Gaussberg: Named Locations (Antarctica) | Gaussberg</skos:scopeNote>
   </skos:Concept>
   <skos:Concept rdf:about="urn:aodn.org.au:geographicextents:concept:1107">
      <skos:prefLabel xml:lang="en">Named Locations (Antarctica) | George V Land</skos:prefLabel>
      <skos:inScheme rdf:resource="urn:aodn.org.au:geographicextents:conceptscheme:1.0"/>
      <gml:BoundedBy>
         <gml:Envelope gml:srsName="http://www.opengis.net/gml/srs/epsg.xml#epsg:4326">
            <gml:lowerCorner>142.03 -90</gml:lowerCorner>
            <gml:upperCorner>153.75 -60</gml:upperCorner>
         </gml:Envelope>
      </gml:BoundedBy>
      <skos:broader rdf:resource="urn:aodn.org.au:geographicextents:concept:10011"/>
      <skos:definition xml:lang="en">Named Locations (Antarctica) | George V Land</skos:definition>
      <skos:scopeNote xml:lang="en">Named Locations (Antarctica) | George V Land: Named Locations (Antarctica) | George V Land</skos:scopeNote>
   </skos:Concept>
   <skos:Concept rdf:about="urn:aodn.org.au:geographicextents:concept:1108">
      <skos:prefLabel xml:lang="en">Named Locations (Antarctica) | Grove Mountains</skos:prefLabel>
      <skos:inScheme rdf:resource="urn:aodn.org.au:geographicextents:conceptscheme:1.0"/>
      <gml:BoundedBy>
         <gml:Envelope gml:srsName="http://www.opengis.net/gml/srs/epsg.xml#epsg:4326">
            <gml:lowerCorner>72.85 -73.45</gml:lowerCorner>
            <gml:upperCorner>76.47 -72.28</gml:upperCorner>
         </gml:Envelope>
      </gml:BoundedBy>
      <skos:broader rdf:resource="urn:aodn.org.au:geographicextents:concept:10011"/>
      <skos:definition xml:lang="en">Named Locations (Antarctica) | Grove Mountains</skos:definition>
      <skos:scopeNote xml:lang="en">Named Locations (Antarctica) | Grove Mountains: Named Locations (Antarctica) | Grove Mountains</skos:scopeNote>
   </skos:Concept>
   <skos:Concept rdf:about="urn:aodn.org.au:geographicextents:concept:1109">
      <skos:prefLabel xml:lang="en">Named Locations (Antarctica) | Hawker island</skos:prefLabel>
      <skos:inScheme rdf:resource="urn:aodn.org.au:geographicextents:conceptscheme:1.0"/>
      <gml:BoundedBy>
         <gml:Envelope gml:srsName="http://www.opengis.net/gml/srs/epsg.xml#epsg:4326">
            <gml:lowerCorner>77.81 -68.65</gml:lowerCorner>
            <gml:upperCorner>77.89 -68.62</gml:upperCorner>
         </gml:Envelope>
      </gml:BoundedBy>
      <skos:broader rdf:resource="urn:aodn.org.au:geographicextents:concept:10011"/>
      <skos:definition xml:lang="en">Named Locations (Antarctica) | Hawker island</skos:definition>
      <skos:scopeNote xml:lang="en">Named Locations (Antarctica) | Hawker island: Named Locations (Antarctica) | Hawker island</skos:scopeNote>
   </skos:Concept>
   <skos:Concept rdf:about="urn:aodn.org.au:geographicextents:concept:1110">
      <skos:prefLabel xml:lang="en">Named Locations (Antarctica) | Holme Bay</skos:prefLabel>
      <skos:inScheme rdf:resource="urn:aodn.org.au:geographicextents:conceptscheme:1.0"/>
      <gml:BoundedBy>
         <gml:Envelope gml:srsName="http://www.opengis.net/gml/srs/epsg.xml#epsg:4326">
            <gml:lowerCorner>62.17 -67.75</gml:lowerCorner>
            <gml:upperCorner>63.11 -67.52</gml:upperCorner>
         </gml:Envelope>
      </gml:BoundedBy>
      <skos:broader rdf:resource="urn:aodn.org.au:geographicextents:concept:10011"/>
      <skos:definition xml:lang="en">Named Locations (Antarctica) | Holme Bay</skos:definition>
      <skos:scopeNote xml:lang="en">Named Locations (Antarctica) | Holme Bay: Named Locations (Antarctica) | Holme Bay</skos:scopeNote>
   </skos:Concept>
   <skos:Concept rdf:about="urn:aodn.org.au:geographicextents:concept:1111">
      <skos:prefLabel xml:lang="en">Named Locations (Antarctica) | Honkala Island</skos:prefLabel>
      <skos:inScheme rdf:resource="urn:aodn.org.au:geographicextents:conceptscheme:1.0"/>
      <gml:BoundedBy>
         <gml:Envelope gml:srsName="http://www.opengis.net/gml/srs/epsg.xml#epsg:4326">
            <gml:lowerCorner>110.58 -66.24</gml:lowerCorner>
            <gml:upperCorner>110.64 -66.22</gml:upperCorner>
         </gml:Envelope>
      </gml:BoundedBy>
      <skos:broader rdf:resource="urn:aodn.org.au:geographicextents:concept:10011"/>
      <skos:definition xml:lang="en">Named Locations (Antarctica) | Honkala Island</skos:definition>
      <skos:scopeNote xml:lang="en">Named Locations (Antarctica) | Honkala Island: Named Locations (Antarctica) | Honkala Island</skos:scopeNote>
   </skos:Concept>
   <skos:Concept rdf:about="urn:aodn.org.au:geographicextents:concept:1112">
      <skos:prefLabel xml:lang="en">Named Locations (Antarctica) | Hop Island</skos:prefLabel>
      <skos:inScheme rdf:resource="urn:aodn.org.au:geographicextents:conceptscheme:1.0"/>
      <gml:BoundedBy>
         <gml:Envelope gml:srsName="http://www.opengis.net/gml/srs/epsg.xml#epsg:4326">
            <gml:lowerCorner>77.63 -68.85</gml:lowerCorner>
            <gml:upperCorner>77.75 -68.81</gml:upperCorner>
         </gml:Envelope>
      </gml:BoundedBy>
      <skos:broader rdf:resource="urn:aodn.org.au:geographicextents:concept:10011"/>
      <skos:definition xml:lang="en">Named Locations (Antarctica) | Hop Island</skos:definition>
      <skos:scopeNote xml:lang="en">Named Locations (Antarctica) | Hop Island: Named Locations (Antarctica) | Hop Island</skos:scopeNote>
   </skos:Concept>
   <skos:Concept rdf:about="urn:aodn.org.au:geographicextents:concept:1114">
      <skos:prefLabel xml:lang="en">Named Locations (Antarctica) | Landing Bluff</skos:prefLabel>
      <skos:inScheme rdf:resource="urn:aodn.org.au:geographicextents:conceptscheme:1.0"/>
      <gml:BoundedBy>
         <gml:Envelope gml:srsName="http://www.opengis.net/gml/srs/epsg.xml#epsg:4326">
            <gml:lowerCorner>73.69 -69.76</gml:lowerCorner>
            <gml:upperCorner>73.72 -69.73</gml:upperCorner>
         </gml:Envelope>
      </gml:BoundedBy>
      <skos:broader rdf:resource="urn:aodn.org.au:geographicextents:concept:10011"/>
      <skos:definition xml:lang="en">Named Locations (Antarctica) | Landing Bluff</skos:definition>
      <skos:scopeNote xml:lang="en">Named Locations (Antarctica) | Landing Bluff: Named Locations (Antarctica) | Landing Bluff</skos:scopeNote>
   </skos:Concept>
   <skos:Concept rdf:about="urn:aodn.org.au:geographicextents:concept:1115">
      <skos:prefLabel xml:lang="en">Named Locations (Antarctica) | Larsemann Hills</skos:prefLabel>
      <skos:inScheme rdf:resource="urn:aodn.org.au:geographicextents:conceptscheme:1.0"/>
      <gml:BoundedBy>
         <gml:Envelope gml:srsName="http://www.opengis.net/gml/srs/epsg.xml#epsg:4326">
            <gml:lowerCorner>76 -69.5</gml:lowerCorner>
            <gml:upperCorner>76.48 -69.33</gml:upperCorner>
         </gml:Envelope>
      </gml:BoundedBy>
      <skos:broader rdf:resource="urn:aodn.org.au:geographicextents:concept:10011"/>
      <skos:definition xml:lang="en">Named Locations (Antarctica) | Larsemann Hills</skos:definition>
      <skos:scopeNote xml:lang="en">Named Locations (Antarctica) | Larsemann Hills: Named Locations (Antarctica) | Larsemann Hills</skos:scopeNote>
   </skos:Concept>
   <skos:Concept rdf:about="urn:aodn.org.au:geographicextents:concept:1116">
      <skos:prefLabel xml:lang="en">Named Locations (Antarctica) | Law Station (Romania)</skos:prefLabel>
      <skos:inScheme rdf:resource="urn:aodn.org.au:geographicextents:conceptscheme:1.0"/>
      <gml:BoundedBy>
         <gml:Envelope gml:srsName="http://www.opengis.net/gml/srs/epsg.xml#epsg:4326">
            <gml:lowerCorner>76.38 -69.38</gml:lowerCorner>
            <gml:upperCorner>76.39 -69.39</gml:upperCorner>
         </gml:Envelope>
      </gml:BoundedBy>
      <skos:broader rdf:resource="urn:aodn.org.au:geographicextents:concept:10011"/>
      <skos:definition xml:lang="en">Named Locations (Antarctica) | Law Station (Romania)</skos:definition>
      <skos:scopeNote xml:lang="en">Named Locations (Antarctica) | Law Station (Romania): Named Locations (Antarctica) | Law Station (Romania)</skos:scopeNote>
   </skos:Concept>
   <skos:Concept rdf:about="urn:aodn.org.au:geographicextents:concept:1117">
      <skos:prefLabel xml:lang="en">Named Locations (Antarctica) | Law Dome</skos:prefLabel>
      <skos:inScheme rdf:resource="urn:aodn.org.au:geographicextents:conceptscheme:1.0"/>
      <gml:BoundedBy>
         <gml:Envelope gml:srsName="http://www.opengis.net/gml/srs/epsg.xml#epsg:4326">
            <gml:lowerCorner>112.16 -67</gml:lowerCorner>
            <gml:upperCorner>113.57 -66.47</gml:upperCorner>
         </gml:Envelope>
      </gml:BoundedBy>
      <skos:broader rdf:resource="urn:aodn.org.au:geographicextents:concept:10011"/>
      <skos:definition xml:lang="en">Named Locations (Antarctica) | Law Dome</skos:definition>
      <skos:scopeNote xml:lang="en">Named Locations (Antarctica) | Law Dome: Named Locations (Antarctica) | Law Dome</skos:scopeNote>
   </skos:Concept>
   <skos:Concept rdf:about="urn:aodn.org.au:geographicextents:concept:1118">
      <skos:prefLabel xml:lang="en">Named Locations (Antarctica) | Loewe Massif</skos:prefLabel>
      <skos:inScheme rdf:resource="urn:aodn.org.au:geographicextents:conceptscheme:1.0"/>
      <gml:BoundedBy>
         <gml:Envelope gml:srsName="http://www.opengis.net/gml/srs/epsg.xml#epsg:4326">
            <gml:lowerCorner>67.56 -70.65</gml:lowerCorner>
            <gml:upperCorner>68.07 -70.51</gml:upperCorner>
         </gml:Envelope>
      </gml:BoundedBy>
      <skos:broader rdf:resource="urn:aodn.org.au:geographicextents:concept:10011"/>
      <skos:definition xml:lang="en">Named Locations (Antarctica) | Loewe Massif</skos:definition>
      <skos:scopeNote xml:lang="en">Named Locations (Antarctica) | Loewe Massif: Named Locations (Antarctica) | Loewe Massif</skos:scopeNote>
   </skos:Concept>
   <skos:Concept rdf:about="urn:aodn.org.au:geographicextents:concept:1119">
      <skos:prefLabel xml:lang="en">Named Locations (Antarctica) | Long Fjord</skos:prefLabel>
      <skos:inScheme rdf:resource="urn:aodn.org.au:geographicextents:conceptscheme:1.0"/>
      <gml:BoundedBy>
         <gml:Envelope gml:srsName="http://www.opengis.net/gml/srs/epsg.xml#epsg:4326">
            <gml:lowerCorner>77.97 -68.57</gml:lowerCorner>
            <gml:upperCorner>78.46 -68.47</gml:upperCorner>
         </gml:Envelope>
      </gml:BoundedBy>
      <skos:broader rdf:resource="urn:aodn.org.au:geographicextents:concept:10011"/>
      <skos:definition xml:lang="en">Named Locations (Antarctica) | Long Fjord</skos:definition>
      <skos:scopeNote xml:lang="en">Named Locations (Antarctica) | Long Fjord: Named Locations (Antarctica) | Long Fjord</skos:scopeNote>
   </skos:Concept>
   <skos:Concept rdf:about="urn:aodn.org.au:geographicextents:concept:1120">
      <skos:prefLabel xml:lang="en">Named Locations (Antarctica) | Mac.Robertson Land</skos:prefLabel>
      <skos:inScheme rdf:resource="urn:aodn.org.au:geographicextents:conceptscheme:1.0"/>
      <gml:BoundedBy>
         <gml:Envelope gml:srsName="http://www.opengis.net/gml/srs/epsg.xml#epsg:4326">
            <gml:lowerCorner>54.6 -75.9</gml:lowerCorner>
            <gml:upperCorner>74.1 -67.1</gml:upperCorner>
         </gml:Envelope>
      </gml:BoundedBy>
      <skos:broader rdf:resource="urn:aodn.org.au:geographicextents:concept:10011"/>
      <skos:definition xml:lang="en">Named Locations (Antarctica) | Mac.Robertson Land</skos:definition>
      <skos:scopeNote xml:lang="en">Named Locations (Antarctica) | Mac.Robertson Land: Named Locations (Antarctica) | Mac.Robertson Land</skos:scopeNote>
   </skos:Concept>
   <skos:Concept rdf:about="urn:aodn.org.au:geographicextents:concept:1121">
      <skos:prefLabel xml:lang="en">Named Locations (Antarctica) | Mac.Robertson Shelf</skos:prefLabel>
      <skos:inScheme rdf:resource="urn:aodn.org.au:geographicextents:conceptscheme:1.0"/>
      <gml:BoundedBy>
         <gml:Envelope gml:srsName="http://www.opengis.net/gml/srs/epsg.xml#epsg:4326">
            <gml:lowerCorner>60 -67.5</gml:lowerCorner>
            <gml:upperCorner>70 -66.5</gml:upperCorner>
         </gml:Envelope>
      </gml:BoundedBy>
      <skos:broader rdf:resource="urn:aodn.org.au:geographicextents:concept:10011"/>
      <skos:definition xml:lang="en">Named Locations (Antarctica) | Mac.Robertson Shelf</skos:definition>
      <skos:scopeNote xml:lang="en">Named Locations (Antarctica) | Mac.Robertson Shelf: Named Locations (Antarctica) | Mac.Robertson Shelf</skos:scopeNote>
   </skos:Concept>
   <skos:Concept rdf:about="urn:aodn.org.au:geographicextents:concept:1122">
      <skos:prefLabel xml:lang="en">Named Locations (Antarctica) | Magnetic Island</skos:prefLabel>
      <skos:inScheme rdf:resource="urn:aodn.org.au:geographicextents:conceptscheme:1.0"/>
      <gml:BoundedBy>
         <gml:Envelope gml:srsName="http://www.opengis.net/gml/srs/epsg.xml#epsg:4326">
            <gml:lowerCorner>77.89 -68.55</gml:lowerCorner>
            <gml:upperCorner>77.92 -68.54</gml:upperCorner>
         </gml:Envelope>
      </gml:BoundedBy>
      <skos:broader rdf:resource="urn:aodn.org.au:geographicextents:concept:10011"/>
      <skos:definition xml:lang="en">Named Locations (Antarctica) | Magnetic Island</skos:definition>
      <skos:scopeNote xml:lang="en">Named Locations (Antarctica) | Magnetic Island: Named Locations (Antarctica) | Magnetic Island</skos:scopeNote>
   </skos:Concept>
   <skos:Concept rdf:about="urn:aodn.org.au:geographicextents:concept:1123">
      <skos:prefLabel xml:lang="en">Named Locations (Antarctica) | Mawson Coast</skos:prefLabel>
      <skos:inScheme rdf:resource="urn:aodn.org.au:geographicextents:conceptscheme:1.0"/>
      <gml:BoundedBy>
         <gml:Envelope gml:srsName="http://www.opengis.net/gml/srs/epsg.xml#epsg:4326">
            <gml:lowerCorner>59.57 -67.7</gml:lowerCorner>
            <gml:upperCorner>66.9 -67.3</gml:upperCorner>
         </gml:Envelope>
      </gml:BoundedBy>
      <skos:broader rdf:resource="urn:aodn.org.au:geographicextents:concept:10011"/>
      <skos:definition xml:lang="en">Named Locations (Antarctica) | Mawson Coast</skos:definition>
      <skos:scopeNote xml:lang="en">Named Locations (Antarctica) | Mawson Coast: Named Locations (Antarctica) | Mawson Coast</skos:scopeNote>
   </skos:Concept>
   <skos:Concept rdf:about="urn:aodn.org.au:geographicextents:concept:135">
      <skos:prefLabel xml:lang="en">Named Locations (Antarctica) | Mawson Station (Australia)</skos:prefLabel>
      <skos:inScheme rdf:resource="urn:aodn.org.au:geographicextents:conceptscheme:1.0"/>
      <gml:BoundedBy>
         <gml:Envelope gml:srsName="http://www.opengis.net/gml/srs/epsg.xml#epsg:4326">
            <gml:lowerCorner>62.87 -67.61</gml:lowerCorner>
            <gml:upperCorner>62.88 -67.6</gml:upperCorner>
         </gml:Envelope>
      </gml:BoundedBy>
      <skos:broader rdf:resource="urn:aodn.org.au:geographicextents:concept:10011"/>
      <skos:definition xml:lang="en">Named Locations (Antarctica) | Mawson Station (Australia)</skos:definition>
      <skos:scopeNote xml:lang="en">Named Locations (Antarctica) | Mawson Station (Australia): Named Locations (Antarctica) | Mawson Station (Australia)</skos:scopeNote>
   </skos:Concept>
   <skos:Concept rdf:about="urn:aodn.org.au:geographicextents:concept:1124">
      <skos:prefLabel xml:lang="en">Named Locations (Antarctica) | McMurdo Station (USA)</skos:prefLabel>
      <skos:inScheme rdf:resource="urn:aodn.org.au:geographicextents:conceptscheme:1.0"/>
      <gml:BoundedBy>
         <gml:Envelope gml:srsName="http://www.opengis.net/gml/srs/epsg.xml#epsg:4326">
            <gml:lowerCorner>166.62 -77.86</gml:lowerCorner>
            <gml:upperCorner>166.81 -77.82</gml:upperCorner>
         </gml:Envelope>
      </gml:BoundedBy>
      <skos:broader rdf:resource="urn:aodn.org.au:geographicextents:concept:10011"/>
      <skos:definition xml:lang="en">Named Locations (Antarctica) | McMurdo Station (USA)</skos:definition>
      <skos:scopeNote xml:lang="en">Named Locations (Antarctica) | McMurdo Station (USA): Named Locations (Antarctica) | McMurdo Station (USA)</skos:scopeNote>
   </skos:Concept>
   <skos:Concept rdf:about="urn:aodn.org.au:geographicextents:concept:1125">
      <skos:prefLabel xml:lang="en">Named Locations (Antarctica) | Mertz Glacier Polynya</skos:prefLabel>
      <skos:inScheme rdf:resource="urn:aodn.org.au:geographicextents:conceptscheme:1.0"/>
      <gml:BoundedBy>
         <gml:Envelope gml:srsName="http://www.opengis.net/gml/srs/epsg.xml#epsg:4326">
            <gml:lowerCorner>142 -67</gml:lowerCorner>
            <gml:upperCorner>146 -66.3</gml:upperCorner>
         </gml:Envelope>
      </gml:BoundedBy>
      <skos:broader rdf:resource="urn:aodn.org.au:geographicextents:concept:10011"/>
      <skos:definition xml:lang="en">Named Locations (Antarctica) | Mertz Glacier Polynya</skos:definition>
      <skos:scopeNote xml:lang="en">Named Locations (Antarctica) | Mertz Glacier Polynya: Named Locations (Antarctica) | Mertz Glacier Polynya</skos:scopeNote>
   </skos:Concept>
   <skos:Concept rdf:about="urn:aodn.org.au:geographicextents:concept:1126">
      <skos:prefLabel xml:lang="en">Named Locations (Antarctica) | Mirny Station (Russia)</skos:prefLabel>
      <skos:inScheme rdf:resource="urn:aodn.org.au:geographicextents:conceptscheme:1.0"/>
      <gml:BoundedBy>
         <gml:Envelope gml:srsName="http://www.opengis.net/gml/srs/epsg.xml#epsg:4326">
            <gml:lowerCorner>92.99 -66.56</gml:lowerCorner>
            <gml:upperCorner>93.01 -66.55</gml:upperCorner>
         </gml:Envelope>
      </gml:BoundedBy>
      <skos:broader rdf:resource="urn:aodn.org.au:geographicextents:concept:10011"/>
      <skos:definition xml:lang="en">Named Locations (Antarctica) | Mirny Station (Russia)</skos:definition>
      <skos:scopeNote xml:lang="en">Named Locations (Antarctica) | Mirny Station (Russia): Named Locations (Antarctica) | Mirny Station (Russia)</skos:scopeNote>
   </skos:Concept>
   <skos:Concept rdf:about="urn:aodn.org.au:geographicextents:concept:1127">
      <skos:prefLabel xml:lang="en">Named Locations (Antarctica) | Murphy Rocks</skos:prefLabel>
      <skos:inScheme rdf:resource="urn:aodn.org.au:geographicextents:conceptscheme:1.0"/>
      <gml:BoundedBy>
         <gml:Envelope gml:srsName="http://www.opengis.net/gml/srs/epsg.xml#epsg:4326">
            <gml:lowerCorner>78.733 -68.233</gml:lowerCorner>
            <gml:upperCorner>78.733 -68.233</gml:upperCorner>
         </gml:Envelope>
      </gml:BoundedBy>
      <skos:broader rdf:resource="urn:aodn.org.au:geographicextents:concept:10011"/>
      <skos:definition xml:lang="en">Named Locations (Antarctica) | Murphy Rocks</skos:definition>
      <skos:scopeNote xml:lang="en">Named Locations (Antarctica) | Murphy Rocks: Named Locations (Antarctica) | Murphy Rocks</skos:scopeNote>
   </skos:Concept>
   <skos:Concept rdf:about="urn:aodn.org.au:geographicextents:concept:1128">
      <skos:prefLabel xml:lang="en">Named Locations (Antarctica) | Murray Monolith</skos:prefLabel>
      <skos:inScheme rdf:resource="urn:aodn.org.au:geographicextents:conceptscheme:1.0"/>
      <gml:BoundedBy>
         <gml:Envelope gml:srsName="http://www.opengis.net/gml/srs/epsg.xml#epsg:4326">
            <gml:lowerCorner>66.888 -67.784</gml:lowerCorner>
            <gml:upperCorner>66.888 -67.784</gml:upperCorner>
         </gml:Envelope>
      </gml:BoundedBy>
      <skos:broader rdf:resource="urn:aodn.org.au:geographicextents:concept:10011"/>
      <skos:definition xml:lang="en">Named Locations (Antarctica) | Murray Monolith</skos:definition>
      <skos:scopeNote xml:lang="en">Named Locations (Antarctica) | Murray Monolith: Named Locations (Antarctica) | Murray Monolith</skos:scopeNote>
   </skos:Concept>
   <skos:Concept rdf:about="urn:aodn.org.au:geographicextents:concept:1129">
      <skos:prefLabel xml:lang="en">Named Locations (Antarctica) | Newcomb Bay</skos:prefLabel>
      <skos:inScheme rdf:resource="urn:aodn.org.au:geographicextents:conceptscheme:1.0"/>
      <gml:BoundedBy>
         <gml:Envelope gml:srsName="http://www.opengis.net/gml/srs/epsg.xml#epsg:4326">
            <gml:lowerCorner>110.49 -66.28</gml:lowerCorner>
            <gml:upperCorner>110.58 -66.25</gml:upperCorner>
         </gml:Envelope>
      </gml:BoundedBy>
      <skos:broader rdf:resource="urn:aodn.org.au:geographicextents:concept:10011"/>
      <skos:definition xml:lang="en">Named Locations (Antarctica) | Newcomb Bay</skos:definition>
      <skos:scopeNote xml:lang="en">Named Locations (Antarctica) | Newcomb Bay: Named Locations (Antarctica) | Newcomb Bay</skos:scopeNote>
   </skos:Concept>
   <skos:Concept rdf:about="urn:aodn.org.au:geographicextents:concept:1131">
      <skos:prefLabel xml:lang="en">Named Locations (Antarctica) | Noonan Cove</skos:prefLabel>
      <skos:inScheme rdf:resource="urn:aodn.org.au:geographicextents:conceptscheme:1.0"/>
      <gml:BoundedBy>
         <gml:Envelope gml:srsName="http://www.opengis.net/gml/srs/epsg.xml#epsg:4326">
            <gml:lowerCorner>110.527 -66.259</gml:lowerCorner>
            <gml:upperCorner>110.527 -66.259</gml:upperCorner>
         </gml:Envelope>
      </gml:BoundedBy>
      <skos:broader rdf:resource="urn:aodn.org.au:geographicextents:concept:10011"/>
      <skos:definition xml:lang="en">Named Locations (Antarctica) | Noonan Cove</skos:definition>
      <skos:scopeNote xml:lang="en">Named Locations (Antarctica) | Noonan Cove: Named Locations (Antarctica) | Noonan Cove</skos:scopeNote>
   </skos:Concept>
   <skos:Concept rdf:about="urn:aodn.org.au:geographicextents:concept:1132">
      <skos:prefLabel xml:lang="en">Named Locations (Antarctica) | O'Brien Bay</skos:prefLabel>
      <skos:inScheme rdf:resource="urn:aodn.org.au:geographicextents:conceptscheme:1.0"/>
      <gml:BoundedBy>
         <gml:Envelope gml:srsName="http://www.opengis.net/gml/srs/epsg.xml#epsg:4326">
            <gml:lowerCorner>110.48 -66.32</gml:lowerCorner>
            <gml:upperCorner>110.57 -66.29</gml:upperCorner>
         </gml:Envelope>
      </gml:BoundedBy>
      <skos:broader rdf:resource="urn:aodn.org.au:geographicextents:concept:10011"/>
      <skos:definition xml:lang="en">Named Locations (Antarctica) | O'Brien Bay</skos:definition>
      <skos:scopeNote xml:lang="en">Named Locations (Antarctica) | O'Brien Bay: Named Locations (Antarctica) | O'Brien Bay</skos:scopeNote>
   </skos:Concept>
   <skos:Concept rdf:about="urn:aodn.org.au:geographicextents:concept:1133">
      <skos:prefLabel xml:lang="en">Named Locations (Antarctica) | O'Gorman Rocks</skos:prefLabel>
      <skos:inScheme rdf:resource="urn:aodn.org.au:geographicextents:conceptscheme:1.0"/>
      <gml:BoundedBy>
         <gml:Envelope gml:srsName="http://www.opengis.net/gml/srs/epsg.xml#epsg:4326">
            <gml:lowerCorner>77.95 -68.571</gml:lowerCorner>
            <gml:upperCorner>77.95 -68.571</gml:upperCorner>
         </gml:Envelope>
      </gml:BoundedBy>
      <skos:broader rdf:resource="urn:aodn.org.au:geographicextents:concept:10011"/>
      <skos:definition xml:lang="en">Named Locations (Antarctica) | O'Gorman Rocks</skos:definition>
      <skos:scopeNote xml:lang="en">Named Locations (Antarctica) | O'Gorman Rocks: Named Locations (Antarctica) | O'Gorman Rocks</skos:scopeNote>
   </skos:Concept>
   <skos:Concept rdf:about="urn:aodn.org.au:geographicextents:concept:1134">
      <skos:prefLabel xml:lang="en">Named Locations (Antarctica) | Penney Bay</skos:prefLabel>
      <skos:inScheme rdf:resource="urn:aodn.org.au:geographicextents:conceptscheme:1.0"/>
      <gml:BoundedBy>
         <gml:Envelope gml:srsName="http://www.opengis.net/gml/srs/epsg.xml#epsg:4326">
            <gml:lowerCorner>110.5 -66.49</gml:lowerCorner>
            <gml:upperCorner>110.74 -66.36</gml:upperCorner>
         </gml:Envelope>
      </gml:BoundedBy>
      <skos:broader rdf:resource="urn:aodn.org.au:geographicextents:concept:10011"/>
      <skos:definition xml:lang="en">Named Locations (Antarctica) | Penney Bay</skos:definition>
      <skos:scopeNote xml:lang="en">Named Locations (Antarctica) | Penney Bay: Named Locations (Antarctica) | Penney Bay</skos:scopeNote>
   </skos:Concept>
   <skos:Concept rdf:about="urn:aodn.org.au:geographicextents:concept:1135">
      <skos:prefLabel xml:lang="en">Named Locations (Antarctica) | Petersen Island</skos:prefLabel>
      <skos:inScheme rdf:resource="urn:aodn.org.au:geographicextents:conceptscheme:1.0"/>
      <gml:BoundedBy>
         <gml:Envelope gml:srsName="http://www.opengis.net/gml/srs/epsg.xml#epsg:4326">
            <gml:lowerCorner>62.88 -67.59</gml:lowerCorner>
            <gml:upperCorner>62.9 -67.57</gml:upperCorner>
         </gml:Envelope>
      </gml:BoundedBy>
      <skos:broader rdf:resource="urn:aodn.org.au:geographicextents:concept:10011"/>
      <skos:definition xml:lang="en">Named Locations (Antarctica) | Petersen Island</skos:definition>
      <skos:scopeNote xml:lang="en">Named Locations (Antarctica) | Petersen Island: Named Locations (Antarctica) | Petersen Island</skos:scopeNote>
   </skos:Concept>
   <skos:Concept rdf:about="urn:aodn.org.au:geographicextents:concept:1136">
      <skos:prefLabel xml:lang="en">Named Locations (Antarctica) | Petersen Bank</skos:prefLabel>
      <skos:inScheme rdf:resource="urn:aodn.org.au:geographicextents:conceptscheme:1.0"/>
      <gml:BoundedBy>
         <gml:Envelope gml:srsName="http://www.opengis.net/gml/srs/epsg.xml#epsg:4326">
            <gml:lowerCorner>110.789 -65.782</gml:lowerCorner>
            <gml:upperCorner>110.789 -65.782</gml:upperCorner>
         </gml:Envelope>
      </gml:BoundedBy>
      <skos:broader rdf:resource="urn:aodn.org.au:geographicextents:concept:10011"/>
      <skos:definition xml:lang="en">Named Locations (Antarctica) | Petersen Bank</skos:definition>
      <skos:scopeNote xml:lang="en">Named Locations (Antarctica) | Petersen Bank: Named Locations (Antarctica) | Petersen Bank</skos:scopeNote>
   </skos:Concept>
   <skos:Concept rdf:about="urn:aodn.org.au:geographicextents:concept:1137">
      <skos:prefLabel xml:lang="en">Named Locations (Antarctica) | Prince Charles Mountains</skos:prefLabel>
      <skos:inScheme rdf:resource="urn:aodn.org.au:geographicextents:conceptscheme:1.0"/>
      <gml:BoundedBy>
         <gml:Envelope gml:srsName="http://www.opengis.net/gml/srs/epsg.xml#epsg:4326">
            <gml:lowerCorner>59.72 -74.6</gml:lowerCorner>
            <gml:upperCorner>69.52 -69.91</gml:upperCorner>
         </gml:Envelope>
      </gml:BoundedBy>
      <skos:broader rdf:resource="urn:aodn.org.au:geographicextents:concept:10011"/>
      <skos:definition xml:lang="en">Named Locations (Antarctica) | Prince Charles Mountains</skos:definition>
      <skos:scopeNote xml:lang="en">Named Locations (Antarctica) | Prince Charles Mountains: Named Locations (Antarctica) | Prince Charles Mountains</skos:scopeNote>
   </skos:Concept>
   <skos:Concept rdf:about="urn:aodn.org.au:geographicextents:concept:1139">
      <skos:prefLabel xml:lang="en">Named Locations (Antarctica) | Princess Elizabeth Trough</skos:prefLabel>
      <skos:inScheme rdf:resource="urn:aodn.org.au:geographicextents:conceptscheme:1.0"/>
      <gml:BoundedBy>
         <gml:Envelope gml:srsName="http://www.opengis.net/gml/srs/epsg.xml#epsg:4326">
            <gml:lowerCorner>75 -66</gml:lowerCorner>
            <gml:upperCorner>90 -60</gml:upperCorner>
         </gml:Envelope>
      </gml:BoundedBy>
      <skos:broader rdf:resource="urn:aodn.org.au:geographicextents:concept:10011"/>
      <skos:definition xml:lang="en">Named Locations (Antarctica) | Princess Elizabeth Trough</skos:definition>
      <skos:scopeNote xml:lang="en">Named Locations (Antarctica) | Princess Elizabeth Trough: Named Locations (Antarctica) | Princess Elizabeth Trough</skos:scopeNote>
   </skos:Concept>
   <skos:Concept rdf:about="urn:aodn.org.au:geographicextents:concept:136">
      <skos:prefLabel xml:lang="en">Named Locations (Antarctica) | Prydz Bay</skos:prefLabel>
      <skos:inScheme rdf:resource="urn:aodn.org.au:geographicextents:conceptscheme:1.0"/>
      <gml:BoundedBy>
         <gml:Envelope gml:srsName="http://www.opengis.net/gml/srs/epsg.xml#epsg:4326">
            <gml:lowerCorner>72.15 -69.93</gml:lowerCorner>
            <gml:upperCorner>78.82 -68.16</gml:upperCorner>
         </gml:Envelope>
      </gml:BoundedBy>
      <skos:broader rdf:resource="urn:aodn.org.au:geographicextents:concept:10011"/>
      <skos:definition xml:lang="en">Named Locations (Antarctica) | Prydz Bay</skos:definition>
      <skos:scopeNote xml:lang="en">Named Locations (Antarctica) | Prydz Bay: Named Locations (Antarctica) | Prydz Bay</skos:scopeNote>
   </skos:Concept>
   <skos:Concept rdf:about="urn:aodn.org.au:geographicextents:concept:137">
      <skos:prefLabel xml:lang="en">Named Locations (Antarctica) | Publications Ice Shelf</skos:prefLabel>
      <skos:inScheme rdf:resource="urn:aodn.org.au:geographicextents:conceptscheme:1.0"/>
      <gml:BoundedBy>
         <gml:Envelope gml:srsName="http://www.opengis.net/gml/srs/epsg.xml#epsg:4326">
            <gml:lowerCorner>74.38 -69.96</gml:lowerCorner>
            <gml:upperCorner>75.95 -69.29</gml:upperCorner>
         </gml:Envelope>
      </gml:BoundedBy>
      <skos:broader rdf:resource="urn:aodn.org.au:geographicextents:concept:10011"/>
      <skos:definition xml:lang="en">Named Locations (Antarctica) | Publications Ice Shelf</skos:definition>
      <skos:scopeNote xml:lang="en">Named Locations (Antarctica) | Publications Ice Shelf: Named Locations (Antarctica) | Publications Ice Shelf</skos:scopeNote>
   </skos:Concept>
   <skos:Concept rdf:about="urn:aodn.org.au:geographicextents:concept:1140">
      <skos:prefLabel xml:lang="en">Named Locations (Antarctica) | Rauer Islands</skos:prefLabel>
      <skos:inScheme rdf:resource="urn:aodn.org.au:geographicextents:conceptscheme:1.0"/>
      <gml:BoundedBy>
         <gml:Envelope gml:srsName="http://www.opengis.net/gml/srs/epsg.xml#epsg:4326">
            <gml:lowerCorner>77.59 -68.92</gml:lowerCorner>
            <gml:upperCorner>78.03 -68.75</gml:upperCorner>
         </gml:Envelope>
      </gml:BoundedBy>
      <skos:broader rdf:resource="urn:aodn.org.au:geographicextents:concept:10011"/>
      <skos:definition xml:lang="en">Named Locations (Antarctica) | Rauer Islands</skos:definition>
      <skos:scopeNote xml:lang="en">Named Locations (Antarctica) | Rauer Islands: Named Locations (Antarctica) | Rauer Islands</skos:scopeNote>
   </skos:Concept>
   <skos:Concept rdf:about="urn:aodn.org.au:geographicextents:concept:1142">
      <skos:prefLabel xml:lang="en">Named Locations (Antarctica) | Richardson Lakes</skos:prefLabel>
      <skos:inScheme rdf:resource="urn:aodn.org.au:geographicextents:conceptscheme:1.0"/>
      <gml:BoundedBy>
         <gml:Envelope gml:srsName="http://www.opengis.net/gml/srs/epsg.xml#epsg:4326">
            <gml:lowerCorner>50.54 -66.86</gml:lowerCorner>
            <gml:upperCorner>50.9 -66.74</gml:upperCorner>
         </gml:Envelope>
      </gml:BoundedBy>
      <skos:broader rdf:resource="urn:aodn.org.au:geographicextents:concept:10011"/>
      <skos:definition xml:lang="en">Named Locations (Antarctica) | Richardson Lakes</skos:definition>
      <skos:scopeNote xml:lang="en">Named Locations (Antarctica) | Richardson Lakes: Named Locations (Antarctica) | Richardson Lakes</skos:scopeNote>
   </skos:Concept>
   <skos:Concept rdf:about="urn:aodn.org.au:geographicextents:concept:1143">
      <skos:prefLabel xml:lang="en">Named Locations (Antarctica) | Sandefjord Bay</skos:prefLabel>
      <skos:inScheme rdf:resource="urn:aodn.org.au:geographicextents:conceptscheme:1.0"/>
      <gml:BoundedBy>
         <gml:Envelope gml:srsName="http://www.opengis.net/gml/srs/epsg.xml#epsg:4326">
            <gml:lowerCorner>73.22 -69.94</gml:lowerCorner>
            <gml:upperCorner>76.75 -69.25</gml:upperCorner>
         </gml:Envelope>
      </gml:BoundedBy>
      <skos:broader rdf:resource="urn:aodn.org.au:geographicextents:concept:10011"/>
      <skos:definition xml:lang="en">Named Locations (Antarctica) | Sandefjord Bay</skos:definition>
      <skos:scopeNote xml:lang="en">Named Locations (Antarctica) | Sandefjord Bay: Named Locations (Antarctica) | Sandefjord Bay</skos:scopeNote>
   </skos:Concept>
   <skos:Concept rdf:about="urn:aodn.org.au:geographicextents:concept:1144">
      <skos:prefLabel xml:lang="en">Named Locations (Antarctica) | Scullin Monolith</skos:prefLabel>
      <skos:inScheme rdf:resource="urn:aodn.org.au:geographicextents:conceptscheme:1.0"/>
      <gml:BoundedBy>
         <gml:Envelope gml:srsName="http://www.opengis.net/gml/srs/epsg.xml#epsg:4326">
            <gml:lowerCorner>66.719 -67.794</gml:lowerCorner>
            <gml:upperCorner>66.719 -67.794</gml:upperCorner>
         </gml:Envelope>
      </gml:BoundedBy>
      <skos:broader rdf:resource="urn:aodn.org.au:geographicextents:concept:10011"/>
      <skos:definition xml:lang="en">Named Locations (Antarctica) | Scullin Monolith</skos:definition>
      <skos:scopeNote xml:lang="en">Named Locations (Antarctica) | Scullin Monolith: Named Locations (Antarctica) | Scullin Monolith</skos:scopeNote>
   </skos:Concept>
   <skos:Concept rdf:about="urn:aodn.org.au:geographicextents:concept:138">
      <skos:prefLabel xml:lang="en">Named Locations (Antarctica) | Shackleton Ice Shelf</skos:prefLabel>
      <skos:inScheme rdf:resource="urn:aodn.org.au:geographicextents:conceptscheme:1.0"/>
      <gml:BoundedBy>
         <gml:Envelope gml:srsName="http://www.opengis.net/gml/srs/epsg.xml#epsg:4326">
            <gml:lowerCorner>95.5 -66.76</gml:lowerCorner>
            <gml:upperCorner>102 -64.73</gml:upperCorner>
         </gml:Envelope>
      </gml:BoundedBy>
      <skos:broader rdf:resource="urn:aodn.org.au:geographicextents:concept:10011"/>
      <skos:definition xml:lang="en">Named Locations (Antarctica) | Shackleton Ice Shelf</skos:definition>
      <skos:scopeNote xml:lang="en">Named Locations (Antarctica) | Shackleton Ice Shelf: Named Locations (Antarctica) | Shackleton Ice Shelf</skos:scopeNote>
   </skos:Concept>
   <skos:Concept rdf:about="urn:aodn.org.au:geographicextents:concept:1145">
      <skos:prefLabel xml:lang="en">Named Locations (Antarctica) | Shannon Bay</skos:prefLabel>
      <skos:inScheme rdf:resource="urn:aodn.org.au:geographicextents:conceptscheme:1.0"/>
      <gml:BoundedBy>
         <gml:Envelope gml:srsName="http://www.opengis.net/gml/srs/epsg.xml#epsg:4326">
            <gml:lowerCorner>110.525 -66.279</gml:lowerCorner>
            <gml:upperCorner>110.525 -66.279</gml:upperCorner>
         </gml:Envelope>
      </gml:BoundedBy>
      <skos:broader rdf:resource="urn:aodn.org.au:geographicextents:concept:10011"/>
      <skos:definition xml:lang="en">Named Locations (Antarctica) | Shannon Bay</skos:definition>
      <skos:scopeNote xml:lang="en">Named Locations (Antarctica) | Shannon Bay: Named Locations (Antarctica) | Shannon Bay</skos:scopeNote>
   </skos:Concept>
   <skos:Concept rdf:about="urn:aodn.org.au:geographicextents:concept:1146">
      <skos:prefLabel xml:lang="en">Named Locations (Antarctica) | Shirley Island</skos:prefLabel>
      <skos:inScheme rdf:resource="urn:aodn.org.au:geographicextents:conceptscheme:1.0"/>
      <gml:BoundedBy>
         <gml:Envelope gml:srsName="http://www.opengis.net/gml/srs/epsg.xml#epsg:4326">
            <gml:lowerCorner>110.47 -66.29</gml:lowerCorner>
            <gml:upperCorner>110.49 -66.28</gml:upperCorner>
         </gml:Envelope>
      </gml:BoundedBy>
      <skos:broader rdf:resource="urn:aodn.org.au:geographicextents:concept:10011"/>
      <skos:definition xml:lang="en">Named Locations (Antarctica) | Shirley Island</skos:definition>
      <skos:scopeNote xml:lang="en">Named Locations (Antarctica) | Shirley Island: Named Locations (Antarctica) | Shirley Island</skos:scopeNote>
   </skos:Concept>
   <skos:Concept rdf:about="urn:aodn.org.au:geographicextents:concept:1153">
      <skos:prefLabel xml:lang="en">Named Locations (Antarctica) | Showa Station (Japan)</skos:prefLabel>
      <skos:inScheme rdf:resource="urn:aodn.org.au:geographicextents:conceptscheme:1.0"/>
      <gml:BoundedBy>
         <gml:Envelope gml:srsName="http://www.opengis.net/gml/srs/epsg.xml#epsg:4326">
            <gml:lowerCorner>39.58 -69.005</gml:lowerCorner>
            <gml:upperCorner>39.58 -69.005</gml:upperCorner>
         </gml:Envelope>
      </gml:BoundedBy>
      <skos:broader rdf:resource="urn:aodn.org.au:geographicextents:concept:10011"/>
      <skos:definition xml:lang="en">Named Locations (Antarctica) | Showa Station (Japan)</skos:definition>
      <skos:scopeNote xml:lang="en">Named Locations (Antarctica) | Showa Station (Japan): Named Locations (Antarctica) | Showa Station (Japan)</skos:scopeNote>
   </skos:Concept>
   <skos:Concept rdf:about="urn:aodn.org.au:geographicextents:concept:1147">
      <skos:prefLabel xml:lang="en">Named Locations (Antarctica) | Sparkes Bay</skos:prefLabel>
      <skos:inScheme rdf:resource="urn:aodn.org.au:geographicextents:conceptscheme:1.0"/>
      <gml:BoundedBy>
         <gml:Envelope gml:srsName="http://www.opengis.net/gml/srs/epsg.xml#epsg:4326">
            <gml:lowerCorner>110.567 -66.359</gml:lowerCorner>
            <gml:upperCorner>110.567 -66.359</gml:upperCorner>
         </gml:Envelope>
      </gml:BoundedBy>
      <skos:broader rdf:resource="urn:aodn.org.au:geographicextents:concept:10011"/>
      <skos:definition xml:lang="en">Named Locations (Antarctica) | Sparkes Bay</skos:definition>
      <skos:scopeNote xml:lang="en">Named Locations (Antarctica) | Sparkes Bay: Named Locations (Antarctica) | Sparkes Bay</skos:scopeNote>
   </skos:Concept>
   <skos:Concept rdf:about="urn:aodn.org.au:geographicextents:concept:1148">
      <skos:prefLabel xml:lang="en">Named Locations (Antarctica) | Stefansson Bay</skos:prefLabel>
      <skos:inScheme rdf:resource="urn:aodn.org.au:geographicextents:conceptscheme:1.0"/>
      <gml:BoundedBy>
         <gml:Envelope gml:srsName="http://www.opengis.net/gml/srs/epsg.xml#epsg:4326">
            <gml:lowerCorner>59.167 -67.333</gml:lowerCorner>
            <gml:upperCorner>59.167 -67.333</gml:upperCorner>
         </gml:Envelope>
      </gml:BoundedBy>
      <skos:broader rdf:resource="urn:aodn.org.au:geographicextents:concept:10011"/>
      <skos:definition xml:lang="en">Named Locations (Antarctica) | Stefansson Bay</skos:definition>
      <skos:scopeNote xml:lang="en">Named Locations (Antarctica) | Stefansson Bay: Named Locations (Antarctica) | Stefansson Bay</skos:scopeNote>
   </skos:Concept>
   <skos:Concept rdf:about="urn:aodn.org.au:geographicextents:concept:1150">
      <skos:prefLabel xml:lang="en">Named Locations (Antarctica) | Stillwell Hills</skos:prefLabel>
      <skos:inScheme rdf:resource="urn:aodn.org.au:geographicextents:conceptscheme:1.0"/>
      <gml:BoundedBy>
         <gml:Envelope gml:srsName="http://www.opengis.net/gml/srs/epsg.xml#epsg:4326">
            <gml:lowerCorner>59.34 -67.48</gml:lowerCorner>
            <gml:upperCorner>59.59 -67.32</gml:upperCorner>
         </gml:Envelope>
      </gml:BoundedBy>
      <skos:broader rdf:resource="urn:aodn.org.au:geographicextents:concept:10011"/>
      <skos:definition xml:lang="en">Named Locations (Antarctica) | Stillwell Hills</skos:definition>
      <skos:scopeNote xml:lang="en">Named Locations (Antarctica) | Stillwell Hills: Named Locations (Antarctica) | Stillwell Hills</skos:scopeNote>
   </skos:Concept>
   <skos:Concept rdf:about="urn:aodn.org.au:geographicextents:concept:1152">
      <skos:prefLabel xml:lang="en">Named Locations (Antarctica) | Svenner Islands</skos:prefLabel>
      <skos:inScheme rdf:resource="urn:aodn.org.au:geographicextents:conceptscheme:1.0"/>
      <gml:BoundedBy>
         <gml:Envelope gml:srsName="http://www.opengis.net/gml/srs/epsg.xml#epsg:4326">
            <gml:lowerCorner>76.911 -69.018</gml:lowerCorner>
            <gml:upperCorner>76.911 -69.018</gml:upperCorner>
         </gml:Envelope>
      </gml:BoundedBy>
      <skos:broader rdf:resource="urn:aodn.org.au:geographicextents:concept:10011"/>
      <skos:definition xml:lang="en">Named Locations (Antarctica) | Svenner Islands</skos:definition>
      <skos:scopeNote xml:lang="en">Named Locations (Antarctica) | Svenner Islands: Named Locations (Antarctica) | Svenner Islands</skos:scopeNote>
   </skos:Concept>
   <skos:Concept rdf:about="urn:aodn.org.au:geographicextents:concept:1154">
      <skos:prefLabel xml:lang="en">Named Locations (Antarctica) | Tryne Fjord</skos:prefLabel>
      <skos:inScheme rdf:resource="urn:aodn.org.au:geographicextents:conceptscheme:1.0"/>
      <gml:BoundedBy>
         <gml:Envelope gml:srsName="http://www.opengis.net/gml/srs/epsg.xml#epsg:4326">
            <gml:lowerCorner>78.3 -68.49</gml:lowerCorner>
            <gml:upperCorner>78.43 -68.42</gml:upperCorner>
         </gml:Envelope>
      </gml:BoundedBy>
      <skos:broader rdf:resource="urn:aodn.org.au:geographicextents:concept:10011"/>
      <skos:definition xml:lang="en">Named Locations (Antarctica) | Tryne Fjord</skos:definition>
      <skos:scopeNote xml:lang="en">Named Locations (Antarctica) | Tryne Fjord: Named Locations (Antarctica) | Tryne Fjord</skos:scopeNote>
   </skos:Concept>
   <skos:Concept rdf:about="urn:aodn.org.au:geographicextents:concept:1155">
      <skos:prefLabel xml:lang="en">Named Locations (Antarctica) | Verner Island</skos:prefLabel>
      <skos:inScheme rdf:resource="urn:aodn.org.au:geographicextents:conceptscheme:1.0"/>
      <gml:BoundedBy>
         <gml:Envelope gml:srsName="http://www.opengis.net/gml/srs/epsg.xml#epsg:4326">
            <gml:lowerCorner>62.883 -67.577</gml:lowerCorner>
            <gml:upperCorner>62.883 -67.577</gml:upperCorner>
         </gml:Envelope>
      </gml:BoundedBy>
      <skos:broader rdf:resource="urn:aodn.org.au:geographicextents:concept:10011"/>
      <skos:definition xml:lang="en">Named Locations (Antarctica) | Verner Island</skos:definition>
      <skos:scopeNote xml:lang="en">Named Locations (Antarctica) | Verner Island: Named Locations (Antarctica) | Verner Island</skos:scopeNote>
   </skos:Concept>
   <skos:Concept rdf:about="urn:aodn.org.au:geographicextents:concept:1157">
      <skos:prefLabel xml:lang="en">Named Locations (Antarctica) | Vestfold Hills</skos:prefLabel>
      <skos:inScheme rdf:resource="urn:aodn.org.au:geographicextents:conceptscheme:1.0"/>
      <gml:BoundedBy>
         <gml:Envelope gml:srsName="http://www.opengis.net/gml/srs/epsg.xml#epsg:4326">
            <gml:lowerCorner>77.82 -68.67</gml:lowerCorner>
            <gml:upperCorner>78.57 -68.42</gml:upperCorner>
         </gml:Envelope>
      </gml:BoundedBy>
      <skos:broader rdf:resource="urn:aodn.org.au:geographicextents:concept:10011"/>
      <skos:definition xml:lang="en">Named Locations (Antarctica) | Vestfold Hills</skos:definition>
      <skos:scopeNote xml:lang="en">Named Locations (Antarctica) | Vestfold Hills: Named Locations (Antarctica) | Vestfold Hills</skos:scopeNote>
   </skos:Concept>
   <skos:Concept rdf:about="urn:aodn.org.au:geographicextents:concept:1158">
      <skos:prefLabel xml:lang="en">Named Locations (Antarctica) | Victoria Land</skos:prefLabel>
      <skos:inScheme rdf:resource="urn:aodn.org.au:geographicextents:conceptscheme:1.0"/>
      <gml:BoundedBy>
         <gml:Envelope gml:srsName="http://www.opengis.net/gml/srs/epsg.xml#epsg:4326">
            <gml:lowerCorner>160 -78</gml:lowerCorner>
            <gml:upperCorner>120 -70.5</gml:upperCorner>
         </gml:Envelope>
      </gml:BoundedBy>
      <skos:broader rdf:resource="urn:aodn.org.au:geographicextents:concept:10011"/>
      <skos:definition xml:lang="en">Named Locations (Antarctica) | Victoria Land</skos:definition>
      <skos:scopeNote xml:lang="en">Named Locations (Antarctica) | Victoria Land: Named Locations (Antarctica) | Victoria Land</skos:scopeNote>
   </skos:Concept>
   <skos:Concept rdf:about="urn:aodn.org.au:geographicextents:concept:140">
      <skos:prefLabel xml:lang="en">Named Locations (Antarctica) | Voyekov Ice Shelf</skos:prefLabel>
      <skos:inScheme rdf:resource="urn:aodn.org.au:geographicextents:conceptscheme:1.0"/>
      <gml:BoundedBy>
         <gml:Envelope gml:srsName="http://www.opengis.net/gml/srs/epsg.xml#epsg:4326">
            <gml:lowerCorner>121.6 -67.05</gml:lowerCorner>
            <gml:upperCorner>129.39 -65.18</gml:upperCorner>
         </gml:Envelope>
      </gml:BoundedBy>
      <skos:broader rdf:resource="urn:aodn.org.au:geographicextents:concept:10011"/>
      <skos:definition xml:lang="en">Named Locations (Antarctica) | Voyekov Ice Shelf</skos:definition>
      <skos:scopeNote xml:lang="en">Named Locations (Antarctica) | Voyekov Ice Shelf: Named Locations (Antarctica) | Voyekov Ice Shelf</skos:scopeNote>
   </skos:Concept>
   <skos:Concept rdf:about="urn:aodn.org.au:geographicextents:concept:1159">
      <skos:prefLabel xml:lang="en">Named Locations (Antarctica) | Welch Island</skos:prefLabel>
      <skos:inScheme rdf:resource="urn:aodn.org.au:geographicextents:conceptscheme:1.0"/>
      <gml:BoundedBy>
         <gml:Envelope gml:srsName="http://www.opengis.net/gml/srs/epsg.xml#epsg:4326">
            <gml:lowerCorner>62.91 -67.57</gml:lowerCorner>
            <gml:upperCorner>62.945 -67.55</gml:upperCorner>
         </gml:Envelope>
      </gml:BoundedBy>
      <skos:broader rdf:resource="urn:aodn.org.au:geographicextents:concept:10011"/>
      <skos:definition xml:lang="en">Named Locations (Antarctica) | Welch Island</skos:definition>
      <skos:scopeNote xml:lang="en">Named Locations (Antarctica) | Welch Island: Named Locations (Antarctica) | Welch Island</skos:scopeNote>
   </skos:Concept>
   <skos:Concept rdf:about="urn:aodn.org.au:geographicextents:concept:141">
      <skos:prefLabel xml:lang="en">Named Locations (Antarctica) | West Ice Shelf</skos:prefLabel>
      <skos:inScheme rdf:resource="urn:aodn.org.au:geographicextents:conceptscheme:1.0"/>
      <gml:BoundedBy>
         <gml:Envelope gml:srsName="http://www.opengis.net/gml/srs/epsg.xml#epsg:4326">
            <gml:lowerCorner>81.35 -67.8</gml:lowerCorner>
            <gml:upperCorner>87.15 -65.46</gml:upperCorner>
         </gml:Envelope>
      </gml:BoundedBy>
      <skos:broader rdf:resource="urn:aodn.org.au:geographicextents:concept:10011"/>
      <skos:definition xml:lang="en">Named Locations (Antarctica) | West Ice Shelf</skos:definition>
      <skos:scopeNote xml:lang="en">Named Locations (Antarctica) | West Ice Shelf: Named Locations (Antarctica) | West Ice Shelf</skos:scopeNote>
   </skos:Concept>
   <skos:Concept rdf:about="urn:aodn.org.au:geographicextents:concept:1160">
      <skos:prefLabel xml:lang="en">Named Locations (Antarctica) | Wilkes Station (Australia)</skos:prefLabel>
      <skos:inScheme rdf:resource="urn:aodn.org.au:geographicextents:conceptscheme:1.0"/>
      <gml:BoundedBy>
         <gml:Envelope gml:srsName="http://www.opengis.net/gml/srs/epsg.xml#epsg:4326">
            <gml:lowerCorner>110.526 -66.257</gml:lowerCorner>
            <gml:upperCorner>110.526 -66.257</gml:upperCorner>
         </gml:Envelope>
      </gml:BoundedBy>
      <skos:broader rdf:resource="urn:aodn.org.au:geographicextents:concept:10011"/>
      <skos:definition xml:lang="en">Named Locations (Antarctica) | Wilkes Station (Australia)</skos:definition>
      <skos:scopeNote xml:lang="en">Named Locations (Antarctica) | Wilkes Station (Australia): Named Locations (Antarctica) | Wilkes Station (Australia)</skos:scopeNote>
   </skos:Concept>
   <skos:Concept rdf:about="urn:aodn.org.au:geographicextents:concept:1161">
      <skos:prefLabel xml:lang="en">Named Locations (Antarctica) | Windmill Islands</skos:prefLabel>
      <skos:inScheme rdf:resource="urn:aodn.org.au:geographicextents:conceptscheme:1.0"/>
      <gml:BoundedBy>
         <gml:Envelope gml:srsName="http://www.opengis.net/gml/srs/epsg.xml#epsg:4326">
            <gml:lowerCorner>110.34 -66.49</gml:lowerCorner>
            <gml:upperCorner>110.66 -66.28</gml:upperCorner>
         </gml:Envelope>
      </gml:BoundedBy>
      <skos:broader rdf:resource="urn:aodn.org.au:geographicextents:concept:10011"/>
      <skos:definition xml:lang="en">Named Locations (Antarctica) | Windmill Islands</skos:definition>
      <skos:scopeNote xml:lang="en">Named Locations (Antarctica) | Windmill Islands: Named Locations (Antarctica) | Windmill Islands</skos:scopeNote>
   </skos:Concept>
   <skos:Concept rdf:about="urn:aodn.org.au:geographicextents:concept:43">
      <skos:prefLabel xml:lang="en">Offshore Islands (Australia) | Ashmore &amp; Cartier Islands</skos:prefLabel>
      <skos:inScheme rdf:resource="urn:aodn.org.au:geographicextents:conceptscheme:1.0"/>
      <gml:BoundedBy>
         <gml:Envelope gml:srsName="http://www.opengis.net/gml/srs/epsg.xml#epsg:4326">
            <gml:lowerCorner>122.8 -12.6</gml:lowerCorner>
            <gml:upperCorner>123.7 -12.1</gml:upperCorner>
         </gml:Envelope>
      </gml:BoundedBy>
      <skos:broader rdf:resource="urn:aodn.org.au:geographicextents:concept:10005"/>
      <skos:definition xml:lang="en">Offshore Islands (Australia) | Ashmore &amp; Cartier Islands</skos:definition>
      <skos:scopeNote xml:lang="en">Offshore Islands (Australia) | Ashmore &amp; Cartier Islands: Offshore Islands (Australia) | Ashmore &amp; Cartier Islands</skos:scopeNote>
   </skos:Concept>
   <skos:Concept rdf:about="urn:aodn.org.au:geographicextents:concept:44">
      <skos:prefLabel xml:lang="en">Offshore Islands (Australia) | Christmas Island</skos:prefLabel>
      <skos:inScheme rdf:resource="urn:aodn.org.au:geographicextents:conceptscheme:1.0"/>
      <gml:BoundedBy>
         <gml:Envelope gml:srsName="http://www.opengis.net/gml/srs/epsg.xml#epsg:4326">
            <gml:lowerCorner>105.1 -11</gml:lowerCorner>
            <gml:upperCorner>106.1 -10</gml:upperCorner>
         </gml:Envelope>
      </gml:BoundedBy>
      <skos:broader rdf:resource="urn:aodn.org.au:geographicextents:concept:10005"/>
      <skos:definition xml:lang="en">Offshore Islands (Australia) | Christmas Island</skos:definition>
      <skos:scopeNote xml:lang="en">Offshore Islands (Australia) | Christmas Island: Offshore Islands (Australia) | Christmas Island</skos:scopeNote>
   </skos:Concept>
   <skos:Concept rdf:about="urn:aodn.org.au:geographicextents:concept:45">
      <skos:prefLabel xml:lang="en">Offshore Islands (Australia) | Cocos (Keeling) Island</skos:prefLabel>
      <skos:inScheme rdf:resource="urn:aodn.org.au:geographicextents:conceptscheme:1.0"/>
      <gml:BoundedBy>
         <gml:Envelope gml:srsName="http://www.opengis.net/gml/srs/epsg.xml#epsg:4326">
            <gml:lowerCorner>96.3 -12.4</gml:lowerCorner>
            <gml:upperCorner>97.3 -11.4</gml:upperCorner>
         </gml:Envelope>
      </gml:BoundedBy>
      <skos:broader rdf:resource="urn:aodn.org.au:geographicextents:concept:10005"/>
      <skos:definition xml:lang="en">Offshore Islands (Australia) | Cocos (Keeling) Island</skos:definition>
      <skos:scopeNote xml:lang="en">Offshore Islands (Australia) | Cocos (Keeling) Island: Offshore Islands (Australia) | Cocos (Keeling) Island</skos:scopeNote>
   </skos:Concept>
   <skos:Concept rdf:about="urn:aodn.org.au:geographicextents:concept:46">
      <skos:prefLabel xml:lang="en">Offshore Islands (Australia) | Heard &amp; McDonald Islands</skos:prefLabel>
      <skos:inScheme rdf:resource="urn:aodn.org.au:geographicextents:conceptscheme:1.0"/>
      <gml:BoundedBy>
         <gml:Envelope gml:srsName="http://www.opengis.net/gml/srs/epsg.xml#epsg:4326">
            <gml:lowerCorner>73 -53.3</gml:lowerCorner>
            <gml:upperCorner>74 -52.8</gml:upperCorner>
         </gml:Envelope>
      </gml:BoundedBy>
      <skos:broader rdf:resource="urn:aodn.org.au:geographicextents:concept:10005"/>
      <skos:definition xml:lang="en">Offshore Islands (Australia) | Heard &amp; McDonald Islands</skos:definition>
      <skos:scopeNote xml:lang="en">Offshore Islands (Australia) | Heard &amp; McDonald Islands: Offshore Islands (Australia) | Heard &amp; McDonald Islands</skos:scopeNote>
   </skos:Concept>
   <skos:Concept rdf:about="urn:aodn.org.au:geographicextents:concept:47">
      <skos:prefLabel xml:lang="en">Offshore Islands (Australia) | Lord Howe Island</skos:prefLabel>
      <skos:inScheme rdf:resource="urn:aodn.org.au:geographicextents:conceptscheme:1.0"/>
      <gml:BoundedBy>
         <gml:Envelope gml:srsName="http://www.opengis.net/gml/srs/epsg.xml#epsg:4326">
            <gml:lowerCorner>158.7 -31.8</gml:lowerCorner>
            <gml:upperCorner>159.3 -31.2</gml:upperCorner>
         </gml:Envelope>
      </gml:BoundedBy>
      <skos:broader rdf:resource="urn:aodn.org.au:geographicextents:concept:10005"/>
      <skos:definition xml:lang="en">Offshore Islands (Australia) | Lord Howe Island</skos:definition>
      <skos:scopeNote xml:lang="en">Offshore Islands (Australia) | Lord Howe Island: Offshore Islands (Australia) | Lord Howe Island</skos:scopeNote>
   </skos:Concept>
   <skos:Concept rdf:about="urn:aodn.org.au:geographicextents:concept:48">
      <skos:prefLabel xml:lang="en">Offshore Islands (Australia) | Macquarie Island</skos:prefLabel>
      <skos:inScheme rdf:resource="urn:aodn.org.au:geographicextents:conceptscheme:1.0"/>
      <gml:BoundedBy>
         <gml:Envelope gml:srsName="http://www.opengis.net/gml/srs/epsg.xml#epsg:4326">
            <gml:lowerCorner>158.5 -55</gml:lowerCorner>
            <gml:upperCorner>159.5 -54</gml:upperCorner>
         </gml:Envelope>
      </gml:BoundedBy>
      <skos:broader rdf:resource="urn:aodn.org.au:geographicextents:concept:10005"/>
      <skos:definition xml:lang="en">Offshore Islands (Australia) | Macquarie Island</skos:definition>
      <skos:scopeNote xml:lang="en">Offshore Islands (Australia) | Macquarie Island: Offshore Islands (Australia) | Macquarie Island</skos:scopeNote>
   </skos:Concept>
   <skos:Concept rdf:about="urn:aodn.org.au:geographicextents:concept:49">
      <skos:prefLabel xml:lang="en">Offshore Islands (Australia) | Norfolk Island</skos:prefLabel>
      <skos:inScheme rdf:resource="urn:aodn.org.au:geographicextents:conceptscheme:1.0"/>
      <gml:BoundedBy>
         <gml:Envelope gml:srsName="http://www.opengis.net/gml/srs/epsg.xml#epsg:4326">
            <gml:lowerCorner>167.7 -29.2</gml:lowerCorner>
            <gml:upperCorner>168.2 -28.9</gml:upperCorner>
         </gml:Envelope>
      </gml:BoundedBy>
      <skos:broader rdf:resource="urn:aodn.org.au:geographicextents:concept:10005"/>
      <skos:definition xml:lang="en">Offshore Islands (Australia) | Norfolk Island</skos:definition>
      <skos:scopeNote xml:lang="en">Offshore Islands (Australia) | Norfolk Island: Offshore Islands (Australia) | Norfolk Island</skos:scopeNote>
   </skos:Concept>
   <skos:Concept rdf:about="urn:aodn.org.au:geographicextents:concept:7">
      <skos:prefLabel xml:lang="en">Regional Seas | Arafura Sea</skos:prefLabel>
      <skos:inScheme rdf:resource="urn:aodn.org.au:geographicextents:conceptscheme:1.0"/>
      <gml:BoundedBy>
         <gml:Envelope gml:srsName="http://www.opengis.net/gml/srs/epsg.xml#epsg:4326">
            <gml:lowerCorner>131 -18</gml:lowerCorner>
            <gml:upperCorner>142 -3</gml:upperCorner>
         </gml:Envelope>
      </gml:BoundedBy>
      <skos:broader rdf:resource="urn:aodn.org.au:geographicextents:concept:10000"/>
      <skos:definition xml:lang="en">Regional Seas | Arafura Sea</skos:definition>
      <skos:scopeNote xml:lang="en">Regional Seas | Arafura Sea: Regional Seas | Arafura Sea</skos:scopeNote>
   </skos:Concept>
   <skos:Concept rdf:about="urn:aodn.org.au:geographicextents:concept:8">
      <skos:prefLabel xml:lang="en">Regional Seas | Bali Sea</skos:prefLabel>
      <skos:inScheme rdf:resource="urn:aodn.org.au:geographicextents:conceptscheme:1.0"/>
      <gml:BoundedBy>
         <gml:Envelope gml:srsName="http://www.opengis.net/gml/srs/epsg.xml#epsg:4326">
            <gml:lowerCorner>114 -9</gml:lowerCorner>
            <gml:upperCorner>117 -7</gml:upperCorner>
         </gml:Envelope>
      </gml:BoundedBy>
      <skos:broader rdf:resource="urn:aodn.org.au:geographicextents:concept:10000"/>
      <skos:definition xml:lang="en">Regional Seas | Bali Sea</skos:definition>
      <skos:scopeNote xml:lang="en">Regional Seas | Bali Sea: Regional Seas | Bali Sea</skos:scopeNote>
   </skos:Concept>
   <skos:Concept rdf:about="urn:aodn.org.au:geographicextents:concept:9">
      <skos:prefLabel xml:lang="en">Regional Seas | Banda Sea</skos:prefLabel>
      <skos:inScheme rdf:resource="urn:aodn.org.au:geographicextents:conceptscheme:1.0"/>
      <gml:BoundedBy>
         <gml:Envelope gml:srsName="http://www.opengis.net/gml/srs/epsg.xml#epsg:4326">
            <gml:lowerCorner>120.5 -8.5</gml:lowerCorner>
            <gml:upperCorner>133 -1</gml:upperCorner>
         </gml:Envelope>
      </gml:BoundedBy>
      <skos:broader rdf:resource="urn:aodn.org.au:geographicextents:concept:10000"/>
      <skos:definition xml:lang="en">Regional Seas | Banda Sea</skos:definition>
      <skos:scopeNote xml:lang="en">Regional Seas | Banda Sea: Regional Seas | Banda Sea</skos:scopeNote>
   </skos:Concept>
   <skos:Concept rdf:about="urn:aodn.org.au:geographicextents:concept:10">
      <skos:prefLabel xml:lang="en">Regional Seas | Bismarck Sea</skos:prefLabel>
      <skos:inScheme rdf:resource="urn:aodn.org.au:geographicextents:conceptscheme:1.0"/>
      <gml:BoundedBy>
         <gml:Envelope gml:srsName="http://www.opengis.net/gml/srs/epsg.xml#epsg:4326">
            <gml:lowerCorner>144 -6.5</gml:lowerCorner>
            <gml:upperCorner>152.5 -2</gml:upperCorner>
         </gml:Envelope>
      </gml:BoundedBy>
      <skos:broader rdf:resource="urn:aodn.org.au:geographicextents:concept:10000"/>
      <skos:definition xml:lang="en">Regional Seas | Bismarck Sea</skos:definition>
      <skos:scopeNote xml:lang="en">Regional Seas | Bismarck Sea: Regional Seas | Bismarck Sea</skos:scopeNote>
   </skos:Concept>
   <skos:Concept rdf:about="urn:aodn.org.au:geographicextents:concept:11">
      <skos:prefLabel xml:lang="en">Regional Seas | Celebes Sea</skos:prefLabel>
      <skos:inScheme rdf:resource="urn:aodn.org.au:geographicextents:conceptscheme:1.0"/>
      <gml:BoundedBy>
         <gml:Envelope gml:srsName="http://www.opengis.net/gml/srs/epsg.xml#epsg:4326">
            <gml:lowerCorner>117 1</gml:lowerCorner>
            <gml:upperCorner>125 8</gml:upperCorner>
         </gml:Envelope>
      </gml:BoundedBy>
      <skos:broader rdf:resource="urn:aodn.org.au:geographicextents:concept:10000"/>
      <skos:definition xml:lang="en">Regional Seas | Celebes Sea</skos:definition>
      <skos:scopeNote xml:lang="en">Regional Seas | Celebes Sea: Regional Seas | Celebes Sea</skos:scopeNote>
   </skos:Concept>
   <skos:Concept rdf:about="urn:aodn.org.au:geographicextents:concept:12">
      <skos:prefLabel xml:lang="en">Regional Seas | Ceram Sea</skos:prefLabel>
      <skos:inScheme rdf:resource="urn:aodn.org.au:geographicextents:conceptscheme:1.0"/>
      <gml:BoundedBy>
         <gml:Envelope gml:srsName="http://www.opengis.net/gml/srs/epsg.xml#epsg:4326">
            <gml:lowerCorner>126 -3</gml:lowerCorner>
            <gml:upperCorner>132 -2</gml:upperCorner>
         </gml:Envelope>
      </gml:BoundedBy>
      <skos:broader rdf:resource="urn:aodn.org.au:geographicextents:concept:10000"/>
      <skos:definition xml:lang="en">Regional Seas | Ceram Sea</skos:definition>
      <skos:scopeNote xml:lang="en">Regional Seas | Ceram Sea: Regional Seas | Ceram Sea</skos:scopeNote>
   </skos:Concept>
   <skos:Concept rdf:about="urn:aodn.org.au:geographicextents:concept:13">
      <skos:prefLabel xml:lang="en">Regional Seas | Coral Sea</skos:prefLabel>
      <skos:inScheme rdf:resource="urn:aodn.org.au:geographicextents:conceptscheme:1.0"/>
      <gml:BoundedBy>
         <gml:Envelope gml:srsName="http://www.opengis.net/gml/srs/epsg.xml#epsg:4326">
            <gml:lowerCorner>142.3 -24</gml:lowerCorner>
            <gml:upperCorner>156 -12</gml:upperCorner>
         </gml:Envelope>
      </gml:BoundedBy>
      <skos:broader rdf:resource="urn:aodn.org.au:geographicextents:concept:10000"/>
      <skos:definition xml:lang="en">Regional Seas | Coral Sea</skos:definition>
      <skos:scopeNote xml:lang="en">Regional Seas | Coral Sea: Regional Seas | Coral Sea</skos:scopeNote>
   </skos:Concept>
   <skos:Concept rdf:about="urn:aodn.org.au:geographicextents:concept:14">
      <skos:prefLabel xml:lang="en">Regional Seas | Flores Sea</skos:prefLabel>
      <skos:inScheme rdf:resource="urn:aodn.org.au:geographicextents:conceptscheme:1.0"/>
      <gml:BoundedBy>
         <gml:Envelope gml:srsName="http://www.opengis.net/gml/srs/epsg.xml#epsg:4326">
            <gml:lowerCorner>117 -8.5</gml:lowerCorner>
            <gml:upperCorner>123 -5.5</gml:upperCorner>
         </gml:Envelope>
      </gml:BoundedBy>
      <skos:broader rdf:resource="urn:aodn.org.au:geographicextents:concept:10000"/>
      <skos:definition xml:lang="en">Regional Seas | Flores Sea</skos:definition>
      <skos:scopeNote xml:lang="en">Regional Seas | Flores Sea: Regional Seas | Flores Sea</skos:scopeNote>
   </skos:Concept>
   <skos:Concept rdf:about="urn:aodn.org.au:geographicextents:concept:15">
      <skos:prefLabel xml:lang="en">Regional Seas | Gulf of Papua</skos:prefLabel>
      <skos:inScheme rdf:resource="urn:aodn.org.au:geographicextents:conceptscheme:1.0"/>
      <gml:BoundedBy>
         <gml:Envelope gml:srsName="http://www.opengis.net/gml/srs/epsg.xml#epsg:4326">
            <gml:lowerCorner>143 -10</gml:lowerCorner>
            <gml:upperCorner>147 -7.5</gml:upperCorner>
         </gml:Envelope>
      </gml:BoundedBy>
      <skos:broader rdf:resource="urn:aodn.org.au:geographicextents:concept:10000"/>
      <skos:definition xml:lang="en">Regional Seas | Gulf of Papua</skos:definition>
      <skos:scopeNote xml:lang="en">Regional Seas | Gulf of Papua: Regional Seas | Gulf of Papua</skos:scopeNote>
   </skos:Concept>
   <skos:Concept rdf:about="urn:aodn.org.au:geographicextents:concept:16">
      <skos:prefLabel xml:lang="en">Regional Seas | Gulf of Thailand</skos:prefLabel>
      <skos:inScheme rdf:resource="urn:aodn.org.au:geographicextents:conceptscheme:1.0"/>
      <gml:BoundedBy>
         <gml:Envelope gml:srsName="http://www.opengis.net/gml/srs/epsg.xml#epsg:4326">
            <gml:lowerCorner>99 7</gml:lowerCorner>
            <gml:upperCorner>105 14</gml:upperCorner>
         </gml:Envelope>
      </gml:BoundedBy>
      <skos:broader rdf:resource="urn:aodn.org.au:geographicextents:concept:10000"/>
      <skos:definition xml:lang="en">Regional Seas | Gulf of Thailand</skos:definition>
      <skos:scopeNote xml:lang="en">Regional Seas | Gulf of Thailand: Regional Seas | Gulf of Thailand</skos:scopeNote>
   </skos:Concept>
   <skos:Concept rdf:about="urn:aodn.org.au:geographicextents:concept:17">
      <skos:prefLabel xml:lang="en">Regional Seas | Java Sea</skos:prefLabel>
      <skos:inScheme rdf:resource="urn:aodn.org.au:geographicextents:conceptscheme:1.0"/>
      <gml:BoundedBy>
         <gml:Envelope gml:srsName="http://www.opengis.net/gml/srs/epsg.xml#epsg:4326">
            <gml:lowerCorner>105 -8</gml:lowerCorner>
            <gml:upperCorner>119 -3</gml:upperCorner>
         </gml:Envelope>
      </gml:BoundedBy>
      <skos:broader rdf:resource="urn:aodn.org.au:geographicextents:concept:10000"/>
      <skos:definition xml:lang="en">Regional Seas | Java Sea</skos:definition>
      <skos:scopeNote xml:lang="en">Regional Seas | Java Sea: Regional Seas | Java Sea</skos:scopeNote>
   </skos:Concept>
   <skos:Concept rdf:about="urn:aodn.org.au:geographicextents:concept:18">
      <skos:prefLabel xml:lang="en">Regional Seas | Makassar Strait</skos:prefLabel>
      <skos:inScheme rdf:resource="urn:aodn.org.au:geographicextents:conceptscheme:1.0"/>
      <gml:BoundedBy>
         <gml:Envelope gml:srsName="http://www.opengis.net/gml/srs/epsg.xml#epsg:4326">
            <gml:lowerCorner>116 -4</gml:lowerCorner>
            <gml:upperCorner>119.5 1</gml:upperCorner>
         </gml:Envelope>
      </gml:BoundedBy>
      <skos:broader rdf:resource="urn:aodn.org.au:geographicextents:concept:10000"/>
      <skos:definition xml:lang="en">Regional Seas | Makassar Strait</skos:definition>
      <skos:scopeNote xml:lang="en">Regional Seas | Makassar Strait: Regional Seas | Makassar Strait</skos:scopeNote>
   </skos:Concept>
   <skos:Concept rdf:about="urn:aodn.org.au:geographicextents:concept:19">
      <skos:prefLabel xml:lang="en">Regional Seas | Molucca Sea</skos:prefLabel>
      <skos:inScheme rdf:resource="urn:aodn.org.au:geographicextents:conceptscheme:1.0"/>
      <gml:BoundedBy>
         <gml:Envelope gml:srsName="http://www.opengis.net/gml/srs/epsg.xml#epsg:4326">
            <gml:lowerCorner>123 -1.5</gml:lowerCorner>
            <gml:upperCorner>128 8</gml:upperCorner>
         </gml:Envelope>
      </gml:BoundedBy>
      <skos:broader rdf:resource="urn:aodn.org.au:geographicextents:concept:10000"/>
      <skos:definition xml:lang="en">Regional Seas | Molucca Sea</skos:definition>
      <skos:scopeNote xml:lang="en">Regional Seas | Molucca Sea: Regional Seas | Molucca Sea</skos:scopeNote>
   </skos:Concept>
   <skos:Concept rdf:about="urn:aodn.org.au:geographicextents:concept:20">
      <skos:prefLabel xml:lang="en">Regional Seas | Savu Sea</skos:prefLabel>
      <skos:inScheme rdf:resource="urn:aodn.org.au:geographicextents:conceptscheme:1.0"/>
      <gml:BoundedBy>
         <gml:Envelope gml:srsName="http://www.opengis.net/gml/srs/epsg.xml#epsg:4326">
            <gml:lowerCorner>118 -11</gml:lowerCorner>
            <gml:upperCorner>125 -8</gml:upperCorner>
         </gml:Envelope>
      </gml:BoundedBy>
      <skos:broader rdf:resource="urn:aodn.org.au:geographicextents:concept:10000"/>
      <skos:definition xml:lang="en">Regional Seas | Savu Sea</skos:definition>
      <skos:scopeNote xml:lang="en">Regional Seas | Savu Sea: Regional Seas | Savu Sea</skos:scopeNote>
   </skos:Concept>
   <skos:Concept rdf:about="urn:aodn.org.au:geographicextents:concept:21">
      <skos:prefLabel xml:lang="en">Regional Seas | Solomon Sea</skos:prefLabel>
      <skos:inScheme rdf:resource="urn:aodn.org.au:geographicextents:conceptscheme:1.0"/>
      <gml:BoundedBy>
         <gml:Envelope gml:srsName="http://www.opengis.net/gml/srs/epsg.xml#epsg:4326">
            <gml:lowerCorner>147 -12</gml:lowerCorner>
            <gml:upperCorner>162 -4.5</gml:upperCorner>
         </gml:Envelope>
      </gml:BoundedBy>
      <skos:broader rdf:resource="urn:aodn.org.au:geographicextents:concept:10000"/>
      <skos:definition xml:lang="en">Regional Seas | Solomon Sea</skos:definition>
      <skos:scopeNote xml:lang="en">Regional Seas | Solomon Sea: Regional Seas | Solomon Sea</skos:scopeNote>
   </skos:Concept>
   <skos:Concept rdf:about="urn:aodn.org.au:geographicextents:concept:22">
      <skos:prefLabel xml:lang="en">Regional Seas | South China Sea</skos:prefLabel>
      <skos:inScheme rdf:resource="urn:aodn.org.au:geographicextents:conceptscheme:1.0"/>
      <gml:BoundedBy>
         <gml:Envelope gml:srsName="http://www.opengis.net/gml/srs/epsg.xml#epsg:4326">
            <gml:lowerCorner>102 -3</gml:lowerCorner>
            <gml:upperCorner>120 25</gml:upperCorner>
         </gml:Envelope>
      </gml:BoundedBy>
      <skos:broader rdf:resource="urn:aodn.org.au:geographicextents:concept:10000"/>
      <skos:definition xml:lang="en">Regional Seas | South China Sea</skos:definition>
      <skos:scopeNote xml:lang="en">Regional Seas | South China Sea: Regional Seas | South China Sea</skos:scopeNote>
   </skos:Concept>
   <skos:Concept rdf:about="urn:aodn.org.au:geographicextents:concept:23">
      <skos:prefLabel xml:lang="en">Regional Seas | Tasman Sea</skos:prefLabel>
      <skos:inScheme rdf:resource="urn:aodn.org.au:geographicextents:conceptscheme:1.0"/>
      <gml:BoundedBy>
         <gml:Envelope gml:srsName="http://www.opengis.net/gml/srs/epsg.xml#epsg:4326">
            <gml:lowerCorner>147 -53</gml:lowerCorner>
            <gml:upperCorner>175 -29</gml:upperCorner>
         </gml:Envelope>
      </gml:BoundedBy>
      <skos:broader rdf:resource="urn:aodn.org.au:geographicextents:concept:10000"/>
      <skos:definition xml:lang="en">Regional Seas | Tasman Sea</skos:definition>
      <skos:scopeNote xml:lang="en">Regional Seas | Tasman Sea: Regional Seas | Tasman Sea</skos:scopeNote>
   </skos:Concept>
   <skos:Concept rdf:about="urn:aodn.org.au:geographicextents:concept:24">
      <skos:prefLabel xml:lang="en">Regional Seas | Timor Sea</skos:prefLabel>
      <skos:inScheme rdf:resource="urn:aodn.org.au:geographicextents:conceptscheme:1.0"/>
      <gml:BoundedBy>
         <gml:Envelope gml:srsName="http://www.opengis.net/gml/srs/epsg.xml#epsg:4326">
            <gml:lowerCorner>123 -15</gml:lowerCorner>
            <gml:upperCorner>133 -8</gml:upperCorner>
         </gml:Envelope>
      </gml:BoundedBy>
      <skos:broader rdf:resource="urn:aodn.org.au:geographicextents:concept:10000"/>
      <skos:definition xml:lang="en">Regional Seas | Timor Sea</skos:definition>
      <skos:scopeNote xml:lang="en">Regional Seas | Timor Sea: Regional Seas | Timor Sea</skos:scopeNote>
   </skos:Concept>
   <skos:Concept rdf:about="urn:aodn.org.au:geographicextents:concept:34">
      <skos:prefLabel xml:lang="en">States, Territories (Australia) | Australian Antarctic Territory</skos:prefLabel>
      <skos:inScheme rdf:resource="urn:aodn.org.au:geographicextents:conceptscheme:1.0"/>
      <gml:BoundedBy>
         <gml:Envelope gml:srsName="http://www.opengis.net/gml/srs/epsg.xml#epsg:4326">
            <gml:lowerCorner>45 -90</gml:lowerCorner>
            <gml:upperCorner>160 -60</gml:upperCorner>
         </gml:Envelope>
      </gml:BoundedBy>
      <skos:broader rdf:resource="urn:aodn.org.au:geographicextents:concept:10003"/>
      <skos:definition xml:lang="en">States, Territories (Australia) | Australian Antarctic Territory</skos:definition>
      <skos:scopeNote xml:lang="en">States, Territories (Australia) | Australian Antarctic Territory: States, Territories (Australia) | Australian Antarctic Territory</skos:scopeNote>
   </skos:Concept>
   <skos:Concept rdf:about="urn:aodn.org.au:geographicextents:concept:35">
      <skos:prefLabel xml:lang="en">States, Territories (Australia) | Australian Capital Territory</skos:prefLabel>
      <skos:inScheme rdf:resource="urn:aodn.org.au:geographicextents:conceptscheme:1.0"/>
      <gml:BoundedBy>
         <gml:Envelope gml:srsName="http://www.opengis.net/gml/srs/epsg.xml#epsg:4326">
            <gml:lowerCorner>148.5 -36</gml:lowerCorner>
            <gml:upperCorner>149.5 -35</gml:upperCorner>
         </gml:Envelope>
      </gml:BoundedBy>
      <skos:broader rdf:resource="urn:aodn.org.au:geographicextents:concept:10003"/>
      <skos:definition xml:lang="en">States, Territories (Australia) | Australian Capital Territory</skos:definition>
      <skos:scopeNote xml:lang="en">States, Territories (Australia) | Australian Capital Territory: States, Territories (Australia) | Australian Capital Territory</skos:scopeNote>
   </skos:Concept>
   <skos:Concept rdf:about="urn:aodn.org.au:geographicextents:concept:36">
      <skos:prefLabel xml:lang="en">States, Territories (Australia) | New South Wales</skos:prefLabel>
      <skos:inScheme rdf:resource="urn:aodn.org.au:geographicextents:conceptscheme:1.0"/>
      <gml:BoundedBy>
         <gml:Envelope gml:srsName="http://www.opengis.net/gml/srs/epsg.xml#epsg:4326">
            <gml:lowerCorner>141 -37.5</gml:lowerCorner>
            <gml:upperCorner>154 -28</gml:upperCorner>
         </gml:Envelope>
      </gml:BoundedBy>
      <skos:broader rdf:resource="urn:aodn.org.au:geographicextents:concept:10003"/>
      <skos:definition xml:lang="en">States, Territories (Australia) | New South Wales</skos:definition>
      <skos:scopeNote xml:lang="en">States, Territories (Australia) | New South Wales: States, Territories (Australia) | New South Wales</skos:scopeNote>
   </skos:Concept>
   <skos:Concept rdf:about="urn:aodn.org.au:geographicextents:concept:37">
      <skos:prefLabel xml:lang="en">States, Territories (Australia) | Northern Territory</skos:prefLabel>
      <skos:inScheme rdf:resource="urn:aodn.org.au:geographicextents:conceptscheme:1.0"/>
      <gml:BoundedBy>
         <gml:Envelope gml:srsName="http://www.opengis.net/gml/srs/epsg.xml#epsg:4326">
            <gml:lowerCorner>129 -26</gml:lowerCorner>
            <gml:upperCorner>138 -11</gml:upperCorner>
         </gml:Envelope>
      </gml:BoundedBy>
      <skos:broader rdf:resource="urn:aodn.org.au:geographicextents:concept:10003"/>
      <skos:definition xml:lang="en">States, Territories (Australia) | Northern Territory</skos:definition>
      <skos:scopeNote xml:lang="en">States, Territories (Australia) | Northern Territory: States, Territories (Australia) | Northern Territory</skos:scopeNote>
   </skos:Concept>
   <skos:Concept rdf:about="urn:aodn.org.au:geographicextents:concept:38">
      <skos:prefLabel xml:lang="en">States, Territories (Australia) | Queensland</skos:prefLabel>
      <skos:inScheme rdf:resource="urn:aodn.org.au:geographicextents:conceptscheme:1.0"/>
      <gml:BoundedBy>
         <gml:Envelope gml:srsName="http://www.opengis.net/gml/srs/epsg.xml#epsg:4326">
            <gml:lowerCorner>138 -29.5</gml:lowerCorner>
            <gml:upperCorner>153.5 -9</gml:upperCorner>
         </gml:Envelope>
      </gml:BoundedBy>
      <skos:broader rdf:resource="urn:aodn.org.au:geographicextents:concept:10003"/>
      <skos:definition xml:lang="en">States, Territories (Australia) | Queensland</skos:definition>
      <skos:scopeNote xml:lang="en">States, Territories (Australia) | Queensland: States, Territories (Australia) | Queensland</skos:scopeNote>
   </skos:Concept>
   <skos:Concept rdf:about="urn:aodn.org.au:geographicextents:concept:39">
      <skos:prefLabel xml:lang="en">States, Territories (Australia) | South Australia</skos:prefLabel>
      <skos:inScheme rdf:resource="urn:aodn.org.au:geographicextents:conceptscheme:1.0"/>
      <gml:BoundedBy>
         <gml:Envelope gml:srsName="http://www.opengis.net/gml/srs/epsg.xml#epsg:4326">
            <gml:lowerCorner>129 -38.5</gml:lowerCorner>
            <gml:upperCorner>141 -26</gml:upperCorner>
         </gml:Envelope>
      </gml:BoundedBy>
      <skos:broader rdf:resource="urn:aodn.org.au:geographicextents:concept:10003"/>
      <skos:definition xml:lang="en">States, Territories (Australia) | South Australia</skos:definition>
      <skos:scopeNote xml:lang="en">States, Territories (Australia) | South Australia: States, Territories (Australia) | South Australia</skos:scopeNote>
   </skos:Concept>
   <skos:Concept rdf:about="urn:aodn.org.au:geographicextents:concept:40">
      <skos:prefLabel xml:lang="en">States, Territories (Australia) | Tasmania</skos:prefLabel>
      <skos:inScheme rdf:resource="urn:aodn.org.au:geographicextents:conceptscheme:1.0"/>
      <gml:BoundedBy>
         <gml:Envelope gml:srsName="http://www.opengis.net/gml/srs/epsg.xml#epsg:4326">
            <gml:lowerCorner>143.6 -44</gml:lowerCorner>
            <gml:upperCorner>148.6 -39.5</gml:upperCorner>
         </gml:Envelope>
      </gml:BoundedBy>
      <skos:broader rdf:resource="urn:aodn.org.au:geographicextents:concept:10003"/>
      <skos:definition xml:lang="en">States, Territories (Australia) | Tasmania</skos:definition>
      <skos:scopeNote xml:lang="en">States, Territories (Australia) | Tasmania: States, Territories (Australia) | Tasmania</skos:scopeNote>
   </skos:Concept>
   <skos:Concept rdf:about="urn:aodn.org.au:geographicextents:concept:41">
      <skos:prefLabel xml:lang="en">States, Territories (Australia) | Victoria</skos:prefLabel>
      <skos:inScheme rdf:resource="urn:aodn.org.au:geographicextents:conceptscheme:1.0"/>
      <gml:BoundedBy>
         <gml:Envelope gml:srsName="http://www.opengis.net/gml/srs/epsg.xml#epsg:4326">
            <gml:lowerCorner>141 -39</gml:lowerCorner>
            <gml:upperCorner>150 -34</gml:upperCorner>
         </gml:Envelope>
      </gml:BoundedBy>
      <skos:broader rdf:resource="urn:aodn.org.au:geographicextents:concept:10003"/>
      <skos:definition xml:lang="en">States, Territories (Australia) | Victoria</skos:definition>
      <skos:scopeNote xml:lang="en">States, Territories (Australia) | Victoria: States, Territories (Australia) | Victoria</skos:scopeNote>
   </skos:Concept>
   <skos:Concept rdf:about="urn:aodn.org.au:geographicextents:concept:42">
      <skos:prefLabel xml:lang="en">States, Territories (Australia) | Western Australia</skos:prefLabel>
      <skos:inScheme rdf:resource="urn:aodn.org.au:geographicextents:conceptscheme:1.0"/>
      <gml:BoundedBy>
         <gml:Envelope gml:srsName="http://www.opengis.net/gml/srs/epsg.xml#epsg:4326">
            <gml:lowerCorner>112.5 -35.5</gml:lowerCorner>
            <gml:upperCorner>129 -13.5</gml:upperCorner>
         </gml:Envelope>
      </gml:BoundedBy>
      <skos:broader rdf:resource="urn:aodn.org.au:geographicextents:concept:10003"/>
      <skos:definition xml:lang="en">States, Territories (Australia) | Western Australia</skos:definition>
      <skos:scopeNote xml:lang="en">States, Territories (Australia) | Western Australia: States, Territories (Australia) | Western Australia</skos:scopeNote>
   </skos:Concept>
</rdf:RDF>